<?xml version="1.0" encoding="utf-8"?>
<!-- Ontoterminology: ALyrA_ontoterminology -->
<!-- Author: Rafail Giannadakis -->
<!-- Creation date: May 18, 2024 -->
<!-- Export date: August 25, 2024 time: 10:01:57 PM -->
<!-- TEDI version: 3.7 -->
<!-- http://ontoterminology.com/tedi -->
<rdf:RDF xmlns="http://www.ontologia.fr/OTB/ALyrA_v.1.0#"
    xml:base="http://www.ontologia.fr/OTB/ALyrA_v.1.0"
    xmlns:rdf="http://www.w3.org/1999/02/22-rdf-syntax-ns#"
    xmlns:owl="http://www.w3.org/2002/07/owl#"
    xmlns:skos="http://www.w3.org/2004/02/skos/core#"
    xmlns:foaf="http://xmlns.com/foaf/0.1/"
    xmlns:dc="http://purl.org/dc/elements/1.1/"
    xmlns:xml="http://www.w3.org/XML/1998/namespace"
    xmlns:xsd="http://www.w3.org/2001/XMLSchema#"
    xmlns:rdfs="http://www.w3.org/2000/01/rdf-schema#"
    xmlns:otv="http://www.ontologia.fr/OTB/otv#"
    xmlns:vs="http://www.w3.org/2003/06/sw-vocab-status/ns#"
    xmlns:vann="http://purl.org/vocab/vann/"
    xmlns:ontolex="http://www.w3.org/ns/lemon/ontolex#">

	<!-- 
	//////////////////////////////////////////////////////////
	//
	// SKOS
	//
	//////////////////////////////////////////////////////////
	-->

	<!--  SKOS Concept Scheme -->

    <skos:ConceptScheme rdf:about="http://www.ontologia.fr/OTB/ALyrA_v.1.0">
        <dc:title>ALyrA_ontoterminology</dc:title>
        <dc:description>This is version 1.0 of the ALyrA ontoterminology (i.e., 'a terminology whose conceptual system is a formal ontology', Roche 2007 ), which focuses on modelling Archaic Lyric poets (799-430 BCΕ). AlyrA stands for "Archaic Lyrical Agora". 
The ontoterminology was created by Rafail Giannadakis (Department of Philology, University of Crete) under the supervision of Dr. Maria Papadopoulou (Department of Philology, University of Crete).
We gratefully acknowledge the generous funding of the European Commission in the context of the TALOS AI for SSH project (Grant agreement ID: 101087269).</dc:description>
        <dc:issued rdf:datatype="http://www.w3.org/2001/XMLSchema#date">2024-5-18</dc:issued>
        <dc:modified rdf:datatype="http://www.w3.org/2001/XMLSchema#date">2024-8-25</dc:modified>
        <dc:creator>Rafail Giannadakis</dc:creator>
        <dc:publisher>University of Crete - TALOS</dc:publisher>
    </skos:ConceptScheme>

	<!--  SKOS Concepts -->

    <skos:Concept rdf:about="#Archaic_Lyric_Composer">
        <skos:inScheme rdf:resource="http://www.ontologia.fr/OTB/ALyrA_v.1.0"/>
        <skos:topConceptOf rdf:resource="http://www.ontologia.fr/OTB/ALyrA_v.1.0"/>
        <rdfs:label xml:lang="en">archaic lyric composer</rdfs:label>
        <skos:prefLabel xml:lang="en">archaic lyric composer</skos:prefLabel>
        <skos:definition xml:lang="en">An Archaic Lyric composer is a person who lived during 7th-early 5th century BCE and wrote a lyric poem.</skos:definition>
        <rdfs:label xml:lang="el">αρχαϊκός λυρικός συνθέτης</rdfs:label>
        <skos:prefLabel xml:lang="el">αρχαϊκός λυρικός συνθέτης</skos:prefLabel>
        <skos:definition xml:lang="el">Ο αρχαϊκός λυρικός συνθέτης είναι ένα πρόσωπο που έζησε κατά τη διάρκεια του 7ου-αρχές του 5ου αιώνα π.Χ. και έγραψε λυρικό ποίημα.</skos:definition>
        <skos:narrower rdf:resource="#Archaic_Lyric_Poet"/>
        <skos:narrower rdf:resource="#Archaic_Lyric_Poetess"/>
        <skos:related rdf:resource="#BCE_century"/>
        <skos:related rdf:resource="#Ancient_Location"/>
        <skos:related rdf:resource="#Ancient_Location"/>
        <skos:related rdf:resource="#Archaic_Lyric_Poem"/>
    </skos:Concept>

    <skos:Concept rdf:about="#Archaic_Lyric_Poem_only_in_ionic_dialect_in_elegiac_couplet">
        <skos:inScheme rdf:resource="http://www.ontologia.fr/OTB/ALyrA_v.1.0"/>
        <rdfs:label xml:lang="en">elegy</rdfs:label>
        <skos:prefLabel xml:lang="en">elegy</skos:prefLabel>
        <skos:definition xml:lang="en">Elegies are poems written in elegiac couplets, with the first line in hexameter and the second line in pentameter, initially used for lamentation (but later had a wide range of themes) and possibly originating from Eastern mourning practices. They can be as short as a single couplet or longer sequences as needed.</skos:definition>
        <rdfs:label xml:lang="el">ελεγεία</rdfs:label>
        <skos:prefLabel xml:lang="el">ελεγεία</skos:prefLabel>
        <skos:definition xml:lang="el">Οι ελεγείες είναι ποιήματα γραμμένα σε ελεγειακά δίστιχα, με τον πρώτο στίχο σε εξάμετρο και τον δεύτερο σε πεντάμετρο. Αρχικά, χρησιμοποιήθηκαν για θρήνους (αλλά αργότερα είχαν ένα ευρύ φάσμα θεμάτων) και πιθανόν προέρχονται από τις ανατολίτικες θρηνητικές πρακτικές. Μπορεί να είναι μικρές σε έκταση (όσο ένα απλό κουπλέ) ή μεγαλύτερες.</skos:definition>
        <skos:broader rdf:resource="#Archaic_Lyric_Poem_only_in_ionic_dialect"/>
        <skos:narrower rdf:resource="#Archaic_Lyric_Poem_only_in_ionic_dialect_in_elegiac_couplet_with_erotic_content"/>
        <skos:narrower rdf:resource="#Archaic_Lyric_Poem_only_in_ionic_dialect_in_elegiac_couplet_with_gnomic_content"/>
        <skos:narrower rdf:resource="#Archaic_Lyric_Poem_only_in_ionic_dialect_in_elegiac_couplet_with_political_content"/>
        <skos:narrower rdf:resource="#Archaic_Lyric_Poem_only_in_ionic_dialect_in_elegiac_couplet_with_war_content"/>
    </skos:Concept>

    <skos:Concept rdf:about="#Archaic_Lyric_Poem">
        <skos:inScheme rdf:resource="http://www.ontologia.fr/OTB/ALyrA_v.1.0"/>
        <skos:topConceptOf rdf:resource="http://www.ontologia.fr/OTB/ALyrA_v.1.0"/>
        <rdfs:label xml:lang="en">archaic lyric poem</rdfs:label>
        <skos:prefLabel xml:lang="en">archaic lyric poem</skos:prefLabel>
        <skos:definition xml:lang="en">"Lyric poetry began as a fixture of ancient Greece, classified against other categories of poetry at the time of classical antiquity: dramas (written in verse) and epic poems. The lyric was far shorter, distinguished also by its focus on the poet’s state of mind and personal themes rather than narrative arc" (Academy of American Poets). So, an Archaic Lyric Poem is such poem written from 7th-early 5th century BCE.</skos:definition>
        <rdfs:label xml:lang="el">αρχαϊκό λυρικό ποίημα</rdfs:label>
        <skos:prefLabel xml:lang="el">αρχαϊκό λυρικό ποίημα</skos:prefLabel>
        <skos:definition xml:lang="el">"Η Λυρική ποίηση ξεκίνησε ως θεσμός της αρχαίας Ελλάδας, ταξινομημένος σε σχέση με άλλες κατηγορίες ποίησης κατά την εποχή της κλασικής αρχαιότητας: τα δραματικά (γραμμένα σε στίχους) και τα επικά ποιήματα. Η λυρική ποίηση ήταν πολύ πιο σύντομη, ενώ διακρινόταν επίσης από την εστίασή της στην ψυχική κατάσταση του ποιητή και σε προσωπικά θέματα και όχι στο αφηγηματικό τόξο" (Ακαδημία Αμερικανών Ποιητών). Έτσι, ένα αρχαϊκό λυρικό ποίημα είναι ένα τέτοιο ποίημα που γράφτηκε από τον 7ο-αρχές του 5ου αιώνα π.Χ.</skos:definition>
        <skos:narrower rdf:resource="#Archaic_Lyric_Poem_only_in_ionic_dialect"/>
        <skos:narrower rdf:resource="#Archaic_Lyric_Poem_in_ionic_or_in_doric_or_in_aeolic_dialect"/>
        <skos:related rdf:resource="#Archaic_Lyric_Composer"/>
    </skos:Concept>

    <skos:Concept rdf:about="#Archaic_Lyric_Poem_in_ionic_or_in_doric_or_in_aeolic_dialect_performed_by_a_chorus_or_by_a_single_performer_dedicated_to_apollo">
        <skos:inScheme rdf:resource="http://www.ontologia.fr/OTB/ALyrA_v.1.0"/>
        <rdfs:label xml:lang="en">paean</rdfs:label>
        <skos:prefLabel xml:lang="en">paean</skos:prefLabel>
        <skos:definition xml:lang="en">Lyric song dedicated to Ancient Greek god Apollo. Alcman, Pindar and Bacchylides are famous composers of paeans.</skos:definition>
        <rdfs:label xml:lang="el">παιάνας</rdfs:label>
        <skos:prefLabel xml:lang="el">παιάνας</skos:prefLabel>
        <skos:definition xml:lang="el">Λυρικό τραγούδι αφιερωμένο στον αρχαίο Έλληνα θεό Απόλλωνα. Ο Αλκμάνας, ο Πίνδαρος και ο Βακχυλίδης είναι διάσημοι συνθέτες παιάνων.</skos:definition>
        <skos:broader rdf:resource="#Archaic_Lyric_Poem_in_ionic_or_in_doric_or_in_aeolic_dialect_performed_by_a_chorus_or_by_a_single_performer_dedicated_to_a_god"/>
    </skos:Concept>

    <skos:Concept rdf:about="#Archaic_Lyric_Poem_only_in_ionic_dialect_in_elegiac_couplet_with_gnomic_content">
        <skos:inScheme rdf:resource="http://www.ontologia.fr/OTB/ALyrA_v.1.0"/>
        <rdfs:label xml:lang="en">gnomic elegy</rdfs:label>
        <skos:prefLabel xml:lang="en">gnomic elegy</skos:prefLabel>
        <skos:definition xml:lang="en">Elegy with gnomic, counseling, biosophical content. Known poets of gnomic elegies are Phocylides and Theognis.</skos:definition>
        <rdfs:label xml:lang="el">γνωμική ελεγεία</rdfs:label>
        <skos:prefLabel xml:lang="el">γνωμική ελεγεία</skos:prefLabel>
        <skos:definition xml:lang="el">Ελεγεία με γνωμικό, συμβουλευτικό, βιοσοφικό περιεχόμενο. Γνωστοί ποιητές γνωστών γνωμικών ελεγειών είναι ο Φωκυλίδης και ο Θεογένης.</skos:definition>
        <skos:broader rdf:resource="#Archaic_Lyric_Poem_only_in_ionic_dialect_in_elegiac_couplet"/>
    </skos:Concept>

    <skos:Concept rdf:about="#Archaic_Lyric_Poem_in_ionic_or_in_doric_or_in_aeolic_dialect_performed_by_a_chorus">
        <skos:inScheme rdf:resource="http://www.ontologia.fr/OTB/ALyrA_v.1.0"/>
        <rdfs:label xml:lang="en">archaic lyric poem in ionic or in doric or in aeolic dialect performed by a chorus</rdfs:label>
        <skos:prefLabel xml:lang="en">archaic lyric poem in ionic or in doric or in aeolic dialect performed by a chorus</skos:prefLabel>
        <skos:definition xml:lang="en">Lyric song performed by a group (chorus) of people (women, men), which were dancing and singing.</skos:definition>
        <rdfs:label xml:lang="el">αρχαϊκό λυρικό ποίημα σε ιωνική ή δωρική ή αιολική διάλεκτο που εκτελείται από χορό</rdfs:label>
        <skos:prefLabel xml:lang="el">αρχαϊκό λυρικό ποίημα σε ιωνική ή δωρική ή αιολική διάλεκτο που εκτελείται από χορό</skos:prefLabel>
        <skos:definition xml:lang="el">Μέλος που εκτελείται από Χορό.</skos:definition>
        <skos:broader rdf:resource="#Archaic_Lyric_Poem_in_ionic_or_in_doric_or_in_aeolic_dialect"/>
        <skos:narrower rdf:resource="#Archaic_Lyric_Poem_in_ionic_or_in_doric_or_in_aeolic_dialect_performed_by_a_chorus_performed_by_a_maidens_chorus"/>
        <skos:narrower rdf:resource="#Archaic_Lyric_Poem_in_ionic_or_in_doric_or_in_aeolic_dialect_performed_by_a_chorus_performed_by_a_non-specific_type_of_chorus"/>
    </skos:Concept>

    <skos:Concept rdf:about="#Archaic_Lyric_Poem_in_ionic_or_in_doric_or_in_aeolic_dialect_performed_by_a_chorus_on_the_way_to_an_altar">
        <skos:inScheme rdf:resource="http://www.ontologia.fr/OTB/ALyrA_v.1.0"/>
        <rdfs:label xml:lang="en">prosodion</rdfs:label>
        <skos:prefLabel xml:lang="en">prosodion</skos:prefLabel>
        <skos:definition xml:lang="en">A lyric song performed on the way to an altar by a chorus. Alcman, Bacchylides and Pindar are famous prosodia composers.</skos:definition>
        <rdfs:label xml:lang="el">προσόδιο</rdfs:label>
        <skos:prefLabel xml:lang="el">προσόδιο</skos:prefLabel>
        <skos:definition xml:lang="el">Ένα λυρικό τραγούδι που ερμηνεύεται στο δρόμο προς το ιερό από μια χορωδία. Ο Αλκμάν, ο Βακχυλίδης και ο Πίνδαρος είναι διάσημοι συνθέτες προσοδίων.</skos:definition>
        <skos:broader rdf:resource="#Archaic_Lyric_Poem_in_ionic_or_in_doric_or_in_aeolic_dialect_performed_by_a_chorus_performed_by_a_non-specific_type_of_chorus"/>
    </skos:Concept>

    <skos:Concept rdf:about="#Archaic_Lyric_Poem_in_ionic_or_in_doric_or_in_aeolic_dialect_performed_by_a_single_performer">
        <skos:inScheme rdf:resource="http://www.ontologia.fr/OTB/ALyrA_v.1.0"/>
        <rdfs:label xml:lang="en">monody</rdfs:label>
        <skos:prefLabel xml:lang="en">monody</skos:prefLabel>
        <skos:definition xml:lang="en">Monodies are characterized by solo performances, where the poet identifies with the singer and expresses personal thoughts and emotions, as they offer a direct and free expression of personality. For instance, in Sapphic odes, the poetess prioritizes her own voice over others.</skos:definition>
        <rdfs:label xml:lang="el">μονωδία</rdfs:label>
        <skos:prefLabel xml:lang="el">μονωδία</skos:prefLabel>
        <skos:definition xml:lang="el">Οι μονωδίες χαρακτηρίζονται από σόλο ερμηνείες, όπου ο ποιητής ταυτίζεται με τον τραγουδιστή και εκφράζει προσωπικές σκέψεις και συναισθήματα, καθώς προσφέρουν μια άμεση και ελεύθερη έκφραση της προσωπικότητας. Για παράδειγμα, στις σαπφικές ωδές, η ποιήτρια δίνει προτεραιότητα στη δική της φωνή έναντι των άλλων.</skos:definition>
        <skos:broader rdf:resource="#Archaic_Lyric_Poem_in_ionic_or_in_doric_or_in_aeolic_dialect"/>
    </skos:Concept>

    <skos:Concept rdf:about="#Archaic_Lyric_Poem_only_in_ionic_dialect">
        <skos:inScheme rdf:resource="http://www.ontologia.fr/OTB/ALyrA_v.1.0"/>
        <rdfs:label xml:lang="en">archaic lyric poem only in ionic dialect</rdfs:label>
        <skos:prefLabel xml:lang="en">archaic lyric poem only in ionic dialect</skos:prefLabel>
        <skos:definition xml:lang="en">Archaic Lyric poem written only in ionic dialect. Ionic greek dialect, a subset of Eastern Greek, originated on the mainland and spread during the Dorian invasions. By the 5th century BC, it was primarily spoken in Ionia, including Asia Minor, Chios, and Samos. It also extended to Euboea and through Ionian colonization to the northern Aegean, Black Sea, and western Mediterranean.</skos:definition>
        <rdfs:label xml:lang="el">αρχαϊκό λυρικό ποίημα μόνο στην ιωνική διάλεκτο</rdfs:label>
        <skos:prefLabel xml:lang="el">αρχαϊκό λυρικό ποίημα μόνο στην ιωνική διάλεκτο</skos:prefLabel>
        <skos:definition xml:lang="el">Αρχαϊκό λυρικό ποίημα μόνο στην ιωνική διάλεκτο.</skos:definition>
        <skos:broader rdf:resource="#Archaic_Lyric_Poem"/>
        <skos:narrower rdf:resource="#Archaic_Lyric_Poem_only_in_ionic_dialect_in_elegiac_couplet"/>
        <skos:narrower rdf:resource="#Archaic_Lyric_Poem_only_in_ionic_dialect_in_iambic_or_trochaic_metre"/>
    </skos:Concept>

    <skos:Concept rdf:about="#Ancient_Location">
        <skos:inScheme rdf:resource="http://www.ontologia.fr/OTB/ALyrA_v.1.0"/>
        <skos:topConceptOf rdf:resource="http://www.ontologia.fr/OTB/ALyrA_v.1.0"/>
        <rdfs:label xml:lang="en">ancient location</rdfs:label>
        <skos:prefLabel xml:lang="en">ancient location</skos:prefLabel>
        <skos:definition xml:lang="en">In the current ontoterminology Ancient Location objects concern the places where the Archaic Lyric Poets were born or lived, while they are inserted with coordinates from the pleiades gazetteer of ancient places (https:pleiades.stoa.orgplaces).</skos:definition>
        <rdfs:label xml:lang="el">αρχαία τοποθεσία</rdfs:label>
        <skos:prefLabel xml:lang="el">αρχαία τοποθεσία</skos:prefLabel>
        <skos:definition xml:lang="el">Στην παρούσα οντοορολογία γίνεται αναφορά στους τόπους όπου γεννήθηκαν ή έζησαν οι αρχαϊκοί λυρικοί ποιητές. Η ακριβής τους τοποθεσία εισάγεται με συντεταγμένες από το ευρετήριο αρχαίων τόπων pleiades (https:pleiades.stoa.orgplaces).</skos:definition>
        <skos:related rdf:resource="#Archaic_Lyric_Composer"/>
        <skos:related rdf:resource="#Archaic_Lyric_Composer"/>
    </skos:Concept>

    <skos:Concept rdf:about="#Archaic_Lyric_Poem_in_ionic_or_in_doric_or_in_aeolic_dialect_performed_by_a_chorus_or_by_a_single_performer_dedicated_to_dionysus">
        <skos:inScheme rdf:resource="http://www.ontologia.fr/OTB/ALyrA_v.1.0"/>
        <rdfs:label xml:lang="en">dithyramb</rdfs:label>
        <skos:prefLabel xml:lang="en">dithyramb</skos:prefLabel>
        <skos:definition xml:lang="en">Devotional hymns of Dionysus. Bacchylides, Pindar and Simonides are known to have composed dithyrambs.</skos:definition>
        <rdfs:label xml:lang="el">διθύραμβος</rdfs:label>
        <skos:prefLabel xml:lang="el">διθύραμβος</skos:prefLabel>
        <skos:definition xml:lang="el">Λατρευτικοί ύμνοι του Διονύσου. Ο Βακχυλίδης, ο Πίνδαρος και ο Σιμωνίδης είναι γνωστό ότι συνέθεσαν διθύραμβους.</skos:definition>
        <skos:broader rdf:resource="#Archaic_Lyric_Poem_in_ionic_or_in_doric_or_in_aeolic_dialect_performed_by_a_chorus_or_by_a_single_performer_dedicated_to_a_god"/>
    </skos:Concept>

    <skos:Concept rdf:about="#Archaic_Lyric_Poem_in_ionic_or_in_doric_or_in_aeolic_dialect_performed_by_a_chorus_or_by_a_single_performer_dedicated_to_a_god">
        <skos:inScheme rdf:resource="http://www.ontologia.fr/OTB/ALyrA_v.1.0"/>
        <rdfs:label xml:lang="en">hymn</rdfs:label>
        <skos:prefLabel xml:lang="en">hymn</skos:prefLabel>
        <skos:definition xml:lang="en">Lyric song dedicated to gods. Multiple poets has composed hymns, sych as Alcaeus, Terpander, Sappho, Alcman et. al.</skos:definition>
        <rdfs:label xml:lang="el">ύμνος</rdfs:label>
        <skos:prefLabel xml:lang="el">ύμνος</skos:prefLabel>
        <skos:definition xml:lang="el">Λυρικό τραγούδι αφιερωμένο στους θεούς. Πολλοί ποιητές έχουν συνθέσει ύμνους, όπως ο Αλκαίος, ο Τέρπανδρος, η Σαπφώ, ο Αλκμάνας κ.ά.</skos:definition>
        <skos:broader rdf:resource="#Archaic_Lyric_Poem_in_ionic_or_in_doric_or_in_aeolic_dialect_performed_by_a_chorus_or_by_a_single_performer"/>
        <skos:narrower rdf:resource="#Archaic_Lyric_Poem_in_ionic_or_in_doric_or_in_aeolic_dialect_performed_by_a_chorus_or_by_a_single_performer_dedicated_to_apollo"/>
        <skos:narrower rdf:resource="#Archaic_Lyric_Poem_in_ionic_or_in_doric_or_in_aeolic_dialect_performed_by_a_chorus_or_by_a_single_performer_dedicated_to_dionysus"/>
    </skos:Concept>

    <skos:Concept rdf:about="#Archaic_Lyric_Poem_only_in_ionic_dialect_in_iambic_or_trochaic_metre">
        <skos:inScheme rdf:resource="http://www.ontologia.fr/OTB/ALyrA_v.1.0"/>
        <rdfs:label xml:lang="en">iamb</rdfs:label>
        <skos:prefLabel xml:lang="en">iamb</skos:prefLabel>
        <skos:definition xml:lang="en">Initially associated with Dionysus, the iamb may have a pre-Hellenic origin as a poetic form. Typically composed in iambic trimeter or trochaic tetrameter, its Ionic version often adopts a first-person perspective, though its context can vary.</skos:definition>
        <rdfs:label xml:lang="el">ίαμβος</rdfs:label>
        <skos:prefLabel xml:lang="el">ίαμβος</skos:prefLabel>
        <skos:definition xml:lang="el">Αρχικά συνδεόμενος με τον Διόνυσο, ο ίαμβος μπορεί να έχει προελληνική προέλευση ως ποιητική μορφή. Συνήθως συντίθεται σε ιαμβικό τρίμετρο ή τροχαϊκό τετράμετρο, η ιωνική εκδοχή του συχνά υιοθετεί την πρωτοπρόσωπη σκοπιά, αν και τα συμφραζόμενα μπορεί να ποικίλλουν.</skos:definition>
        <skos:broader rdf:resource="#Archaic_Lyric_Poem_only_in_ionic_dialect"/>
    </skos:Concept>

    <skos:Concept rdf:about="#Archaic_Lyric_Poem_in_ionic_or_in_doric_or_in_aeolic_dialect_performed_by_a_chorus_or_by_a_single_performer">
        <skos:inScheme rdf:resource="http://www.ontologia.fr/OTB/ALyrA_v.1.0"/>
        <rdfs:label xml:lang="en">archaic lyric poem in ionic or in doric or in aeolic dialect performed by a chorus or by a single performer</rdfs:label>
        <skos:prefLabel xml:lang="en">archaic lyric poem in ionic or in doric or in aeolic dialect performed by a chorus or by a single performer</skos:prefLabel>
        <skos:definition xml:lang="en">Melos which was performed either by one person or by a chorus.</skos:definition>
        <rdfs:label xml:lang="el">αρχαϊκό λυρικό ποίημα σε ιωνική ή δωρική ή αιολική διάλεκτο που εκτελείται από χορό ή από έναν μόνο ερμηνευτή</rdfs:label>
        <skos:prefLabel xml:lang="el">αρχαϊκό λυρικό ποίημα σε ιωνική ή δωρική ή αιολική διάλεκτο που εκτελείται από χορό ή από έναν μόνο ερμηνευτή</skos:prefLabel>
        <skos:definition xml:lang="el">Μέλος που εκτελείται από χορό ή από έναν μόνο ερμηνευτή.</skos:definition>
        <skos:broader rdf:resource="#Archaic_Lyric_Poem_in_ionic_or_in_doric_or_in_aeolic_dialect"/>
        <skos:narrower rdf:resource="#Archaic_Lyric_Poem_in_ionic_or_in_doric_or_in_aeolic_dialect_performed_by_a_chorus_or_by_a_single_performer_dedicated_to_a_god"/>
        <skos:narrower rdf:resource="#Archaic_Lyric_Poem_in_ionic_or_in_doric_or_in_aeolic_dialect_performed_by_a_chorus_or_by_a_single_performer_dedicated_to_living"/>
    </skos:Concept>

    <skos:Concept rdf:about="#Archaic_Lyric_Poem_in_ionic_or_in_doric_or_in_aeolic_dialect_performed_by_a_chorus_or_by_a_single_performer_dedicated_to_dead">
        <skos:inScheme rdf:resource="http://www.ontologia.fr/OTB/ALyrA_v.1.0"/>
        <rdfs:label xml:lang="en">threnos</rdfs:label>
        <skos:prefLabel xml:lang="en">threnos</skos:prefLabel>
        <skos:definition xml:lang="en">Lyric song dedicated to a dead human being. Anacreon, Pindar and Simonides are famous for their such compositions.</skos:definition>
        <rdfs:label xml:lang="el">θρήνος</rdfs:label>
        <skos:prefLabel xml:lang="el">θρήνος</skos:prefLabel>
        <skos:definition xml:lang="el">Λυρικό τραγούδι αφιερωμένο σε έναν νεκρό άνθρωπο. Ο Ανακρέων, ο Πίνδαρος και ο Σιμωνίδης είναι διάσημοι για τέτοιες συνθέσεις τους.</skos:definition>
        <skos:broader rdf:resource="#Archaic_Lyric_Poem_in_ionic_or_in_doric_or_in_aeolic_dialect_performed_by_a_chorus_or_by_a_single_performer_dedicated_to_living"/>
    </skos:Concept>

    <skos:Concept rdf:about="#Archaic_Lyric_Poem_in_ionic_or_in_doric_or_in_aeolic_dialect">
        <skos:inScheme rdf:resource="http://www.ontologia.fr/OTB/ALyrA_v.1.0"/>
        <rdfs:label xml:lang="en">melos</rdfs:label>
        <skos:prefLabel xml:lang="en">melos</skos:prefLabel>
        <skos:definition xml:lang="en">Melos is the hypernym of the Archaic Lyric poems, which were written in ionic (except of the iamb and elegy), aeolic and doric dialect.</skos:definition>
        <rdfs:label xml:lang="el">μέλος</rdfs:label>
        <skos:prefLabel xml:lang="el">μέλος</skos:prefLabel>
        <skos:definition xml:lang="el">Το Μέλος είναι το υπερώνυμο των αρχαϊκών λυρικών ποιημάτων, τα οποία ήταν γραμμένα σε ιωνική (εκτός από τον ίαμβο και την ελεγεία), αιολική και δωρική διάλεκτο.</skos:definition>
        <skos:broader rdf:resource="#Archaic_Lyric_Poem"/>
        <skos:narrower rdf:resource="#Archaic_Lyric_Poem_in_ionic_or_in_doric_or_in_aeolic_dialect_performed_by_a_chorus_or_by_a_single_performer"/>
        <skos:narrower rdf:resource="#Archaic_Lyric_Poem_in_ionic_or_in_doric_or_in_aeolic_dialect_performed_by_a_single_performer"/>
        <skos:narrower rdf:resource="#Archaic_Lyric_Poem_in_ionic_or_in_doric_or_in_aeolic_dialect_performed_by_a_chorus"/>
    </skos:Concept>

    <skos:Concept rdf:about="#Archaic_Lyric_Poem_only_in_ionic_dialect_in_elegiac_couplet_with_war_content">
        <skos:inScheme rdf:resource="http://www.ontologia.fr/OTB/ALyrA_v.1.0"/>
        <rdfs:label xml:lang="en">war elegy</rdfs:label>
        <skos:prefLabel xml:lang="en">war elegy</skos:prefLabel>
        <skos:definition xml:lang="en">Elegy with war content. Tyrtaeus and Callinus are famous poets of such elegy.</skos:definition>
        <rdfs:label xml:lang="el">πολεμική ελεγεία</rdfs:label>
        <skos:prefLabel xml:lang="el">πολεμική ελεγεία</skos:prefLabel>
        <skos:definition xml:lang="el">Ελεγεία με πολεμικό χαρακτήρα. Ο Τυρταίος και ο Καλλίνικος είναι διάσημοι ποιητές τέτοιων ελεγειών.</skos:definition>
        <skos:broader rdf:resource="#Archaic_Lyric_Poem_only_in_ionic_dialect_in_elegiac_couplet"/>
    </skos:Concept>

    <skos:Concept rdf:about="#Archaic_Lyric_Poem_in_ionic_or_in_doric_or_in_aeolic_dialect_performed_by_a_chorus_with_imitation_expressions">
        <skos:inScheme rdf:resource="http://www.ontologia.fr/OTB/ALyrA_v.1.0"/>
        <rdfs:label xml:lang="en">hyporcheme</rdfs:label>
        <skos:prefLabel xml:lang="en">hyporcheme</skos:prefLabel>
        <skos:definition xml:lang="en">A lyric song accompanied by imitative movements. Bacchylides and Pindar are famous for composing hyporchemes.</skos:definition>
        <rdfs:label xml:lang="el">υπόρχημα</rdfs:label>
        <skos:prefLabel xml:lang="el">υπόρχημα</skos:prefLabel>
        <skos:definition xml:lang="el">Ένα λυρικό τραγούδι που συνοδεύεται από μιμητικές κινήσεις. Ο Βακχυλίδης και ο Πίνδαρος φημίζονται για τη σύνθεση υπορχημάτων.</skos:definition>
        <skos:broader rdf:resource="#Archaic_Lyric_Poem_in_ionic_or_in_doric_or_in_aeolic_dialect_performed_by_a_chorus_performed_by_a_non-specific_type_of_chorus"/>
    </skos:Concept>

    <skos:Concept rdf:about="#Archaic_Lyric_Poem_in_ionic_or_in_doric_or_in_aeolic_dialect_performed_by_a_chorus_or_by_a_single_performer_dedicated_to_wedding_couple">
        <skos:inScheme rdf:resource="http://www.ontologia.fr/OTB/ALyrA_v.1.0"/>
        <rdfs:label xml:lang="en">epithalamion</rdfs:label>
        <skos:prefLabel xml:lang="en">epithalamion</skos:prefLabel>
        <skos:definition xml:lang="en">Epithalamium is a song dedicated to a wedding couple sung at the nuptial residence. Sappho is famous for her such songs.</skos:definition>
        <rdfs:label xml:lang="el">επιθαλάμιο</rdfs:label>
        <skos:prefLabel xml:lang="el">επιθαλάμιο</skos:prefLabel>
        <skos:definition xml:lang="el">Το Επιθαλάμιο είναι ένα τραγούδι αφιερωμένο σε ένα γαμήλιο ζευγάρι που τραγουδιέται στη γαμήλια κατοικία. Η Σαπφώ είναι γνωστή για τα επιθαλάμιά της.</skos:definition>
        <skos:broader rdf:resource="#Archaic_Lyric_Poem_in_ionic_or_in_doric_or_in_aeolic_dialect_performed_by_a_chorus_or_by_a_single_performer_dedicated_to_living"/>
    </skos:Concept>

    <skos:Concept rdf:about="#Archaic_Lyric_Poem_only_in_ionic_dialect_in_elegiac_couplet_with_political_content">
        <skos:inScheme rdf:resource="http://www.ontologia.fr/OTB/ALyrA_v.1.0"/>
        <rdfs:label xml:lang="en">political elegy</rdfs:label>
        <skos:prefLabel xml:lang="en">political elegy</skos:prefLabel>
        <skos:definition xml:lang="en">Elegy with political content. Solon Atheniensis is a famous poet who composed such elegies.</skos:definition>
        <rdfs:label xml:lang="el">πολιτική ελεγεία</rdfs:label>
        <skos:prefLabel xml:lang="el">πολιτική ελεγεία</skos:prefLabel>
        <skos:definition xml:lang="el">Ελεγεία με πολιτικό χαρακτήρα. Ο Τυρταίος και ο Καλλίνικος είναι διάσημοι ποιητές τέτοιων ελεγειών.</skos:definition>
        <skos:broader rdf:resource="#Archaic_Lyric_Poem_only_in_ionic_dialect_in_elegiac_couplet"/>
    </skos:Concept>

    <skos:Concept rdf:about="#Archaic_Lyric_Poem_in_ionic_or_in_doric_or_in_aeolic_dialect_performed_by_a_chorus_performed_by_a_non-specific_type_of_chorus">
        <skos:inScheme rdf:resource="http://www.ontologia.fr/OTB/ALyrA_v.1.0"/>
        <rdfs:label xml:lang="en">archaic lyric poem in ionic or doric or aeolic dialect performed by a chorus of no particular type</rdfs:label>
        <skos:definition xml:lang="en">An Archaic Lyric poem in Ionic or Doric or Aeolic dialect performed by a chorus of no particular type.</skos:definition>
        <rdfs:label xml:lang="el">αρχαϊκό λυρικό ποίημα σε ιωνική ή δωρική ή αιολική διάλεκτο που εκτελείται από χορό μη συγκεκριμένου τύπου</rdfs:label>
        <skos:prefLabel xml:lang="el">αρχαϊκό λυρικό ποίημα σε ιωνική ή δωρική ή αιολική διάλεκτο που εκτελείται από χορό μη συγκεκριμένου τύπου</skos:prefLabel>
        <skos:definition xml:lang="el">Αρχαϊκό λυρικό ποίημα σε ιωνική ή δωρική ή αιολική διάλεκτο που εκτελείται από χορό μη συγκεκριμένου τύπου.</skos:definition>
        <skos:broader rdf:resource="#Archaic_Lyric_Poem_in_ionic_or_in_doric_or_in_aeolic_dialect_performed_by_a_chorus"/>
        <skos:narrower rdf:resource="#Archaic_Lyric_Poem_in_ionic_or_in_doric_or_in_aeolic_dialect_performed_by_a_chorus_during_bride_procession"/>
        <skos:narrower rdf:resource="#Archaic_Lyric_Poem_in_ionic_or_in_doric_or_in_aeolic_dialect_performed_by_a_chorus_with_imitation_expressions"/>
        <skos:narrower rdf:resource="#Archaic_Lyric_Poem_in_ionic_or_in_doric_or_in_aeolic_dialect_performed_by_a_chorus_on_the_way_to_an_altar"/>
    </skos:Concept>

    <skos:Concept rdf:about="#BCE_century">
        <skos:inScheme rdf:resource="http://www.ontologia.fr/OTB/ALyrA_v.1.0"/>
        <skos:topConceptOf rdf:resource="http://www.ontologia.fr/OTB/ALyrA_v.1.0"/>
        <rdfs:label xml:lang="en">before common era century</rdfs:label>
        <skos:prefLabel xml:lang="en">before common era century</skos:prefLabel>
        <skos:definition xml:lang="en">Century that is BCE.</skos:definition>
        <rdfs:label xml:lang="el">προχριστιανικός αιώνας</rdfs:label>
        <skos:prefLabel xml:lang="el">προχριστιανικός αιώνας</skos:prefLabel>
        <skos:definition xml:lang="el"> Προχριστιανικός αιώνας.</skos:definition>
        <skos:related rdf:resource="#Archaic_Lyric_Composer"/>
    </skos:Concept>

    <skos:Concept rdf:about="#Archaic_Lyric_Poetess">
        <skos:inScheme rdf:resource="http://www.ontologia.fr/OTB/ALyrA_v.1.0"/>
        <rdfs:label xml:lang="en">archaic lyric poetess</rdfs:label>
        <skos:prefLabel xml:lang="en">archaic lyric poetess</skos:prefLabel>
        <skos:definition xml:lang="en">An Archaic Lyric poetess (woman) is a person who lived during 7th-early 5th century BCE and wrote Archaic Lyric poetry.</skos:definition>
        <rdfs:label xml:lang="el">αρχαϊκή λυρική ποιήτρια</rdfs:label>
        <skos:prefLabel xml:lang="el">αρχαϊκή λυρική ποιήτρια</skos:prefLabel>
        <skos:definition xml:lang="el">Η αρχαϊκή λυρική ποιήτρια είναι πρόσωπο που έζησε κατά τον 7ο-αρχές του 5ου αιώνα π.Χ. και έγραψε αρχαϊκή λυρική ποίηση.</skos:definition>
        <skos:broader rdf:resource="#Archaic_Lyric_Composer"/>
    </skos:Concept>

    <skos:Concept rdf:about="#Archaic_Lyric_Poem_in_ionic_or_in_doric_or_in_aeolic_dialect_performed_by_a_chorus_performed_by_a_maidens_chorus">
        <skos:inScheme rdf:resource="http://www.ontologia.fr/OTB/ALyrA_v.1.0"/>
        <rdfs:label xml:lang="en">partheneion</rdfs:label>
        <skos:prefLabel xml:lang="en">partheneion</skos:prefLabel>
        <skos:definition xml:lang="en">A lyric song performed by a maidens chorus. Alcman, Pindar and Bacchylides are famous for composing Partheneia.</skos:definition>
        <rdfs:label xml:lang="el">παρθένειο</rdfs:label>
        <skos:prefLabel xml:lang="el">παρθένειο</skos:prefLabel>
        <skos:definition xml:lang="el">Ένα λυρικό τραγούδι που ερμηνεύεται από μια χορωδία νεανίδων. Ο Αλκμάνας, ο Πίνδαρος και ο Βακχυλίδης φημίζονται για τη σύνθεση των Παρθενείων.</skos:definition>
        <skos:broader rdf:resource="#Archaic_Lyric_Poem_in_ionic_or_in_doric_or_in_aeolic_dialect_performed_by_a_chorus"/>
    </skos:Concept>

    <skos:Concept rdf:about="#Archaic_Lyric_Poem_in_ionic_or_in_doric_or_in_aeolic_dialect_performed_by_a_chorus_or_by_a_single_performer_dedicated_to_winners_in_athletic_events">
        <skos:inScheme rdf:resource="http://www.ontologia.fr/OTB/ALyrA_v.1.0"/>
        <rdfs:label xml:lang="en">epinikion</rdfs:label>
        <skos:prefLabel xml:lang="en">epinikion</skos:prefLabel>
        <skos:definition xml:lang="en">Lyric song of praise winners of sports games. Pindar, Bacchylides and Ibicus are who composed epinikia.</skos:definition>
        <rdfs:label xml:lang="el">επίνικος</rdfs:label>
        <skos:prefLabel xml:lang="el">επίνικος</skos:prefLabel>
        <skos:definition xml:lang="el">Λυρικό τραγούδι αφιερωμένο σε νικητή αθλητικών αγώνων. Ο Πίνδαρος, ο Βακχυλίδης και ο Ίβυκος είναι αυτοί που συνέθεσαν επινίκια τραγούδια.</skos:definition>
        <skos:broader rdf:resource="#Archaic_Lyric_Poem_in_ionic_or_in_doric_or_in_aeolic_dialect_performed_by_a_chorus_or_by_a_single_performer_dedicated_to_living"/>
    </skos:Concept>

    <skos:Concept rdf:about="#Archaic_Lyric_Poem_in_ionic_or_in_doric_or_in_aeolic_dialect_performed_by_a_chorus_or_by_a_single_performer_dedicated_to_living">
        <skos:inScheme rdf:resource="http://www.ontologia.fr/OTB/ALyrA_v.1.0"/>
        <rdfs:label xml:lang="en">enkomion</rdfs:label>
        <skos:prefLabel xml:lang="en">enkomion</skos:prefLabel>
        <skos:definition xml:lang="en">Lyric song of praise for living people. Pindar, Bacchylides and Ibicus are important figures in enkomion composition.</skos:definition>
        <rdfs:label xml:lang="el">εγκώμιο</rdfs:label>
        <skos:prefLabel xml:lang="el">εγκώμιο</skos:prefLabel>
        <skos:definition xml:lang="el">Λυρικό τραγούδι επαίνου για ανθρώπους στη διάρκεια της ζωής τους. Ο Πίνδαρος, ο Βακχυλίδης και ο Ίβυκος είναι σημαντικές μορφές της σύνθεσης του εγκωμίου.</skos:definition>
        <skos:broader rdf:resource="#Archaic_Lyric_Poem_in_ionic_or_in_doric_or_in_aeolic_dialect_performed_by_a_chorus_or_by_a_single_performer"/>
        <skos:narrower rdf:resource="#Archaic_Lyric_Poem_in_ionic_or_in_doric_or_in_aeolic_dialect_performed_by_a_chorus_or_by_a_single_performer_dedicated_to_dead"/>
        <skos:narrower rdf:resource="#Archaic_Lyric_Poem_in_ionic_or_in_doric_or_in_aeolic_dialect_performed_by_a_chorus_or_by_a_single_performer_dedicated_to_wedding_couple"/>
        <skos:narrower rdf:resource="#Archaic_Lyric_Poem_in_ionic_or_in_doric_or_in_aeolic_dialect_performed_by_a_chorus_or_by_a_single_performer_dedicated_to_winners_in_athletic_events"/>
    </skos:Concept>

    <skos:Concept rdf:about="#Archaic_Lyric_Poem_in_ionic_or_in_doric_or_in_aeolic_dialect_performed_by_a_chorus_during_bride_procession">
        <skos:inScheme rdf:resource="http://www.ontologia.fr/OTB/ALyrA_v.1.0"/>
        <rdfs:label xml:lang="en">hymenaios</rdfs:label>
        <skos:prefLabel xml:lang="en">hymenaios</skos:prefLabel>
        <skos:definition xml:lang="en">A lyric song sung during the procession of the bride to the groom's house. Sappho is famous for her such songs.</skos:definition>
        <rdfs:label xml:lang="el">υμέναιος</rdfs:label>
        <skos:prefLabel xml:lang="el">υμέναιος</skos:prefLabel>
        <skos:definition xml:lang="el">Ένα λυρικό τραγούδι που εκτελείται κατά τη διάρκεια της πομπής της νύφης προς το σπίτι του γαμπρού. Η Σαπφώ είναι διάσημη για τους υμεναίους της.</skos:definition>
        <skos:broader rdf:resource="#Archaic_Lyric_Poem_in_ionic_or_in_doric_or_in_aeolic_dialect_performed_by_a_chorus_performed_by_a_non-specific_type_of_chorus"/>
    </skos:Concept>

    <skos:Concept rdf:about="#Archaic_Lyric_Poet">
        <skos:inScheme rdf:resource="http://www.ontologia.fr/OTB/ALyrA_v.1.0"/>
        <rdfs:label xml:lang="en">archaic lyric poet</rdfs:label>
        <skos:prefLabel xml:lang="en">archaic lyric poet</skos:prefLabel>
        <skos:definition xml:lang="en">An Archaic Lyric poet is a person (man) who lived during 7th-early 5th century BCE and wrote Archaic Lyric poetry.</skos:definition>
        <rdfs:label xml:lang="el">αρχαϊκός λυρικός ποιητής</rdfs:label>
        <skos:prefLabel xml:lang="el">αρχαϊκός λυρικός ποιητής</skos:prefLabel>
        <skos:definition xml:lang="el">Ο αρχαϊκός λυρικός ποιητής είναι ένα πρόσωπο που έζησε κατά τον 7ο-αρχές του 5ου αιώνα π.Χ. και έγραψε αρχαϊκή λυρική ποίηση.</skos:definition>
        <skos:broader rdf:resource="#Archaic_Lyric_Composer"/>
    </skos:Concept>

    <skos:Concept rdf:about="#Archaic_Lyric_Poem_only_in_ionic_dialect_in_elegiac_couplet_with_erotic_content">
        <skos:inScheme rdf:resource="http://www.ontologia.fr/OTB/ALyrA_v.1.0"/>
        <rdfs:label xml:lang="en">erotic elegy</rdfs:label>
        <skos:prefLabel xml:lang="en">erotic elegy</skos:prefLabel>
        <skos:definition xml:lang="en">Elegy with erotic content. Famous poet who composed erotic elegies is Mimnermus.</skos:definition>
        <rdfs:label xml:lang="el">ερωτική ελεγεία</rdfs:label>
        <skos:prefLabel xml:lang="el">ερωτική ελεγεία</skos:prefLabel>
        <skos:definition xml:lang="el">Ελεγεία με ερωτικό χαρακτήρα. Διάσημος ποιητής που συνέθεσε ερωτικές ελεγείες είναι ο Μίμνερμος.</skos:definition>
        <skos:broader rdf:resource="#Archaic_Lyric_Poem_only_in_ionic_dialect_in_elegiac_couplet"/>
    </skos:Concept>

	<!-- 
	//////////////////////////////////////////////////////////
	//
	// OWL
	//
	//////////////////////////////////////////////////////////
	-->

	<!--  OWL Ontology -->

    <owl:Ontology rdf:about="http://www.ontologia.fr/OTB/ALyrA_v.1.0">
        <dc:title>ALyrA_ontoterminology</dc:title>
        <dc:description>This is version 1.0 of the ALyrA ontoterminology (i.e., 'a terminology whose conceptual system is a formal ontology', Roche 2007 ), which focuses on modelling Archaic Lyric poets (799-430 BCΕ). AlyrA stands for "Archaic Lyrical Agora". 
The ontoterminology was created by Rafail Giannadakis (Department of Philology, University of Crete) under the supervision of Dr. Maria Papadopoulou (Department of Philology, University of Crete).
We gratefully acknowledge the generous funding of the European Commission in the context of the TALOS AI for SSH project (Grant agreement ID: 101087269).</dc:description>
        <dc:issued rdf:datatype="http://www.w3.org/2001/XMLSchema#date">2024-5-18</dc:issued>
        <dc:modified rdf:datatype="http://www.w3.org/2001/XMLSchema#date">2024-8-25</dc:modified>
        <dc:creator>Rafail Giannadakis</dc:creator>
        <dc:publisher>University of Crete - TALOS</dc:publisher>
    </owl:Ontology>

	<!--  OWL Object Properties -->

    <owl:ObjectProperty rdf:about="#residentedBy">
        <rdfs:label>residentedBy</rdfs:label>
        <rdfs:domain>
            <owl:Class>
                <owl:unionOf rdf:parseType="Collection">
                    <rdf:Description rdf:about="#Ancient_Location"/>
                </owl:unionOf>
            </owl:Class>
        </rdfs:domain>
        <rdfs:range>
            <owl:Class>
                <owl:unionOf rdf:parseType="Collection">
                    <rdf:Description rdf:about="#Archaic_Lyric_Composer"/>
                </owl:unionOf>
            </owl:Class>
        </rdfs:range>
    </owl:ObjectProperty>

    <owl:ObjectProperty rdf:about="#bornIn">
        <rdfs:label>bornIn</rdfs:label>
        <rdfs:domain>
            <owl:Class>
                <owl:unionOf rdf:parseType="Collection">
                    <rdf:Description rdf:about="#Archaic_Lyric_Composer"/>
                </owl:unionOf>
            </owl:Class>
        </rdfs:domain>
        <rdfs:range>
            <owl:Class>
                <owl:unionOf rdf:parseType="Collection">
                    <rdf:Description rdf:about="#Ancient_Location"/>
                </owl:unionOf>
            </owl:Class>
        </rdfs:range>
    </owl:ObjectProperty>

    <owl:ObjectProperty rdf:about="#isWrittenBy">
        <rdfs:label>isWrittenBy</rdfs:label>
        <rdfs:domain>
            <owl:Class>
                <owl:unionOf rdf:parseType="Collection">
                    <rdf:Description rdf:about="#Archaic_Lyric_Poem"/>
                </owl:unionOf>
            </owl:Class>
        </rdfs:domain>
        <rdfs:range>
            <owl:Class>
                <owl:unionOf rdf:parseType="Collection">
                    <rdf:Description rdf:about="#Archaic_Lyric_Composer"/>
                </owl:unionOf>
            </owl:Class>
        </rdfs:range>
    </owl:ObjectProperty>

    <owl:ObjectProperty rdf:about="#centuryOfLiving">
        <rdfs:label>centuryOfLiving</rdfs:label>
        <rdfs:domain>
            <owl:Class>
                <owl:unionOf rdf:parseType="Collection">
                    <rdf:Description rdf:about="#Archaic_Lyric_Composer"/>
                </owl:unionOf>
            </owl:Class>
        </rdfs:domain>
        <rdfs:range>
            <owl:Class>
                <owl:unionOf rdf:parseType="Collection">
                    <rdf:Description rdf:about="#BCE_century"/>
                </owl:unionOf>
            </owl:Class>
        </rdfs:range>
    </owl:ObjectProperty>

    <owl:ObjectProperty rdf:about="#stayedIn">
        <rdfs:label>stayedIn</rdfs:label>
        <rdfs:domain>
            <owl:Class>
                <owl:unionOf rdf:parseType="Collection">
                    <rdf:Description rdf:about="#Archaic_Lyric_Composer"/>
                </owl:unionOf>
            </owl:Class>
        </rdfs:domain>
        <rdfs:range>
            <owl:Class>
                <owl:unionOf rdf:parseType="Collection">
                    <rdf:Description rdf:about="#Ancient_Location"/>
                </owl:unionOf>
            </owl:Class>
        </rdfs:range>
    </owl:ObjectProperty>

    <owl:ObjectProperty rdf:about="#isCenturyOf">
        <rdfs:label>isCenturyOf</rdfs:label>
        <rdfs:domain>
            <owl:Class>
                <owl:unionOf rdf:parseType="Collection">
                    <rdf:Description rdf:about="#BCE_century"/>
                </owl:unionOf>
            </owl:Class>
        </rdfs:domain>
        <rdfs:range>
            <owl:Class>
                <owl:unionOf rdf:parseType="Collection">
                    <rdf:Description rdf:about="#Archaic_Lyric_Composer"/>
                </owl:unionOf>
            </owl:Class>
        </rdfs:range>
    </owl:ObjectProperty>

    <owl:ObjectProperty rdf:about="#hasWritten">
        <rdfs:label>hasWritten</rdfs:label>
        <rdfs:domain>
            <owl:Class>
                <owl:unionOf rdf:parseType="Collection">
                    <rdf:Description rdf:about="#Archaic_Lyric_Composer"/>
                </owl:unionOf>
            </owl:Class>
        </rdfs:domain>
        <rdfs:range>
            <owl:Class>
                <owl:unionOf rdf:parseType="Collection">
                    <rdf:Description rdf:about="#Archaic_Lyric_Poem"/>
                </owl:unionOf>
            </owl:Class>
        </rdfs:range>
    </owl:ObjectProperty>

    <owl:ObjectProperty rdf:about="#isBirthPlaceOf">
        <rdfs:label>isBirthPlaceOf</rdfs:label>
        <rdfs:domain>
            <owl:Class>
                <owl:unionOf rdf:parseType="Collection">
                    <rdf:Description rdf:about="#Ancient_Location"/>
                </owl:unionOf>
            </owl:Class>
        </rdfs:domain>
        <rdfs:range>
            <owl:Class>
                <owl:unionOf rdf:parseType="Collection">
                    <rdf:Description rdf:about="#Archaic_Lyric_Composer"/>
                </owl:unionOf>
            </owl:Class>
        </rdfs:range>
    </owl:ObjectProperty>

	<!--  OWL Data Properties -->

    <owl:DatatypeProperty rdf:about="#passageChosenEn">
        <rdfs:label>passageChosenEn</rdfs:label>
        <rdfs:domain>
            <owl:Class>
                <owl:unionOf rdf:parseType="Collection">
                    <rdf:Description rdf:about="#Archaic_Lyric_Composer"/>
                </owl:unionOf>
            </owl:Class>
        </rdfs:domain>
        <rdfs:range rdf:resource="http://www.w3.org/2001/XMLSchema#string"/>
    </owl:DatatypeProperty>

    <owl:DatatypeProperty rdf:about="#pleiadesCoordinates">
        <rdfs:label>pleiadesCoordinates</rdfs:label>
        <rdfs:domain>
            <owl:Class>
                <owl:unionOf rdf:parseType="Collection">
                    <rdf:Description rdf:about="#Ancient_Location"/>
                </owl:unionOf>
            </owl:Class>
        </rdfs:domain>
        <rdfs:range rdf:resource="http://www.w3.org/2000/01/rdf-schema#Literal"/>
    </owl:DatatypeProperty>

    <owl:DatatypeProperty rdf:about="#tlgIdentifyingNumber">
        <rdfs:label>tlgIdentifyingNumber</rdfs:label>
        <rdfs:domain>
            <owl:Class>
                <owl:unionOf rdf:parseType="Collection">
                    <rdf:Description rdf:about="#Archaic_Lyric_Composer"/>
                </owl:unionOf>
            </owl:Class>
        </rdfs:domain>
        <rdfs:range rdf:resource="http://www.w3.org/2000/01/rdf-schema#Literal"/>
    </owl:DatatypeProperty>

    <owl:DatatypeProperty rdf:about="#endsIn">
        <rdfs:label>endsIn</rdfs:label>
        <rdfs:domain>
            <owl:Class>
                <owl:unionOf rdf:parseType="Collection">
                    <rdf:Description rdf:about="#BCE_century"/>
                </owl:unionOf>
            </owl:Class>
        </rdfs:domain>
        <rdfs:range rdf:resource="http://www.w3.org/2001/XMLSchema#decimal"/>
    </owl:DatatypeProperty>

    <owl:DatatypeProperty rdf:about="#startsIn">
        <rdfs:label>startsIn</rdfs:label>
        <rdfs:domain>
            <owl:Class>
                <owl:unionOf rdf:parseType="Collection">
                    <rdf:Description rdf:about="#BCE_century"/>
                </owl:unionOf>
            </owl:Class>
        </rdfs:domain>
        <rdfs:range rdf:resource="http://www.w3.org/2001/XMLSchema#decimal"/>
    </owl:DatatypeProperty>

    <owl:DatatypeProperty rdf:about="#passageChoselEl">
        <rdfs:label>passageChoselEl</rdfs:label>
        <rdfs:domain>
            <owl:Class>
                <owl:unionOf rdf:parseType="Collection">
                    <rdf:Description rdf:about="#Archaic_Lyric_Composer"/>
                </owl:unionOf>
            </owl:Class>
        </rdfs:domain>
        <rdfs:range rdf:resource="http://www.w3.org/2001/XMLSchema#string"/>
    </owl:DatatypeProperty>

	<!--  OWL Classes -->

    <owl:Class rdf:about="#Archaic_Lyric_Composer">
        <rdfs:label xml:lang="en">archaic lyric composer</rdfs:label>
        <skos:prefLabel xml:lang="en">archaic lyric composer</skos:prefLabel>
        <skos:definition xml:lang="en">An Archaic Lyric composer is a person who lived during 7th-early 5th century BCE and wrote a lyric poem.</skos:definition>
        <rdfs:label xml:lang="el">αρχαϊκός λυρικός συνθέτης</rdfs:label>
        <skos:prefLabel xml:lang="el">αρχαϊκός λυρικός συνθέτης</skos:prefLabel>
        <skos:definition xml:lang="el">Ο αρχαϊκός λυρικός συνθέτης είναι ένα πρόσωπο που έζησε κατά τη διάρκεια του 7ου-αρχές του 5ου αιώνα π.Χ. και έγραψε λυρικό ποίημα.</skos:definition>
        <owl:disjointWith rdf:resource="#Ancient_Location"/>
        <owl:disjointWith rdf:resource="#Archaic_Lyric_Poem"/>
        <owl:disjointWith rdf:resource="#BCE_century"/>
        <rdfs:subClassOf>
            <owl:Restriction>
                <owl:onProperty rdf:resource="#ownDifference"/>
                <owl:hasValue rdf:resource="#archaic_lyric_composer"/>
            </owl:Restriction>
        </rdfs:subClassOf>
        <rdfs:subClassOf>
            <owl:Restriction>
                <owl:onProperty rdf:resource="#centuryOfLiving"/>
                <owl:someValuesFrom rdf:resource="#BCE_century"/>
            </owl:Restriction>
        </rdfs:subClassOf>
        <rdfs:subClassOf>
            <owl:Restriction>
                <owl:onProperty rdf:resource="#stayedIn"/>
                <owl:someValuesFrom rdf:resource="#Ancient_Location"/>
            </owl:Restriction>
        </rdfs:subClassOf>
        <rdfs:subClassOf>
            <owl:Restriction>
                <owl:onProperty rdf:resource="#bornIn"/>
                <owl:someValuesFrom rdf:resource="#Ancient_Location"/>
            </owl:Restriction>
        </rdfs:subClassOf>
        <rdfs:subClassOf>
            <owl:Restriction>
                <owl:onProperty rdf:resource="#hasWritten"/>
                <owl:someValuesFrom rdf:resource="#Archaic_Lyric_Poem"/>
            </owl:Restriction>
        </rdfs:subClassOf>
        <rdfs:subClassOf>
            <owl:Restriction>
                <owl:onProperty rdf:resource="#tlgIdentifyingNumber"/>
                <owl:someValuesFrom rdf:resource="http://www.w3.org/2000/01/rdf-schema#Literal"/>
            </owl:Restriction>
        </rdfs:subClassOf>
        <rdfs:subClassOf>
            <owl:Restriction>
                <owl:onProperty rdf:resource="#passageChosenEn"/>
                <owl:someValuesFrom rdf:resource="http://www.w3.org/2001/XMLSchema#string"/>
            </owl:Restriction>
        </rdfs:subClassOf>
        <rdfs:subClassOf>
            <owl:Restriction>
                <owl:onProperty rdf:resource="#passageChoselEl"/>
                <owl:someValuesFrom rdf:resource="http://www.w3.org/2001/XMLSchema#string"/>
            </owl:Restriction>
        </rdfs:subClassOf>
    </owl:Class>

    <owl:Class rdf:about="#Archaic_Lyric_Poem_only_in_ionic_dialect_in_elegiac_couplet">
        <rdfs:label xml:lang="en">elegy</rdfs:label>
        <skos:prefLabel xml:lang="en">elegy</skos:prefLabel>
        <skos:definition xml:lang="en">Elegies are poems written in elegiac couplets, with the first line in hexameter and the second line in pentameter, initially used for lamentation (but later had a wide range of themes) and possibly originating from Eastern mourning practices. They can be as short as a single couplet or longer sequences as needed.</skos:definition>
        <rdfs:label xml:lang="el">ελεγεία</rdfs:label>
        <skos:prefLabel xml:lang="el">ελεγεία</skos:prefLabel>
        <skos:definition xml:lang="el">Οι ελεγείες είναι ποιήματα γραμμένα σε ελεγειακά δίστιχα, με τον πρώτο στίχο σε εξάμετρο και τον δεύτερο σε πεντάμετρο. Αρχικά, χρησιμοποιήθηκαν για θρήνους (αλλά αργότερα είχαν ένα ευρύ φάσμα θεμάτων) και πιθανόν προέρχονται από τις ανατολίτικες θρηνητικές πρακτικές. Μπορεί να είναι μικρές σε έκταση (όσο ένα απλό κουπλέ) ή μεγαλύτερες.</skos:definition>
        <rdfs:subClassOf rdf:resource="#Archaic_Lyric_Poem_only_in_ionic_dialect"/>
        <owl:disjointWith rdf:resource="#Archaic_Lyric_Poem_only_in_ionic_dialect_in_iambic_or_trochaic_metre"/>
        <rdfs:subClassOf>
            <owl:Restriction>
                <owl:onProperty rdf:resource="#ownDifference"/>
                <owl:hasValue rdf:resource="#in_elegiac_couplet"/>
            </owl:Restriction>
        </rdfs:subClassOf>
    </owl:Class>

    <owl:Class rdf:about="#Archaic_Lyric_Poem">
        <rdfs:label xml:lang="en">archaic lyric poem</rdfs:label>
        <skos:prefLabel xml:lang="en">archaic lyric poem</skos:prefLabel>
        <skos:definition xml:lang="en">"Lyric poetry began as a fixture of ancient Greece, classified against other categories of poetry at the time of classical antiquity: dramas (written in verse) and epic poems. The lyric was far shorter, distinguished also by its focus on the poet’s state of mind and personal themes rather than narrative arc" (Academy of American Poets). So, an Archaic Lyric Poem is such poem written from 7th-early 5th century BCE.</skos:definition>
        <rdfs:label xml:lang="el">αρχαϊκό λυρικό ποίημα</rdfs:label>
        <skos:prefLabel xml:lang="el">αρχαϊκό λυρικό ποίημα</skos:prefLabel>
        <skos:definition xml:lang="el">"Η Λυρική ποίηση ξεκίνησε ως θεσμός της αρχαίας Ελλάδας, ταξινομημένος σε σχέση με άλλες κατηγορίες ποίησης κατά την εποχή της κλασικής αρχαιότητας: τα δραματικά (γραμμένα σε στίχους) και τα επικά ποιήματα. Η λυρική ποίηση ήταν πολύ πιο σύντομη, ενώ διακρινόταν επίσης από την εστίασή της στην ψυχική κατάσταση του ποιητή και σε προσωπικά θέματα και όχι στο αφηγηματικό τόξο" (Ακαδημία Αμερικανών Ποιητών). Έτσι, ένα αρχαϊκό λυρικό ποίημα είναι ένα τέτοιο ποίημα που γράφτηκε από τον 7ο-αρχές του 5ου αιώνα π.Χ.</skos:definition>
        <owl:disjointWith rdf:resource="#Ancient_Location"/>
        <owl:disjointWith rdf:resource="#Archaic_Lyric_Composer"/>
        <owl:disjointWith rdf:resource="#BCE_century"/>
        <rdfs:subClassOf>
            <owl:Restriction>
                <owl:onProperty rdf:resource="#ownDifference"/>
                <owl:hasValue rdf:resource="#archaic_lyric_poem"/>
            </owl:Restriction>
        </rdfs:subClassOf>
        <rdfs:subClassOf>
            <owl:Restriction>
                <owl:onProperty rdf:resource="#isWrittenBy"/>
                <owl:someValuesFrom rdf:resource="#Archaic_Lyric_Composer"/>
            </owl:Restriction>
        </rdfs:subClassOf>
    </owl:Class>

    <owl:Class rdf:about="#Archaic_Lyric_Poem_in_ionic_or_in_doric_or_in_aeolic_dialect_performed_by_a_chorus_or_by_a_single_performer_dedicated_to_apollo">
        <rdfs:label xml:lang="en">paean</rdfs:label>
        <skos:prefLabel xml:lang="en">paean</skos:prefLabel>
        <skos:definition xml:lang="en">Lyric song dedicated to Ancient Greek god Apollo. Alcman, Pindar and Bacchylides are famous composers of paeans.</skos:definition>
        <rdfs:label xml:lang="el">παιάνας</rdfs:label>
        <skos:prefLabel xml:lang="el">παιάνας</skos:prefLabel>
        <skos:definition xml:lang="el">Λυρικό τραγούδι αφιερωμένο στον αρχαίο Έλληνα θεό Απόλλωνα. Ο Αλκμάνας, ο Πίνδαρος και ο Βακχυλίδης είναι διάσημοι συνθέτες παιάνων.</skos:definition>
        <rdfs:subClassOf rdf:resource="#Archaic_Lyric_Poem_in_ionic_or_in_doric_or_in_aeolic_dialect_performed_by_a_chorus_or_by_a_single_performer_dedicated_to_a_god"/>
        <owl:disjointWith rdf:resource="#Archaic_Lyric_Poem_in_ionic_or_in_doric_or_in_aeolic_dialect_performed_by_a_chorus_or_by_a_single_performer_dedicated_to_dionysus"/>
        <rdfs:subClassOf>
            <owl:Restriction>
                <owl:onProperty rdf:resource="#ownDifference"/>
                <owl:hasValue rdf:resource="#dedicated_to_apollo"/>
            </owl:Restriction>
        </rdfs:subClassOf>
    </owl:Class>

    <owl:Class rdf:about="#Archaic_Lyric_Poem_only_in_ionic_dialect_in_elegiac_couplet_with_gnomic_content">
        <rdfs:label xml:lang="en">gnomic elegy</rdfs:label>
        <skos:prefLabel xml:lang="en">gnomic elegy</skos:prefLabel>
        <skos:definition xml:lang="en">Elegy with gnomic, counseling, biosophical content. Known poets of gnomic elegies are Phocylides and Theognis.</skos:definition>
        <rdfs:label xml:lang="el">γνωμική ελεγεία</rdfs:label>
        <skos:prefLabel xml:lang="el">γνωμική ελεγεία</skos:prefLabel>
        <skos:definition xml:lang="el">Ελεγεία με γνωμικό, συμβουλευτικό, βιοσοφικό περιεχόμενο. Γνωστοί ποιητές γνωστών γνωμικών ελεγειών είναι ο Φωκυλίδης και ο Θεογένης.</skos:definition>
        <rdfs:subClassOf rdf:resource="#Archaic_Lyric_Poem_only_in_ionic_dialect_in_elegiac_couplet"/>
        <owl:disjointWith rdf:resource="#Archaic_Lyric_Poem_only_in_ionic_dialect_in_elegiac_couplet_with_erotic_content"/>
        <owl:disjointWith rdf:resource="#Archaic_Lyric_Poem_only_in_ionic_dialect_in_elegiac_couplet_with_political_content"/>
        <owl:disjointWith rdf:resource="#Archaic_Lyric_Poem_only_in_ionic_dialect_in_elegiac_couplet_with_war_content"/>
        <rdfs:subClassOf>
            <owl:Restriction>
                <owl:onProperty rdf:resource="#ownDifference"/>
                <owl:hasValue rdf:resource="#with_specific_content"/>
            </owl:Restriction>
        </rdfs:subClassOf>
        <rdfs:subClassOf>
            <owl:Restriction>
                <owl:onProperty rdf:resource="#ownDifference"/>
                <owl:hasValue rdf:resource="#with_gnomic_content"/>
            </owl:Restriction>
        </rdfs:subClassOf>
    </owl:Class>

    <owl:Class rdf:about="#Archaic_Lyric_Poem_in_ionic_or_in_doric_or_in_aeolic_dialect_performed_by_a_chorus">
        <rdfs:label xml:lang="en">archaic lyric poem in ionic or in doric or in aeolic dialect performed by a chorus</rdfs:label>
        <skos:prefLabel xml:lang="en">archaic lyric poem in ionic or in doric or in aeolic dialect performed by a chorus</skos:prefLabel>
        <skos:definition xml:lang="en">Lyric song performed by a group (chorus) of people (women, men), which were dancing and singing.</skos:definition>
        <rdfs:label xml:lang="el">αρχαϊκό λυρικό ποίημα σε ιωνική ή δωρική ή αιολική διάλεκτο που εκτελείται από χορό</rdfs:label>
        <skos:prefLabel xml:lang="el">αρχαϊκό λυρικό ποίημα σε ιωνική ή δωρική ή αιολική διάλεκτο που εκτελείται από χορό</skos:prefLabel>
        <skos:definition xml:lang="el">Μέλος που εκτελείται από Χορό.</skos:definition>
        <rdfs:subClassOf rdf:resource="#Archaic_Lyric_Poem_in_ionic_or_in_doric_or_in_aeolic_dialect"/>
        <owl:disjointWith rdf:resource="#Archaic_Lyric_Poem_in_ionic_or_in_doric_or_in_aeolic_dialect_performed_by_a_chorus_or_by_a_single_performer"/>
        <owl:disjointWith rdf:resource="#Archaic_Lyric_Poem_in_ionic_or_in_doric_or_in_aeolic_dialect_performed_by_a_single_performer"/>
        <rdfs:subClassOf>
            <owl:Restriction>
                <owl:onProperty rdf:resource="#ownDifference"/>
                <owl:hasValue rdf:resource="#performed_by_a_chorus"/>
            </owl:Restriction>
        </rdfs:subClassOf>
    </owl:Class>

    <owl:Class rdf:about="#Archaic_Lyric_Poem_in_ionic_or_in_doric_or_in_aeolic_dialect_performed_by_a_chorus_on_the_way_to_an_altar">
        <rdfs:label xml:lang="en">prosodion</rdfs:label>
        <skos:prefLabel xml:lang="en">prosodion</skos:prefLabel>
        <skos:definition xml:lang="en">A lyric song performed on the way to an altar by a chorus. Alcman, Bacchylides and Pindar are famous prosodia composers.</skos:definition>
        <rdfs:label xml:lang="el">προσόδιο</rdfs:label>
        <skos:prefLabel xml:lang="el">προσόδιο</skos:prefLabel>
        <skos:definition xml:lang="el">Ένα λυρικό τραγούδι που ερμηνεύεται στο δρόμο προς το ιερό από μια χορωδία. Ο Αλκμάν, ο Βακχυλίδης και ο Πίνδαρος είναι διάσημοι συνθέτες προσοδίων.</skos:definition>
        <rdfs:subClassOf rdf:resource="#Archaic_Lyric_Poem_in_ionic_or_in_doric_or_in_aeolic_dialect_performed_by_a_chorus_performed_by_a_non-specific_type_of_chorus"/>
        <owl:disjointWith rdf:resource="#Archaic_Lyric_Poem_in_ionic_or_in_doric_or_in_aeolic_dialect_performed_by_a_chorus_during_bride_procession"/>
        <rdfs:subClassOf>
            <owl:Restriction>
                <owl:onProperty rdf:resource="#ownDifference"/>
                <owl:hasValue rdf:resource="#on_the_way_to_an_altar"/>
            </owl:Restriction>
        </rdfs:subClassOf>
    </owl:Class>

    <owl:Class rdf:about="#Archaic_Lyric_Poem_in_ionic_or_in_doric_or_in_aeolic_dialect_performed_by_a_single_performer">
        <rdfs:label xml:lang="en">monody</rdfs:label>
        <skos:prefLabel xml:lang="en">monody</skos:prefLabel>
        <skos:definition xml:lang="en">Monodies are characterized by solo performances, where the poet identifies with the singer and expresses personal thoughts and emotions, as they offer a direct and free expression of personality. For instance, in Sapphic odes, the poetess prioritizes her own voice over others.</skos:definition>
        <rdfs:label xml:lang="el">μονωδία</rdfs:label>
        <skos:prefLabel xml:lang="el">μονωδία</skos:prefLabel>
        <skos:definition xml:lang="el">Οι μονωδίες χαρακτηρίζονται από σόλο ερμηνείες, όπου ο ποιητής ταυτίζεται με τον τραγουδιστή και εκφράζει προσωπικές σκέψεις και συναισθήματα, καθώς προσφέρουν μια άμεση και ελεύθερη έκφραση της προσωπικότητας. Για παράδειγμα, στις σαπφικές ωδές, η ποιήτρια δίνει προτεραιότητα στη δική της φωνή έναντι των άλλων.</skos:definition>
        <rdfs:subClassOf rdf:resource="#Archaic_Lyric_Poem_in_ionic_or_in_doric_or_in_aeolic_dialect"/>
        <owl:disjointWith rdf:resource="#Archaic_Lyric_Poem_in_ionic_or_in_doric_or_in_aeolic_dialect_performed_by_a_chorus_or_by_a_single_performer"/>
        <owl:disjointWith rdf:resource="#Archaic_Lyric_Poem_in_ionic_or_in_doric_or_in_aeolic_dialect_performed_by_a_chorus"/>
        <rdfs:subClassOf>
            <owl:Restriction>
                <owl:onProperty rdf:resource="#ownDifference"/>
                <owl:hasValue rdf:resource="#performed_by_a_single_performer"/>
            </owl:Restriction>
        </rdfs:subClassOf>
    </owl:Class>

    <owl:Class rdf:about="#Archaic_Lyric_Poem_only_in_ionic_dialect">
        <rdfs:label xml:lang="en">archaic lyric poem only in ionic dialect</rdfs:label>
        <skos:prefLabel xml:lang="en">archaic lyric poem only in ionic dialect</skos:prefLabel>
        <skos:definition xml:lang="en">Archaic Lyric poem written only in ionic dialect. Ionic greek dialect, a subset of Eastern Greek, originated on the mainland and spread during the Dorian invasions. By the 5th century BC, it was primarily spoken in Ionia, including Asia Minor, Chios, and Samos. It also extended to Euboea and through Ionian colonization to the northern Aegean, Black Sea, and western Mediterranean.</skos:definition>
        <rdfs:label xml:lang="el">αρχαϊκό λυρικό ποίημα μόνο στην ιωνική διάλεκτο</rdfs:label>
        <skos:prefLabel xml:lang="el">αρχαϊκό λυρικό ποίημα μόνο στην ιωνική διάλεκτο</skos:prefLabel>
        <skos:definition xml:lang="el">Αρχαϊκό λυρικό ποίημα μόνο στην ιωνική διάλεκτο.</skos:definition>
        <rdfs:subClassOf rdf:resource="#Archaic_Lyric_Poem"/>
        <owl:disjointWith rdf:resource="#Archaic_Lyric_Poem_in_ionic_or_in_doric_or_in_aeolic_dialect"/>
        <rdfs:subClassOf>
            <owl:Restriction>
                <owl:onProperty rdf:resource="#ownDifference"/>
                <owl:hasValue rdf:resource="#only_in_ionic_dialect"/>
            </owl:Restriction>
        </rdfs:subClassOf>
    </owl:Class>

    <owl:Class rdf:about="#Ancient_Location">
        <rdfs:label xml:lang="en">ancient location</rdfs:label>
        <skos:prefLabel xml:lang="en">ancient location</skos:prefLabel>
        <skos:definition xml:lang="en">In the current ontoterminology Ancient Location objects concern the places where the Archaic Lyric Poets were born or lived, while they are inserted with coordinates from the pleiades gazetteer of ancient places (https:pleiades.stoa.orgplaces).</skos:definition>
        <rdfs:label xml:lang="el">αρχαία τοποθεσία</rdfs:label>
        <skos:prefLabel xml:lang="el">αρχαία τοποθεσία</skos:prefLabel>
        <skos:definition xml:lang="el">Στην παρούσα οντοορολογία γίνεται αναφορά στους τόπους όπου γεννήθηκαν ή έζησαν οι αρχαϊκοί λυρικοί ποιητές. Η ακριβής τους τοποθεσία εισάγεται με συντεταγμένες από το ευρετήριο αρχαίων τόπων pleiades (https:pleiades.stoa.orgplaces).</skos:definition>
        <owl:disjointWith rdf:resource="#Archaic_Lyric_Composer"/>
        <owl:disjointWith rdf:resource="#Archaic_Lyric_Poem"/>
        <owl:disjointWith rdf:resource="#BCE_century"/>
        <rdfs:subClassOf>
            <owl:Restriction>
                <owl:onProperty rdf:resource="#ownDifference"/>
                <owl:hasValue rdf:resource="#ancient_location"/>
            </owl:Restriction>
        </rdfs:subClassOf>
        <rdfs:subClassOf>
            <owl:Restriction>
                <owl:onProperty rdf:resource="#residentedBy"/>
                <owl:someValuesFrom rdf:resource="#Archaic_Lyric_Composer"/>
            </owl:Restriction>
        </rdfs:subClassOf>
        <rdfs:subClassOf>
            <owl:Restriction>
                <owl:onProperty rdf:resource="#isBirthPlaceOf"/>
                <owl:someValuesFrom rdf:resource="#Archaic_Lyric_Composer"/>
            </owl:Restriction>
        </rdfs:subClassOf>
        <rdfs:subClassOf>
            <owl:Restriction>
                <owl:onProperty rdf:resource="#pleiadesCoordinates"/>
                <owl:someValuesFrom rdf:resource="http://www.w3.org/2000/01/rdf-schema#Literal"/>
            </owl:Restriction>
        </rdfs:subClassOf>
    </owl:Class>

    <owl:Class rdf:about="#Archaic_Lyric_Poem_in_ionic_or_in_doric_or_in_aeolic_dialect_performed_by_a_chorus_or_by_a_single_performer_dedicated_to_dionysus">
        <rdfs:label xml:lang="en">dithyramb</rdfs:label>
        <skos:prefLabel xml:lang="en">dithyramb</skos:prefLabel>
        <skos:definition xml:lang="en">Devotional hymns of Dionysus. Bacchylides, Pindar and Simonides are known to have composed dithyrambs.</skos:definition>
        <rdfs:label xml:lang="el">διθύραμβος</rdfs:label>
        <skos:prefLabel xml:lang="el">διθύραμβος</skos:prefLabel>
        <skos:definition xml:lang="el">Λατρευτικοί ύμνοι του Διονύσου. Ο Βακχυλίδης, ο Πίνδαρος και ο Σιμωνίδης είναι γνωστό ότι συνέθεσαν διθύραμβους.</skos:definition>
        <rdfs:subClassOf rdf:resource="#Archaic_Lyric_Poem_in_ionic_or_in_doric_or_in_aeolic_dialect_performed_by_a_chorus_or_by_a_single_performer_dedicated_to_a_god"/>
        <owl:disjointWith rdf:resource="#Archaic_Lyric_Poem_in_ionic_or_in_doric_or_in_aeolic_dialect_performed_by_a_chorus_or_by_a_single_performer_dedicated_to_apollo"/>
        <rdfs:subClassOf>
            <owl:Restriction>
                <owl:onProperty rdf:resource="#ownDifference"/>
                <owl:hasValue rdf:resource="#dedicated_to_dionysus"/>
            </owl:Restriction>
        </rdfs:subClassOf>
    </owl:Class>

    <owl:Class rdf:about="#Archaic_Lyric_Poem_in_ionic_or_in_doric_or_in_aeolic_dialect_performed_by_a_chorus_or_by_a_single_performer_dedicated_to_a_god">
        <rdfs:label xml:lang="en">hymn</rdfs:label>
        <skos:prefLabel xml:lang="en">hymn</skos:prefLabel>
        <skos:definition xml:lang="en">Lyric song dedicated to gods. Multiple poets has composed hymns, sych as Alcaeus, Terpander, Sappho, Alcman et. al.</skos:definition>
        <rdfs:label xml:lang="el">ύμνος</rdfs:label>
        <skos:prefLabel xml:lang="el">ύμνος</skos:prefLabel>
        <skos:definition xml:lang="el">Λυρικό τραγούδι αφιερωμένο στους θεούς. Πολλοί ποιητές έχουν συνθέσει ύμνους, όπως ο Αλκαίος, ο Τέρπανδρος, η Σαπφώ, ο Αλκμάνας κ.ά.</skos:definition>
        <rdfs:subClassOf rdf:resource="#Archaic_Lyric_Poem_in_ionic_or_in_doric_or_in_aeolic_dialect_performed_by_a_chorus_or_by_a_single_performer"/>
        <owl:disjointWith rdf:resource="#Archaic_Lyric_Poem_in_ionic_or_in_doric_or_in_aeolic_dialect_performed_by_a_chorus_or_by_a_single_performer_dedicated_to_living"/>
        <rdfs:subClassOf>
            <owl:Restriction>
                <owl:onProperty rdf:resource="#ownDifference"/>
                <owl:hasValue rdf:resource="#dedicated_to_a_god"/>
            </owl:Restriction>
        </rdfs:subClassOf>
    </owl:Class>

    <owl:Class rdf:about="#Archaic_Lyric_Poem_only_in_ionic_dialect_in_iambic_or_trochaic_metre">
        <rdfs:label xml:lang="en">iamb</rdfs:label>
        <skos:prefLabel xml:lang="en">iamb</skos:prefLabel>
        <skos:definition xml:lang="en">Initially associated with Dionysus, the iamb may have a pre-Hellenic origin as a poetic form. Typically composed in iambic trimeter or trochaic tetrameter, its Ionic version often adopts a first-person perspective, though its context can vary.</skos:definition>
        <rdfs:label xml:lang="el">ίαμβος</rdfs:label>
        <skos:prefLabel xml:lang="el">ίαμβος</skos:prefLabel>
        <skos:definition xml:lang="el">Αρχικά συνδεόμενος με τον Διόνυσο, ο ίαμβος μπορεί να έχει προελληνική προέλευση ως ποιητική μορφή. Συνήθως συντίθεται σε ιαμβικό τρίμετρο ή τροχαϊκό τετράμετρο, η ιωνική εκδοχή του συχνά υιοθετεί την πρωτοπρόσωπη σκοπιά, αν και τα συμφραζόμενα μπορεί να ποικίλλουν.</skos:definition>
        <rdfs:subClassOf rdf:resource="#Archaic_Lyric_Poem_only_in_ionic_dialect"/>
        <owl:disjointWith rdf:resource="#Archaic_Lyric_Poem_only_in_ionic_dialect_in_elegiac_couplet"/>
        <rdfs:subClassOf>
            <owl:Restriction>
                <owl:onProperty rdf:resource="#ownDifference"/>
                <owl:hasValue rdf:resource="#in_iambic_or_trochaic_metre"/>
            </owl:Restriction>
        </rdfs:subClassOf>
    </owl:Class>

    <owl:Class rdf:about="#Archaic_Lyric_Poem_in_ionic_or_in_doric_or_in_aeolic_dialect_performed_by_a_chorus_or_by_a_single_performer">
        <rdfs:label xml:lang="en">archaic lyric poem in ionic or in doric or in aeolic dialect performed by a chorus or by a single performer</rdfs:label>
        <skos:prefLabel xml:lang="en">archaic lyric poem in ionic or in doric or in aeolic dialect performed by a chorus or by a single performer</skos:prefLabel>
        <skos:definition xml:lang="en">Melos which was performed either by one person or by a chorus.</skos:definition>
        <rdfs:label xml:lang="el">αρχαϊκό λυρικό ποίημα σε ιωνική ή δωρική ή αιολική διάλεκτο που εκτελείται από χορό ή από έναν μόνο ερμηνευτή</rdfs:label>
        <skos:prefLabel xml:lang="el">αρχαϊκό λυρικό ποίημα σε ιωνική ή δωρική ή αιολική διάλεκτο που εκτελείται από χορό ή από έναν μόνο ερμηνευτή</skos:prefLabel>
        <skos:definition xml:lang="el">Μέλος που εκτελείται από χορό ή από έναν μόνο ερμηνευτή.</skos:definition>
        <rdfs:subClassOf rdf:resource="#Archaic_Lyric_Poem_in_ionic_or_in_doric_or_in_aeolic_dialect"/>
        <owl:disjointWith rdf:resource="#Archaic_Lyric_Poem_in_ionic_or_in_doric_or_in_aeolic_dialect_performed_by_a_chorus"/>
        <owl:disjointWith rdf:resource="#Archaic_Lyric_Poem_in_ionic_or_in_doric_or_in_aeolic_dialect_performed_by_a_single_performer"/>
        <rdfs:subClassOf>
            <owl:Restriction>
                <owl:onProperty rdf:resource="#ownDifference"/>
                <owl:hasValue rdf:resource="#performed_by_a_chorus_or_by_a_single_performer"/>
            </owl:Restriction>
        </rdfs:subClassOf>
    </owl:Class>

    <owl:Class rdf:about="#Archaic_Lyric_Poem_in_ionic_or_in_doric_or_in_aeolic_dialect_performed_by_a_chorus_or_by_a_single_performer_dedicated_to_dead">
        <rdfs:label xml:lang="en">threnos</rdfs:label>
        <skos:prefLabel xml:lang="en">threnos</skos:prefLabel>
        <skos:definition xml:lang="en">Lyric song dedicated to a dead human being. Anacreon, Pindar and Simonides are famous for their such compositions.</skos:definition>
        <rdfs:label xml:lang="el">θρήνος</rdfs:label>
        <skos:prefLabel xml:lang="el">θρήνος</skos:prefLabel>
        <skos:definition xml:lang="el">Λυρικό τραγούδι αφιερωμένο σε έναν νεκρό άνθρωπο. Ο Ανακρέων, ο Πίνδαρος και ο Σιμωνίδης είναι διάσημοι για τέτοιες συνθέσεις τους.</skos:definition>
        <rdfs:subClassOf rdf:resource="#Archaic_Lyric_Poem_in_ionic_or_in_doric_or_in_aeolic_dialect_performed_by_a_chorus_or_by_a_single_performer_dedicated_to_living"/>
        <owl:disjointWith rdf:resource="#Archaic_Lyric_Poem_in_ionic_or_in_doric_or_in_aeolic_dialect_performed_by_a_chorus_or_by_a_single_performer_dedicated_to_wedding_couple"/>
        <owl:disjointWith rdf:resource="#Archaic_Lyric_Poem_in_ionic_or_in_doric_or_in_aeolic_dialect_performed_by_a_chorus_or_by_a_single_performer_dedicated_to_winners_in_athletic_events"/>
        <rdfs:subClassOf>
            <owl:Restriction>
                <owl:onProperty rdf:resource="#ownDifference"/>
                <owl:hasValue rdf:resource="#dedicated_to_a_dead_being"/>
            </owl:Restriction>
        </rdfs:subClassOf>
    </owl:Class>

    <owl:Class rdf:about="#Archaic_Lyric_Poem_in_ionic_or_in_doric_or_in_aeolic_dialect">
        <rdfs:label xml:lang="en">melos</rdfs:label>
        <skos:prefLabel xml:lang="en">melos</skos:prefLabel>
        <skos:definition xml:lang="en">Melos is the hypernym of the Archaic Lyric poems, which were written in ionic (except of the iamb and elegy), aeolic and doric dialect.</skos:definition>
        <rdfs:label xml:lang="el">μέλος</rdfs:label>
        <skos:prefLabel xml:lang="el">μέλος</skos:prefLabel>
        <skos:definition xml:lang="el">Το Μέλος είναι το υπερώνυμο των αρχαϊκών λυρικών ποιημάτων, τα οποία ήταν γραμμένα σε ιωνική (εκτός από τον ίαμβο και την ελεγεία), αιολική και δωρική διάλεκτο.</skos:definition>
        <rdfs:subClassOf rdf:resource="#Archaic_Lyric_Poem"/>
        <owl:disjointWith rdf:resource="#Archaic_Lyric_Poem_only_in_ionic_dialect"/>
        <rdfs:subClassOf>
            <owl:Restriction>
                <owl:onProperty rdf:resource="#ownDifference"/>
                <owl:hasValue rdf:resource="#in_ionic_or_in_doric_or_in_aeolic_dialect"/>
            </owl:Restriction>
        </rdfs:subClassOf>
    </owl:Class>

    <owl:Class rdf:about="#Archaic_Lyric_Poem_only_in_ionic_dialect_in_elegiac_couplet_with_war_content">
        <rdfs:label xml:lang="en">war elegy</rdfs:label>
        <skos:prefLabel xml:lang="en">war elegy</skos:prefLabel>
        <skos:definition xml:lang="en">Elegy with war content. Tyrtaeus and Callinus are famous poets of such elegy.</skos:definition>
        <rdfs:label xml:lang="el">πολεμική ελεγεία</rdfs:label>
        <skos:prefLabel xml:lang="el">πολεμική ελεγεία</skos:prefLabel>
        <skos:definition xml:lang="el">Ελεγεία με πολεμικό χαρακτήρα. Ο Τυρταίος και ο Καλλίνικος είναι διάσημοι ποιητές τέτοιων ελεγειών.</skos:definition>
        <rdfs:subClassOf rdf:resource="#Archaic_Lyric_Poem_only_in_ionic_dialect_in_elegiac_couplet"/>
        <owl:disjointWith rdf:resource="#Archaic_Lyric_Poem_only_in_ionic_dialect_in_elegiac_couplet_with_erotic_content"/>
        <owl:disjointWith rdf:resource="#Archaic_Lyric_Poem_only_in_ionic_dialect_in_elegiac_couplet_with_gnomic_content"/>
        <owl:disjointWith rdf:resource="#Archaic_Lyric_Poem_only_in_ionic_dialect_in_elegiac_couplet_with_political_content"/>
        <rdfs:subClassOf>
            <owl:Restriction>
                <owl:onProperty rdf:resource="#ownDifference"/>
                <owl:hasValue rdf:resource="#with_specific_content"/>
            </owl:Restriction>
        </rdfs:subClassOf>
        <rdfs:subClassOf>
            <owl:Restriction>
                <owl:onProperty rdf:resource="#ownDifference"/>
                <owl:hasValue rdf:resource="#with_war_content"/>
            </owl:Restriction>
        </rdfs:subClassOf>
    </owl:Class>

    <owl:Class rdf:about="#Archaic_Lyric_Poem_in_ionic_or_in_doric_or_in_aeolic_dialect_performed_by_a_chorus_with_imitation_expressions">
        <rdfs:label xml:lang="en">hyporcheme</rdfs:label>
        <skos:prefLabel xml:lang="en">hyporcheme</skos:prefLabel>
        <skos:definition xml:lang="en">A lyric song accompanied by imitative movements. Bacchylides and Pindar are famous for composing hyporchemes.</skos:definition>
        <rdfs:label xml:lang="el">υπόρχημα</rdfs:label>
        <skos:prefLabel xml:lang="el">υπόρχημα</skos:prefLabel>
        <skos:definition xml:lang="el">Ένα λυρικό τραγούδι που συνοδεύεται από μιμητικές κινήσεις. Ο Βακχυλίδης και ο Πίνδαρος φημίζονται για τη σύνθεση υπορχημάτων.</skos:definition>
        <rdfs:subClassOf rdf:resource="#Archaic_Lyric_Poem_in_ionic_or_in_doric_or_in_aeolic_dialect_performed_by_a_chorus_performed_by_a_non-specific_type_of_chorus"/>
        <rdfs:subClassOf>
            <owl:Restriction>
                <owl:onProperty rdf:resource="#ownDifference"/>
                <owl:hasValue rdf:resource="#with_specific_content"/>
            </owl:Restriction>
        </rdfs:subClassOf>
        <rdfs:subClassOf>
            <owl:Restriction>
                <owl:onProperty rdf:resource="#ownDifference"/>
                <owl:hasValue rdf:resource="#with_imitation_content"/>
            </owl:Restriction>
        </rdfs:subClassOf>
    </owl:Class>

    <owl:Class rdf:about="#Archaic_Lyric_Poem_in_ionic_or_in_doric_or_in_aeolic_dialect_performed_by_a_chorus_or_by_a_single_performer_dedicated_to_wedding_couple">
        <rdfs:label xml:lang="en">epithalamion</rdfs:label>
        <skos:prefLabel xml:lang="en">epithalamion</skos:prefLabel>
        <skos:definition xml:lang="en">Epithalamium is a song dedicated to a wedding couple sung at the nuptial residence. Sappho is famous for her such songs.</skos:definition>
        <rdfs:label xml:lang="el">επιθαλάμιο</rdfs:label>
        <skos:prefLabel xml:lang="el">επιθαλάμιο</skos:prefLabel>
        <skos:definition xml:lang="el">Το Επιθαλάμιο είναι ένα τραγούδι αφιερωμένο σε ένα γαμήλιο ζευγάρι που τραγουδιέται στη γαμήλια κατοικία. Η Σαπφώ είναι γνωστή για τα επιθαλάμιά της.</skos:definition>
        <rdfs:subClassOf rdf:resource="#Archaic_Lyric_Poem_in_ionic_or_in_doric_or_in_aeolic_dialect_performed_by_a_chorus_or_by_a_single_performer_dedicated_to_living"/>
        <owl:disjointWith rdf:resource="#Archaic_Lyric_Poem_in_ionic_or_in_doric_or_in_aeolic_dialect_performed_by_a_chorus_or_by_a_single_performer_dedicated_to_dead"/>
        <owl:disjointWith rdf:resource="#Archaic_Lyric_Poem_in_ionic_or_in_doric_or_in_aeolic_dialect_performed_by_a_chorus_or_by_a_single_performer_dedicated_to_winners_in_athletic_events"/>
        <rdfs:subClassOf>
            <owl:Restriction>
                <owl:onProperty rdf:resource="#ownDifference"/>
                <owl:hasValue rdf:resource="#dedicated_to_wedding_couple"/>
            </owl:Restriction>
        </rdfs:subClassOf>
    </owl:Class>

    <owl:Class rdf:about="#Archaic_Lyric_Poem_only_in_ionic_dialect_in_elegiac_couplet_with_political_content">
        <rdfs:label xml:lang="en">political elegy</rdfs:label>
        <skos:prefLabel xml:lang="en">political elegy</skos:prefLabel>
        <skos:definition xml:lang="en">Elegy with political content. Solon Atheniensis is a famous poet who composed such elegies.</skos:definition>
        <rdfs:label xml:lang="el">πολιτική ελεγεία</rdfs:label>
        <skos:prefLabel xml:lang="el">πολιτική ελεγεία</skos:prefLabel>
        <skos:definition xml:lang="el">Ελεγεία με πολιτικό χαρακτήρα. Ο Τυρταίος και ο Καλλίνικος είναι διάσημοι ποιητές τέτοιων ελεγειών.</skos:definition>
        <rdfs:subClassOf rdf:resource="#Archaic_Lyric_Poem_only_in_ionic_dialect_in_elegiac_couplet"/>
        <owl:disjointWith rdf:resource="#Archaic_Lyric_Poem_only_in_ionic_dialect_in_elegiac_couplet_with_erotic_content"/>
        <owl:disjointWith rdf:resource="#Archaic_Lyric_Poem_only_in_ionic_dialect_in_elegiac_couplet_with_gnomic_content"/>
        <owl:disjointWith rdf:resource="#Archaic_Lyric_Poem_only_in_ionic_dialect_in_elegiac_couplet_with_war_content"/>
        <rdfs:subClassOf>
            <owl:Restriction>
                <owl:onProperty rdf:resource="#ownDifference"/>
                <owl:hasValue rdf:resource="#with_specific_content"/>
            </owl:Restriction>
        </rdfs:subClassOf>
        <rdfs:subClassOf>
            <owl:Restriction>
                <owl:onProperty rdf:resource="#ownDifference"/>
                <owl:hasValue rdf:resource="#with_political_content"/>
            </owl:Restriction>
        </rdfs:subClassOf>
    </owl:Class>

    <owl:Class rdf:about="#Archaic_Lyric_Poem_in_ionic_or_in_doric_or_in_aeolic_dialect_performed_by_a_chorus_performed_by_a_non-specific_type_of_chorus">
        <rdfs:label xml:lang="en">archaic lyric poem in ionic or doric or aeolic dialect performed by a chorus of no particular type</rdfs:label>
        <skos:definition xml:lang="en">An Archaic Lyric poem in Ionic or Doric or Aeolic dialect performed by a chorus of no particular type.</skos:definition>
        <rdfs:label xml:lang="el">αρχαϊκό λυρικό ποίημα σε ιωνική ή δωρική ή αιολική διάλεκτο που εκτελείται από χορό μη συγκεκριμένου τύπου</rdfs:label>
        <skos:prefLabel xml:lang="el">αρχαϊκό λυρικό ποίημα σε ιωνική ή δωρική ή αιολική διάλεκτο που εκτελείται από χορό μη συγκεκριμένου τύπου</skos:prefLabel>
        <skos:definition xml:lang="el">Αρχαϊκό λυρικό ποίημα σε ιωνική ή δωρική ή αιολική διάλεκτο που εκτελείται από χορό μη συγκεκριμένου τύπου.</skos:definition>
        <rdfs:subClassOf rdf:resource="#Archaic_Lyric_Poem_in_ionic_or_in_doric_or_in_aeolic_dialect_performed_by_a_chorus"/>
        <owl:disjointWith rdf:resource="#Archaic_Lyric_Poem_in_ionic_or_in_doric_or_in_aeolic_dialect_performed_by_a_chorus_performed_by_a_maidens_chorus"/>
        <rdfs:subClassOf>
            <owl:Restriction>
                <owl:onProperty rdf:resource="#ownDifference"/>
                <owl:hasValue rdf:resource="#performed_by_a_non-specific_type_of_chorus"/>
            </owl:Restriction>
        </rdfs:subClassOf>
    </owl:Class>

    <owl:Class rdf:about="#BCE_century">
        <rdfs:label xml:lang="en">before common era century</rdfs:label>
        <skos:prefLabel xml:lang="en">before common era century</skos:prefLabel>
        <skos:definition xml:lang="en">Century that is BCE.</skos:definition>
        <rdfs:label xml:lang="el">προχριστιανικός αιώνας</rdfs:label>
        <skos:prefLabel xml:lang="el">προχριστιανικός αιώνας</skos:prefLabel>
        <skos:definition xml:lang="el"> Προχριστιανικός αιώνας.</skos:definition>
        <owl:disjointWith rdf:resource="#Ancient_Location"/>
        <owl:disjointWith rdf:resource="#Archaic_Lyric_Composer"/>
        <owl:disjointWith rdf:resource="#Archaic_Lyric_Poem"/>
        <rdfs:subClassOf>
            <owl:Restriction>
                <owl:onProperty rdf:resource="#ownDifference"/>
                <owl:hasValue rdf:resource="#before_common_era_century"/>
            </owl:Restriction>
        </rdfs:subClassOf>
        <rdfs:subClassOf>
            <owl:Restriction>
                <owl:onProperty rdf:resource="#isCenturyOf"/>
                <owl:someValuesFrom rdf:resource="#Archaic_Lyric_Composer"/>
            </owl:Restriction>
        </rdfs:subClassOf>
        <rdfs:subClassOf>
            <owl:Restriction>
                <owl:onProperty rdf:resource="#startsIn"/>
                <owl:someValuesFrom rdf:resource="http://www.w3.org/2001/XMLSchema#decimal"/>
            </owl:Restriction>
        </rdfs:subClassOf>
        <rdfs:subClassOf>
            <owl:Restriction>
                <owl:onProperty rdf:resource="#endsIn"/>
                <owl:someValuesFrom rdf:resource="http://www.w3.org/2001/XMLSchema#decimal"/>
            </owl:Restriction>
        </rdfs:subClassOf>
    </owl:Class>

    <owl:Class rdf:about="#Archaic_Lyric_Poetess">
        <rdfs:label xml:lang="en">archaic lyric poetess</rdfs:label>
        <skos:prefLabel xml:lang="en">archaic lyric poetess</skos:prefLabel>
        <skos:definition xml:lang="en">An Archaic Lyric poetess (woman) is a person who lived during 7th-early 5th century BCE and wrote Archaic Lyric poetry.</skos:definition>
        <rdfs:label xml:lang="el">αρχαϊκή λυρική ποιήτρια</rdfs:label>
        <skos:prefLabel xml:lang="el">αρχαϊκή λυρική ποιήτρια</skos:prefLabel>
        <skos:definition xml:lang="el">Η αρχαϊκή λυρική ποιήτρια είναι πρόσωπο που έζησε κατά τον 7ο-αρχές του 5ου αιώνα π.Χ. και έγραψε αρχαϊκή λυρική ποίηση.</skos:definition>
        <rdfs:subClassOf rdf:resource="#Archaic_Lyric_Composer"/>
        <owl:disjointWith rdf:resource="#Archaic_Lyric_Poet"/>
        <rdfs:subClassOf>
            <owl:Restriction>
                <owl:onProperty rdf:resource="#ownDifference"/>
                <owl:hasValue rdf:resource="#female"/>
            </owl:Restriction>
        </rdfs:subClassOf>
    </owl:Class>

    <owl:Class rdf:about="#Archaic_Lyric_Poem_in_ionic_or_in_doric_or_in_aeolic_dialect_performed_by_a_chorus_performed_by_a_maidens_chorus">
        <rdfs:label xml:lang="en">partheneion</rdfs:label>
        <skos:prefLabel xml:lang="en">partheneion</skos:prefLabel>
        <skos:definition xml:lang="en">A lyric song performed by a maidens chorus. Alcman, Pindar and Bacchylides are famous for composing Partheneia.</skos:definition>
        <rdfs:label xml:lang="el">παρθένειο</rdfs:label>
        <skos:prefLabel xml:lang="el">παρθένειο</skos:prefLabel>
        <skos:definition xml:lang="el">Ένα λυρικό τραγούδι που ερμηνεύεται από μια χορωδία νεανίδων. Ο Αλκμάνας, ο Πίνδαρος και ο Βακχυλίδης φημίζονται για τη σύνθεση των Παρθενείων.</skos:definition>
        <rdfs:subClassOf rdf:resource="#Archaic_Lyric_Poem_in_ionic_or_in_doric_or_in_aeolic_dialect_performed_by_a_chorus"/>
        <owl:disjointWith rdf:resource="#Archaic_Lyric_Poem_in_ionic_or_in_doric_or_in_aeolic_dialect_performed_by_a_chorus_performed_by_a_non-specific_type_of_chorus"/>
        <rdfs:subClassOf>
            <owl:Restriction>
                <owl:onProperty rdf:resource="#ownDifference"/>
                <owl:hasValue rdf:resource="#performed_by_a_maidens_chorus"/>
            </owl:Restriction>
        </rdfs:subClassOf>
    </owl:Class>

    <owl:Class rdf:about="#Archaic_Lyric_Poem_in_ionic_or_in_doric_or_in_aeolic_dialect_performed_by_a_chorus_or_by_a_single_performer_dedicated_to_winners_in_athletic_events">
        <rdfs:label xml:lang="en">epinikion</rdfs:label>
        <skos:prefLabel xml:lang="en">epinikion</skos:prefLabel>
        <skos:definition xml:lang="en">Lyric song of praise winners of sports games. Pindar, Bacchylides and Ibicus are who composed epinikia.</skos:definition>
        <rdfs:label xml:lang="el">επίνικος</rdfs:label>
        <skos:prefLabel xml:lang="el">επίνικος</skos:prefLabel>
        <skos:definition xml:lang="el">Λυρικό τραγούδι αφιερωμένο σε νικητή αθλητικών αγώνων. Ο Πίνδαρος, ο Βακχυλίδης και ο Ίβυκος είναι αυτοί που συνέθεσαν επινίκια τραγούδια.</skos:definition>
        <rdfs:subClassOf rdf:resource="#Archaic_Lyric_Poem_in_ionic_or_in_doric_or_in_aeolic_dialect_performed_by_a_chorus_or_by_a_single_performer_dedicated_to_living"/>
        <owl:disjointWith rdf:resource="#Archaic_Lyric_Poem_in_ionic_or_in_doric_or_in_aeolic_dialect_performed_by_a_chorus_or_by_a_single_performer_dedicated_to_dead"/>
        <owl:disjointWith rdf:resource="#Archaic_Lyric_Poem_in_ionic_or_in_doric_or_in_aeolic_dialect_performed_by_a_chorus_or_by_a_single_performer_dedicated_to_wedding_couple"/>
        <rdfs:subClassOf>
            <owl:Restriction>
                <owl:onProperty rdf:resource="#ownDifference"/>
                <owl:hasValue rdf:resource="#dedicated_to_winners_in_athletic_events"/>
            </owl:Restriction>
        </rdfs:subClassOf>
    </owl:Class>

    <owl:Class rdf:about="#Archaic_Lyric_Poem_in_ionic_or_in_doric_or_in_aeolic_dialect_performed_by_a_chorus_or_by_a_single_performer_dedicated_to_living">
        <rdfs:label xml:lang="en">enkomion</rdfs:label>
        <skos:prefLabel xml:lang="en">enkomion</skos:prefLabel>
        <skos:definition xml:lang="en">Lyric song of praise for living people. Pindar, Bacchylides and Ibicus are important figures in enkomion composition.</skos:definition>
        <rdfs:label xml:lang="el">εγκώμιο</rdfs:label>
        <skos:prefLabel xml:lang="el">εγκώμιο</skos:prefLabel>
        <skos:definition xml:lang="el">Λυρικό τραγούδι επαίνου για ανθρώπους στη διάρκεια της ζωής τους. Ο Πίνδαρος, ο Βακχυλίδης και ο Ίβυκος είναι σημαντικές μορφές της σύνθεσης του εγκωμίου.</skos:definition>
        <rdfs:subClassOf rdf:resource="#Archaic_Lyric_Poem_in_ionic_or_in_doric_or_in_aeolic_dialect_performed_by_a_chorus_or_by_a_single_performer"/>
        <owl:disjointWith rdf:resource="#Archaic_Lyric_Poem_in_ionic_or_in_doric_or_in_aeolic_dialect_performed_by_a_chorus_or_by_a_single_performer_dedicated_to_a_god"/>
        <rdfs:subClassOf>
            <owl:Restriction>
                <owl:onProperty rdf:resource="#ownDifference"/>
                <owl:hasValue rdf:resource="#dedicated_to_mortal"/>
            </owl:Restriction>
        </rdfs:subClassOf>
    </owl:Class>

    <owl:Class rdf:about="#Archaic_Lyric_Poem_in_ionic_or_in_doric_or_in_aeolic_dialect_performed_by_a_chorus_during_bride_procession">
        <rdfs:label xml:lang="en">hymenaios</rdfs:label>
        <skos:prefLabel xml:lang="en">hymenaios</skos:prefLabel>
        <skos:definition xml:lang="en">A lyric song sung during the procession of the bride to the groom's house. Sappho is famous for her such songs.</skos:definition>
        <rdfs:label xml:lang="el">υμέναιος</rdfs:label>
        <skos:prefLabel xml:lang="el">υμέναιος</skos:prefLabel>
        <skos:definition xml:lang="el">Ένα λυρικό τραγούδι που εκτελείται κατά τη διάρκεια της πομπής της νύφης προς το σπίτι του γαμπρού. Η Σαπφώ είναι διάσημη για τους υμεναίους της.</skos:definition>
        <rdfs:subClassOf rdf:resource="#Archaic_Lyric_Poem_in_ionic_or_in_doric_or_in_aeolic_dialect_performed_by_a_chorus_performed_by_a_non-specific_type_of_chorus"/>
        <owl:disjointWith rdf:resource="#Archaic_Lyric_Poem_in_ionic_or_in_doric_or_in_aeolic_dialect_performed_by_a_chorus_on_the_way_to_an_altar"/>
        <rdfs:subClassOf>
            <owl:Restriction>
                <owl:onProperty rdf:resource="#ownDifference"/>
                <owl:hasValue rdf:resource="#during_bride_procession"/>
            </owl:Restriction>
        </rdfs:subClassOf>
    </owl:Class>

    <owl:Class rdf:about="#Archaic_Lyric_Poet">
        <rdfs:label xml:lang="en">archaic lyric poet</rdfs:label>
        <skos:prefLabel xml:lang="en">archaic lyric poet</skos:prefLabel>
        <skos:definition xml:lang="en">An Archaic Lyric poet is a person (man) who lived during 7th-early 5th century BCE and wrote Archaic Lyric poetry.</skos:definition>
        <rdfs:label xml:lang="el">αρχαϊκός λυρικός ποιητής</rdfs:label>
        <skos:prefLabel xml:lang="el">αρχαϊκός λυρικός ποιητής</skos:prefLabel>
        <skos:definition xml:lang="el">Ο αρχαϊκός λυρικός ποιητής είναι ένα πρόσωπο που έζησε κατά τον 7ο-αρχές του 5ου αιώνα π.Χ. και έγραψε αρχαϊκή λυρική ποίηση.</skos:definition>
        <rdfs:subClassOf rdf:resource="#Archaic_Lyric_Composer"/>
        <owl:disjointWith rdf:resource="#Archaic_Lyric_Poetess"/>
        <rdfs:subClassOf>
            <owl:Restriction>
                <owl:onProperty rdf:resource="#ownDifference"/>
                <owl:hasValue rdf:resource="#male"/>
            </owl:Restriction>
        </rdfs:subClassOf>
    </owl:Class>

    <owl:Class rdf:about="#Archaic_Lyric_Poem_only_in_ionic_dialect_in_elegiac_couplet_with_erotic_content">
        <rdfs:label xml:lang="en">erotic elegy</rdfs:label>
        <skos:prefLabel xml:lang="en">erotic elegy</skos:prefLabel>
        <skos:definition xml:lang="en">Elegy with erotic content. Famous poet who composed erotic elegies is Mimnermus.</skos:definition>
        <rdfs:label xml:lang="el">ερωτική ελεγεία</rdfs:label>
        <skos:prefLabel xml:lang="el">ερωτική ελεγεία</skos:prefLabel>
        <skos:definition xml:lang="el">Ελεγεία με ερωτικό χαρακτήρα. Διάσημος ποιητής που συνέθεσε ερωτικές ελεγείες είναι ο Μίμνερμος.</skos:definition>
        <rdfs:subClassOf rdf:resource="#Archaic_Lyric_Poem_only_in_ionic_dialect_in_elegiac_couplet"/>
        <owl:disjointWith rdf:resource="#Archaic_Lyric_Poem_only_in_ionic_dialect_in_elegiac_couplet_with_gnomic_content"/>
        <owl:disjointWith rdf:resource="#Archaic_Lyric_Poem_only_in_ionic_dialect_in_elegiac_couplet_with_political_content"/>
        <owl:disjointWith rdf:resource="#Archaic_Lyric_Poem_only_in_ionic_dialect_in_elegiac_couplet_with_war_content"/>
        <rdfs:subClassOf>
            <owl:Restriction>
                <owl:onProperty rdf:resource="#ownDifference"/>
                <owl:hasValue rdf:resource="#with_specific_content"/>
            </owl:Restriction>
        </rdfs:subClassOf>
        <rdfs:subClassOf>
            <owl:Restriction>
                <owl:onProperty rdf:resource="#ownDifference"/>
                <owl:hasValue rdf:resource="#with_erotic_content"/>
            </owl:Restriction>
        </rdfs:subClassOf>
    </owl:Class>

	<!--  OWL Individuals -->

    <owl:NamedIndividual rdf:about="#elegies_simonides">
        <rdfs:label xml:lang="en">elegies_simonides</rdfs:label>
        <skos:prefLabel xml:lang="en">elegies_simonides</skos:prefLabel>
        <rdf:type rdf:resource="#Archaic_Lyric_Poem_only_in_ionic_dialect_in_elegiac_couplet"/>
        <isWrittenBy rdf:resource="#simonides_ceus"/>    </owl:NamedIndividual>

    <owl:NamedIndividual rdf:about="#erotic_odes_alcman">
        <rdfs:label xml:lang="en">erotic_odes_alcman</rdfs:label>
        <skos:prefLabel xml:lang="en">erotic_odes_alcman</skos:prefLabel>
        <rdf:type rdf:resource="#Archaic_Lyric_Poem_in_ionic_or_in_doric_or_in_aeolic_dialect_performed_by_a_single_performer"/>
        <isWrittenBy rdf:resource="#alcman_lacedaemonius"/>    </owl:NamedIndividual>

    <owl:NamedIndividual rdf:about="#threnoi_anacreon">
        <rdfs:label xml:lang="en">threnoi_anacreon</rdfs:label>
        <skos:prefLabel xml:lang="en">threnoi_anacreon</skos:prefLabel>
        <rdf:type rdf:resource="#Archaic_Lyric_Poem_in_ionic_or_in_doric_or_in_aeolic_dialect_performed_by_a_chorus_or_by_a_single_performer_dedicated_to_dead"/>
        <isWrittenBy rdf:resource="#anacreon_teius"/>    </owl:NamedIndividual>

    <owl:NamedIndividual rdf:about="#partheneia_pindarus">
        <rdfs:label xml:lang="en">partheneia_pindarus</rdfs:label>
        <skos:prefLabel xml:lang="en">partheneia_pindarus</skos:prefLabel>
        <rdf:type rdf:resource="#Archaic_Lyric_Poem_in_ionic_or_in_doric_or_in_aeolic_dialect_performed_by_a_chorus_performed_by_a_maidens_chorus"/>
        <isWrittenBy rdf:resource="#pindarus_boeotus"/>    </owl:NamedIndividual>

    <owl:NamedIndividual rdf:about="#war_elegies_tyrtaeus">
        <rdfs:label xml:lang="en">war_elegies_tyrtaeus</rdfs:label>
        <skos:prefLabel xml:lang="en">war_elegies_tyrtaeus</skos:prefLabel>
        <rdf:type rdf:resource="#Archaic_Lyric_Poem_only_in_ionic_dialect_in_elegiac_couplet_with_war_content"/>
        <isWrittenBy rdf:resource="#tyrtaeus_lacedaemonius"/>    </owl:NamedIndividual>

    <owl:NamedIndividual rdf:about="#callinus_ephesius">
        <rdfs:label xml:lang="en">callinus_ephesius</rdfs:label>
        <skos:prefLabel xml:lang="en">callinus_ephesius</skos:prefLabel>
        <rdf:type rdf:resource="#Archaic_Lyric_Poet"/>
        <passageChosenEn rdf:datatype="http://www.w3.org/2001/XMLSchema#string">The_Elegiac_Poems_of_Callinus,_CURFRAG.tlg-0243.1,_translated_by_Edmonts:_How_long_will_ye_lie_idle?_When,_young_men,_will_ye_show_a_stout_heart?_Have_ye_no_shame_of_your_sloth_before_them_that_dwell_round_about_you?_Purpose_ye_to_sit_in_peace_though_the_land_is_full_of_war?_..._and_let_every_man_cast_his_javelin_once_more_as_he_dies._For_''tis_an_honourable_thing_and_a_glorious_to_a_man_to_fight_the_foe_for_land_and_children_and_wedded_wife;_and_death_shall_befall_only_when_the_Fates_ordain_it._Nay,_so_soon_as_war_is_mingled_let_each_go_forward_spear_in_poise_and_shield_before_stout_heart;_for_by_no_means_may_a_man_escape_death,_nay_not_if_he_come_of_immortal_lineage._Oftentime,_it_may_be,_he_returneth_safe_from_the_conflict_of_battle_and_the_thud_of_spears,_and_the_doom_of_death_cometh_upon_him_at_home;_yet_such_is_not_dear_to_the_people_nor_regretted,_whereas_if_aught_happen_to_the_other_sort_he_is_bewailed_of_small_and_great._When_a_brave_man_dieth_the_whole_people_regretteth_him,_and_while_he_lives_he_is_as_good_as_a_demigod;_for_in_their_eyes_he_is_a_tower,_seeing_that_he_doeth_single-handed_as_good_work_as_many_together._(Edmonds,_J._M._(1931)._The_Elegiac_Poems_of_Callinus_in_Elegy_and_Iambus_[English_Translation]._Cambridge,_MA:_Harvard_University_Press._London:_William_Heinemann_Ltd._(Original_work_published_1931)._Retrieved_May_4,_2024,_from_https:www.perseus.tufts.eduhoppertext?doc=Perseus%3Atext%3A2008.01.0479%3Avolume%3D1%3Atext%3D1%3Asection%3D2#note1:~:text=as%20many%20together.-,CURFRAG.tlg%2D0243.1,-%E2%80%9D%20Stobaeus%20Anthology)</passageChosenEn>
        <tlgIdentifyingNumber>tlg0243</tlgIdentifyingNumber>
        <passageChoselEl rdf:datatype="http://www.w3.org/2001/XMLSchema#string">Καλλίνος,_απ._1_West,_μετ._Σ._Μενάνδρου:_Ως_πότε_πια_κατάκοιτοι;_ορμήν_πότε_θα_βρείτε;_|_δεν_ντρέπεσθε_τους_γείτονες_για_την_οκνιάν_αυτή;_|_Ε!_παλικάρια,_ειρηνικά_πως_κάθεστε_θαρρείτε_|_και_ωστόσο_γύρω_ο_πόλεμος_όλη_την_γη_κρατεί…_|_................._|_Είναι_τιμή_κι_είναι_χαρά_στο_παλικάρι_η_μάχη_|_για_την_πατρίδα,_την_καλή_γυναίκα,_τα_παιδιά._|_Ο_θάνατος_τότε_θα_᾽ρθει,_όταν_η_Μοίρα_λάχει·_|_μόνο_καθείς_ας_ορθωθεί_μ᾽_ατρόμητη_καρδιά,_|_και_ας_δράξει_αμέσως_το_σπαθί_κι_ας_ζώσει_τ᾽_άρματά_του_|_και_όσό_᾽ναι_του_πολέμου_αρχή,_ας_δράμει_εκεί_μπροστά,_|_γιατί_να_φύγει_αδύνατο_την_μοίρα_του_θανάτου,_|_και_αν_η_γενιά_του_από_θεούς_αθάνατου_ς_βαστά·_|_κάποτ᾽_αν_απ᾽_τον_πόλεμο_δειλά_λιποτακτήσει,_|_μέσα_στο_σπίτι_βρίσκει_τον_η_ώρα_του_η_στερνή._|_Μα_τούτον_ποιος_τον_αγαπά_και_ποιος_θα_τον_ποθήσει;_|_ενώ_τον_άλλο_ένας_λαός,_αν_πάθει,_τον_πονεί._|_Γιατί_ο_λαός_ολάκερος_θρηνεί_το_παλικάρι,_|_σαν_αποθάνει·_κι_έχουν_τον_ημίθεο_όσο_ζει_|_σαν_πύργ᾽_όλοι_κατάματα_θωρούν_τον_με_καμάρι_|_γιατί_μονάχος_κάμνει_αυτός_όσα_πολλοί_μαζί!_(Τσέλικας,_Σ._(επ.)._ΚΑΛΛΙΝΟΣ:_απ._1_West._Ανθολογία_Αρχαϊκής_Λυρικής_Ποίησης._Ανακτήθηκε_4_Μαΐου_2024,_από_https:www.greek-language.grdigitalResourcesancient_greekanthologypoetrybrowse.html?text_id=48)</passageChoselEl>
        <hasWritten rdf:resource="#war_elegy_callinus"/>        <centuryOfLiving rdf:resource="#7th_century_BCE"/>        <bornIn rdf:resource="#ephesus"/>        <rdfs:seeAlso rdf:resource="https://www.britannica.com/biography/Callinus"/>
        <rdfs:seeAlso rdf:resource="https://www.perseus.tufts.edu/hopper/text?doc=Perseus%3Atext%3A2008.01.0479%3Avolume%3D1%3Atext%3D1%3Asection%3D2"/>
        <rdfs:seeAlso rdf:resource="https://topostext.org/people/2039"/>
        <rdfs:seeAlso rdf:resource="https://www.perseus.tufts.edu/hopper/text?doc=Perseus%3Atext%3A2008.01.0479%3Avolume%3D1%3Atext%3D1"/>
        <rdfs:seeAlso rdf:resource="https://catalog.perseus.org/catalog/urn:cite:perseus:author.310"/>
        <rdfs:seeAlso rdf:resource="https://catalog.perseus.org/catalog/urn:cts:greekLit:tlg0243.tlg001"/>
    </owl:NamedIndividual>

    <owl:NamedIndividual rdf:about="#archilochus_parius">
        <rdfs:label xml:lang="en">archilochus_parius</rdfs:label>
        <skos:prefLabel xml:lang="en">archilochus_parius</skos:prefLabel>
        <rdf:type rdf:resource="#Archaic_Lyric_Poet"/>
        <skos:note>By shakko - Own work, CC BY-SA 3.0, Bust of a bearded man (Archilochus?). Roman copy (c. 2nd century BC) of Greek original (4th century BC)https:commons.wikimedia.orgwindex.php?curid=7408002</skos:note>
        <passageChosenEn rdf:datatype="http://www.w3.org/2001/XMLSchema#string">Elegiac_Poems_(Archilochus),_CURFRAG.tlg-0232.6,_translated_by_Edmonts:_the_shield_I_left_because_I_must,_poor_blameless_armament!_beside_a_bush,_gives_joy_now_to_some_Saian,_but_myself_I_have_saved._What_care_I_for_that_shield?_It_shall_go_with_a_curse._I''ll_get_me_another_e''en_as_good._(Edmonds,_J._M._(1931)._Archilochus_in_Elegy_and_Iambus_[English_Translation]._Cambridge,_MA:_Harvard_University_Press._London:_William_Heinemann_Ltd._(Original_work_published_1931)._Retrieved_May_4,_2024,_from_https:www.perseus.tufts.eduhoppertext?doc=Perseus:text:2008.01.0480:volume=2:text=21:section=2&amp;highlight=shield#:~:text=e%27en%20as%20good.-,CURFRAG.tlg%2D0232.6,-%E2%80%9D%20Plutarch%20Spartan)</passageChosenEn>
        <tlgIdentifyingNumber>tlg0232</tlgIdentifyingNumber>
        <passageChoselEl rdf:datatype="http://www.w3.org/2001/XMLSchema#string">Αρχίλοχος,_απ._5_West,_μετ._Θ._Κ._Στεφανόπουλος:_Με_την_ασπίδα_μου_κάποιος_Σάιος,_το_ξέρω,_αγάλλεται._|_Ήταν_όπλο_αψεγάδιαστο,_κι_εγώ_την_εγκατέλειψα_πλάι_στο_θάμνο,_|_όμως_δεν_το_᾽θελα·_έσωσα_τη_ζωή_μου._|_Τι_με_νοιάζει_πια_η_ασπίδα_εκείνη;_Ώρα_καλή·_|_θα_ξαναβρώ_άλλη,_όχι_κατώτερη._(Στεφανόπουλου,_Θ._Κ.,_Τσιτσιρίδη,_Στ.,_Αντζουλή,_Λ.,_&amp;_Κριτσέλη,_Γ._(χ.χ.)._ΑΡΧΙΛΟΧΟΣ:_25._–_Απόσπασμα_5_West._Ανθολογία_Αρχαίας_Ελληνικής_Γραμματείας._Ανακτήθηκε_4_Μαΐου_2024,_από_https:www.greek-language.grdigitalResourcesancient_greekanthologyliteraturebrowse.html?text_id=50)</passageChoselEl>
        <hasWritten rdf:resource="#elegies_archilochus"/>        <hasWritten rdf:resource="#iambs_archilochus"/>        <hasWritten rdf:resource="#hymns_archilochus"/>        <centuryOfLiving rdf:resource="#7th_century_BCE"/>        <bornIn rdf:resource="#paros"/>        <stayedIn rdf:resource="#thasos_settlement"/>        <foaf:depiction rdf:resource="https://upload.wikimedia.org/wikipedia/commons/thumb/e/eb/Archilochus_01_pushkin.jpg/800px-Archilochus_01_pushkin.jpg"/>
        <rdfs:seeAlso rdf:resource="https://catalog.perseus.org/catalog/urn:cite:perseus:author.175"/>
        <rdfs:seeAlso rdf:resource="https://en.wikipedia.org/wiki/Archilochus"/>
        <rdfs:seeAlso rdf:resource="https://www.britannica.com/biography/Archilochus-Greek-author"/>
        <rdfs:seeAlso rdf:resource="https://www.perseus.tufts.edu/hopper/text?doc=Perseus%3Atext%3A2008.01.0480%3Avolume%3D2%3Atext%3D21"/>
        <rdfs:seeAlso rdf:resource="https://el.wikipedia.org/wiki/%CE%91%CF%81%CF%87%CE%AF%CE%BB%CE%BF%CF%87%CE%BF%CF%82"/>
        <rdfs:seeAlso rdf:resource="https://www.wikidata.org/wiki/Q201323"/>
        <rdfs:seeAlso rdf:resource="https://en.wikiquote.org/wiki/Archilochus"/>
    </owl:NamedIndividual>

    <owl:NamedIndividual rdf:about="#sappho_lesbia">
        <rdfs:label xml:lang="en">sappho_lesbia</rdfs:label>
        <skos:prefLabel xml:lang="en">sappho_lesbia</skos:prefLabel>
        <rdf:type rdf:resource="#Archaic_Lyric_Poetess"/>
        <skos:note>By Charles Mengin - Sappho (1877) by Charles Mengin (1853–1933). One tradition claims that Sappho committed suicide by jumping off the Leucadian cliff., Public Domain, https:commons.wikimedia.orgwindex.php?curid=1753564</skos:note>
        <passageChosenEn rdf:datatype="http://www.w3.org/2001/XMLSchema#string">Sappho,_fr._50:_The_man_who_is_pretty_is_so_only_as_far_as_he_looks;_the_man_who_is_good_is_already_beautiful._(Sententiaeantiquae._(2012,_March_14)._Sappho,_fragment_50._SENTENTIAE_ANTIQUAE._https:sententiaeantiquae.com20120314sappho-fragment-50)</passageChosenEn>
        <tlgIdentifyingNumber>tlg0009</tlgIdentifyingNumber>
        <passageChoselEl rdf:datatype="http://www.w3.org/2001/XMLSchema#string">απφώ,_απ._50_Lobel-Page_μετ._Ι.Ν._Καζάζη:_Αυτός_που_είναι_ωραίος,_είναι_ωραίος_στην_όψη,_αυτός_όμως_που_είναι_και_καλός,_θα_είναι_αυτόματα_και_ωραίος._(Τσέλικας,_Σ._(επ.)._ΣΑΠΦΩ:_απ._50_Lobel-Page._Ανθολογία_Αρχαϊκής_Λυρικής_Ποίησης._Ανακτήθηκε_4_Μαΐου_2024,_από_https:www.greek-language.grdigitalResourcesancient_greekanthologypoetrybrowse.html?text_id=296)</passageChoselEl>
        <hasWritten rdf:resource="#hymenaios_sappho"/>        <hasWritten rdf:resource="#epithalamia_sappho"/>        <hasWritten rdf:resource="#hymns_sappho"/>        <hasWritten rdf:resource="#erotic_odes_sappho"/>        <centuryOfLiving rdf:resource="#6th_century_BCE"/>        <centuryOfLiving rdf:resource="#7th_century_BCE"/>        <bornIn rdf:resource="#lesbos"/>        <stayedIn rdf:resource="#sicilia"/>        <rdfs:seeAlso rdf:resource="https://www.perseus.tufts.edu/hopper/text?doc=Perseus%3Atext%3A1999.04.0004%3Aalphabetic+letter%3DS%3Aentry+group%3D2%3Aentry%3Dsappho"/>
        <rdfs:seeAlso rdf:resource="https://catalog.perseus.org/catalog/urn:cite:perseus:author.1245"/>
        <rdfs:seeAlso rdf:resource="https://catalog.perseus.org/?f%5Btg_facet%5D%5B%5D=Sappho&amp;f%5Bwork_lang%5D%5B%5D=grc&amp;per_page=10&amp;q=tg_no_token%3A%5BS+TO+T%5D&amp;sort=auth_name+asc%2C+work_title+asc"/>
        <rdfs:seeAlso rdf:resource="https://www.perseus.tufts.edu/hopper/text?doc=Perseus%3Atext%3A1999.04.0104%3Aalphabetic+letter%3DS%3Aentry+group%3D4%3Aentry%3Dsappho-bio-1"/>
        <rdfs:seeAlso rdf:resource="https://catalog.perseus.org/catalog/urn:cts:greekLit:tlg0009.tlg002"/>
        <rdfs:seeAlso rdf:resource="https://catalog.perseus.org/catalog/urn:cts:greekLit:tlg0009.tlg001"/>
        <rdfs:seeAlso rdf:resource="https://www.perseus.tufts.edu/hopper/text?doc=Perseus:text:1999.04.0104:entry=sappho-bio-1"/>
        <foaf:depiction rdf:resource="https://upload.wikimedia.org/wikipedia/commons/b/b1/1877_Charles_Mengin_-_Sappho.jpg"/>
    </owl:NamedIndividual>

    <owl:NamedIndividual rdf:about="#anacreon_teius">
        <rdfs:label xml:lang="en">anacreon_teius</rdfs:label>
        <skos:prefLabel xml:lang="en">anacreon_teius</skos:prefLabel>
        <rdf:type rdf:resource="#Archaic_Lyric_Poet"/>
        <skos:note>By ChrisO - Own work, CC BY-SA 3.0, Anacreon depicted in the act of singing and playing his lyre.
https:commons.wikimedia.orgwindex.php?curid=4678744</skos:note>
        <tlgIdentifyingNumber>tlg0237</tlgIdentifyingNumber>
        <hasWritten rdf:resource="#elegies_anacreon"/>        <hasWritten rdf:resource="#iambs_anacreon"/>        <hasWritten rdf:resource="#hymns_anacreon"/>        <hasWritten rdf:resource="#threnoi_anacreon"/>        <hasWritten rdf:resource="#erotic_odes_anacreon"/>        <hasWritten rdf:resource="#sympotic_odes_alcaeus"/>        <centuryOfLiving rdf:resource="#6th_century_BCE"/>        <bornIn rdf:resource="#teos"/>        <stayedIn rdf:resource="#abdera"/>        <stayedIn rdf:resource="#samos"/>        <stayedIn rdf:resource="#teos"/>        <stayedIn rdf:resource="#athens"/>        <foaf:depiction rdf:resource="https://upload.wikimedia.org/wikipedia/commons/thumb/9/97/Anacreon_monte_calvo.jpg/330px-Anacreon_monte_calvo.jpg"/>
        <rdfs:seeAlso rdf:resource="https://catalog.perseus.org/catalog/urn:cite:perseus:author.84"/>
        <rdfs:seeAlso rdf:resource="https://en.wikipedia.org/wiki/Anacreon"/>
        <rdfs:seeAlso rdf:resource="https://www.britannica.com/biography/Anacreon"/>
        <rdfs:seeAlso rdf:resource="https://chs.harvard.edu/chapter/14-anacreon/"/>
        <rdfs:seeAlso rdf:resource="https://www.cambridge.org/core/books/abs/cambridge-companion-to-greek-lyric/anacreon-and-the-anacreontea/D6B462BA668AD3899E02267A62386720"/>
        <rdfs:seeAlso rdf:resource="https://www.poetryfoundation.org/poets/anacreon"/>
        <rdfs:seeAlso rdf:resource="https://lsj.gr/wiki/Anacreon"/>
        <rdfs:seeAlso rdf:resource="https://www.perseus.tufts.edu/hopper/text?doc=Perseus%3Atext%3A1999.04.0004%3Aentry%3Danacreon"/>
        <rdfs:seeAlso rdf:resource="https://catalog.perseus.org/catalog/urn:cts:greekLit:tlg0237.tlg004"/>
        <rdfs:seeAlso rdf:resource="https://catalog.perseus.org/catalog/urn:cts:greekLit:tlg0237.tlg002"/>
        <rdfs:seeAlso rdf:resource="https://catalog.perseus.org/catalog/urn:cts:greekLit:tlg0237.tlg001"/>
    </owl:NamedIndividual>

    <owl:NamedIndividual rdf:about="#erotic_odes_alcaeus">
        <rdfs:label xml:lang="en">erotic_odes_alcaeus</rdfs:label>
        <skos:prefLabel xml:lang="en">erotic_odes_alcaeus</skos:prefLabel>
        <rdf:type rdf:resource="#Archaic_Lyric_Poem_in_ionic_or_in_doric_or_in_aeolic_dialect_performed_by_a_single_performer"/>
        <isWrittenBy rdf:resource="#alcaeus_lesbius"/>    </owl:NamedIndividual>

    <owl:NamedIndividual rdf:about="#mimnermus_lyricus">
        <rdfs:label xml:lang="en">mimnermus_lyricus</rdfs:label>
        <skos:prefLabel xml:lang="en">mimnermus_lyricus</skos:prefLabel>
        <rdf:type rdf:resource="#Archaic_Lyric_Poet"/>
        <passageChosenEn rdf:datatype="http://www.w3.org/2001/XMLSchema#string">The_Elegies_of_Mimnermus,_CURFRAG.tlg-0255.1,_translated_by_Edmonts:_But_what_life_would_there_be,_what_joy,_without_golden_Aphrodite?_May_I_die_when_I_be_no_more_concerned_with_secret_love_and_suasive_gifts_and_the_bed,_such_things_as_are_the_very_flowers_of_youth,_pleasant_alike_to_man_and_woman._And_when_dolorous_Age_cometh,_that_maketh_a_man_both_foul_without_and_evil_within,ill_cares_do_wear_and_wear_his_heart,_he_hath_no_more_the_joy_of_looking_one_the_sunlight,_to_children_he_is_hateful,_to_women_contemptible,_so_grievous_hath_God_made_Age._(Edmonds,_J._M._(1931)._The_Elegies_of_Mimnermus_in_Elegy_and_Iambus_[English_Translation]._Cambridge,_MA:_Harvard_University_Press._London:_William_Heinemann_Ltd._(Original_work_published_1931)._Retrieved_May_4,_2024,_from_https:www.perseus.tufts.eduhoppertext?doc=Perseus%3Atext%3A2008.01.0479%3Avolume%3D1%3Atext%3D4%3Asection%3D2#:~:text=God%20made%20Age.-,%20Stobaeus%20Anthology)</passageChosenEn>
        <tlgIdentifyingNumber>tlg0255</tlgIdentifyingNumber>
        <passageChoselEl rdf:datatype="http://www.w3.org/2001/XMLSchema#string">Μίμνερμος,_απ._1_West_μετ._I._Ν._Καζάζη:_Τι_είναι_η_ζωή,_και_ποια_η_γλύκα_της_δίχως_την_Αφροδίτη_τη_χρυσή;_Ν_άφηνα_την_πνοή_μου,_όταν_θα_έπαυαν_όλα_τούτα_να_μ᾽_ενδιαφέρουν,_οι_κρυφές_αγάπες,_τα_γλυκά_σαν_μέλι_δώρα_τους_και_το_κρεβάτι_—_άνθη_συναρπαστικά_που_στολίζουν_τη_νιότη_αντρών_και_γυναικών._Μα_όταν_επιδράμει_οδυνηρό_το_γήρας,_αυτό_που_ασχημίζει_τον_άνθρωπο_και_τον_εξευτελίζει,_εξουθενωτικό_άγχος_βασανίζει_την_ψυχή_του,_και_πια_δεν_χαίρεται_να_αντικρίζει_το_φως_του_ήλιου·_γιατί_οι_άγουροι_τον_αποφεύγουν,_και_οι_γυναίκες_τον_περιφρονούν_—_τόσο_σκληρά_έκαμε_ο_θεός_τα_γηρατειά!_(Τσέλικας,_Σ._(επ.)._Μίμνερμος:_απ._1_West._Ανθολογία_Αρχαϊκής_Λυρικής_Ποίησης._Ανακτήθηκε_4_Μαΐου_2024,_από_https:www.greek-language.grdigitalResourcesancient_greekanthologypoetrybrowse.html?text_id=64#m2)</passageChoselEl>
        <hasWritten rdf:resource="#erotic_elegies_mimnermus"/>        <centuryOfLiving rdf:resource="#7th_century_BCE"/>        <stayedIn rdf:resource="#colophon"/>        <stayedIn rdf:resource="#smyrna"/>        <rdfs:seeAlso rdf:resource="https://www.perseus.tufts.edu/hopper/text?doc=Perseus%3Atext%3A2008.01.0479%3Avolume%3D1%3Atext%3D4%3Asection%3D2"/>
        <rdfs:seeAlso rdf:resource="https://catalog.perseus.org/catalog/urn:cite:perseus:author.938"/>
        <rdfs:seeAlso rdf:resource="https://www.wikidata.org/wiki/Q316129"/>
        <rdfs:seeAlso rdf:resource="https://catalog.perseus.org/catalog/urn:cts:greekLit:tlg0255.tlg002"/>
        <rdfs:seeAlso rdf:resource="https://catalog.perseus.org/catalog/urn:cts:greekLit:tlg0255.tlg001"/>
    </owl:NamedIndividual>

    <owl:NamedIndividual rdf:about="#7th_century_BCE">
        <rdfs:label xml:lang="en">7th_century_BCE</rdfs:label>
        <skos:prefLabel xml:lang="en">7th_century_BCE</skos:prefLabel>
        <rdf:type rdf:resource="#BCE_century"/>
        <startsIn rdf:datatype="http://www.w3.org/2001/XMLSchema#decimal">-699</startsIn>
        <endsIn rdf:datatype="http://www.w3.org/2001/XMLSchema#decimal">-600</endsIn>
        <isCenturyOf rdf:resource="#mimnermus_lyricus"/>        <isCenturyOf rdf:resource="#tyrtaeus_lacedaemonius"/>        <isCenturyOf rdf:resource="#solon_atheniensis"/>        <isCenturyOf rdf:resource="#stesichorus_himeraeus"/>        <isCenturyOf rdf:resource="#terpander_lesbius"/>        <isCenturyOf rdf:resource="#callinus_ephesius"/>        <isCenturyOf rdf:resource="#sappho_lesbia"/>        <isCenturyOf rdf:resource="#alcman_lacedaemonius"/>        <isCenturyOf rdf:resource="#archilochus_parius"/>        <isCenturyOf rdf:resource="#semonides_amorginus"/>        <isCenturyOf rdf:resource="#alcaeus_lesbius"/>    </owl:NamedIndividual>

    <owl:NamedIndividual rdf:about="#enkomion_pindarus">
        <rdfs:label xml:lang="en">enkomion_pindarus</rdfs:label>
        <skos:prefLabel xml:lang="en">enkomion_pindarus</skos:prefLabel>
        <rdf:type rdf:resource="#Archaic_Lyric_Poem_in_ionic_or_in_doric_or_in_aeolic_dialect_performed_by_a_chorus_or_by_a_single_performer_dedicated_to_living"/>
        <isWrittenBy rdf:resource="#pindarus_boeotus"/>    </owl:NamedIndividual>

    <owl:NamedIndividual rdf:about="#erotic_odes_anacreon">
        <rdfs:label xml:lang="en">erotic_odes_anacreon</rdfs:label>
        <skos:prefLabel xml:lang="en">erotic_odes_anacreon</skos:prefLabel>
        <rdf:type rdf:resource="#Archaic_Lyric_Poem_in_ionic_or_in_doric_or_in_aeolic_dialect_performed_by_a_single_performer"/>
        <isWrittenBy rdf:resource="#anacreon_teius"/>    </owl:NamedIndividual>

    <owl:NamedIndividual rdf:about="#smyrna">
        <rdfs:label xml:lang="en">smyrna</rdfs:label>
        <skos:prefLabel xml:lang="en">smyrna</skos:prefLabel>
        <rdf:type rdf:resource="#Ancient_Location"/>
        <pleiadesCoordinates>38.41719605,27.141387</pleiadesCoordinates>
        <residentedBy rdf:resource="#mimnermus_lyricus"/>        <rdfs:seeAlso rdf:resource="https://pleiades.stoa.org/places/550771"/>
        <rdfs:seeAlso rdf:resource="https://www.trismegistos.org/place/41382"/>
        <rdfs:seeAlso rdf:resource="https://en.wikipedia.org/wiki/%C4%B0zmir"/>
        <rdfs:seeAlso rdf:resource="http://www.perseus.tufts.edu/hopper/text?doc=Perseus%3Atext%3A1999.04.0006%3Aalphabetic+letter%3DS%3Aentry+group%3D8%3Aentry%3Dsmyrna"/>
    </owl:NamedIndividual>

    <owl:NamedIndividual rdf:about="#partheneia_alcman">
        <rdfs:label xml:lang="en">partheneia_alcman</rdfs:label>
        <skos:prefLabel xml:lang="en">partheneia_alcman</skos:prefLabel>
        <rdf:type rdf:resource="#Archaic_Lyric_Poem_in_ionic_or_in_doric_or_in_aeolic_dialect_performed_by_a_chorus_performed_by_a_maidens_chorus"/>
        <isWrittenBy rdf:resource="#alcman_lacedaemonius"/>    </owl:NamedIndividual>

    <owl:NamedIndividual rdf:about="#akragas">
        <rdfs:label xml:lang="en">akragas</rdfs:label>
        <skos:prefLabel xml:lang="en">akragas</skos:prefLabel>
        <rdf:type rdf:resource="#Ancient_Location"/>
        <pleiadesCoordinates>37.290594,13.585475</pleiadesCoordinates>
        <residentedBy rdf:resource="#pindarus_boeotus"/>        <rdfs:seeAlso rdf:resource="https://pleiades.stoa.org/places/462086"/>
        <rdfs:seeAlso rdf:resource="https://topostext.org/place/373136PAkr"/>
        <rdfs:seeAlso rdf:resource="https://en.wikipedia.org/wiki/Agrigento"/>
        <rdfs:seeAlso rdf:resource="http://www.geonames.org/2525764/agrigento.html"/>
        <rdfs:seeAlso rdf:resource="https://www.wikidata.org/wiki/Q13678"/>
        <rdfs:seeAlso rdf:resource="http://www.trismegistos.org/place/22270"/>
    </owl:NamedIndividual>

    <owl:NamedIndividual rdf:about="#paeans_bacchylides">
        <rdfs:label xml:lang="en">paeans_bacchylides</rdfs:label>
        <skos:prefLabel xml:lang="en">paeans_bacchylides</skos:prefLabel>
        <rdf:type rdf:resource="#Archaic_Lyric_Poem_in_ionic_or_in_doric_or_in_aeolic_dialect_performed_by_a_chorus_or_by_a_single_performer_dedicated_to_apollo"/>
        <isWrittenBy rdf:resource="#bacchylides_ceus"/>    </owl:NamedIndividual>

    <owl:NamedIndividual rdf:about="#iambs_hipponax">
        <rdfs:label xml:lang="en">iambs_hipponax</rdfs:label>
        <skos:prefLabel xml:lang="en">iambs_hipponax</skos:prefLabel>
        <rdf:type rdf:resource="#Archaic_Lyric_Poem_only_in_ionic_dialect_in_iambic_or_trochaic_metre"/>
        <isWrittenBy rdf:resource="#hipponax_ephesius"/>    </owl:NamedIndividual>

    <owl:NamedIndividual rdf:about="#alcman_lacedaemonius">
        <rdfs:label xml:lang="en">alcman_lacedaemonius</rdfs:label>
        <skos:prefLabel xml:lang="en">alcman_lacedaemonius</skos:prefLabel>
        <rdf:type rdf:resource="#Archaic_Lyric_Poet"/>
        <skos:note>By ellenm1 - Roman-period mosaic portrait of Alcman from Gerasa, 3rd century AD. Flickr: Mosaic Portrait of the Poet Alkman, CC BY 2.0, https:commons.wikimedia.orgwindex.php?curid=140276390</skos:note>
        <passageChosenEn rdf:datatype="http://www.w3.org/2001/XMLSchema#string">Alcman,_fr._14_transl._Cambell:_Come,_Muse,_clear-voiced_Muse_of_many_songs,_singer_always,_begin_a_new_song_for_girls_to_sing._(Campbell,_D._(n.d.)._Alcman_Fr._14._In_Greek_Lyric,_Volume_II._Harvard_University_Press._Retrieved_4_May_2024,_from_https:www.loebclassics.comviewalcman-fragments1988pb_LCL143.407.xml)</passageChosenEn>
        <tlgIdentifyingNumber>tlg0291</tlgIdentifyingNumber>
        <passageChoselEl rdf:datatype="http://www.w3.org/2001/XMLSchema#string">Αλκμάν,_απ._14a_Page_μετ._Ι.Ν._Καζάζης:_Έλα,_Μούσα,_γλυκόλαλη_Μούσα_μου,_με_τα_πλούσια,_μελωδικά_τραγούδια_σου_για_κάθε_περίσταση,_κι_άρχισε_έναν_καινούριο_σκοπό_να_τραγουδήσουν_τα_κορίτσια._(Τσέλικας,_Σ._(επ.)._ΑΛΚΜΑΝ:_απ._14a_Page._Ανθολογία_Αρχαϊκής_Λυρικής_Ποίησης._Ανακτήθηκε_4_Μαΐου_2024,_από_https:www.greek-language.grdigitalResourcesancient_greekanthologypoetrybrowse.html?text_id=143)</passageChoselEl>
        <hasWritten rdf:resource="#partheneia_alcman"/>        <hasWritten rdf:resource="#prosodia_alcman"/>        <hasWritten rdf:resource="#hymns_alcman"/>        <hasWritten rdf:resource="#paeans_alcman"/>        <hasWritten rdf:resource="#erotic_odes_alcman"/>        <centuryOfLiving rdf:resource="#7th_century_BCE"/>        <bornIn rdf:resource="#sardis"/>        <stayedIn rdf:resource="#sparta"/>        <foaf:depiction rdf:resource="https://upload.wikimedia.org/wikipedia/commons/9/9e/Mosaic_Portrait_of_the_Poet_Alcman_%28cropped%29.jpg"/>
        <rdfs:seeAlso rdf:resource="https://catalog.perseus.org/catalog/urn:cite:perseus:author.57"/>
        <rdfs:seeAlso rdf:resource="https://www.perseus.tufts.edu/hopper/text?doc=Perseus%3Atext%3A1999.04.0104%3Aalphabetic+letter%3DA%3Aentry+group%3D14%3Aentry%3Dalcman-bio-1"/>
        <rdfs:seeAlso rdf:resource="https://catalog.perseus.org/catalog/urn:cts:greekLit:tlg0291.tlg001.opp-eng1"/>
        <rdfs:seeAlso rdf:resource="https://logeion.uchicago.edu/Alcman"/>
        <rdfs:seeAlso rdf:resource="https://en.wikipedia.org/wiki/Alcman"/>
        <rdfs:seeAlso rdf:resource="https://www.britannica.com/biography/Alcman"/>
        <rdfs:seeAlso rdf:resource="https://el.wikipedia.org/wiki/%CE%91%CE%BB%CE%BA%CE%BC%CE%AC%CE%BD"/>
        <rdfs:seeAlso rdf:resource="https://chs.harvard.edu/primary-source/alcman-partheneion-sb/"/>
        <rdfs:seeAlso rdf:resource="https://www.britannica.com/biography/Alcaeus"/>
    </owl:NamedIndividual>

    <owl:NamedIndividual rdf:about="#miletus">
        <rdfs:label xml:lang="en">miletus</rdfs:label>
        <skos:prefLabel xml:lang="en">miletus</skos:prefLabel>
        <rdf:type rdf:resource="#Ancient_Location"/>
        <pleiadesCoordinates>37.53046444,27.2788084839</pleiadesCoordinates>
        <isBirthPlaceOf rdf:resource="#phocylides_milesius"/>        <rdfs:seeAlso rdf:resource="https://pleiades.stoa.org/places/599799"/>
        <rdfs:seeAlso rdf:resource="https://en.wikipedia.org/wiki/Miletus"/>
        <rdfs:seeAlso rdf:resource="http://www.geonames.org/9534929/miletos.html"/>
        <rdfs:seeAlso rdf:resource="http://www.trismegistos.org/place/1375"/>
        <rdfs:seeAlso rdf:resource="https://www.wikidata.org/wiki/Q169460"/>
        <rdfs:seeAlso rdf:resource="http://www.geonames.org/9534929/miletos.html"/>
    </owl:NamedIndividual>

    <owl:NamedIndividual rdf:about="#enkomion_ibycus">
        <rdfs:label xml:lang="en">enkomion_ibycus</rdfs:label>
        <skos:prefLabel xml:lang="en">enkomion_ibycus</skos:prefLabel>
        <rdf:type rdf:resource="#Archaic_Lyric_Poem_in_ionic_or_in_doric_or_in_aeolic_dialect_performed_by_a_chorus_or_by_a_single_performer_dedicated_to_living"/>
        <isWrittenBy rdf:resource="#ibycus_rheginus"/>    </owl:NamedIndividual>

    <owl:NamedIndividual rdf:about="#colophon">
        <rdfs:label xml:lang="en">colophon</rdfs:label>
        <skos:prefLabel xml:lang="en">colophon</skos:prefLabel>
        <rdf:type rdf:resource="#Ancient_Location"/>
        <pleiadesCoordinates>38.108253,27.1483085</pleiadesCoordinates>
        <residentedBy rdf:resource="#mimnermus_lyricus"/>        <rdfs:seeAlso rdf:resource="https://pleiades.stoa.org/places/599577"/>
        <rdfs:seeAlso rdf:resource="http://www.trismegistos.org/place/1142"/>
        <rdfs:seeAlso rdf:resource="http://www.geonames.org/9794266/colophon-greek-bath.html"/>
        <rdfs:seeAlso rdf:resource="https://en.wikipedia.org/wiki/Colophon_(city)"/>
        <rdfs:seeAlso rdf:resource="http://www.perseus.tufts.edu/hopper/text?doc=Perseus%3Atext%3A1999.04.0006%3Aalphabetic+letter%3DC%3Aentry+group%3D8%3Aentry%3Dcolophon"/>
    </owl:NamedIndividual>

    <owl:NamedIndividual rdf:about="#epinikoi_simonides">
        <rdfs:label xml:lang="en">epinikoi_simonides</rdfs:label>
        <skos:prefLabel xml:lang="en">epinikoi_simonides</skos:prefLabel>
        <rdf:type rdf:resource="#Archaic_Lyric_Poem_in_ionic_or_in_doric_or_in_aeolic_dialect_performed_by_a_chorus_or_by_a_single_performer_dedicated_to_winners_in_athletic_events"/>
        <isWrittenBy rdf:resource="#simonides_ceus"/>    </owl:NamedIndividual>

    <owl:NamedIndividual rdf:about="#amorgos">
        <rdfs:label xml:lang="en">amorgos</rdfs:label>
        <skos:prefLabel xml:lang="en">amorgos</skos:prefLabel>
        <rdf:type rdf:resource="#Ancient_Location"/>
        <pleiadesCoordinates>36.8482485331,25.8978389099</pleiadesCoordinates>
        <residentedBy rdf:resource="#semonides_amorginus"/>        <rdfs:seeAlso rdf:resource="https://pleiades.stoa.org/places/599484"/>
        <rdfs:seeAlso rdf:resource="https://topostext.org/place/368259IAmo"/>
        <rdfs:seeAlso rdf:resource="https://de.wikisource.org/wiki/RE:Amorgos"/>
        <rdfs:seeAlso rdf:resource="https://www.trismegistos.org/place/3592"/>
    </owl:NamedIndividual>

    <owl:NamedIndividual rdf:about="#paros">
        <rdfs:label xml:lang="en">paros</rdfs:label>
        <skos:prefLabel xml:lang="en">paros</skos:prefLabel>
        <rdf:type rdf:resource="#Ancient_Location"/>
        <pleiadesCoordinates>37.0637200811,25.1981285553</pleiadesCoordinates>
        <isBirthPlaceOf rdf:resource="#archilochus_parius"/>        <rdfs:seeAlso rdf:resource="https://pleiades.stoa.org/places/599868"/>
        <rdfs:seeAlso rdf:resource="https://www.wikidata.org/wiki/Q201272"/>
        <rdfs:seeAlso rdf:resource="https://www.trismegistos.org/place/1613"/>
        <rdfs:seeAlso rdf:resource="https://www.geonames.org/255720/nisi-paros.html"/>
        <rdfs:seeAlso rdf:resource="https://en.wikipedia.org/wiki/Paros"/>
    </owl:NamedIndividual>

    <owl:NamedIndividual rdf:about="#alcaeus_lesbius">
        <rdfs:label xml:lang="en">alcaeus_lesbius</rdfs:label>
        <skos:prefLabel xml:lang="en">alcaeus_lesbius</skos:prefLabel>
        <rdf:type rdf:resource="#Archaic_Lyric_Poet"/>
        <skos:note>By Brygos Painter - Alcaeus and Sappho, Attic red-figure calathus, c. 470 BC, Staatliche Antikensammlungen (Inv. 2416). User:Bibi Saint-Pol, own work, 2007-02-10, Public Domain, https:commons.wikimedia.orgwindex.php?curid=2751067</skos:note>
        <passageChosenEn rdf:datatype="http://www.w3.org/2001/XMLSchema#string">Tr._J._Henderson,_Alcaeus_fr._Lobel-Page_335_(Sympotic):_We_should_not_surrender_our_hearts_to_our_troubles,_for_we_shall_make_no_headway_by_grieving,_Bycchis:_the_best_of_remedies_is_to_bring_wine_and_get_drunk._(Henderson,_J._(n.d.)._Alcaeus._Loeb_Classical_Library._Retrieved_4_May_2024,_from_https:www.loebclassics.comviewalcaeus-fragments1982pb_LCL142.373.xml)</passageChosenEn>
        <tlgIdentifyingNumber>tlg0383</tlgIdentifyingNumber>
        <passageChoselEl rdf:datatype="http://www.w3.org/2001/XMLSchema#string">Αλκαίος,_απ._Lobel-Page_335,_μετ._Ηλ._Βουτιερίδης:_Δεν_πρέπει_την_ψυχή_ν᾽_αφήνουμε_στις_λύπες·_|_γιατί_κι_αν_λυπηθούμε_δε_θα_ωφεληθούμε_|_τίποτα,_ω_Βάκχε._Σαν_το_πιο_καλό_θεράπιο_|_δίνοντας_στην_ψυχή_μας_το_κρασί,_ας_μεθούμε._(Τσέλικας,_Σ._(επ.)._ΑΛΚΑΙΟΣ:_απ._335_Lobel-Page._Ανθολογία_Αρχαϊκής_Λυρικής_Ποίησης._Ανακτήθηκε_4_Μαΐου_2024,_από_https:www.greek-language.grdigitalResourcesancient_greekanthologypoetrybrowse.html?text_id=252)</passageChoselEl>
        <hasWritten rdf:resource="#hymns_alcaeus"/>        <hasWritten rdf:resource="#erotic_odes_alcaeus"/>        <hasWritten rdf:resource="#sympotic_odes_alcaeus"/>        <hasWritten rdf:resource="#warlike_odes_alcaeus"/>        <centuryOfLiving rdf:resource="#6th_century_BCE"/>        <centuryOfLiving rdf:resource="#7th_century_BCE"/>        <bornIn rdf:resource="#lesbos"/>        <stayedIn rdf:resource="#aegypt"/>        <stayedIn rdf:resource="#lesbos"/>        <rdfs:seeAlso rdf:resource="https://catalog.perseus.org/catalog/urn:cite:perseus:author.51"/>
        <rdfs:seeAlso rdf:resource="https://en.wikipedia.org/wiki/Alcaeus"/>
        <rdfs:seeAlso rdf:resource="https://www.britannica.com/biography/Alcaeus"/>
        <rdfs:seeAlso rdf:resource="https://repository.kallipos.gr/handle/11419/8620"/>
        <rdfs:seeAlso rdf:resource="https://chs.harvard.edu/curated-article/gregory-nagy-did-sappho-and-alcaeus-ever-meet-symmetries-of-myth-and-ritual-in-performing-the-songs-of-ancient-lesbos/"/>
        <rdfs:seeAlso rdf:resource="https://www.oxfordreference.com/display/10.1093/oi/authority.20110803095400481"/>
        <rdfs:seeAlso rdf:resource="https://www.attalus.org/names/a/alcaeus.html"/>
        <foaf:depiction rdf:resource="https://upload.wikimedia.org/wikipedia/commons/thumb/9/99/Alkaios_Sappho_Staatliche_Antikensammlungen_2416_n1.jpg/440px-Alkaios_Sappho_Staatliche_Antikensammlungen_2416_n1.jpg"/>
        <rdfs:seeAlso rdf:resource="https://catalog.perseus.org/catalog/urn:cts:greekLit:tlg0383.tlg001"/>
    </owl:NamedIndividual>

    <owl:NamedIndividual rdf:about="#gnomic_elegies_phocylides">
        <rdfs:label xml:lang="en">gnomic_elegies_phocylides</rdfs:label>
        <skos:prefLabel xml:lang="en">gnomic_elegies_phocylides</skos:prefLabel>
        <rdf:type rdf:resource="#Archaic_Lyric_Poem_only_in_ionic_dialect_in_elegiac_couplet_with_gnomic_content"/>
        <isWrittenBy rdf:resource="#phocylides_milesius"/>    </owl:NamedIndividual>

    <owl:NamedIndividual rdf:about="#boeotia">
        <rdfs:label xml:lang="en">boeotia</rdfs:label>
        <skos:prefLabel xml:lang="en">boeotia</skos:prefLabel>
        <rdf:type rdf:resource="#Ancient_Location"/>
        <pleiadesCoordinates>38.3168971672,23.1349191419</pleiadesCoordinates>
        <isBirthPlaceOf rdf:resource="#pindarus_boeotus"/>        <rdfs:seeAlso rdf:resource="https://pleiades.stoa.org/places/540689"/>
        <rdfs:seeAlso rdf:resource="https://en.wikipedia.org/wiki/Boeotia"/>
        <rdfs:seeAlso rdf:resource="https://topostext.org/place/384233RBoi"/>
        <rdfs:seeAlso rdf:resource="https://www.trismegistos.org/place/446"/>
    </owl:NamedIndividual>

    <owl:NamedIndividual rdf:about="#prosodia_alcman">
        <rdfs:label xml:lang="en">prosodia_alcman</rdfs:label>
        <skos:prefLabel xml:lang="en">prosodia_alcman</skos:prefLabel>
        <rdf:type rdf:resource="#Archaic_Lyric_Poem_in_ionic_or_in_doric_or_in_aeolic_dialect_performed_by_a_chorus_on_the_way_to_an_altar"/>
        <isWrittenBy rdf:resource="#alcman_lacedaemonius"/>    </owl:NamedIndividual>

    <owl:NamedIndividual rdf:about="#threnoi_pindarus">
        <rdfs:label xml:lang="en">threnoi_pindarus</rdfs:label>
        <skos:prefLabel xml:lang="en">threnoi_pindarus</skos:prefLabel>
        <rdf:type rdf:resource="#Archaic_Lyric_Poem_in_ionic_or_in_doric_or_in_aeolic_dialect_performed_by_a_chorus_or_by_a_single_performer_dedicated_to_dead"/>
        <isWrittenBy rdf:resource="#pindarus_boeotus"/>    </owl:NamedIndividual>

    <owl:NamedIndividual rdf:about="#lesbos">
        <rdfs:label xml:lang="en">lesbos</rdfs:label>
        <skos:prefLabel xml:lang="en">lesbos</skos:prefLabel>
        <rdf:type rdf:resource="#Ancient_Location"/>
        <pleiadesCoordinates>39.1785448797,26.2377523591</pleiadesCoordinates>
        <isBirthPlaceOf rdf:resource="#alcaeus_lesbius"/>        <isBirthPlaceOf rdf:resource="#sappho_lesbia"/>        <isBirthPlaceOf rdf:resource="#terpander_lesbius"/>        <rdfs:seeAlso rdf:resource="https://pleiades.stoa.org/places/550696"/>
        <rdfs:seeAlso rdf:resource="https://en.wikipedia.org/wiki/Lesbos"/>
        <rdfs:seeAlso rdf:resource="https://topostext.org/place/392261ILes"/>
        <rdfs:seeAlso rdf:resource="https://www.wikidata.org/"/>
        <rdfs:seeAlso rdf:resource="http://www.trismegistos.org/place/1242"/>
    </owl:NamedIndividual>

    <owl:NamedIndividual rdf:about="#solon_atheniensis">
        <rdfs:label xml:lang="en">solon_atheniensis</rdfs:label>
        <skos:prefLabel xml:lang="en">solon_atheniensis</skos:prefLabel>
        <rdf:type rdf:resource="#Archaic_Lyric_Poet"/>
        <skos:note>By M. A. Barth - "Solon demands to pledge respect for his laws", book illustration (Augsburg 1832). 'Vorzeit und Gegenwart", Augsbourg, 1832, Public Domain, https:commons.wikimedia.orgwindex.php?curid=74939386</skos:note>
        <tlgIdentifyingNumber>tlg0263</tlgIdentifyingNumber>
        <hasWritten rdf:resource="#political_elegies_solon"/>        <centuryOfLiving rdf:resource="#6th_century_BCE"/>        <centuryOfLiving rdf:resource="#7th_century_BCE"/>        <bornIn rdf:resource="#athens"/>        <foaf:depiction rdf:resource="https://upload.wikimedia.org/wikipedia/commons/f/f6/Solon_demands_to_pledge_respect_for_his_laws.jpg"/>
        <rdfs:seeAlso rdf:resource="https://www.perseus.tufts.edu/hopper/text?doc=Perseus%3Atext%3A2008.01.0479%3Avolume%3D1%3Atext%3D5%3Asection%3D2"/>
        <rdfs:seeAlso rdf:resource="https://www.perseus.tufts.edu/hopper/text?doc=Perseus%3Atext%3A1999.04.0004%3Aalphabetic+letter%3DS%3Aentry+group%3D6%3Aentry%3Dsolon"/>
        <rdfs:seeAlso rdf:resource="https://catalog.perseus.org/catalog/urn:cts:greekLit:tlg0007.tlg007"/>
        <rdfs:seeAlso rdf:resource="https://catalog.perseus.org/catalog/urn:cts:greekLit:tlg0263.tlg001"/>
    </owl:NamedIndividual>

    <owl:NamedIndividual rdf:about="#prosodia_bacchylides">
        <rdfs:label xml:lang="en">prosodia_bacchylides</rdfs:label>
        <skos:prefLabel xml:lang="en">prosodia_bacchylides</skos:prefLabel>
        <rdf:type rdf:resource="#Archaic_Lyric_Poem_in_ionic_or_in_doric_or_in_aeolic_dialect_performed_by_a_chorus_on_the_way_to_an_altar"/>
        <isWrittenBy rdf:resource="#bacchylides_ceus"/>    </owl:NamedIndividual>

    <owl:NamedIndividual rdf:about="#klazomenai">
        <rdfs:label xml:lang="en">klazomenai</rdfs:label>
        <skos:prefLabel xml:lang="en">klazomenai</skos:prefLabel>
        <rdf:type rdf:resource="#Ancient_Location"/>
        <pleiadesCoordinates>38.3614575859,26.770567899</pleiadesCoordinates>
        <residentedBy rdf:resource="#hipponax_ephesius"/>        <rdfs:seeAlso rdf:resource="https://pleiades.stoa.org/places/550650"/>
        <rdfs:seeAlso rdf:resource="https://pleiades.stoa.org/places/550651"/>
        <rdfs:seeAlso rdf:resource="https://en.wikipedia.org/wiki/Klazomenai"/>
        <rdfs:seeAlso rdf:resource="https://topostext.org/place/384268PKla"/>
    </owl:NamedIndividual>

    <owl:NamedIndividual rdf:about="#phocylides_milesius">
        <rdfs:label xml:lang="en">phocylides_milesius</rdfs:label>
        <skos:prefLabel xml:lang="en">phocylides_milesius</skos:prefLabel>
        <rdf:type rdf:resource="#Archaic_Lyric_Poet"/>
        <tlgIdentifyingNumber>tlg1604</tlgIdentifyingNumber>
        <hasWritten rdf:resource="#gnomic_elegies_phocylides"/>        <centuryOfLiving rdf:resource="#6th_century_BCE"/>        <bornIn rdf:resource="#miletus"/>        <rdfs:seeAlso rdf:resource="https://www.perseus.tufts.edu/hopper/text?doc=Perseus%3Atext%3A2008.01.0479%3Avolume%3D1%3Atext%3D9"/>
        <rdfs:seeAlso rdf:resource="https://www.perseus.tufts.edu/hopper/text?doc=Perseus%3Atext%3A2008.01.0479%3Avolume%3D1%3Atext%3D9%3Asection%3D2"/>
        <rdfs:seeAlso rdf:resource="https://catalog.perseus.org/catalog/urn:cite:perseus:author.1116"/>
        <rdfs:seeAlso rdf:resource="https://www.wikidata.org/wiki/Q972799"/>
        <rdfs:seeAlso rdf:resource="https://anthologiagraeca.org/authors/291/"/>
        <rdfs:seeAlso rdf:resource="https://quod.lib.umich.edu/cgi/t/text/pageviewer-idx?c=moa;cc=moa;rgn=full%20text;idno=ACL3129.0003.001;didno=ACL3129.0003.001;view=image;seq=00000350"/>
        <rdfs:seeAlso rdf:resource="https://catalog.perseus.org/catalog/urn:cts:greekLit:tlg1604.tlg002"/>
    </owl:NamedIndividual>

    <owl:NamedIndividual rdf:about="#elegies_anacreon">
        <rdfs:label xml:lang="en">elegies_anacreon</rdfs:label>
        <skos:prefLabel xml:lang="en">elegies_anacreon</skos:prefLabel>
        <rdf:type rdf:resource="#Archaic_Lyric_Poem_only_in_ionic_dialect_in_elegiac_couplet"/>
        <isWrittenBy rdf:resource="#anacreon_teius"/>    </owl:NamedIndividual>

    <owl:NamedIndividual rdf:about="#sparta">
        <rdfs:label xml:lang="en">sparta</rdfs:label>
        <skos:prefLabel xml:lang="en">sparta</skos:prefLabel>
        <rdf:type rdf:resource="#Ancient_Location"/>
        <pleiadesCoordinates>37.0818455246,22.4246825462</pleiadesCoordinates>
        <residentedBy rdf:resource="#alcman_lacedaemonius"/>        <isBirthPlaceOf rdf:resource="#tyrtaeus_lacedaemonius"/>        <rdfs:seeAlso rdf:resource="https://pleiades.stoa.org/places/570685"/>
        <rdfs:seeAlso rdf:resource="http://www.trismegistos.org/place/2181"/>
        <rdfs:seeAlso rdf:resource="https://www.wikidata.org/wiki/Q5690"/>
        <rdfs:seeAlso rdf:resource="https://www.geonames.org/253394/sparta.html"/>
        <rdfs:seeAlso rdf:resource="https://en.wikipedia.org/wiki/Sparta"/>
        <rdfs:seeAlso rdf:resource="https://topostext.org/place/371224PSpa"/>
    </owl:NamedIndividual>

    <owl:NamedIndividual rdf:about="#megara">
        <rdfs:label xml:lang="en">megara</rdfs:label>
        <skos:prefLabel xml:lang="en">megara</skos:prefLabel>
        <rdf:type rdf:resource="#Ancient_Location"/>
        <pleiadesCoordinates>37.985078,23.340163</pleiadesCoordinates>
        <isBirthPlaceOf rdf:resource="#theognis_megarensis"/>        <rdfs:seeAlso rdf:resource="https://pleiades.stoa.org/places/570468"/>
        <rdfs:seeAlso rdf:resource="https://topostext.org/place/380233PMeg"/>
        <rdfs:seeAlso rdf:resource="https://en.wikipedia.org/wiki/Megara"/>
        <rdfs:seeAlso rdf:resource="http://www.perseus.tufts.edu/hopper/text?doc=Perseus%3Atext%3A1999.04.0064%3Aalphabetic+letter%3DM%3Aentry+group%3D8%3Aentry%3Dmegara-geo02"/>
        <rdfs:seeAlso rdf:resource="https://en.wikipedia.org/wiki/Megaris"/>
    </owl:NamedIndividual>

    <owl:NamedIndividual rdf:about="#sicilia">
        <rdfs:label xml:lang="en">sicilia</rdfs:label>
        <skos:prefLabel xml:lang="en">sicilia</skos:prefLabel>
        <rdf:type rdf:resource="#Ancient_Location"/>
        <pleiadesCoordinates>37.6288545273,13.9945590442</pleiadesCoordinates>
        <residentedBy rdf:resource="#simonides_ceus"/>        <residentedBy rdf:resource="#sappho_lesbia"/>        <rdfs:seeAlso rdf:resource="https://pleiades.stoa.org/places/462492"/>
        <rdfs:seeAlso rdf:resource="https://en.wikipedia.org/wiki/Sicily"/>
        <rdfs:seeAlso rdf:resource="http://www.perseus.tufts.edu/hopper/text?doc=Perseus%3Atext%3A1999.04.0064%3Aalphabetic+letter%3DS%3Aentry+group%3D12%3Aentry%3Dsicilia-geo"/>
        <rdfs:seeAlso rdf:resource="http://www.geonames.org/"/>
        <rdfs:seeAlso rdf:resource="https://www.wikidata.org/wiki/Q4951156"/>
        <rdfs:seeAlso rdf:resource="https://www.trismegistos.org/place/2132"/>
    </owl:NamedIndividual>

    <owl:NamedIndividual rdf:about="#enkomion_bacchylides">
        <rdfs:label xml:lang="en">enkomion_bacchylides</rdfs:label>
        <skos:prefLabel xml:lang="en">enkomion_bacchylides</skos:prefLabel>
        <rdf:type rdf:resource="#Archaic_Lyric_Poem_in_ionic_or_in_doric_or_in_aeolic_dialect_performed_by_a_chorus_or_by_a_single_performer_dedicated_to_living"/>
        <isWrittenBy rdf:resource="#bacchylides_ceus"/>    </owl:NamedIndividual>

    <owl:NamedIndividual rdf:about="#paeans_pindarus">
        <rdfs:label xml:lang="en">paeans_pindarus</rdfs:label>
        <skos:prefLabel xml:lang="en">paeans_pindarus</skos:prefLabel>
        <rdf:type rdf:resource="#Archaic_Lyric_Poem_in_ionic_or_in_doric_or_in_aeolic_dialect_performed_by_a_chorus_or_by_a_single_performer_dedicated_to_apollo"/>
        <isWrittenBy rdf:resource="#pindarus_boeotus"/>    </owl:NamedIndividual>

    <owl:NamedIndividual rdf:about="#choral_ibycus">
        <rdfs:label xml:lang="en">choral_ibycus</rdfs:label>
        <skos:prefLabel xml:lang="en">choral_ibycus</skos:prefLabel>
        <rdf:type rdf:resource="#Archaic_Lyric_Poem_in_ionic_or_in_doric_or_in_aeolic_dialect_performed_by_a_chorus"/>
        <isWrittenBy rdf:resource="#ibycus_rheginus"/>    </owl:NamedIndividual>

    <owl:NamedIndividual rdf:about="#elegies_archilochus">
        <rdfs:label xml:lang="en">elegies_archilochus</rdfs:label>
        <skos:prefLabel xml:lang="en">elegies_archilochus</skos:prefLabel>
        <rdf:type rdf:resource="#Archaic_Lyric_Poem_only_in_ionic_dialect_in_elegiac_couplet"/>
        <isWrittenBy rdf:resource="#archilochus_parius"/>    </owl:NamedIndividual>

    <owl:NamedIndividual rdf:about="#dithyrambs_simonides">
        <rdfs:label xml:lang="en">dithyrambs_simonides</rdfs:label>
        <skos:prefLabel xml:lang="en">dithyrambs_simonides</skos:prefLabel>
        <rdf:type rdf:resource="#Archaic_Lyric_Poem_in_ionic_or_in_doric_or_in_aeolic_dialect_performed_by_a_chorus_or_by_a_single_performer_dedicated_to_dionysus"/>
        <isWrittenBy rdf:resource="#simonides_ceus"/>    </owl:NamedIndividual>

    <owl:NamedIndividual rdf:about="#pindarus_boeotus">
        <rdfs:label xml:lang="en">pindarus_boeotus</rdfs:label>
        <skos:prefLabel xml:lang="en">pindarus_boeotus</skos:prefLabel>
        <rdf:type rdf:resource="#Archaic_Lyric_Poet"/>
        <skos:note>By Ancient Roman frescos of Pompeii - Enthroned Pindar with lyre, Muse and poetess. Antique fresco in Pompeii
https:pompeiiinpictures.compompeiiinpicturesindex.htm, Public Domain, https:commons.wikimedia.orgwindex.php?curid=94696565</skos:note>
        <passageChosenEn rdf:datatype="http://www.w3.org/2001/XMLSchema#string">Pythian_7_transl_Svarlien:_The_great_city_of_Athens_is_the_most_beautiful_prelude_of_song,_which_the_widely_powerful_race_of_the_Alcmaeonids_can_lay_as_a_foundation_of_odes_in_honor_of_their_horses._[5]_What_fatherland,_what_family_will_you_name_that_is_more_illustrious_in_Greece?_For_in_all_cities_the_story_[10]_of_the_citizens_of_Erechtheus_makes_the_rounds,_Apollo,_how_they_made_your_dwelling_in_divine_Pytho_a_marvel_to_see._Five_Isthmian_victories_lead_my_song_forward,_and_one_outstanding_triumph_[15]_at_Zeus''_Olympian_games,_and_two_from_Cirrha—_yours,_Megacles,_and_your_ancestors''._I_rejoice_at_this_new_success;_but_I_grieve_that_fine_deeds_are_repaid_with_envy._[20]_It_is_true_what_they_say:_the_abiding_bloom_of_good_fortune_brings_with_it_both_good_and_bad._(Arnson_Svarlien,_D._(n.d.)._Pindar,_Pythian_7._Retrieved_12_May_2024,_from_https:www.perseus.tufts.eduhoppertext?doc=Perseus%3Atext%3A1999.01.0162%3Abook%3DP.%3Apoem%3D7)</passageChosenEn>
        <tlgIdentifyingNumber>tlg0033</tlgIdentifyingNumber>
        <hasWritten rdf:resource="#hyporchemes_pindarus"/>        <hasWritten rdf:resource="#partheneia_pindarus"/>        <hasWritten rdf:resource="#prosodia_pindarus"/>        <hasWritten rdf:resource="#dithyrambs_pindarus"/>        <hasWritten rdf:resource="#enkomion_pindarus"/>        <hasWritten rdf:resource="#epinikoi_pindarus"/>        <hasWritten rdf:resource="#paeans_pindarus"/>        <hasWritten rdf:resource="#threnoi_pindarus"/>        <centuryOfLiving rdf:resource="#5th_century_BCE"/>        <centuryOfLiving rdf:resource="#6th_century_BCE"/>        <bornIn rdf:resource="#boeotia"/>        <stayedIn rdf:resource="#akragas"/>        <stayedIn rdf:resource="#athens"/>        <stayedIn rdf:resource="#syrakousai"/>        <rdfs:seeAlso rdf:resource="https://www.perseus.tufts.edu/hopper/collection?collection=Perseus%3Acorpus%3Aperseus%2Cauthor%2CPindar"/>
        <rdfs:seeAlso rdf:resource="https://catalog.perseus.org/catalog/urn:cite:perseus:author.1126"/>
        <rdfs:seeAlso rdf:resource="https://catalog.perseus.org/catalog/urn:cts:greekLit:tlg0033.tlg005"/>
        <rdfs:seeAlso rdf:resource="https://catalog.perseus.org/catalog/urn:cts:greekLit:tlg0033.tlg004"/>
        <rdfs:seeAlso rdf:resource="https://catalog.perseus.org/catalog/urn:cts:greekLit:tlg0033.tlg003"/>
        <rdfs:seeAlso rdf:resource="https://catalog.perseus.org/catalog/urn:cts:greekLit:tlg0033.tlg001"/>
        <rdfs:seeAlso rdf:resource="https://catalog.perseus.org/catalog/urn:cts:greekLit:tlg0033.tlg002"/>
        <rdfs:seeAlso rdf:resource="https://www.trismegistos.org/author/690"/>
        <foaf:depiction rdf:resource="https://upload.wikimedia.org/wikipedia/commons/d/d7/VIII.1.a%2C_Pompeii._June_2017._Painted_panel_from_west_end_of_south_wall_of_enthroned_Pindar_with_lyre%2C_with_Muse_and_poetess.jpg"/>
    </owl:NamedIndividual>

    <owl:NamedIndividual rdf:about="#threnoi_simonides">
        <rdfs:label xml:lang="en">threnoi_simonides</rdfs:label>
        <skos:prefLabel xml:lang="en">threnoi_simonides</skos:prefLabel>
        <rdf:type rdf:resource="#Archaic_Lyric_Poem_in_ionic_or_in_doric_or_in_aeolic_dialect_performed_by_a_chorus_or_by_a_single_performer_dedicated_to_dead"/>
        <isWrittenBy rdf:resource="#simonides_ceus"/>    </owl:NamedIndividual>

    <owl:NamedIndividual rdf:about="#political_elegies_solon">
        <rdfs:label xml:lang="en">political_elegies_solon</rdfs:label>
        <skos:prefLabel xml:lang="en">political_elegies_solon</skos:prefLabel>
        <rdf:type rdf:resource="#Archaic_Lyric_Poem_only_in_ionic_dialect_in_elegiac_couplet_with_political_content"/>
        <isWrittenBy rdf:resource="#solon_atheniensis"/>    </owl:NamedIndividual>

    <owl:NamedIndividual rdf:about="#partheneia_bacchylides">
        <rdfs:label xml:lang="en">partheneia_bacchylides</rdfs:label>
        <skos:prefLabel xml:lang="en">partheneia_bacchylides</skos:prefLabel>
        <rdf:type rdf:resource="#Archaic_Lyric_Poem_in_ionic_or_in_doric_or_in_aeolic_dialect_performed_by_a_chorus_performed_by_a_maidens_chorus"/>
        <isWrittenBy rdf:resource="#bacchylides_ceus"/>    </owl:NamedIndividual>

    <owl:NamedIndividual rdf:about="#iambs_archilochus">
        <rdfs:label xml:lang="en">iambs_archilochus</rdfs:label>
        <skos:prefLabel xml:lang="en">iambs_archilochus</skos:prefLabel>
        <rdf:type rdf:resource="#Archaic_Lyric_Poem_only_in_ionic_dialect_in_iambic_or_trochaic_metre"/>
        <isWrittenBy rdf:resource="#archilochus_parius"/>    </owl:NamedIndividual>

    <owl:NamedIndividual rdf:about="#keos">
        <rdfs:label xml:lang="en">keos</rdfs:label>
        <skos:prefLabel xml:lang="en">keos</skos:prefLabel>
        <rdf:type rdf:resource="#Ancient_Location"/>
        <pleiadesCoordinates>37.61385947,24.3265549158</pleiadesCoordinates>
        <isBirthPlaceOf rdf:resource="#bacchylides_ceus"/>        <isBirthPlaceOf rdf:resource="#simonides_ceus"/>        <rdfs:seeAlso rdf:resource="https://pleiades.stoa.org/places/570348"/>
        <rdfs:seeAlso rdf:resource="https://en.wikipedia.org/wiki/Kea_(island)"/>
        <rdfs:seeAlso rdf:resource="https://topostext.org/place/376243IKeo"/>
        <rdfs:seeAlso rdf:resource="http://www.trismegistos.org/place/1032"/>
    </owl:NamedIndividual>

    <owl:NamedIndividual rdf:about="#epithalamia_sappho">
        <rdfs:label xml:lang="en">epithalamia_sappho</rdfs:label>
        <skos:prefLabel xml:lang="en">epithalamia_sappho</skos:prefLabel>
        <rdf:type rdf:resource="#Archaic_Lyric_Poem_in_ionic_or_in_doric_or_in_aeolic_dialect_performed_by_a_chorus_or_by_a_single_performer_dedicated_to_wedding_couple"/>
        <isWrittenBy rdf:resource="#sappho_lesbia"/>    </owl:NamedIndividual>

    <owl:NamedIndividual rdf:about="#stesichorus_himeraeus">
        <rdfs:label xml:lang="en">stesichorus_himeraeus</rdfs:label>
        <skos:prefLabel xml:lang="en">stesichorus_himeraeus</skos:prefLabel>
        <rdf:type rdf:resource="#Archaic_Lyric_Poet"/>
        <skos:note>Από Pirizz at Ιταλικά Βικιπαίδεια - Stesichorus - Bellini Garden, Catania, Italy - September 2010. Transferred from it.wikipedia to Commons by OrbiliusMagister., Κοινό Κτήμα, https:commons.wikimedia.orgwindex.php?curid=12861189</skos:note>
        <passageChosenEn rdf:datatype="http://www.w3.org/2001/XMLSchema#string">Stesichorus,_fr._192_tr._Campbell:_That_story_is_not_true,_and_you_did_not_go_on_the_well-benched_ships_and_you_did_not_reach_the_citadel_of_Troy;_(Campbell,_D._A._(n.d.)._Stesichorus,_ΕΛΕΝΑ:_ΠΑΛΙΝΩΙΔΙΑΙ._Loeb_Classical_Library._Retrieved_5_May_2024,_from_https:www.loebclassics.comviewstesichorus_i-fragments1991pb_LCL476.93.xml)'_tlgIdentifyingNumber:_'tlg0292</passageChosenEn>
        <tlgIdentifyingNumber>tlg0292</tlgIdentifyingNumber>
        <passageChoselEl rdf:datatype="http://www.w3.org/2001/XMLSchema#string">Στησίχορος,_απ._192_Page_μετ._Ι.Ν._Καζάζης:_Δεν_αληθεύει_αυτή_η_ιστορία·_ούτε_σε_καράβια_καλοσκάμνιστα_μπήκες_εσύ_ποτέ,_ούτε_έφτασες_στης_Τροίας_την_ακρόπολη._(Τσέλικας,_Σ._(επ.)._ΣΤΗΣΙΧΟΡΟΣ:_απ._192_Page._Ανθολογία_Αρχαϊκής_Λυρικής_Ποίησης._Ανακτήθηκε_4_Μαΐου_2024,_από_https:www.greek-language.grdigitalResourcesancient_greekanthologypoetrybrowse.html?text_id=199)</passageChoselEl>
        <hasWritten rdf:resource="#choral_stesichorus"/>        <centuryOfLiving rdf:resource="#6th_century_BCE"/>        <centuryOfLiving rdf:resource="#7th_century_BCE"/>        <bornIn rdf:resource="#himera"/>        <foaf:depiction rdf:resource="https://upload.wikimedia.org/wikipedia/commons/e/e5/Stesichorus.jpg"/>
        <rdfs:seeAlso rdf:resource="https://www.perseus.tufts.edu/hopper/text?doc=PersEnc+S.stesichorus"/>
        <rdfs:seeAlso rdf:resource="https://catalog.perseus.tufts.edu/catalog/urn:cts:greekLit:tlg0292.tlg001.opp-grc3"/>
        <rdfs:seeAlso rdf:resource="https://catalog.perseus.tufts.edu/catalog/urn:cite:perseus:author.1328"/>
        <rdfs:seeAlso rdf:resource="https://www.loebclassics.com/view/stesichorus_i-fragments/1991/pb_LCL476.61.xml?readMode=recto"/>
        <rdfs:seeAlso rdf:resource="https://en.wikipedia.org/wiki/Stesichorus"/>
        <rdfs:seeAlso rdf:resource="https://www.britannica.com/biography/Stesichorus"/>
        <rdfs:seeAlso rdf:resource="https://classics-at.chs.harvard.edu/classics6-evanthia-tsitsibakou-vasalos-stesichorus-%E1%BC%B0%CE%BB%CE%B9%CE%BF%CF%85-%CF%80%CE%B5%CF%81%CF%83%CE%B9%CF%82-and-the-epic-tradition/"/>
        <rdfs:seeAlso rdf:resource="https://topostext.org/people/695"/>
    </owl:NamedIndividual>

    <owl:NamedIndividual rdf:about="#iambs_semonides">
        <rdfs:label xml:lang="en">iambs_semonides</rdfs:label>
        <skos:prefLabel xml:lang="en">iambs_semonides</skos:prefLabel>
        <rdf:type rdf:resource="#Archaic_Lyric_Poem_only_in_ionic_dialect_in_iambic_or_trochaic_metre"/>
        <isWrittenBy rdf:resource="#semonides_amorginus"/>    </owl:NamedIndividual>

    <owl:NamedIndividual rdf:about="#sympotic_odes_anacreon">
        <rdfs:label xml:lang="en">sympotic_odes_anacreon</rdfs:label>
        <skos:prefLabel xml:lang="en">sympotic_odes_anacreon</skos:prefLabel>
        <rdf:type rdf:resource="#Archaic_Lyric_Poem_in_ionic_or_in_doric_or_in_aeolic_dialect_performed_by_a_single_performer"/>
        <isWrittenBy rdf:resource="#anacreon_teius"/>    </owl:NamedIndividual>

    <owl:NamedIndividual rdf:about="#ananius_iambographus">
        <rdfs:label xml:lang="en">ananius_iambographus</rdfs:label>
        <skos:prefLabel xml:lang="en">ananius_iambographus</skos:prefLabel>
        <rdf:type rdf:resource="#Archaic_Lyric_Poet"/>
        <tlgIdentifyingNumber>tlg0238</tlgIdentifyingNumber>
        <hasWritten rdf:resource="#iambs_ananius"/>        <centuryOfLiving rdf:resource="#6th_century_BCE"/>        <rdfs:seeAlso rdf:resource="https://en.wikipedia.org/wiki/Ananius"/>
        <rdfs:seeAlso rdf:resource="https://catalog.perseus.org/catalog/urn:cite:perseus:author.85"/>
        <rdfs:seeAlso rdf:resource="https://www.wikidata.org/wiki/Q3615044"/>
        <rdfs:seeAlso rdf:resource="https://www.perseus.tufts.edu/hopper/text.jsp?doc=Perseus%3Atext%3A1999.04.0104%3Aalphabetic+letter%3DA%3Aentry+group%3D21%3Aentry%3Dananius-bio-1"/>
        <rdfs:seeAlso rdf:resource="https://catalog.perseus.org/catalog/urn:cts:greekLit:tlg0238.tlg001"/>
        <rdfs:seeAlso rdf:resource="https://quod.lib.umich.edu/cgi/t/text/pageviewer-idx?c=moa;cc=moa;rgn=full%20text;idno=ACL3129.0001.001;didno=ACL3129.0001.001;view=image;seq=00000173"/>
    </owl:NamedIndividual>

    <owl:NamedIndividual rdf:about="#sardis">
        <rdfs:label xml:lang="en">sardis</rdfs:label>
        <skos:prefLabel xml:lang="en">sardis</skos:prefLabel>
        <rdf:type rdf:resource="#Ancient_Location"/>
        <pleiadesCoordinates>38.488314,28.040286</pleiadesCoordinates>
        <isBirthPlaceOf rdf:resource="#alcman_lacedaemonius"/>        <rdfs:seeAlso rdf:resource="https://pleiades.stoa.org/places/550867"/>
        <rdfs:seeAlso rdf:resource="https://en.wikipedia.org/wiki/Sardis"/>
        <rdfs:seeAlso rdf:resource="https://topostext.org/place/385280PSar"/>
        <rdfs:seeAlso rdf:resource="http://www.perseus.tufts.edu/hopper/text?doc=Perseus%3Atext%3A1999.04.0064%3Aalphabetic+letter%3DS%3Aentry+group%3D5%3Aentry%3Dsardes-geo"/>
        <rdfs:seeAlso rdf:resource="http://www.geonames.org/9986360/sardes.html"/>
        <rdfs:seeAlso rdf:resource="https://www.trismegistos.org/place/2090"/>
    </owl:NamedIndividual>

    <owl:NamedIndividual rdf:about="#rhegium">
        <rdfs:label xml:lang="en">rhegium</rdfs:label>
        <skos:prefLabel xml:lang="en">rhegium</skos:prefLabel>
        <rdf:type rdf:resource="#Ancient_Location"/>
        <pleiadesCoordinates>38.109279,15.64393</pleiadesCoordinates>
        <isBirthPlaceOf rdf:resource="#ibycus_rheginus"/>        <rdfs:seeAlso rdf:resource="https://pleiades.stoa.org/places/452416"/>
        <rdfs:seeAlso rdf:resource="https://en.wikipedia.org/wiki/Reggio_Calabria"/>
        <rdfs:seeAlso rdf:resource="https://topostext.org/place/381156PRhe"/>
    </owl:NamedIndividual>

    <owl:NamedIndividual rdf:about="#warlike_odes_alcaeus">
        <rdfs:label xml:lang="en">warlike_odes_alcaeus</rdfs:label>
        <skos:prefLabel xml:lang="en">warlike_odes_alcaeus</skos:prefLabel>
        <rdf:type rdf:resource="#Archaic_Lyric_Poem_in_ionic_or_in_doric_or_in_aeolic_dialect_performed_by_a_single_performer"/>
        <isWrittenBy rdf:resource="#alcaeus_lesbius"/>    </owl:NamedIndividual>

    <owl:NamedIndividual rdf:about="#hyporchemes_pindarus">
        <rdfs:label xml:lang="en">hyporchemes_pindarus</rdfs:label>
        <skos:prefLabel xml:lang="en">hyporchemes_pindarus</skos:prefLabel>
        <rdf:type rdf:resource="#Archaic_Lyric_Poem_in_ionic_or_in_doric_or_in_aeolic_dialect_performed_by_a_chorus_with_imitation_expressions"/>
        <isWrittenBy rdf:resource="#pindarus_boeotus"/>    </owl:NamedIndividual>

    <owl:NamedIndividual rdf:about="#hymns_anacreon">
        <rdfs:label xml:lang="en">hymns_anacreon</rdfs:label>
        <skos:prefLabel xml:lang="en">hymns_anacreon</skos:prefLabel>
        <rdf:type rdf:resource="#Archaic_Lyric_Poem_in_ionic_or_in_doric_or_in_aeolic_dialect_performed_by_a_chorus_or_by_a_single_performer_dedicated_to_a_god"/>
        <isWrittenBy rdf:resource="#anacreon_teius"/>    </owl:NamedIndividual>

    <owl:NamedIndividual rdf:about="#himera">
        <rdfs:label xml:lang="en">himera</rdfs:label>
        <skos:prefLabel xml:lang="en">himera</skos:prefLabel>
        <rdf:type rdf:resource="#Ancient_Location"/>
        <pleiadesCoordinates>37.9698366164,13.8223437955</pleiadesCoordinates>
        <isBirthPlaceOf rdf:resource="#stesichorus_himeraeus"/>        <rdfs:seeAlso rdf:resource="https://pleiades.stoa.org/places/462244"/>
        <rdfs:seeAlso rdf:resource="https://topostext.org/place/380138PHim"/>
        <rdfs:seeAlso rdf:resource="https://en.wikipedia.org/wiki/Himera"/>
        <rdfs:seeAlso rdf:resource="https://www.wikidata.org/wiki/Q1111219"/>
        <rdfs:seeAlso rdf:resource="https://www.trismegistos.org/place/33123"/>
    </owl:NamedIndividual>

    <owl:NamedIndividual rdf:about="#hymns_alcaeus">
        <rdfs:label xml:lang="en">hymns_alcaeus</rdfs:label>
        <skos:prefLabel xml:lang="en">hymns_alcaeus</skos:prefLabel>
        <rdf:type rdf:resource="#Archaic_Lyric_Poem_in_ionic_or_in_doric_or_in_aeolic_dialect_performed_by_a_chorus_or_by_a_single_performer_dedicated_to_a_god"/>
        <isWrittenBy rdf:resource="#alcaeus_lesbius"/>    </owl:NamedIndividual>

    <owl:NamedIndividual rdf:about="#teos">
        <rdfs:label xml:lang="en">teos</rdfs:label>
        <skos:prefLabel xml:lang="en">teos</skos:prefLabel>
        <rdf:type rdf:resource="#Ancient_Location"/>
        <pleiadesCoordinates>38.185491,26.785397</pleiadesCoordinates>
        <isBirthPlaceOf rdf:resource="#anacreon_teius"/>        <rdfs:seeAlso rdf:resource="https://pleiades.stoa.org/places/550913"/>
        <rdfs:seeAlso rdf:resource="https://en.wikipedia.org/wiki/Teos"/>
        <rdfs:seeAlso rdf:resource="https://topostext.org/place/382268PTeo"/>
        <rdfs:seeAlso rdf:resource="http://www.trismegistos.org/place/2314"/>
    </owl:NamedIndividual>

    <owl:NamedIndividual rdf:about="#dithyrambs_pindarus">
        <rdfs:label xml:lang="en">dithyrambs_pindarus</rdfs:label>
        <skos:prefLabel xml:lang="en">dithyrambs_pindarus</skos:prefLabel>
        <rdf:type rdf:resource="#Archaic_Lyric_Poem_in_ionic_or_in_doric_or_in_aeolic_dialect_performed_by_a_chorus_or_by_a_single_performer_dedicated_to_dionysus"/>
        <isWrittenBy rdf:resource="#pindarus_boeotus"/>    </owl:NamedIndividual>

    <owl:NamedIndividual rdf:about="#theognis_megarensis">
        <rdfs:label xml:lang="en">theognis_megarensis</rdfs:label>
        <skos:prefLabel xml:lang="en">theognis_megarensis</skos:prefLabel>
        <rdf:type rdf:resource="#Archaic_Lyric_Poet"/>
        <skos:note>By Mitteilungen des Deutschen Archäologischen Instituts, Athenische Abteilung - A kylix from Tanagra, Boeotia, 5th century B.C. A symposiast sings ὦ παίδων κάλλιστε, the beginning of a verse by Theognis https:archive.orgstreammitteilungen09deut#page392mode2up, Public Domain, https:commons.wikimedia.orgwindex.php?curid=7774895</skos:note>
        <passageChosenEn rdf:datatype="http://www.w3.org/2001/XMLSchema#string">The_Elegiac_Poems_of_Theognis,_Book_I,_237-254_trans._Edmonds:_I_have_given_thee_wings_to_fly_with_ease_aloft_the_boundless_sea_and_all_the_land._No_meal_or_feast_but_thou''lt_be_there,_couched_''twixt_the_lips_of_many_a_guest,_and_lovely_youths_shall_sing_thee_clear_and_well_in_orderly_wise_to_the_clear-voiced_flute._And_when_thou_comest_to_go_down_to_the_lamentable_house_of_Hades_in_the_depths_of_the_gloomy_earth,_never,_albeit_thou_be_dead,_shalt_thou_lose_thy_fame,_but_men_will_think_of_thee_as_one_of_immortal_name,_Cyrnus,_who_rangeth_the_land_of_Greece_and_the_isles_thereof_—crossing_the_fishy_unharvestable_deep_not_upon_horseback_mounted_but_sped_of_the_glorious_gifts_of_the_violet-crownad_Muses_unto_all_that_care_to_receive_thee;_and_living_as_they_thou_shalt_be_a_song_unto_posterity_so_long_as_Earth_and_Sun_abide._Yet_as_for_me,_thou_hast_no_respect_for_me,_great_or_small,_but_deceivest_me_with_words_as_if_I_were_a_little_child._(Edmonds,_J._M._(1931)._The_Elegiac_Poems_of_Theognis:_Book_I_in_Elegy_and_Iambus_[English_Translation]._Cambridge,_MA:_Harvard_University_Press._London:_William_Heinemann_Ltd._(Original_work_published_1931)._Retrieved_May_4,_2024,_from_https:www.perseus.tufts.eduhoppertext?doc=Perseus%3Atext%3A2008.01.0479%3Avolume%3D1%3Atext%3D11%3Asection%3D2#note1:~:text=assuredly%20be%20taken.-,237%2D254,-I%20have%20given)</passageChosenEn>
        <tlgIdentifyingNumber>tlg0002</tlgIdentifyingNumber>
        <passageChoselEl rdf:datatype="http://www.w3.org/2001/XMLSchema#string">Θέογνις,_Ελεγίαι_237-254_μετ._Μ._Ζ._Κοπιδάκης:_Κύρνε,_σου_χάρισα_φτερά_ανάλαφρα_να_σε_σηκώσουν_πάνω_από_την_απέραντη_θάλασσα_και_ολάκερη_την_οικουμένη._Παντού_σε_όλα_τα_συμπόσια_και_τις_γιορτές_θα_βρίσκεσαι_και_συ,_όλοι_τους_θα_᾽χουνε_για_σε_να_λένε._Παίζοντας_μικρούς_γλυκόλαλους_αυλούς_άντρες_ερωτικοί_θα_τραγουδούν_για_σένα_ωραία_και_τρυφερά_τραγούδια._Κι_όταν_στα_σπλάχνα_της_μαύρης_γης_θα_κατεβείς,_όταν_θα_φτάσεις_στο_πολυστέναχτο_παλάτι_του_Άδη,_ούτε_και_τότε,_αν_και_νεκρός,_θα_ξεχαστείς._Όλοι_θα_σε_θυμούνται,_αθάνατο_θα_᾽ναι_στους_ανθρώπους_το_όνομά_σου._Κύρνε,_στη_γη_της_Ελλάδας_θα_τριγυρνάς_και_στα_νησιά,_πάνω_από_την_άκαρπη_θάλασσα,_όπου_ζουν_τα_ψάρια,_θα_περνοδιαβαίνεις._Δεν_θα_᾽σαι_σε_άλογα_καβάλα,_τα_λαμπρά_δώρα_των_Μουσών,_που_έχουν_στεφάνια_από_μενεξέδες_στα_μαλλιά,_αυτά_θα_σε_ταξιδεύουν._Θα_᾽σαι_στη_συντροφιά_όσων_και_τώρα_και_στους_αιώνες_που_᾽ρχονται_αγαπούνε_το_τραγούδι_-ώσπου_θα_στέκει_η_γη_και_ο_ήλιος_θα_φωτίζει._Μα_ούτε_τόσο_δα_δεν_με_προσέχεις,_και_σαν_μικρό_παιδί_με_υποσχέσεις_ανεκπλήρωτες_με_ξεγελάς._(Στεφανόπουλου,_Θ._Κ.,_Τσιτσιρίδη,_Στ.,_Αντζουλή,_Λ.,_&amp;_Κριτσέλη,_Γ._(χ.χ.)._ΘΕΟΓΝΙΣ:_30._–_«Ἐλεγεῖαι»_237-254._Ανθολογία_Αρχαίας_Ελληνικής_Γραμματείας._Ανακτήθηκε_4_Μαΐου_2024,_από_https:www.greek-language.grdigitalResourcesancient_greekanthologyliteraturebrowse.html?text_id=50)</passageChoselEl>
        <hasWritten rdf:resource="#gnomic_elegies_theognis"/>        <centuryOfLiving rdf:resource="#6th_century_BCE"/>        <bornIn rdf:resource="#megara"/>        <foaf:depiction rdf:resource="https://upload.wikimedia.org/wikipedia/commons/7/7f/Tanagra%2C_5th_century_kylix_a_symposiast_sings_Theognis_o_paidon_kalliste.png"/>
        <rdfs:seeAlso rdf:resource="https://www.perseus.tufts.edu/hopper/text?doc=Perseus%3Atext%3A2008.01.0479%3Avolume%3D1%3Atext%3D11%3Asection%3D2"/>
        <rdfs:seeAlso rdf:resource="https://www.perseus.tufts.edu/hopper/text?doc=Perseus%3Atext%3A2008.01.0479%3Avolume%3D1%3Atext%3D11%3Asection%3D1"/>
        <rdfs:seeAlso rdf:resource="https://catalog.perseus.org/catalog/urn:cts:greekLit:tlg0002.tlg001"/>
        <rdfs:seeAlso rdf:resource="https://catalog.perseus.org/catalog/urn:cts:greekLit:tlg0002.tlg004"/>
        <rdfs:seeAlso rdf:resource="https://catalog.perseus.org/?f%5Btg_facet%5D%5B%5D=Theognis&amp;f%5Bwork_lang%5D%5B%5D=grc&amp;q=tg_no_token%3A%5BT+TO+U%5D&amp;sort=title_display+asc"/>
        <rdfs:seeAlso rdf:resource="https://www.perseus.tufts.edu/hopper/text?doc=Perseus%3Atext%3A1999.04.0104%3Aalphabetic+letter%3DT%3Aentry+group%3D11%3Aentry%3Dtheognis-bio-1"/>
        <rdfs:seeAlso rdf:resource="https://en.wikipedia.org/wiki/Theognis_of_Megara"/>
        <rdfs:seeAlso rdf:resource="https://www.wikidata.org/wiki/Q336115"/>
    </owl:NamedIndividual>

    <owl:NamedIndividual rdf:about="#athens">
        <rdfs:label xml:lang="en">athens</rdfs:label>
        <skos:prefLabel xml:lang="en">athens</skos:prefLabel>
        <rdf:type rdf:resource="#Ancient_Location"/>
        <pleiadesCoordinates>37.9718132251,23.7235488821</pleiadesCoordinates>
        <residentedBy rdf:resource="#anacreon_teius"/>        <residentedBy rdf:resource="#simonides_ceus"/>        <residentedBy rdf:resource="#pindarus_boeotus"/>        <isBirthPlaceOf rdf:resource="#solon_atheniensis"/>        <rdfs:seeAlso rdf:resource="https://pleiades.stoa.org/places/579885"/>
        <rdfs:seeAlso rdf:resource="https://topostext.org/place/380237PAth"/>
        <rdfs:seeAlso rdf:resource="https://en.wikipedia.org/wiki/Athens"/>
        <rdfs:seeAlso rdf:resource="https://www.wikidata.org/wiki/Q1524"/>
        <rdfs:seeAlso rdf:resource="http://www.trismegistos.org/place/364"/>
        <rdfs:seeAlso rdf:resource="http://www.geonames.org/264371/athens.html"/>
    </owl:NamedIndividual>

    <owl:NamedIndividual rdf:about="#sympotic_odes_alcaeus">
        <rdfs:label xml:lang="en">sympotic_odes_alcaeus</rdfs:label>
        <skos:prefLabel xml:lang="en">sympotic_odes_alcaeus</skos:prefLabel>
        <rdf:type rdf:resource="#Archaic_Lyric_Poem_in_ionic_or_in_doric_or_in_aeolic_dialect_performed_by_a_single_performer"/>
        <isWrittenBy rdf:resource="#alcaeus_lesbius"/>    </owl:NamedIndividual>

    <owl:NamedIndividual rdf:about="#aegypt">
        <rdfs:label xml:lang="en">aegypt</rdfs:label>
        <skos:prefLabel xml:lang="en">aegypt</skos:prefLabel>
        <rdf:type rdf:resource="#Ancient_Location"/>
        <pleiadesCoordinates>16.1010829332,31.4591482445</pleiadesCoordinates>
        <residentedBy rdf:resource="#alcaeus_lesbius"/>        <rdfs:seeAlso rdf:resource="https://pleiades.stoa.org/places/981503"/>
        <rdfs:seeAlso rdf:resource="https://en.wikipedia.org/wiki/Ancient_Egypt"/>
        <rdfs:seeAlso rdf:resource="https://www.trismegistos.org/place/49"/>
    </owl:NamedIndividual>

    <owl:NamedIndividual rdf:about="#choral_stesichorus">
        <rdfs:label xml:lang="en">choral_stesichorus</rdfs:label>
        <skos:prefLabel xml:lang="en">choral_stesichorus</skos:prefLabel>
        <rdf:type rdf:resource="#Archaic_Lyric_Poem_in_ionic_or_in_doric_or_in_aeolic_dialect_performed_by_a_chorus"/>
        <isWrittenBy rdf:resource="#stesichorus_himeraeus"/>    </owl:NamedIndividual>

    <owl:NamedIndividual rdf:about="#erotic_elegies_mimnermus">
        <rdfs:label xml:lang="en">erotic_elegies_mimnermus</rdfs:label>
        <skos:prefLabel xml:lang="en">erotic_elegies_mimnermus</skos:prefLabel>
        <rdf:type rdf:resource="#Archaic_Lyric_Poem_only_in_ionic_dialect_in_elegiac_couplet_with_erotic_content"/>
        <isWrittenBy rdf:resource="#mimnermus_lyricus"/>    </owl:NamedIndividual>

    <owl:NamedIndividual rdf:about="#thasos_settlement">
        <rdfs:label xml:lang="en">thasos_settlement</rdfs:label>
        <skos:prefLabel xml:lang="en">thasos_settlement</skos:prefLabel>
        <rdf:type rdf:resource="#Ancient_Location"/>
        <pleiadesCoordinates>40.78201,24.717535</pleiadesCoordinates>
        <residentedBy rdf:resource="#archilochus_parius"/>        <rdfs:seeAlso rdf:resource="https://pleiades.stoa.org/places/501634"/>
        <rdfs:seeAlso rdf:resource="https://topostext.org/place/408247PTha"/>
        <rdfs:seeAlso rdf:resource="http://www.perseus.tufts.edu/hopper/text?doc=Perseus:text:1999.04.0006"/>
        <rdfs:seeAlso rdf:resource="https://www.geonames.org/6633834/thasos.html"/>
        <rdfs:seeAlso rdf:resource="https://www.trismegistos.org/place/2346"/>
    </owl:NamedIndividual>

    <owl:NamedIndividual rdf:about="#5th_century_BCE">
        <rdfs:label xml:lang="en">5th_century_BCE</rdfs:label>
        <skos:prefLabel xml:lang="en">5th_century_BCE</skos:prefLabel>
        <rdf:type rdf:resource="#BCE_century"/>
        <startsIn rdf:datatype="http://www.w3.org/2001/XMLSchema#decimal">-499</startsIn>
        <endsIn rdf:datatype="http://www.w3.org/2001/XMLSchema#decimal">-400</endsIn>
        <isCenturyOf rdf:resource="#pindarus_boeotus"/>        <isCenturyOf rdf:resource="#bacchylides_ceus"/>        <isCenturyOf rdf:resource="#simonides_ceus"/>    </owl:NamedIndividual>

    <owl:NamedIndividual rdf:about="#samos">
        <rdfs:label xml:lang="en">samos</rdfs:label>
        <skos:prefLabel xml:lang="en">samos</skos:prefLabel>
        <rdf:type rdf:resource="#Ancient_Location"/>
        <pleiadesCoordinates>37.7324600706,26.8391253467</pleiadesCoordinates>
        <residentedBy rdf:resource="#ibycus_rheginus"/>        <residentedBy rdf:resource="#anacreon_teius"/>        <isBirthPlaceOf rdf:resource="#semonides_amorginus"/>        <rdfs:seeAlso rdf:resource="https://pleiades.stoa.org/places/599926"/>
        <rdfs:seeAlso rdf:resource="http://www.trismegistos.org/place/2081"/>
        <rdfs:seeAlso rdf:resource="https://www.wikidata.org/wiki/Q156882"/>
        <rdfs:seeAlso rdf:resource="https://topostext.org/place/377269PSam"/>
    </owl:NamedIndividual>

    <owl:NamedIndividual rdf:about="#gnomic_elegies_theognis">
        <rdfs:label xml:lang="en">gnomic_elegies_theognis</rdfs:label>
        <skos:prefLabel xml:lang="en">gnomic_elegies_theognis</skos:prefLabel>
        <rdf:type rdf:resource="#Archaic_Lyric_Poem_only_in_ionic_dialect_in_elegiac_couplet_with_gnomic_content"/>
        <isWrittenBy rdf:resource="#theognis_megarensis"/>    </owl:NamedIndividual>

    <owl:NamedIndividual rdf:about="#simonides_ceus">
        <rdfs:label xml:lang="en">simonides_ceus</rdfs:label>
        <skos:prefLabel xml:lang="en">simonides_ceus</skos:prefLabel>
        <rdf:type rdf:resource="#Archaic_Lyric_Poet"/>
        <skos:note>By Michel Wolgemut, Wilhelm Pleydenwurff; Text: Hartmann Schedel - Imaginary portrait of Simonides from the Nuremberg Chronicle (1493)
Self-scanned, Public Domain, https:commons.wikimedia.orgwindex.php?curid=1129423</skos:note>
        <tlgIdentifyingNumber>tlg0261</tlgIdentifyingNumber>
        <hasWritten rdf:resource="#elegies_simonides"/>        <hasWritten rdf:resource="#dithyrambs_simonides"/>        <hasWritten rdf:resource="#epinikoi_simonides"/>        <hasWritten rdf:resource="#threnoi_simonides"/>        <centuryOfLiving rdf:resource="#5th_century_BCE"/>        <centuryOfLiving rdf:resource="#6th_century_BCE"/>        <bornIn rdf:resource="#keos"/>        <stayedIn rdf:resource="#athens"/>        <stayedIn rdf:resource="#sicilia"/>        <foaf:depiction rdf:resource="https://upload.wikimedia.org/wikipedia/commons/2/2e/Nuremberg_chronicles_f_60r_3.png"/>
        <rdfs:seeAlso rdf:resource="https://www.perseus.tufts.edu/hopper/text?doc=Perseus%3Atext%3A1999.04.0004%3Aentry%3Dsimonides"/>
        <rdfs:seeAlso rdf:resource="https://catalog.perseus.org/catalog/urn:cite:perseus:author.1292"/>
        <rdfs:seeAlso rdf:resource="https://www.perseus.tufts.edu/hopper/text?doc=Perseus%3Atext%3A2008.01.0480%3Avolume%3D2%3Atext%3D22"/>
        <rdfs:seeAlso rdf:resource="https://catalog.perseus.org/?f%5Btg_facet%5D%5B%5D=Simonides&amp;q=tg_no_token%3A%5BS+TO+T%5D"/>
        <rdfs:seeAlso rdf:resource="https://anthologiagraeca.org/authors/22/"/>
        <rdfs:seeAlso rdf:resource="https://www.wikidata.org/wiki/Q273003"/>
        <rdfs:seeAlso rdf:resource="https://en.wikipedia.org/wiki/Simonides_of_Ceos"/>
    </owl:NamedIndividual>

    <owl:NamedIndividual rdf:about="#ibycus_rheginus">
        <rdfs:label xml:lang="en">ibycus_rheginus</rdfs:label>
        <skos:prefLabel xml:lang="en">ibycus_rheginus</skos:prefLabel>
        <rdf:type rdf:resource="#Archaic_Lyric_Poet"/>
        <skos:note>By Heinrich Schwemminger - The Cranes of Ibycus, by Heinrich Schwemminger, illustrating Schiller's poem of that name
https:digital.belvedere.atobjects2534die-kraniche-des-ibykus, Public Domain, https:commons.wikimedia.orgwindex.php?curid=74330706</skos:note>
        <tlgIdentifyingNumber>tlg0293</tlgIdentifyingNumber>
        <hasWritten rdf:resource="#choral_ibycus"/>        <hasWritten rdf:resource="#enkomion_ibycus"/>        <centuryOfLiving rdf:resource="#6th_century_BCE"/>        <bornIn rdf:resource="#rhegium"/>        <stayedIn rdf:resource="#samos"/>        <foaf:depiction rdf:resource="https://upload.wikimedia.org/wikipedia/commons/d/de/Heinrich_Schwemminger_-_Die_Kraniche_des_Ibykus_-_3739_-_Kunsthistorisches_Museum.jpg"/>
        <rdfs:seeAlso rdf:resource="https://catalog.perseus.org/catalog/urn:cts:greekLit:tlg0293.tlg001.opp-eng1"/>
        <rdfs:seeAlso rdf:resource="https://catalog.perseus.org/catalog/urn:cite:perseus:author.760"/>
        <rdfs:seeAlso rdf:resource="https://quod.lib.umich.edu/cgi/t/text/pageviewer-idx?c=moa;cc=moa;rgn=full%20text;idno=ACL3129.0002.001;didno=ACL3129.0002.001;view=image;seq=00000567"/>
        <rdfs:seeAlso rdf:resource="https://en.wikipedia.org/wiki/Ibycus"/>
        <rdfs:seeAlso rdf:resource="https://web.archive.org/web/20120212233258/http://www.csad.ox.ac.uk/POXY/VExhibition/images/1790.jpg"/>
    </owl:NamedIndividual>

    <owl:NamedIndividual rdf:about="#hyporcheme_bacchylides">
        <rdfs:label xml:lang="en">hyporcheme_bacchylides</rdfs:label>
        <skos:prefLabel xml:lang="en">hyporcheme_bacchylides</skos:prefLabel>
        <rdf:type rdf:resource="#Archaic_Lyric_Poem_in_ionic_or_in_doric_or_in_aeolic_dialect_performed_by_a_chorus_with_imitation_expressions"/>
        <isWrittenBy rdf:resource="#bacchylides_ceus"/>    </owl:NamedIndividual>

    <owl:NamedIndividual rdf:about="#epinikoi_pindarus">
        <rdfs:label xml:lang="en">epinikoi_pindarus</rdfs:label>
        <skos:prefLabel xml:lang="en">epinikoi_pindarus</skos:prefLabel>
        <rdf:type rdf:resource="#Archaic_Lyric_Poem_in_ionic_or_in_doric_or_in_aeolic_dialect_performed_by_a_chorus_or_by_a_single_performer_dedicated_to_winners_in_athletic_events"/>
        <isWrittenBy rdf:resource="#pindarus_boeotus"/>    </owl:NamedIndividual>

    <owl:NamedIndividual rdf:about="#6th_century_BCE">
        <rdfs:label xml:lang="en">6th_century_BCE</rdfs:label>
        <skos:prefLabel xml:lang="en">6th_century_BCE</skos:prefLabel>
        <rdf:type rdf:resource="#BCE_century"/>
        <startsIn rdf:datatype="http://www.w3.org/2001/XMLSchema#decimal">-599</startsIn>
        <endsIn rdf:datatype="http://www.w3.org/2001/XMLSchema#decimal">-500</endsIn>
        <isCenturyOf rdf:resource="#alcaeus_lesbius"/>        <isCenturyOf rdf:resource="#anacreon_teius"/>        <isCenturyOf rdf:resource="#pindarus_boeotus"/>        <isCenturyOf rdf:resource="#sappho_lesbia"/>        <isCenturyOf rdf:resource="#ananius_iambographus"/>        <isCenturyOf rdf:resource="#stesichorus_himeraeus"/>        <isCenturyOf rdf:resource="#theognis_megarensis"/>        <isCenturyOf rdf:resource="#solon_atheniensis"/>        <isCenturyOf rdf:resource="#ibycus_rheginus"/>        <isCenturyOf rdf:resource="#phocylides_milesius"/>        <isCenturyOf rdf:resource="#hipponax_ephesius"/>        <isCenturyOf rdf:resource="#bacchylides_ceus"/>        <isCenturyOf rdf:resource="#simonides_ceus"/>    </owl:NamedIndividual>

    <owl:NamedIndividual rdf:about="#epinikoi_bacchylides">
        <rdfs:label xml:lang="en">epinikoi_bacchylides</rdfs:label>
        <skos:prefLabel xml:lang="en">epinikoi_bacchylides</skos:prefLabel>
        <rdf:type rdf:resource="#Archaic_Lyric_Poem_in_ionic_or_in_doric_or_in_aeolic_dialect_performed_by_a_chorus_or_by_a_single_performer_dedicated_to_winners_in_athletic_events"/>
        <isWrittenBy rdf:resource="#bacchylides_ceus"/>    </owl:NamedIndividual>

    <owl:NamedIndividual rdf:about="#abdera">
        <rdfs:label xml:lang="en">abdera</rdfs:label>
        <skos:prefLabel xml:lang="en">abdera</skos:prefLabel>
        <rdf:type rdf:resource="#Ancient_Location"/>
        <pleiadesCoordinates>40.9328277487,24.9743082598</pleiadesCoordinates>
        <residentedBy rdf:resource="#anacreon_teius"/>        <rdfs:seeAlso rdf:resource="https://pleiades.stoa.org/places/501323"/>
        <rdfs:seeAlso rdf:resource="https://topostext.org/place/410250PAbd"/>
        <rdfs:seeAlso rdf:resource="http://www.trismegistos.org/place/14"/>
        <rdfs:seeAlso rdf:resource="http://www.perseus.tufts.edu/hopper/text?doc=Perseus%3Atext%3A1999.04.0064%3Aalphabetic+letter%3DA%3Aentry+group%3D1%3Aentry%3Dabdera-geo"/>
        <rdfs:seeAlso rdf:resource="http://www.perseus.tufts.edu/hopper/text?doc=Perseus:text:1999.04.0006:entry=abdera"/>
    </owl:NamedIndividual>

    <owl:NamedIndividual rdf:about="#paeans_alcman">
        <rdfs:label xml:lang="en">paeans_alcman</rdfs:label>
        <skos:prefLabel xml:lang="en">paeans_alcman</skos:prefLabel>
        <rdf:type rdf:resource="#Archaic_Lyric_Poem_in_ionic_or_in_doric_or_in_aeolic_dialect_performed_by_a_chorus_or_by_a_single_performer_dedicated_to_apollo"/>
        <isWrittenBy rdf:resource="#alcman_lacedaemonius"/>    </owl:NamedIndividual>

    <owl:NamedIndividual rdf:about="#iambs_anacreon">
        <rdfs:label xml:lang="en">iambs_anacreon</rdfs:label>
        <skos:prefLabel xml:lang="en">iambs_anacreon</skos:prefLabel>
        <rdf:type rdf:resource="#Archaic_Lyric_Poem_only_in_ionic_dialect_in_iambic_or_trochaic_metre"/>
        <isWrittenBy rdf:resource="#anacreon_teius"/>    </owl:NamedIndividual>

    <owl:NamedIndividual rdf:about="#hymns_terpander">
        <rdfs:label xml:lang="en">hymns_terpander</rdfs:label>
        <skos:prefLabel xml:lang="en">hymns_terpander</skos:prefLabel>
        <rdf:type rdf:resource="#Archaic_Lyric_Poem_in_ionic_or_in_doric_or_in_aeolic_dialect_performed_by_a_chorus_or_by_a_single_performer_dedicated_to_a_god"/>
        <isWrittenBy rdf:resource="#terpander_lesbius"/>    </owl:NamedIndividual>

    <owl:NamedIndividual rdf:about="#hipponax_ephesius">
        <rdfs:label xml:lang="en">hipponax_ephesius</rdfs:label>
        <skos:prefLabel xml:lang="en">hipponax_ephesius</skos:prefLabel>
        <rdf:type rdf:resource="#Archaic_Lyric_Poet"/>
        <skos:note>By Published by Guillaume Rouille(1518?-1589) - Hipponax of Ephesus was an Ancient Greek iambic poet. "Promptuarii Iconum Insigniorum ", Public Domain, https:commons.wikimedia.orgwindex.php?curid=8660255</skos:note>
        <passageChosenEn rdf:datatype="http://www.w3.org/2001/XMLSchema#string">Hipponax,_fr._68_West:_Two_days_are_sweetest_for_a_woman,_the_day_a_man_marries_her_and_the_day_he_carries_her_out_dead._(Hawkins,_L._(n.d.)._Hipponax_&amp;_Misogyny_in_Ancient_Greece._World_History_Encyclopedia._Retrieved_5_May_2024,_from_https:www.worldhistory.orgarticle188hipponax--misogyny-in-ancient-greece)</passageChosenEn>
        <tlgIdentifyingNumber>tlg0233</tlgIdentifyingNumber>
        <passageChoselEl rdf:datatype="http://www.w3.org/2001/XMLSchema#string">Ιππώναξ,_απ._68_West_μετ._Σ._Μενάρδος:_Δυο_μέρες_της_γυναίκας_είν᾽_οι_πιο_γλυκές,_του_γάμου_η_μια_κι_η_άλλη…_της_κηδείας_της._(Τσέλικας,_Σ._(επ.)._ΙΠΠΩΝΑΞ:_απ._68_West._Ανθολογία_Αρχαϊκής_Λυρικής_Ποίησης._Ανακτήθηκε_4_Μαΐου_2024,_από_https:www.greek-language.grdigitalResourcesancient_greekanthologypoetrybrowse.html?text_id=122)</passageChoselEl>
        <hasWritten rdf:resource="#iambs_hipponax"/>        <centuryOfLiving rdf:resource="#6th_century_BCE"/>        <bornIn rdf:resource="#ephesus"/>        <stayedIn rdf:resource="#klazomenai"/>        <foaf:depiction rdf:resource="https://upload.wikimedia.org/wikipedia/commons/8/87/Hipponax_of_Ephesus.jpg"/>
        <rdfs:seeAlso rdf:resource="https://catalog.perseus.org/catalog/urn:cite:perseus:author.741"/>
        <rdfs:seeAlso rdf:resource="https://catalog.perseus.org/catalog/urn:cts:greekLit:tlg0233.tlg001"/>
        <rdfs:seeAlso rdf:resource="https://www.perseus.tufts.edu/hopper/text?doc=Perseus:text:1999.04.0104:entry=hipponax-bio-1"/>
        <rdfs:seeAlso rdf:resource="https://en.wikipedia.org/wiki/Hipponax"/>
        <rdfs:seeAlso rdf:resource="https://en.wikiquote.org/wiki/Hipponax"/>
    </owl:NamedIndividual>

    <owl:NamedIndividual rdf:about="#hymns_sappho">
        <rdfs:label xml:lang="en">hymns_sappho</rdfs:label>
        <skos:prefLabel xml:lang="en">hymns_sappho</skos:prefLabel>
        <rdf:type rdf:resource="#Archaic_Lyric_Poem_in_ionic_or_in_doric_or_in_aeolic_dialect_performed_by_a_chorus_or_by_a_single_performer_dedicated_to_a_god"/>
        <isWrittenBy rdf:resource="#sappho_lesbia"/>    </owl:NamedIndividual>

    <owl:NamedIndividual rdf:about="#hymns_archilochus">
        <rdfs:label xml:lang="en">hymns_archilochus</rdfs:label>
        <skos:prefLabel xml:lang="en">hymns_archilochus</skos:prefLabel>
        <rdf:type rdf:resource="#Archaic_Lyric_Poem_in_ionic_or_in_doric_or_in_aeolic_dialect_performed_by_a_chorus_or_by_a_single_performer_dedicated_to_a_god"/>
        <isWrittenBy rdf:resource="#archilochus_parius"/>    </owl:NamedIndividual>

    <owl:NamedIndividual rdf:about="#hymenaios_sappho">
        <rdfs:label xml:lang="en">hymenaios_sappho</rdfs:label>
        <skos:prefLabel xml:lang="en">hymenaios_sappho</skos:prefLabel>
        <rdf:type rdf:resource="#Archaic_Lyric_Poem_in_ionic_or_in_doric_or_in_aeolic_dialect_performed_by_a_chorus_during_bride_procession"/>
        <isWrittenBy rdf:resource="#sappho_lesbia"/>    </owl:NamedIndividual>

    <owl:NamedIndividual rdf:about="#erotic_odes_sappho">
        <rdfs:label xml:lang="en">erotic_odes_sappho</rdfs:label>
        <skos:prefLabel xml:lang="en">erotic_odes_sappho</skos:prefLabel>
        <rdf:type rdf:resource="#Archaic_Lyric_Poem_in_ionic_or_in_doric_or_in_aeolic_dialect_performed_by_a_single_performer"/>
        <isWrittenBy rdf:resource="#sappho_lesbia"/>    </owl:NamedIndividual>

    <owl:NamedIndividual rdf:about="#iambs_ananius">
        <rdfs:label xml:lang="en">iambs_ananius</rdfs:label>
        <skos:prefLabel xml:lang="en">iambs_ananius</skos:prefLabel>
        <rdf:type rdf:resource="#Archaic_Lyric_Poem_only_in_ionic_dialect_in_iambic_or_trochaic_metre"/>
        <isWrittenBy rdf:resource="#ananius_iambographus"/>    </owl:NamedIndividual>

    <owl:NamedIndividual rdf:about="#dithyrambs_bacchylides">
        <rdfs:label xml:lang="en">dithyrambs_bacchylides</rdfs:label>
        <skos:prefLabel xml:lang="en">dithyrambs_bacchylides</skos:prefLabel>
        <rdf:type rdf:resource="#Archaic_Lyric_Poem_in_ionic_or_in_doric_or_in_aeolic_dialect_performed_by_a_chorus_or_by_a_single_performer_dedicated_to_dionysus"/>
        <isWrittenBy rdf:resource="#bacchylides_ceus"/>    </owl:NamedIndividual>

    <owl:NamedIndividual rdf:about="#war_elegy_callinus">
        <rdfs:label xml:lang="en">war_elegy_callinus</rdfs:label>
        <skos:prefLabel xml:lang="en">war_elegy_callinus</skos:prefLabel>
        <rdf:type rdf:resource="#Archaic_Lyric_Poem_only_in_ionic_dialect_in_elegiac_couplet_with_war_content"/>
        <isWrittenBy rdf:resource="#callinus_ephesius"/>    </owl:NamedIndividual>

    <owl:NamedIndividual rdf:about="#bacchylides_ceus">
        <rdfs:label xml:lang="en">bacchylides_ceus</rdfs:label>
        <skos:prefLabel xml:lang="en">bacchylides_ceus</skos:prefLabel>
        <rdf:type rdf:resource="#Archaic_Lyric_Poet"/>
        <skos:note>By The Egypt Exploration Society - Bacchylides, Encomia fr. 5, preserved by a 1st-century BC or AD papyrus form Oxyrhynchus (P.Oxy. 1361 fr. 4). B.P. Grenfell &amp; A.S. Hunt, The Oxyrhycnhus Papyri: Part XI. (London: The Egypt Exploration Society, 1915), Public Domain, https:commons.wikimedia.orgwindex.php?curid=16001182</skos:note>
        <tlgIdentifyingNumber>tlg0199</tlgIdentifyingNumber>
        <hasWritten rdf:resource="#hyporcheme_bacchylides"/>        <hasWritten rdf:resource="#partheneia_bacchylides"/>        <hasWritten rdf:resource="#prosodia_bacchylides"/>        <hasWritten rdf:resource="#dithyrambs_bacchylides"/>        <hasWritten rdf:resource="#enkomion_bacchylides"/>        <hasWritten rdf:resource="#epinikoi_bacchylides"/>        <hasWritten rdf:resource="#paeans_bacchylides"/>        <centuryOfLiving rdf:resource="#5th_century_BCE"/>        <centuryOfLiving rdf:resource="#6th_century_BCE"/>        <bornIn rdf:resource="#keos"/>        <stayedIn rdf:resource="#syrakousai"/>        <rdfs:seeAlso rdf:resource="https://catalog.perseus.org/catalog/urn:cite:perseus:author.254"/>
        <rdfs:seeAlso rdf:resource="https://el.wikipedia.org/wiki/%CE%92%CE%B1%CE%BA%CF%87%CF%85%CE%BB%CE%AF%CE%B4%CE%B7%CF%82"/>
        <rdfs:seeAlso rdf:resource="https://en.wikipedia.org/wiki/Bacchylides"/>
        <rdfs:seeAlso rdf:resource="https://www.britannica.com/biography/Bacchylides"/>
        <rdfs:seeAlso rdf:resource="https://www.perseus.tufts.edu/hopper/text?doc=Perseus%3Atext%3A1999.01.0064%3Abook%3DEp"/>
        <rdfs:seeAlso rdf:resource="https://www.perseus.tufts.edu/hopper/text?doc=Perseus%3Atext%3A1999.01.0064%3Abook%3DDith%3Apoem%3D17"/>
        <rdfs:seeAlso rdf:resource="https://www.loebclassics.com/view/LCL461/1992/volume.xml"/>
        <rdfs:seeAlso rdf:resource="https://www.perseus.tufts.edu/hopper/collection?collection=Perseus%3Acorpus%3Aperseus%2Cwork%2CBacchylides%2C%20Epinicians"/>
        <rdfs:seeAlso rdf:resource="https://www.perseus.tufts.edu/hopper/text?doc=Perseus%3Atext%3A1999.01.0064%3Abook%3DDith"/>
        <foaf:depiction rdf:resource="https://upload.wikimedia.org/wikipedia/commons/0/01/P.Oxy._XI_1361_fr._4.jpg"/>
    </owl:NamedIndividual>

    <owl:NamedIndividual rdf:about="#terpander_lesbius">
        <rdfs:label xml:lang="en">terpander_lesbius</rdfs:label>
        <skos:prefLabel xml:lang="en">terpander_lesbius</skos:prefLabel>
        <rdf:type rdf:resource="#Archaic_Lyric_Poet"/>
        <tlgIdentifyingNumber>tlg0299</tlgIdentifyingNumber>
        <hasWritten rdf:resource="#hymns_terpander"/>        <centuryOfLiving rdf:resource="#7th_century_BCE"/>        <bornIn rdf:resource="#lesbos"/>        <rdfs:seeAlso rdf:resource="https://en.wikipedia.org/wiki/Terpander"/>
        <rdfs:seeAlso rdf:resource="https://www.perseus.tufts.edu/hopper/text?doc=Perseus:text:1999.04.0104:entry=terpander-bio-1"/>
        <rdfs:seeAlso rdf:resource="https://chs.harvard.edu/chapter/iii-inventions-of-terpander/"/>
        <rdfs:seeAlso rdf:resource="https://catalog.perseus.org/catalog/urn:cite:perseus:author.1364"/>
        <rdfs:seeAlso rdf:resource="https://catalog.perseus.org/catalog/urn:cts:greekLit:tlg0299.tlg001"/>
        <rdfs:seeAlso rdf:resource="https://quod.lib.umich.edu/cgi/t/text/pageviewer-idx?c=moa;cc=moa;rgn=full%20text;idno=ACL3129.0003.001;didno=ACL3129.0003.001;view=image;seq=00001010"/>
    </owl:NamedIndividual>

    <owl:NamedIndividual rdf:about="#tyrtaeus_lacedaemonius">
        <rdfs:label xml:lang="en">tyrtaeus_lacedaemonius</rdfs:label>
        <skos:prefLabel xml:lang="en">tyrtaeus_lacedaemonius</skos:prefLabel>
        <rdf:type rdf:resource="#Archaic_Lyric_Poet"/>
        <skos:note>By Gustave Moreau - Gustave Moreau, "Tyrtée"
https:dessins-musee-moreau.froutilspeintures_total.php, Public Domain, https:commons.wikimedia.orgwindex.php?curid=127502347</skos:note>
        <passageChosenEn rdf:datatype="http://www.w3.org/2001/XMLSchema#string">The_Elegiac_Poems_of_Tyrtaeus,_CURFRAG.tlg-0266.2_translated_by_Edmonds:_They_heard_the_voice_of_Phoebus_and_brought_home_from_Pytho_oracles_of_the_God_and_words_of_sure_fulfilment;_for_thus_the_Lord_of_the_Silver_Bow,_Far-Shooting_Apollo_of_the_Golden_Hair,_gave_answer_from_out_his_rich_sanctuary:_The_beginning_of_counsel_shall_belong_to_the_God-honoured_Kings_whose_care_is_the_delightsome_city_of_Sparta,_and_to_the_men_of_elder_birth;_after_them_shall_the_commons,_answering_them_back_with_forthright_ordinances,_both_say_things_honourable_and_do_all_that_is_right,_nor_give_the_city_any_crooked_counsel;_so_shall_the_common_people_have_victory_and_might;_for_this_hath_Phoebus_declared_unto_their_city_in_these_matters._(Edmonds,_J._M._(1931)._The_Elegiac_Poems_of_Tyrtaeus_in_Elegy_and_Iambus_[English_Translation]._Cambridge,_MA:_Harvard_University_Press._London:_William_Heinemann_Ltd._(Original_work_published_1931)._Retrieved_May_4,_2024,_from_https:www.perseus.tufts.eduhoppertext?doc=Perseus%3Atext%3A2008.01.0479%3Avolume%3D1%3Atext%3D2%3Asection%3D2#:~:text=in%20these%20matters.-,CURFRAG.tlg%2D0266.2,-%E2%80%9D%20Plutarch%20Life)</passageChosenEn>
        <tlgIdentifyingNumber>tlg0266</tlgIdentifyingNumber>
        <passageChoselEl rdf:datatype="http://www.w3.org/2001/XMLSchema#string">Τυρταίος,_απ._4_West_μετ._Κ._Τοπούζης:_Τον_Φοίβο_οι_απεσταλμένοι_όταν_άκουσαν,_|_στην_πατρίδα_τους_έφεραν_του_θεού_τη_μαντεία_|_και_τα_θεία_του_λόγια._|_«Τις_αποφάσεις_να_παίρνουν_οι_θεοτίμητοι_άρχοντες,_|_που_έχουν_την_έγνοια_της_ολολάτρευτης_Σπάρτης,_|_και_οι_γέροντες_όσοι_πρωτότοκοι_ήταν._|_Και_μετά_οι_πολίτες,_|_με_τους_δίκαιους_νόμους_πράττοντας_σύμφωνα,_|_τα_σωστά_ν᾽_αποδέχονται_και_να_πράττουν_τα_δίκαια,_|_χωρίς_τα_ανάκατα_να_προτείνουν_στην_πόλη·_|_και_το_λαό_η_δύναμη_ν᾽_ακολουθά_και_η_νίκη»._|_Έτσι_ο_Φοίβος_για_την_πόλη_καθόρισε._(Τσέλικας,_Σ._(επ.)._ΤΥΡΤΑΙΟΣ:_απ._4_West._Ανθολογία_Αρχαϊκής_Λυρικής_Ποίησης._Ανακτήθηκε_4_Μαΐου_2024,_από_https:www.greek-language.grdigitalResourcesancient_greekanthologypoetrybrowse.html?text_id=51)</passageChoselEl>
        <hasWritten rdf:resource="#war_elegies_tyrtaeus"/>        <centuryOfLiving rdf:resource="#7th_century_BCE"/>        <bornIn rdf:resource="#sparta"/>        <foaf:depiction rdf:resource="https://upload.wikimedia.org/wikipedia/commons/2/20/Moreau_-_Tyrt%C3%A9e%2C_cat.96.jpg"/>
        <rdfs:seeAlso rdf:resource="https://www.perseus.tufts.edu/hopper/text?doc=Perseus%3Atext%3A2008.01.0479%3Avolume%3D1%3Atext%3D2"/>
        <rdfs:seeAlso rdf:resource="https://www.perseus.tufts.edu/hopper/text?doc=Perseus%3Atext%3A2008.01.0479%3Avolume%3D1%3Atext%3D2%3Asection%3D2"/>
        <rdfs:seeAlso rdf:resource="https://catalog.perseus.org/catalog/urn:cite:perseus:author.1442"/>
        <rdfs:seeAlso rdf:resource="https://www.trismegistos.org/authorwork/6452"/>
        <rdfs:seeAlso rdf:resource="https://chs.harvard.edu/chapter/part-i-greece-11-tyrtaeus-the-lame-general/"/>
        <rdfs:seeAlso rdf:resource="https://www.oxfordreference.com/display/10.1093/acref/9780199545568.001.0001/acref-9780199545568-e-6628"/>
        <rdfs:seeAlso rdf:resource="https://catalog.perseus.org/catalog/urn:cts:greekLit:tlg0266.tlg001"/>
        <rdfs:seeAlso rdf:resource="https://quod.lib.umich.edu/cgi/t/text/pageviewer-idx?c=moa;cc=moa;rgn=full%20text;idno=ACL3129.0003.001;didno=ACL3129.0003.001;view=image;seq=00001205"/>
        <rdfs:seeAlso rdf:resource="https://en.wikipedia.org/wiki/Tyrtaeus"/>
    </owl:NamedIndividual>

    <owl:NamedIndividual rdf:about="#hymns_alcman">
        <rdfs:label xml:lang="en">hymns_alcman</rdfs:label>
        <skos:prefLabel xml:lang="en">hymns_alcman</skos:prefLabel>
        <rdf:type rdf:resource="#Archaic_Lyric_Poem_in_ionic_or_in_doric_or_in_aeolic_dialect_performed_by_a_chorus_or_by_a_single_performer_dedicated_to_a_god"/>
        <isWrittenBy rdf:resource="#alcman_lacedaemonius"/>    </owl:NamedIndividual>

    <owl:NamedIndividual rdf:about="#semonides_amorginus">
        <rdfs:label xml:lang="en">semonides_amorginus</rdfs:label>
        <skos:prefLabel xml:lang="en">semonides_amorginus</skos:prefLabel>
        <rdf:type rdf:resource="#Archaic_Lyric_Poet"/>
        <passageChosenEn rdf:datatype="http://www.w3.org/2001/XMLSchema#string">Semonides,_Iambi,_CURFRAG.tlg-0260.3_translated_by_Edmonds:_There''s_much_time_for_us_to_lie_dead_in,_yet_we_live_years_few_in_number_and_live_them_ill._(Edmonds,_J._M._(1931)._Iambi,_Semonides_in_Elegy_and_Iambus_[English_Translation]._Cambridge,_MA:_Harvard_University_Press._London:_William_Heinemann_Ltd._(Original_work_published_1931)._Retrieved_May_4,_2024,_from_https:www.perseus.tufts.eduhoppertext?doc=Perseus%3Atext%3A2008.01.0480%3Avolume%3D2%3Atext%3D22%3Asection%3D2#:~:text=live%20them%20ill.-,CURFRAG.tlg%2D0260.3,-%E2%80%9D%20Stobaeus%20Anthology)</passageChosenEn>
        <tlgIdentifyingNumber>tlg0260</tlgIdentifyingNumber>
        <passageChoselEl rdf:datatype="http://www.w3.org/2001/XMLSchema#string">Σημωνίδης,_απ._3_West_μετ._Ηλ._Βουτιερίδης:_Για_να_πεθάνουμε_έχουμε_καιρόν_όσον_κι_αν_θέμε,_μα_ζούμε_χρόνια_λιγοστά_και_συφορές_γεμάτα._(Τσέλικας,_Σ._(επ.)._Σημωνίδης:_απ._3_West._Ανθολογία_Αρχαϊκής_Λυρικής_Ποίησης._Ανακτήθηκε_4_Μαΐου_2024,_από_https:www.greek-language.grdigitalResourcesancient_greekanthologypoetrybrowse.html?text_id=58)</passageChoselEl>
        <hasWritten rdf:resource="#iambs_semonides"/>        <centuryOfLiving rdf:resource="#7th_century_BCE"/>        <bornIn rdf:resource="#samos"/>        <stayedIn rdf:resource="#amorgos"/>        <rdfs:seeAlso rdf:resource="https://www.perseus.tufts.edu/hopper/text?doc=Perseus%3Atext%3A2008.01.0480%3Avolume%3D2%3Atext%3D22"/>
        <rdfs:seeAlso rdf:resource="https://www.perseus.tufts.edu/hopper/text?doc=Perseus%3Atext%3A2008.01.0480%3Avolume%3D2%3Atext%3D22%3Asection%3D1"/>
        <rdfs:seeAlso rdf:resource="https://catalog.perseus.org/catalog/urn:cite:perseus:author.1267"/>
        <rdfs:seeAlso rdf:resource="https://www.wikidata.org/wiki/Q381049"/>
        <rdfs:seeAlso rdf:resource="https://catalog.perseus.org/catalog/urn:cts:greekLit:tlg0260.tlg001"/>
        <rdfs:seeAlso rdf:resource="https://quod.lib.umich.edu/cgi/t/text/pageviewer-idx?c=moa;cc=moa;rgn=full%20text;idno=ACL3129.0003.001;didno=ACL3129.0003.001;view=image;seq=00000839"/>
        <rdfs:seeAlso rdf:resource="https://en.wikipedia.org/wiki/Semonides_of_Amorgos"/>
    </owl:NamedIndividual>

    <owl:NamedIndividual rdf:about="#ephesus">
        <rdfs:label xml:lang="en">ephesus</rdfs:label>
        <skos:prefLabel xml:lang="en">ephesus</skos:prefLabel>
        <rdf:type rdf:resource="#Ancient_Location"/>
        <pleiadesCoordinates>37.9407625,27.340307</pleiadesCoordinates>
        <isBirthPlaceOf rdf:resource="#hipponax_ephesius"/>        <isBirthPlaceOf rdf:resource="#callinus_ephesius"/>        <rdfs:seeAlso rdf:resource="https://pleiades.stoa.org/places/599612"/>
        <rdfs:seeAlso rdf:resource="https://www.wikidata.org/wiki/Q64699469"/>
        <rdfs:seeAlso rdf:resource="https://www.wikidata.org/wiki/Q47611"/>
        <rdfs:seeAlso rdf:resource="https://en.wikipedia.org/wiki/Ephesus"/>
        <rdfs:seeAlso rdf:resource="http://www.perseus.tufts.edu/hopper/text?doc=Perseus%3Atext%3A1999.04.0064%3Aalphabetic+letter%3DE%3Aentry+group%3D4%3Aentry%3Dephesus-geo"/>
        <rdfs:seeAlso rdf:resource="https://topostext.org/place/379273PEph"/>
    </owl:NamedIndividual>

    <owl:NamedIndividual rdf:about="#syrakousai">
        <rdfs:label xml:lang="en">syrakousai</rdfs:label>
        <skos:prefLabel xml:lang="en">syrakousai</skos:prefLabel>
        <rdf:type rdf:resource="#Ancient_Location"/>
        <pleiadesCoordinates>37.0700365425,15.2831354804</pleiadesCoordinates>
        <residentedBy rdf:resource="#pindarus_boeotus"/>        <residentedBy rdf:resource="#bacchylides_ceus"/>        <rdfs:seeAlso rdf:resource="https://pleiades.stoa.org/places/462503"/>
        <rdfs:seeAlso rdf:resource="https://www.wikidata.org/wiki/Q13670"/>
        <rdfs:seeAlso rdf:resource="http://www.trismegistos.org/place/2210"/>
        <rdfs:seeAlso rdf:resource="http://www.geonames.org/2523083/siracusa.html"/>
        <rdfs:seeAlso rdf:resource="https://en.wikipedia.org/wiki/Syracuse,_Sicily"/>
    </owl:NamedIndividual>

    <owl:NamedIndividual rdf:about="#prosodia_pindarus">
        <rdfs:label xml:lang="en">prosodia_pindarus</rdfs:label>
        <skos:prefLabel xml:lang="en">prosodia_pindarus</skos:prefLabel>
        <rdf:type rdf:resource="#Archaic_Lyric_Poem_in_ionic_or_in_doric_or_in_aeolic_dialect_performed_by_a_chorus_on_the_way_to_an_altar"/>
        <isWrittenBy rdf:resource="#pindarus_boeotus"/>    </owl:NamedIndividual>

	<!-- 
	//////////////////////////////////////////////////////////
	//
	// OntoLex-Lemon
	//
	//////////////////////////////////////////////////////////
	-->

    <ontolex:LexicalEntry rdf:about="#epithalamion_en">
        <ontolex:lexicalForm>
            <ontolex:Form rdf:about="#form_epithalamion_en">
                <ontolex:writtenRep xml:lang="en">epithalamion</ontolex:writtenRep>
            </ontolex:Form>
        </ontolex:lexicalForm>
        <ontolex:evokes>
            <ontolex:LexicalConcept rdf:about="#lexical_concept_epithalamion_en">
                <ontolex:isEvokedBy rdf:resource="#epithalamion_en"/>
                <skos:definition xml:lang="en">Epithalamium is a song dedicated to a wedding couple sung at the nuptial residence. Sappho is famous for her such songs.</skos:definition>
            </ontolex:LexicalConcept>
        </ontolex:evokes>
        <ontolex:denotes rdf:resource="#Archaic_Lyric_Poem_in_ionic_or_in_doric_or_in_aeolic_dialect_performed_by_a_chorus_or_by_a_single_performer_dedicated_to_wedding_couple"/>
    </ontolex:LexicalEntry>

    <ontolex:LexicalEntry rdf:about="#threnos_en">
        <ontolex:lexicalForm>
            <ontolex:Form rdf:about="#form_threnos_en">
                <ontolex:writtenRep xml:lang="en">threnos</ontolex:writtenRep>
            </ontolex:Form>
        </ontolex:lexicalForm>
        <ontolex:evokes>
            <ontolex:LexicalConcept rdf:about="#lexical_concept_threnos_en">
                <ontolex:isEvokedBy rdf:resource="#threnos_en"/>
                <skos:definition xml:lang="en">Lyric song dedicated to a dead human being. Anacreon, Pindar and Simonides are famous for their such compositions.</skos:definition>
            </ontolex:LexicalConcept>
        </ontolex:evokes>
        <ontolex:denotes rdf:resource="#Archaic_Lyric_Poem_in_ionic_or_in_doric_or_in_aeolic_dialect_performed_by_a_chorus_or_by_a_single_performer_dedicated_to_dead"/>
    </ontolex:LexicalEntry>

    <ontolex:LexicalEntry rdf:about="#archaic_lyric_poetess_en">
        <ontolex:lexicalForm>
            <ontolex:Form rdf:about="#form_archaic_lyric_poetess_en">
                <ontolex:writtenRep xml:lang="en">archaic lyric poetess</ontolex:writtenRep>
            </ontolex:Form>
        </ontolex:lexicalForm>
        <ontolex:evokes>
            <ontolex:LexicalConcept rdf:about="#lexical_concept_archaic_lyric_poetess_en">
                <ontolex:isEvokedBy rdf:resource="#archaic_lyric_poetess_en"/>
                <skos:definition xml:lang="en">An Archaic Lyric poetess (woman) is a person who lived during 7th-early 5th century BCE and wrote Archaic Lyric poetry.</skos:definition>
            </ontolex:LexicalConcept>
        </ontolex:evokes>
        <ontolex:denotes rdf:resource="#Archaic_Lyric_Poetess"/>
    </ontolex:LexicalEntry>

    <ontolex:LexicalEntry rdf:about="#dithyramb_en">
        <ontolex:lexicalForm>
            <ontolex:Form rdf:about="#form_dithyramb_en">
                <ontolex:writtenRep xml:lang="en">dithyramb</ontolex:writtenRep>
            </ontolex:Form>
        </ontolex:lexicalForm>
        <ontolex:evokes>
            <ontolex:LexicalConcept rdf:about="#lexical_concept_dithyramb_en">
                <ontolex:isEvokedBy rdf:resource="#dithyramb_en"/>
                <skos:definition xml:lang="en">Devotional hymns of Dionysus. Bacchylides, Pindar and Simonides are known to have composed dithyrambs.</skos:definition>
            </ontolex:LexicalConcept>
        </ontolex:evokes>
        <ontolex:denotes rdf:resource="#Archaic_Lyric_Poem_in_ionic_or_in_doric_or_in_aeolic_dialect_performed_by_a_chorus_or_by_a_single_performer_dedicated_to_dionysus"/>
    </ontolex:LexicalEntry>

    <ontolex:LexicalEntry rdf:about="#archaic_lyric_poem_in_ionic_or_in_doric_or_in_aeolic_dialect_performed_by_a_chorus_or_by_a_single_performer_en">
        <ontolex:lexicalForm>
            <ontolex:Form rdf:about="#form_archaic_lyric_poem_in_ionic_or_in_doric_or_in_aeolic_dialect_performed_by_a_chorus_or_by_a_single_performer_en">
                <ontolex:writtenRep xml:lang="en">archaic lyric poem in ionic or in doric or in aeolic dialect performed by a chorus or by a single performer</ontolex:writtenRep>
            </ontolex:Form>
        </ontolex:lexicalForm>
        <ontolex:evokes>
            <ontolex:LexicalConcept rdf:about="#lexical_concept_archaic_lyric_poem_in_ionic_or_in_doric_or_in_aeolic_dialect_performed_by_a_chorus_or_by_a_single_performer_en">
                <ontolex:isEvokedBy rdf:resource="#archaic_lyric_poem_in_ionic_or_in_doric_or_in_aeolic_dialect_performed_by_a_chorus_or_by_a_single_performer_en"/>
                <skos:definition xml:lang="en">Melos which was performed either by one person or by a chorus.</skos:definition>
            </ontolex:LexicalConcept>
        </ontolex:evokes>
        <ontolex:denotes rdf:resource="#Archaic_Lyric_Poem_in_ionic_or_in_doric_or_in_aeolic_dialect_performed_by_a_chorus_or_by_a_single_performer"/>
    </ontolex:LexicalEntry>

    <ontolex:LexicalEntry rdf:about="#hyporcheme_en">
        <ontolex:lexicalForm>
            <ontolex:Form rdf:about="#form_hyporcheme_en">
                <ontolex:writtenRep xml:lang="en">hyporcheme</ontolex:writtenRep>
            </ontolex:Form>
        </ontolex:lexicalForm>
        <ontolex:evokes>
            <ontolex:LexicalConcept rdf:about="#lexical_concept_hyporcheme_en">
                <ontolex:isEvokedBy rdf:resource="#hyporcheme_en"/>
                <skos:definition xml:lang="en">A lyric song accompanied by imitative movements. Bacchylides and Pindar are famous for composing hyporchemes.</skos:definition>
            </ontolex:LexicalConcept>
        </ontolex:evokes>
        <ontolex:denotes rdf:resource="#Archaic_Lyric_Poem_in_ionic_or_in_doric_or_in_aeolic_dialect_performed_by_a_chorus_with_imitation_expressions"/>
    </ontolex:LexicalEntry>

    <ontolex:LexicalEntry rdf:about="#archaic_lyric_poem_en">
        <ontolex:lexicalForm>
            <ontolex:Form rdf:about="#form_archaic_lyric_poem_en">
                <ontolex:writtenRep xml:lang="en">archaic lyric poem</ontolex:writtenRep>
            </ontolex:Form>
        </ontolex:lexicalForm>
        <ontolex:evokes>
            <ontolex:LexicalConcept rdf:about="#lexical_concept_archaic_lyric_poem_en">
                <ontolex:isEvokedBy rdf:resource="#archaic_lyric_poem_en"/>
                <skos:definition xml:lang="en">"Lyric poetry began as a fixture of ancient Greece, classified against other categories of poetry at the time of classical antiquity: dramas (written in verse) and epic poems. The lyric was far shorter, distinguished also by its focus on the poet’s state of mind and personal themes rather than narrative arc" (Academy of American Poets). So, an Archaic Lyric Poem is such poem written from 7th-early 5th century BCE.</skos:definition>
            </ontolex:LexicalConcept>
        </ontolex:evokes>
        <ontolex:denotes rdf:resource="#Archaic_Lyric_Poem"/>
    </ontolex:LexicalEntry>

    <ontolex:LexicalEntry rdf:about="#before_common_era_century_en">
        <ontolex:lexicalForm>
            <ontolex:Form rdf:about="#form_before_common_era_century_en">
                <ontolex:writtenRep xml:lang="en">before common era century</ontolex:writtenRep>
            </ontolex:Form>
        </ontolex:lexicalForm>
        <ontolex:evokes>
            <ontolex:LexicalConcept rdf:about="#lexical_concept_before_common_era_century_en">
                <ontolex:isEvokedBy rdf:resource="#before_common_era_century_en"/>
                <skos:definition xml:lang="en">Century that is BCE.</skos:definition>
            </ontolex:LexicalConcept>
        </ontolex:evokes>
        <ontolex:denotes rdf:resource="#BCE_century"/>
    </ontolex:LexicalEntry>

    <ontolex:LexicalEntry rdf:about="#elegy_en">
        <ontolex:lexicalForm>
            <ontolex:Form rdf:about="#form_elegy_en">
                <ontolex:writtenRep xml:lang="en">elegy</ontolex:writtenRep>
            </ontolex:Form>
        </ontolex:lexicalForm>
        <ontolex:evokes>
            <ontolex:LexicalConcept rdf:about="#lexical_concept_elegy_en">
                <ontolex:isEvokedBy rdf:resource="#elegy_en"/>
                <skos:definition xml:lang="en">Elegies are poems written in elegiac couplets, with the first line in hexameter and the second line in pentameter, initially used for lamentation (but later had a wide range of themes) and possibly originating from Eastern mourning practices. They can be as short as a single couplet or longer sequences as needed.</skos:definition>
            </ontolex:LexicalConcept>
        </ontolex:evokes>
        <ontolex:denotes rdf:resource="#Archaic_Lyric_Poem_only_in_ionic_dialect_in_elegiac_couplet"/>
    </ontolex:LexicalEntry>

    <ontolex:LexicalEntry rdf:about="#archaic_lyric_poem_only_in_ionic_dialect_en">
        <ontolex:lexicalForm>
            <ontolex:Form rdf:about="#form_archaic_lyric_poem_only_in_ionic_dialect_en">
                <ontolex:writtenRep xml:lang="en">archaic lyric poem only in ionic dialect</ontolex:writtenRep>
            </ontolex:Form>
        </ontolex:lexicalForm>
        <ontolex:evokes>
            <ontolex:LexicalConcept rdf:about="#lexical_concept_archaic_lyric_poem_only_in_ionic_dialect_en">
                <ontolex:isEvokedBy rdf:resource="#archaic_lyric_poem_only_in_ionic_dialect_en"/>
                <skos:definition xml:lang="en">Archaic Lyric poem written only in ionic dialect. Ionic greek dialect, a subset of Eastern Greek, originated on the mainland and spread during the Dorian invasions. By the 5th century BC, it was primarily spoken in Ionia, including Asia Minor, Chios, and Samos. It also extended to Euboea and through Ionian colonization to the northern Aegean, Black Sea, and western Mediterranean.</skos:definition>
            </ontolex:LexicalConcept>
        </ontolex:evokes>
        <ontolex:denotes rdf:resource="#Archaic_Lyric_Poem_only_in_ionic_dialect"/>
    </ontolex:LexicalEntry>

    <ontolex:LexicalEntry rdf:about="#paean_en">
        <ontolex:lexicalForm>
            <ontolex:Form rdf:about="#form_paean_en">
                <ontolex:writtenRep xml:lang="en">paean</ontolex:writtenRep>
            </ontolex:Form>
        </ontolex:lexicalForm>
        <ontolex:evokes>
            <ontolex:LexicalConcept rdf:about="#lexical_concept_paean_en">
                <ontolex:isEvokedBy rdf:resource="#paean_en"/>
                <skos:definition xml:lang="en">Lyric song dedicated to Ancient Greek god Apollo. Alcman, Pindar and Bacchylides are famous composers of paeans.</skos:definition>
            </ontolex:LexicalConcept>
        </ontolex:evokes>
        <ontolex:denotes rdf:resource="#Archaic_Lyric_Poem_in_ionic_or_in_doric_or_in_aeolic_dialect_performed_by_a_chorus_or_by_a_single_performer_dedicated_to_apollo"/>
    </ontolex:LexicalEntry>

    <ontolex:LexicalEntry rdf:about="#melos_en">
        <ontolex:lexicalForm>
            <ontolex:Form rdf:about="#form_melos_en">
                <ontolex:writtenRep xml:lang="en">melos</ontolex:writtenRep>
            </ontolex:Form>
        </ontolex:lexicalForm>
        <ontolex:evokes>
            <ontolex:LexicalConcept rdf:about="#lexical_concept_melos_en">
                <ontolex:isEvokedBy rdf:resource="#melos_en"/>
                <skos:definition xml:lang="en">Melos is the hypernym of the Archaic Lyric poems, which were written in ionic (except of the iamb and elegy), aeolic and doric dialect.</skos:definition>
            </ontolex:LexicalConcept>
        </ontolex:evokes>
        <ontolex:denotes rdf:resource="#Archaic_Lyric_Poem_in_ionic_or_in_doric_or_in_aeolic_dialect"/>
    </ontolex:LexicalEntry>

    <ontolex:LexicalEntry rdf:about="#archaic_lyric_composer_en">
        <ontolex:lexicalForm>
            <ontolex:Form rdf:about="#form_archaic_lyric_composer_en">
                <ontolex:writtenRep xml:lang="en">archaic lyric composer</ontolex:writtenRep>
            </ontolex:Form>
        </ontolex:lexicalForm>
        <ontolex:evokes>
            <ontolex:LexicalConcept rdf:about="#lexical_concept_archaic_lyric_composer_en">
                <ontolex:isEvokedBy rdf:resource="#archaic_lyric_composer_en"/>
                <skos:definition xml:lang="en">An Archaic Lyric composer is a person who lived during 7th-early 5th century BCE and wrote a lyric poem.</skos:definition>
            </ontolex:LexicalConcept>
        </ontolex:evokes>
        <ontolex:denotes rdf:resource="#Archaic_Lyric_Composer"/>
    </ontolex:LexicalEntry>

    <ontolex:LexicalEntry rdf:about="#hymn_en">
        <ontolex:lexicalForm>
            <ontolex:Form rdf:about="#form_hymn_en">
                <ontolex:writtenRep xml:lang="en">hymn</ontolex:writtenRep>
            </ontolex:Form>
        </ontolex:lexicalForm>
        <ontolex:evokes>
            <ontolex:LexicalConcept rdf:about="#lexical_concept_hymn_en">
                <ontolex:isEvokedBy rdf:resource="#hymn_en"/>
                <skos:definition xml:lang="en">Lyric song dedicated to gods. Multiple poets has composed hymns, sych as Alcaeus, Terpander, Sappho, Alcman et. al.</skos:definition>
            </ontolex:LexicalConcept>
        </ontolex:evokes>
        <ontolex:denotes rdf:resource="#Archaic_Lyric_Poem_in_ionic_or_in_doric_or_in_aeolic_dialect_performed_by_a_chorus_or_by_a_single_performer_dedicated_to_a_god"/>
    </ontolex:LexicalEntry>

    <ontolex:LexicalEntry rdf:about="#archaic_lyric_poet_en">
        <ontolex:lexicalForm>
            <ontolex:Form rdf:about="#form_archaic_lyric_poet_en">
                <ontolex:writtenRep xml:lang="en">archaic lyric poet</ontolex:writtenRep>
            </ontolex:Form>
        </ontolex:lexicalForm>
        <ontolex:evokes>
            <ontolex:LexicalConcept rdf:about="#lexical_concept_archaic_lyric_poet_en">
                <ontolex:isEvokedBy rdf:resource="#archaic_lyric_poet_en"/>
                <skos:definition xml:lang="en">An Archaic Lyric poet is a person (man) who lived during 7th-early 5th century BCE and wrote Archaic Lyric poetry.</skos:definition>
            </ontolex:LexicalConcept>
        </ontolex:evokes>
        <ontolex:denotes rdf:resource="#Archaic_Lyric_Poet"/>
    </ontolex:LexicalEntry>

    <ontolex:LexicalEntry rdf:about="#prosodion_en">
        <ontolex:lexicalForm>
            <ontolex:Form rdf:about="#form_prosodion_en">
                <ontolex:writtenRep xml:lang="en">prosodion</ontolex:writtenRep>
            </ontolex:Form>
        </ontolex:lexicalForm>
        <ontolex:evokes>
            <ontolex:LexicalConcept rdf:about="#lexical_concept_prosodion_en">
                <ontolex:isEvokedBy rdf:resource="#prosodion_en"/>
                <skos:definition xml:lang="en">A lyric song performed on the way to an altar by a chorus. Alcman, Bacchylides and Pindar are famous prosodia composers.</skos:definition>
            </ontolex:LexicalConcept>
        </ontolex:evokes>
        <ontolex:denotes rdf:resource="#Archaic_Lyric_Poem_in_ionic_or_in_doric_or_in_aeolic_dialect_performed_by_a_chorus_on_the_way_to_an_altar"/>
    </ontolex:LexicalEntry>

    <ontolex:LexicalEntry rdf:about="#hymenaios_en">
        <ontolex:lexicalForm>
            <ontolex:Form rdf:about="#form_hymenaios_en">
                <ontolex:writtenRep xml:lang="en">hymenaios</ontolex:writtenRep>
            </ontolex:Form>
        </ontolex:lexicalForm>
        <ontolex:evokes>
            <ontolex:LexicalConcept rdf:about="#lexical_concept_hymenaios_en">
                <ontolex:isEvokedBy rdf:resource="#hymenaios_en"/>
                <skos:definition xml:lang="en">A lyric song sung during the procession of the bride to the groom's house. Sappho is famous for her such songs.</skos:definition>
            </ontolex:LexicalConcept>
        </ontolex:evokes>
        <ontolex:denotes rdf:resource="#Archaic_Lyric_Poem_in_ionic_or_in_doric_or_in_aeolic_dialect_performed_by_a_chorus_during_bride_procession"/>
    </ontolex:LexicalEntry>

    <ontolex:LexicalEntry rdf:about="#enkomion_en">
        <ontolex:lexicalForm>
            <ontolex:Form rdf:about="#form_enkomion_en">
                <ontolex:writtenRep xml:lang="en">enkomion</ontolex:writtenRep>
            </ontolex:Form>
        </ontolex:lexicalForm>
        <ontolex:evokes>
            <ontolex:LexicalConcept rdf:about="#lexical_concept_enkomion_en">
                <ontolex:isEvokedBy rdf:resource="#enkomion_en"/>
                <skos:definition xml:lang="en">Lyric song of praise for living people. Pindar, Bacchylides and Ibicus are important figures in enkomion composition.</skos:definition>
            </ontolex:LexicalConcept>
        </ontolex:evokes>
        <ontolex:denotes rdf:resource="#Archaic_Lyric_Poem_in_ionic_or_in_doric_or_in_aeolic_dialect_performed_by_a_chorus_or_by_a_single_performer_dedicated_to_living"/>
    </ontolex:LexicalEntry>

    <ontolex:LexicalEntry rdf:about="#iamb_en">
        <ontolex:lexicalForm>
            <ontolex:Form rdf:about="#form_iamb_en">
                <ontolex:writtenRep xml:lang="en">iamb</ontolex:writtenRep>
            </ontolex:Form>
        </ontolex:lexicalForm>
        <ontolex:evokes>
            <ontolex:LexicalConcept rdf:about="#lexical_concept_iamb_en">
                <ontolex:isEvokedBy rdf:resource="#iamb_en"/>
                <skos:definition xml:lang="en">Initially associated with Dionysus, the iamb may have a pre-Hellenic origin as a poetic form. Typically composed in iambic trimeter or trochaic tetrameter, its Ionic version often adopts a first-person perspective, though its context can vary.</skos:definition>
            </ontolex:LexicalConcept>
        </ontolex:evokes>
        <ontolex:denotes rdf:resource="#Archaic_Lyric_Poem_only_in_ionic_dialect_in_iambic_or_trochaic_metre"/>
    </ontolex:LexicalEntry>

    <ontolex:LexicalEntry rdf:about="#epinikion_en">
        <ontolex:lexicalForm>
            <ontolex:Form rdf:about="#form_epinikion_en">
                <ontolex:writtenRep xml:lang="en">epinikion</ontolex:writtenRep>
            </ontolex:Form>
        </ontolex:lexicalForm>
        <ontolex:evokes>
            <ontolex:LexicalConcept rdf:about="#lexical_concept_epinikion_en">
                <ontolex:isEvokedBy rdf:resource="#epinikion_en"/>
                <skos:definition xml:lang="en">Lyric song of praise winners of sports games. Pindar, Bacchylides and Ibicus are who composed epinikia.</skos:definition>
            </ontolex:LexicalConcept>
        </ontolex:evokes>
        <ontolex:denotes rdf:resource="#Archaic_Lyric_Poem_in_ionic_or_in_doric_or_in_aeolic_dialect_performed_by_a_chorus_or_by_a_single_performer_dedicated_to_winners_in_athletic_events"/>
    </ontolex:LexicalEntry>

    <ontolex:LexicalEntry rdf:about="#gnomic_elegy_en">
        <ontolex:lexicalForm>
            <ontolex:Form rdf:about="#form_gnomic_elegy_en">
                <ontolex:writtenRep xml:lang="en">gnomic elegy</ontolex:writtenRep>
            </ontolex:Form>
        </ontolex:lexicalForm>
        <ontolex:evokes>
            <ontolex:LexicalConcept rdf:about="#lexical_concept_gnomic_elegy_en">
                <ontolex:isEvokedBy rdf:resource="#gnomic_elegy_en"/>
                <skos:definition xml:lang="en">Elegy with gnomic, counseling, biosophical content. Known poets of gnomic elegies are Phocylides and Theognis.</skos:definition>
            </ontolex:LexicalConcept>
        </ontolex:evokes>
        <ontolex:denotes rdf:resource="#Archaic_Lyric_Poem_only_in_ionic_dialect_in_elegiac_couplet_with_gnomic_content"/>
    </ontolex:LexicalEntry>

    <ontolex:LexicalEntry rdf:about="#political_elegy_en">
        <ontolex:lexicalForm>
            <ontolex:Form rdf:about="#form_political_elegy_en">
                <ontolex:writtenRep xml:lang="en">political elegy</ontolex:writtenRep>
            </ontolex:Form>
        </ontolex:lexicalForm>
        <ontolex:evokes>
            <ontolex:LexicalConcept rdf:about="#lexical_concept_political_elegy_en">
                <ontolex:isEvokedBy rdf:resource="#political_elegy_en"/>
                <skos:definition xml:lang="en">Elegy with political content. Solon Atheniensis is a famous poet who composed such elegies.</skos:definition>
            </ontolex:LexicalConcept>
        </ontolex:evokes>
        <ontolex:denotes rdf:resource="#Archaic_Lyric_Poem_only_in_ionic_dialect_in_elegiac_couplet_with_political_content"/>
    </ontolex:LexicalEntry>

    <ontolex:LexicalEntry rdf:about="#ancient_location_en">
        <ontolex:lexicalForm>
            <ontolex:Form rdf:about="#form_ancient_location_en">
                <ontolex:writtenRep xml:lang="en">ancient location</ontolex:writtenRep>
            </ontolex:Form>
        </ontolex:lexicalForm>
        <ontolex:evokes>
            <ontolex:LexicalConcept rdf:about="#lexical_concept_ancient_location_en">
                <ontolex:isEvokedBy rdf:resource="#ancient_location_en"/>
                <skos:definition xml:lang="en">In the current ontoterminology Ancient Location objects concern the places where the Archaic Lyric Poets were born or lived, while they are inserted with coordinates from the pleiades gazetteer of ancient places (https:pleiades.stoa.orgplaces).</skos:definition>
            </ontolex:LexicalConcept>
        </ontolex:evokes>
        <ontolex:denotes rdf:resource="#Ancient_Location"/>
    </ontolex:LexicalEntry>

    <ontolex:LexicalEntry rdf:about="#erotic_elegy_en">
        <ontolex:lexicalForm>
            <ontolex:Form rdf:about="#form_erotic_elegy_en">
                <ontolex:writtenRep xml:lang="en">erotic elegy</ontolex:writtenRep>
            </ontolex:Form>
        </ontolex:lexicalForm>
        <ontolex:evokes>
            <ontolex:LexicalConcept rdf:about="#lexical_concept_erotic_elegy_en">
                <ontolex:isEvokedBy rdf:resource="#erotic_elegy_en"/>
                <skos:definition xml:lang="en">Elegy with erotic content. Famous poet who composed erotic elegies is Mimnermus.</skos:definition>
            </ontolex:LexicalConcept>
        </ontolex:evokes>
        <ontolex:denotes rdf:resource="#Archaic_Lyric_Poem_only_in_ionic_dialect_in_elegiac_couplet_with_erotic_content"/>
    </ontolex:LexicalEntry>

    <ontolex:LexicalEntry rdf:about="#partheneion_en">
        <ontolex:lexicalForm>
            <ontolex:Form rdf:about="#form_partheneion_en">
                <ontolex:writtenRep xml:lang="en">partheneion</ontolex:writtenRep>
            </ontolex:Form>
        </ontolex:lexicalForm>
        <ontolex:evokes>
            <ontolex:LexicalConcept rdf:about="#lexical_concept_partheneion_en">
                <ontolex:isEvokedBy rdf:resource="#partheneion_en"/>
                <skos:definition xml:lang="en">A lyric song performed by a maidens chorus. Alcman, Pindar and Bacchylides are famous for composing Partheneia.</skos:definition>
            </ontolex:LexicalConcept>
        </ontolex:evokes>
        <ontolex:denotes rdf:resource="#Archaic_Lyric_Poem_in_ionic_or_in_doric_or_in_aeolic_dialect_performed_by_a_chorus_performed_by_a_maidens_chorus"/>
    </ontolex:LexicalEntry>

    <ontolex:LexicalEntry rdf:about="#archaic_lyric_poem_in_ionic_or_in_doric_or_in_aeolic_dialect_performed_by_a_chorus_en">
        <ontolex:lexicalForm>
            <ontolex:Form rdf:about="#form_archaic_lyric_poem_in_ionic_or_in_doric_or_in_aeolic_dialect_performed_by_a_chorus_en">
                <ontolex:writtenRep xml:lang="en">archaic lyric poem in ionic or in doric or in aeolic dialect performed by a chorus</ontolex:writtenRep>
            </ontolex:Form>
        </ontolex:lexicalForm>
        <ontolex:evokes>
            <ontolex:LexicalConcept rdf:about="#lexical_concept_archaic_lyric_poem_in_ionic_or_in_doric_or_in_aeolic_dialect_performed_by_a_chorus_en">
                <ontolex:isEvokedBy rdf:resource="#archaic_lyric_poem_in_ionic_or_in_doric_or_in_aeolic_dialect_performed_by_a_chorus_en"/>
                <skos:definition xml:lang="en">Lyric song performed by a group (chorus) of people (women, men), which were dancing and singing.</skos:definition>
            </ontolex:LexicalConcept>
        </ontolex:evokes>
        <ontolex:denotes rdf:resource="#Archaic_Lyric_Poem_in_ionic_or_in_doric_or_in_aeolic_dialect_performed_by_a_chorus"/>
    </ontolex:LexicalEntry>

    <ontolex:LexicalEntry rdf:about="#archaic_lyric_poem_in_ionic_or_doric_or_aeolic_dialect_performed_by_a_chorus_of_no_particular_type_en">
        <ontolex:lexicalForm>
            <ontolex:Form rdf:about="#form_archaic_lyric_poem_in_ionic_or_doric_or_aeolic_dialect_performed_by_a_chorus_of_no_particular_type_en">
                <ontolex:writtenRep xml:lang="en">archaic lyric poem in ionic or doric or aeolic dialect performed by a chorus of no particular type</ontolex:writtenRep>
            </ontolex:Form>
        </ontolex:lexicalForm>
        <ontolex:evokes>
            <ontolex:LexicalConcept rdf:about="#lexical_concept_archaic_lyric_poem_in_ionic_or_doric_or_aeolic_dialect_performed_by_a_chorus_of_no_particular_type_en">
                <ontolex:isEvokedBy rdf:resource="#archaic_lyric_poem_in_ionic_or_doric_or_aeolic_dialect_performed_by_a_chorus_of_no_particular_type_en"/>
                <skos:definition xml:lang="en">An Archaic Lyric poem in Ionic or Doric or Aeolic dialect performed by a chorus of no particular type.</skos:definition>
            </ontolex:LexicalConcept>
        </ontolex:evokes>
        <ontolex:denotes rdf:resource="#Archaic_Lyric_Poem_in_ionic_or_in_doric_or_in_aeolic_dialect_performed_by_a_chorus_performed_by_a_non-specific_type_of_chorus"/>
    </ontolex:LexicalEntry>

    <ontolex:LexicalEntry rdf:about="#monody_en">
        <ontolex:lexicalForm>
            <ontolex:Form rdf:about="#form_monody_en">
                <ontolex:writtenRep xml:lang="en">monody</ontolex:writtenRep>
            </ontolex:Form>
        </ontolex:lexicalForm>
        <ontolex:evokes>
            <ontolex:LexicalConcept rdf:about="#lexical_concept_monody_en">
                <ontolex:isEvokedBy rdf:resource="#monody_en"/>
                <skos:definition xml:lang="en">Monodies are characterized by solo performances, where the poet identifies with the singer and expresses personal thoughts and emotions, as they offer a direct and free expression of personality. For instance, in Sapphic odes, the poetess prioritizes her own voice over others.</skos:definition>
            </ontolex:LexicalConcept>
        </ontolex:evokes>
        <ontolex:denotes rdf:resource="#Archaic_Lyric_Poem_in_ionic_or_in_doric_or_in_aeolic_dialect_performed_by_a_single_performer"/>
    </ontolex:LexicalEntry>

    <ontolex:LexicalEntry rdf:about="#war_elegy_en">
        <ontolex:lexicalForm>
            <ontolex:Form rdf:about="#form_war_elegy_en">
                <ontolex:writtenRep xml:lang="en">war elegy</ontolex:writtenRep>
            </ontolex:Form>
        </ontolex:lexicalForm>
        <ontolex:evokes>
            <ontolex:LexicalConcept rdf:about="#lexical_concept_war_elegy_en">
                <ontolex:isEvokedBy rdf:resource="#war_elegy_en"/>
                <skos:definition xml:lang="en">Elegy with war content. Tyrtaeus and Callinus are famous poets of such elegy.</skos:definition>
            </ontolex:LexicalConcept>
        </ontolex:evokes>
        <ontolex:denotes rdf:resource="#Archaic_Lyric_Poem_only_in_ionic_dialect_in_elegiac_couplet_with_war_content"/>
    </ontolex:LexicalEntry>

    <ontolex:LexicalEntry rdf:about="#αρχαϊκό_λυρικό_ποίημα_μόνο_στην_ιωνική_διάλεκτο_el">
        <ontolex:lexicalForm>
            <ontolex:Form rdf:about="#form_αρχαϊκό_λυρικό_ποίημα_μόνο_στην_ιωνική_διάλεκτο_el">
                <ontolex:writtenRep xml:lang="el">αρχαϊκό λυρικό ποίημα μόνο στην ιωνική διάλεκτο</ontolex:writtenRep>
            </ontolex:Form>
        </ontolex:lexicalForm>
        <ontolex:evokes>
            <ontolex:LexicalConcept rdf:about="#lexical_concept_αρχαϊκό_λυρικό_ποίημα_μόνο_στην_ιωνική_διάλεκτο_el">
                <ontolex:isEvokedBy rdf:resource="#αρχαϊκό_λυρικό_ποίημα_μόνο_στην_ιωνική_διάλεκτο_el"/>
                <skos:definition xml:lang="el">Αρχαϊκό λυρικό ποίημα μόνο στην ιωνική διάλεκτο.</skos:definition>
            </ontolex:LexicalConcept>
        </ontolex:evokes>
        <ontolex:denotes rdf:resource="#Archaic_Lyric_Poem_only_in_ionic_dialect"/>
    </ontolex:LexicalEntry>

    <ontolex:LexicalEntry rdf:about="#αρχαία_τοποθεσία_el">
        <ontolex:lexicalForm>
            <ontolex:Form rdf:about="#form_αρχαία_τοποθεσία_el">
                <ontolex:writtenRep xml:lang="el">αρχαία τοποθεσία</ontolex:writtenRep>
            </ontolex:Form>
        </ontolex:lexicalForm>
        <ontolex:evokes>
            <ontolex:LexicalConcept rdf:about="#lexical_concept_αρχαία_τοποθεσία_el">
                <ontolex:isEvokedBy rdf:resource="#αρχαία_τοποθεσία_el"/>
                <skos:definition xml:lang="el">Στην παρούσα οντοορολογία γίνεται αναφορά στους τόπους όπου γεννήθηκαν ή έζησαν οι αρχαϊκοί λυρικοί ποιητές. Η ακριβής τους τοποθεσία εισάγεται με συντεταγμένες από το ευρετήριο αρχαίων τόπων pleiades (https:pleiades.stoa.orgplaces).</skos:definition>
            </ontolex:LexicalConcept>
        </ontolex:evokes>
        <ontolex:denotes rdf:resource="#Ancient_Location"/>
    </ontolex:LexicalEntry>

    <ontolex:LexicalEntry rdf:about="#πολεμική_ελεγεία_el">
        <ontolex:lexicalForm>
            <ontolex:Form rdf:about="#form_πολεμική_ελεγεία_el">
                <ontolex:writtenRep xml:lang="el">πολεμική ελεγεία</ontolex:writtenRep>
            </ontolex:Form>
        </ontolex:lexicalForm>
        <ontolex:evokes>
            <ontolex:LexicalConcept rdf:about="#lexical_concept_πολεμική_ελεγεία_el">
                <ontolex:isEvokedBy rdf:resource="#πολεμική_ελεγεία_el"/>
                <skos:definition xml:lang="el">Ελεγεία με πολεμικό χαρακτήρα. Ο Τυρταίος και ο Καλλίνικος είναι διάσημοι ποιητές τέτοιων ελεγειών.</skos:definition>
            </ontolex:LexicalConcept>
        </ontolex:evokes>
        <ontolex:denotes rdf:resource="#Archaic_Lyric_Poem_only_in_ionic_dialect_in_elegiac_couplet_with_war_content"/>
    </ontolex:LexicalEntry>

    <ontolex:LexicalEntry rdf:about="#αρχαϊκή_λυρική_ποιήτρια_el">
        <ontolex:lexicalForm>
            <ontolex:Form rdf:about="#form_αρχαϊκή_λυρική_ποιήτρια_el">
                <ontolex:writtenRep xml:lang="el">αρχαϊκή λυρική ποιήτρια</ontolex:writtenRep>
            </ontolex:Form>
        </ontolex:lexicalForm>
        <ontolex:evokes>
            <ontolex:LexicalConcept rdf:about="#lexical_concept_αρχαϊκή_λυρική_ποιήτρια_el">
                <ontolex:isEvokedBy rdf:resource="#αρχαϊκή_λυρική_ποιήτρια_el"/>
                <skos:definition xml:lang="el">Η αρχαϊκή λυρική ποιήτρια είναι πρόσωπο που έζησε κατά τον 7ο-αρχές του 5ου αιώνα π.Χ. και έγραψε αρχαϊκή λυρική ποίηση.</skos:definition>
            </ontolex:LexicalConcept>
        </ontolex:evokes>
        <ontolex:denotes rdf:resource="#Archaic_Lyric_Poetess"/>
    </ontolex:LexicalEntry>

    <ontolex:LexicalEntry rdf:about="#αρχαϊκός_λυρικός_συνθέτης_el">
        <ontolex:lexicalForm>
            <ontolex:Form rdf:about="#form_αρχαϊκός_λυρικός_συνθέτης_el">
                <ontolex:writtenRep xml:lang="el">αρχαϊκός λυρικός συνθέτης</ontolex:writtenRep>
            </ontolex:Form>
        </ontolex:lexicalForm>
        <ontolex:evokes>
            <ontolex:LexicalConcept rdf:about="#lexical_concept_αρχαϊκός_λυρικός_συνθέτης_el">
                <ontolex:isEvokedBy rdf:resource="#αρχαϊκός_λυρικός_συνθέτης_el"/>
                <skos:definition xml:lang="el">Ο αρχαϊκός λυρικός συνθέτης είναι ένα πρόσωπο που έζησε κατά τη διάρκεια του 7ου-αρχές του 5ου αιώνα π.Χ. και έγραψε λυρικό ποίημα.</skos:definition>
            </ontolex:LexicalConcept>
        </ontolex:evokes>
        <ontolex:denotes rdf:resource="#Archaic_Lyric_Composer"/>
    </ontolex:LexicalEntry>

    <ontolex:LexicalEntry rdf:about="#αρχαϊκό_λυρικό_ποίημα_σε_ιωνική_ή_δωρική_ή_αιολική_διάλεκτο_που_εκτελείται_από_χορό_ή_από_έναν_μόνο_ερμηνευτή_el">
        <ontolex:lexicalForm>
            <ontolex:Form rdf:about="#form_αρχαϊκό_λυρικό_ποίημα_σε_ιωνική_ή_δωρική_ή_αιολική_διάλεκτο_που_εκτελείται_από_χορό_ή_από_έναν_μόνο_ερμηνευτή_el">
                <ontolex:writtenRep xml:lang="el">αρχαϊκό λυρικό ποίημα σε ιωνική ή δωρική ή αιολική διάλεκτο που εκτελείται από χορό ή από έναν μόνο ερμηνευτή</ontolex:writtenRep>
            </ontolex:Form>
        </ontolex:lexicalForm>
        <ontolex:evokes>
            <ontolex:LexicalConcept rdf:about="#lexical_concept_αρχαϊκό_λυρικό_ποίημα_σε_ιωνική_ή_δωρική_ή_αιολική_διάλεκτο_που_εκτελείται_από_χορό_ή_από_έναν_μόνο_ερμηνευτή_el">
                <ontolex:isEvokedBy rdf:resource="#αρχαϊκό_λυρικό_ποίημα_σε_ιωνική_ή_δωρική_ή_αιολική_διάλεκτο_που_εκτελείται_από_χορό_ή_από_έναν_μόνο_ερμηνευτή_el"/>
                <skos:definition xml:lang="el">Μέλος που εκτελείται από χορό ή από έναν μόνο ερμηνευτή.</skos:definition>
            </ontolex:LexicalConcept>
        </ontolex:evokes>
        <ontolex:denotes rdf:resource="#Archaic_Lyric_Poem_in_ionic_or_in_doric_or_in_aeolic_dialect_performed_by_a_chorus_or_by_a_single_performer"/>
    </ontolex:LexicalEntry>

    <ontolex:LexicalEntry rdf:about="#θρήνος_el">
        <ontolex:lexicalForm>
            <ontolex:Form rdf:about="#form_θρήνος_el">
                <ontolex:writtenRep xml:lang="el">θρήνος</ontolex:writtenRep>
            </ontolex:Form>
        </ontolex:lexicalForm>
        <ontolex:evokes>
            <ontolex:LexicalConcept rdf:about="#lexical_concept_θρήνος_el">
                <ontolex:isEvokedBy rdf:resource="#θρήνος_el"/>
                <skos:definition xml:lang="el">Λυρικό τραγούδι αφιερωμένο σε έναν νεκρό άνθρωπο. Ο Ανακρέων, ο Πίνδαρος και ο Σιμωνίδης είναι διάσημοι για τέτοιες συνθέσεις τους.</skos:definition>
            </ontolex:LexicalConcept>
        </ontolex:evokes>
        <ontolex:denotes rdf:resource="#Archaic_Lyric_Poem_in_ionic_or_in_doric_or_in_aeolic_dialect_performed_by_a_chorus_or_by_a_single_performer_dedicated_to_dead"/>
    </ontolex:LexicalEntry>

    <ontolex:LexicalEntry rdf:about="#διθύραμβος_el">
        <ontolex:lexicalForm>
            <ontolex:Form rdf:about="#form_διθύραμβος_el">
                <ontolex:writtenRep xml:lang="el">διθύραμβος</ontolex:writtenRep>
            </ontolex:Form>
        </ontolex:lexicalForm>
        <ontolex:evokes>
            <ontolex:LexicalConcept rdf:about="#lexical_concept_διθύραμβος_el">
                <ontolex:isEvokedBy rdf:resource="#διθύραμβος_el"/>
                <skos:definition xml:lang="el">Λατρευτικοί ύμνοι του Διονύσου. Ο Βακχυλίδης, ο Πίνδαρος και ο Σιμωνίδης είναι γνωστό ότι συνέθεσαν διθύραμβους.</skos:definition>
            </ontolex:LexicalConcept>
        </ontolex:evokes>
        <ontolex:denotes rdf:resource="#Archaic_Lyric_Poem_in_ionic_or_in_doric_or_in_aeolic_dialect_performed_by_a_chorus_or_by_a_single_performer_dedicated_to_dionysus"/>
    </ontolex:LexicalEntry>

    <ontolex:LexicalEntry rdf:about="#ερωτική_ελεγεία_el">
        <ontolex:lexicalForm>
            <ontolex:Form rdf:about="#form_ερωτική_ελεγεία_el">
                <ontolex:writtenRep xml:lang="el">ερωτική ελεγεία</ontolex:writtenRep>
            </ontolex:Form>
        </ontolex:lexicalForm>
        <ontolex:evokes>
            <ontolex:LexicalConcept rdf:about="#lexical_concept_ερωτική_ελεγεία_el">
                <ontolex:isEvokedBy rdf:resource="#ερωτική_ελεγεία_el"/>
                <skos:definition xml:lang="el">Ελεγεία με ερωτικό χαρακτήρα. Διάσημος ποιητής που συνέθεσε ερωτικές ελεγείες είναι ο Μίμνερμος.</skos:definition>
            </ontolex:LexicalConcept>
        </ontolex:evokes>
        <ontolex:denotes rdf:resource="#Archaic_Lyric_Poem_only_in_ionic_dialect_in_elegiac_couplet_with_erotic_content"/>
    </ontolex:LexicalEntry>

    <ontolex:LexicalEntry rdf:about="#πολιτική_ελεγεία_el">
        <ontolex:lexicalForm>
            <ontolex:Form rdf:about="#form_πολιτική_ελεγεία_el">
                <ontolex:writtenRep xml:lang="el">πολιτική ελεγεία</ontolex:writtenRep>
            </ontolex:Form>
        </ontolex:lexicalForm>
        <ontolex:evokes>
            <ontolex:LexicalConcept rdf:about="#lexical_concept_πολιτική_ελεγεία_el">
                <ontolex:isEvokedBy rdf:resource="#πολιτική_ελεγεία_el"/>
                <skos:definition xml:lang="el">Ελεγεία με πολιτικό χαρακτήρα. Ο Τυρταίος και ο Καλλίνικος είναι διάσημοι ποιητές τέτοιων ελεγειών.</skos:definition>
            </ontolex:LexicalConcept>
        </ontolex:evokes>
        <ontolex:denotes rdf:resource="#Archaic_Lyric_Poem_only_in_ionic_dialect_in_elegiac_couplet_with_political_content"/>
    </ontolex:LexicalEntry>

    <ontolex:LexicalEntry rdf:about="#ύμνος_el">
        <ontolex:lexicalForm>
            <ontolex:Form rdf:about="#form_ύμνος_el">
                <ontolex:writtenRep xml:lang="el">ύμνος</ontolex:writtenRep>
            </ontolex:Form>
        </ontolex:lexicalForm>
        <ontolex:evokes>
            <ontolex:LexicalConcept rdf:about="#lexical_concept_ύμνος_el">
                <ontolex:isEvokedBy rdf:resource="#ύμνος_el"/>
                <skos:definition xml:lang="el">Λυρικό τραγούδι αφιερωμένο στους θεούς. Πολλοί ποιητές έχουν συνθέσει ύμνους, όπως ο Αλκαίος, ο Τέρπανδρος, η Σαπφώ, ο Αλκμάνας κ.ά.</skos:definition>
            </ontolex:LexicalConcept>
        </ontolex:evokes>
        <ontolex:denotes rdf:resource="#Archaic_Lyric_Poem_in_ionic_or_in_doric_or_in_aeolic_dialect_performed_by_a_chorus_or_by_a_single_performer_dedicated_to_a_god"/>
    </ontolex:LexicalEntry>

    <ontolex:LexicalEntry rdf:about="#επιθαλάμιο_el">
        <ontolex:lexicalForm>
            <ontolex:Form rdf:about="#form_επιθαλάμιο_el">
                <ontolex:writtenRep xml:lang="el">επιθαλάμιο</ontolex:writtenRep>
            </ontolex:Form>
        </ontolex:lexicalForm>
        <ontolex:evokes>
            <ontolex:LexicalConcept rdf:about="#lexical_concept_επιθαλάμιο_el">
                <ontolex:isEvokedBy rdf:resource="#επιθαλάμιο_el"/>
                <skos:definition xml:lang="el">Το Επιθαλάμιο είναι ένα τραγούδι αφιερωμένο σε ένα γαμήλιο ζευγάρι που τραγουδιέται στη γαμήλια κατοικία. Η Σαπφώ είναι γνωστή για τα επιθαλάμιά της.</skos:definition>
            </ontolex:LexicalConcept>
        </ontolex:evokes>
        <ontolex:denotes rdf:resource="#Archaic_Lyric_Poem_in_ionic_or_in_doric_or_in_aeolic_dialect_performed_by_a_chorus_or_by_a_single_performer_dedicated_to_wedding_couple"/>
    </ontolex:LexicalEntry>

    <ontolex:LexicalEntry rdf:about="#αρχαϊκό_λυρικό_ποίημα_σε_ιωνική_ή_δωρική_ή_αιολική_διάλεκτο_που_εκτελείται_από_χορό_μη_συγκεκριμένου_τύπου_el">
        <ontolex:lexicalForm>
            <ontolex:Form rdf:about="#form_αρχαϊκό_λυρικό_ποίημα_σε_ιωνική_ή_δωρική_ή_αιολική_διάλεκτο_που_εκτελείται_από_χορό_μη_συγκεκριμένου_τύπου_el">
                <ontolex:writtenRep xml:lang="el">αρχαϊκό λυρικό ποίημα σε ιωνική ή δωρική ή αιολική διάλεκτο που εκτελείται από χορό μη συγκεκριμένου τύπου</ontolex:writtenRep>
            </ontolex:Form>
        </ontolex:lexicalForm>
        <ontolex:evokes>
            <ontolex:LexicalConcept rdf:about="#lexical_concept_αρχαϊκό_λυρικό_ποίημα_σε_ιωνική_ή_δωρική_ή_αιολική_διάλεκτο_που_εκτελείται_από_χορό_μη_συγκεκριμένου_τύπου_el">
                <ontolex:isEvokedBy rdf:resource="#αρχαϊκό_λυρικό_ποίημα_σε_ιωνική_ή_δωρική_ή_αιολική_διάλεκτο_που_εκτελείται_από_χορό_μη_συγκεκριμένου_τύπου_el"/>
                <skos:definition xml:lang="el">Αρχαϊκό λυρικό ποίημα σε ιωνική ή δωρική ή αιολική διάλεκτο που εκτελείται από χορό μη συγκεκριμένου τύπου.</skos:definition>
            </ontolex:LexicalConcept>
        </ontolex:evokes>
        <ontolex:denotes rdf:resource="#Archaic_Lyric_Poem_in_ionic_or_in_doric_or_in_aeolic_dialect_performed_by_a_chorus_performed_by_a_non-specific_type_of_chorus"/>
    </ontolex:LexicalEntry>

    <ontolex:LexicalEntry rdf:about="#υμέναιος_el">
        <ontolex:lexicalForm>
            <ontolex:Form rdf:about="#form_υμέναιος_el">
                <ontolex:writtenRep xml:lang="el">υμέναιος</ontolex:writtenRep>
            </ontolex:Form>
        </ontolex:lexicalForm>
        <ontolex:evokes>
            <ontolex:LexicalConcept rdf:about="#lexical_concept_υμέναιος_el">
                <ontolex:isEvokedBy rdf:resource="#υμέναιος_el"/>
                <skos:definition xml:lang="el">Ένα λυρικό τραγούδι που εκτελείται κατά τη διάρκεια της πομπής της νύφης προς το σπίτι του γαμπρού. Η Σαπφώ είναι διάσημη για τους υμεναίους της.</skos:definition>
            </ontolex:LexicalConcept>
        </ontolex:evokes>
        <ontolex:denotes rdf:resource="#Archaic_Lyric_Poem_in_ionic_or_in_doric_or_in_aeolic_dialect_performed_by_a_chorus_during_bride_procession"/>
    </ontolex:LexicalEntry>

    <ontolex:LexicalEntry rdf:about="#παιάνας_el">
        <ontolex:lexicalForm>
            <ontolex:Form rdf:about="#form_παιάνας_el">
                <ontolex:writtenRep xml:lang="el">παιάνας</ontolex:writtenRep>
            </ontolex:Form>
        </ontolex:lexicalForm>
        <ontolex:evokes>
            <ontolex:LexicalConcept rdf:about="#lexical_concept_παιάνας_el">
                <ontolex:isEvokedBy rdf:resource="#παιάνας_el"/>
                <skos:definition xml:lang="el">Λυρικό τραγούδι αφιερωμένο στον αρχαίο Έλληνα θεό Απόλλωνα. Ο Αλκμάνας, ο Πίνδαρος και ο Βακχυλίδης είναι διάσημοι συνθέτες παιάνων.</skos:definition>
            </ontolex:LexicalConcept>
        </ontolex:evokes>
        <ontolex:denotes rdf:resource="#Archaic_Lyric_Poem_in_ionic_or_in_doric_or_in_aeolic_dialect_performed_by_a_chorus_or_by_a_single_performer_dedicated_to_apollo"/>
    </ontolex:LexicalEntry>

    <ontolex:LexicalEntry rdf:about="#αρχαϊκός_λυρικός_ποιητής_el">
        <ontolex:lexicalForm>
            <ontolex:Form rdf:about="#form_αρχαϊκός_λυρικός_ποιητής_el">
                <ontolex:writtenRep xml:lang="el">αρχαϊκός λυρικός ποιητής</ontolex:writtenRep>
            </ontolex:Form>
        </ontolex:lexicalForm>
        <ontolex:evokes>
            <ontolex:LexicalConcept rdf:about="#lexical_concept_αρχαϊκός_λυρικός_ποιητής_el">
                <ontolex:isEvokedBy rdf:resource="#αρχαϊκός_λυρικός_ποιητής_el"/>
                <skos:definition xml:lang="el">Ο αρχαϊκός λυρικός ποιητής είναι ένα πρόσωπο που έζησε κατά τον 7ο-αρχές του 5ου αιώνα π.Χ. και έγραψε αρχαϊκή λυρική ποίηση.</skos:definition>
            </ontolex:LexicalConcept>
        </ontolex:evokes>
        <ontolex:denotes rdf:resource="#Archaic_Lyric_Poet"/>
    </ontolex:LexicalEntry>

    <ontolex:LexicalEntry rdf:about="#προχριστιανικός_αιώνας_el">
        <ontolex:lexicalForm>
            <ontolex:Form rdf:about="#form_προχριστιανικός_αιώνας_el">
                <ontolex:writtenRep xml:lang="el">προχριστιανικός αιώνας</ontolex:writtenRep>
            </ontolex:Form>
        </ontolex:lexicalForm>
        <ontolex:evokes>
            <ontolex:LexicalConcept rdf:about="#lexical_concept_προχριστιανικός_αιώνας_el">
                <ontolex:isEvokedBy rdf:resource="#προχριστιανικός_αιώνας_el"/>
                <skos:definition xml:lang="el"> Προχριστιανικός αιώνας.</skos:definition>
            </ontolex:LexicalConcept>
        </ontolex:evokes>
        <ontolex:denotes rdf:resource="#BCE_century"/>
    </ontolex:LexicalEntry>

    <ontolex:LexicalEntry rdf:about="#υπόρχημα_el">
        <ontolex:lexicalForm>
            <ontolex:Form rdf:about="#form_υπόρχημα_el">
                <ontolex:writtenRep xml:lang="el">υπόρχημα</ontolex:writtenRep>
            </ontolex:Form>
        </ontolex:lexicalForm>
        <ontolex:evokes>
            <ontolex:LexicalConcept rdf:about="#lexical_concept_υπόρχημα_el">
                <ontolex:isEvokedBy rdf:resource="#υπόρχημα_el"/>
                <skos:definition xml:lang="el">Ένα λυρικό τραγούδι που συνοδεύεται από μιμητικές κινήσεις. Ο Βακχυλίδης και ο Πίνδαρος φημίζονται για τη σύνθεση υπορχημάτων.</skos:definition>
            </ontolex:LexicalConcept>
        </ontolex:evokes>
        <ontolex:denotes rdf:resource="#Archaic_Lyric_Poem_in_ionic_or_in_doric_or_in_aeolic_dialect_performed_by_a_chorus_with_imitation_expressions"/>
    </ontolex:LexicalEntry>

    <ontolex:LexicalEntry rdf:about="#γνωμική_ελεγεία_el">
        <ontolex:lexicalForm>
            <ontolex:Form rdf:about="#form_γνωμική_ελεγεία_el">
                <ontolex:writtenRep xml:lang="el">γνωμική ελεγεία</ontolex:writtenRep>
            </ontolex:Form>
        </ontolex:lexicalForm>
        <ontolex:evokes>
            <ontolex:LexicalConcept rdf:about="#lexical_concept_γνωμική_ελεγεία_el">
                <ontolex:isEvokedBy rdf:resource="#γνωμική_ελεγεία_el"/>
                <skos:definition xml:lang="el">Ελεγεία με γνωμικό, συμβουλευτικό, βιοσοφικό περιεχόμενο. Γνωστοί ποιητές γνωστών γνωμικών ελεγειών είναι ο Φωκυλίδης και ο Θεογένης.</skos:definition>
            </ontolex:LexicalConcept>
        </ontolex:evokes>
        <ontolex:denotes rdf:resource="#Archaic_Lyric_Poem_only_in_ionic_dialect_in_elegiac_couplet_with_gnomic_content"/>
    </ontolex:LexicalEntry>

    <ontolex:LexicalEntry rdf:about="#αρχαϊκό_λυρικό_ποίημα_σε_ιωνική_ή_δωρική_ή_αιολική_διάλεκτο_που_εκτελείται_από_χορό_el">
        <ontolex:lexicalForm>
            <ontolex:Form rdf:about="#form_αρχαϊκό_λυρικό_ποίημα_σε_ιωνική_ή_δωρική_ή_αιολική_διάλεκτο_που_εκτελείται_από_χορό_el">
                <ontolex:writtenRep xml:lang="el">αρχαϊκό λυρικό ποίημα σε ιωνική ή δωρική ή αιολική διάλεκτο που εκτελείται από χορό</ontolex:writtenRep>
            </ontolex:Form>
        </ontolex:lexicalForm>
        <ontolex:evokes>
            <ontolex:LexicalConcept rdf:about="#lexical_concept_αρχαϊκό_λυρικό_ποίημα_σε_ιωνική_ή_δωρική_ή_αιολική_διάλεκτο_που_εκτελείται_από_χορό_el">
                <ontolex:isEvokedBy rdf:resource="#αρχαϊκό_λυρικό_ποίημα_σε_ιωνική_ή_δωρική_ή_αιολική_διάλεκτο_που_εκτελείται_από_χορό_el"/>
                <skos:definition xml:lang="el">Μέλος που εκτελείται από Χορό.</skos:definition>
            </ontolex:LexicalConcept>
        </ontolex:evokes>
        <ontolex:denotes rdf:resource="#Archaic_Lyric_Poem_in_ionic_or_in_doric_or_in_aeolic_dialect_performed_by_a_chorus"/>
    </ontolex:LexicalEntry>

    <ontolex:LexicalEntry rdf:about="#εγκώμιο_el">
        <ontolex:lexicalForm>
            <ontolex:Form rdf:about="#form_εγκώμιο_el">
                <ontolex:writtenRep xml:lang="el">εγκώμιο</ontolex:writtenRep>
            </ontolex:Form>
        </ontolex:lexicalForm>
        <ontolex:evokes>
            <ontolex:LexicalConcept rdf:about="#lexical_concept_εγκώμιο_el">
                <ontolex:isEvokedBy rdf:resource="#εγκώμιο_el"/>
                <skos:definition xml:lang="el">Λυρικό τραγούδι επαίνου για ανθρώπους στη διάρκεια της ζωής τους. Ο Πίνδαρος, ο Βακχυλίδης και ο Ίβυκος είναι σημαντικές μορφές της σύνθεσης του εγκωμίου.</skos:definition>
            </ontolex:LexicalConcept>
        </ontolex:evokes>
        <ontolex:denotes rdf:resource="#Archaic_Lyric_Poem_in_ionic_or_in_doric_or_in_aeolic_dialect_performed_by_a_chorus_or_by_a_single_performer_dedicated_to_living"/>
    </ontolex:LexicalEntry>

    <ontolex:LexicalEntry rdf:about="#παρθένειο_el">
        <ontolex:lexicalForm>
            <ontolex:Form rdf:about="#form_παρθένειο_el">
                <ontolex:writtenRep xml:lang="el">παρθένειο</ontolex:writtenRep>
            </ontolex:Form>
        </ontolex:lexicalForm>
        <ontolex:evokes>
            <ontolex:LexicalConcept rdf:about="#lexical_concept_παρθένειο_el">
                <ontolex:isEvokedBy rdf:resource="#παρθένειο_el"/>
                <skos:definition xml:lang="el">Ένα λυρικό τραγούδι που ερμηνεύεται από μια χορωδία νεανίδων. Ο Αλκμάνας, ο Πίνδαρος και ο Βακχυλίδης φημίζονται για τη σύνθεση των Παρθενείων.</skos:definition>
            </ontolex:LexicalConcept>
        </ontolex:evokes>
        <ontolex:denotes rdf:resource="#Archaic_Lyric_Poem_in_ionic_or_in_doric_or_in_aeolic_dialect_performed_by_a_chorus_performed_by_a_maidens_chorus"/>
    </ontolex:LexicalEntry>

    <ontolex:LexicalEntry rdf:about="#ίαμβος_el">
        <ontolex:lexicalForm>
            <ontolex:Form rdf:about="#form_ίαμβος_el">
                <ontolex:writtenRep xml:lang="el">ίαμβος</ontolex:writtenRep>
            </ontolex:Form>
        </ontolex:lexicalForm>
        <ontolex:evokes>
            <ontolex:LexicalConcept rdf:about="#lexical_concept_ίαμβος_el">
                <ontolex:isEvokedBy rdf:resource="#ίαμβος_el"/>
                <skos:definition xml:lang="el">Αρχικά συνδεόμενος με τον Διόνυσο, ο ίαμβος μπορεί να έχει προελληνική προέλευση ως ποιητική μορφή. Συνήθως συντίθεται σε ιαμβικό τρίμετρο ή τροχαϊκό τετράμετρο, η ιωνική εκδοχή του συχνά υιοθετεί την πρωτοπρόσωπη σκοπιά, αν και τα συμφραζόμενα μπορεί να ποικίλλουν.</skos:definition>
            </ontolex:LexicalConcept>
        </ontolex:evokes>
        <ontolex:denotes rdf:resource="#Archaic_Lyric_Poem_only_in_ionic_dialect_in_iambic_or_trochaic_metre"/>
    </ontolex:LexicalEntry>

    <ontolex:LexicalEntry rdf:about="#μονωδία_el">
        <ontolex:lexicalForm>
            <ontolex:Form rdf:about="#form_μονωδία_el">
                <ontolex:writtenRep xml:lang="el">μονωδία</ontolex:writtenRep>
            </ontolex:Form>
        </ontolex:lexicalForm>
        <ontolex:evokes>
            <ontolex:LexicalConcept rdf:about="#lexical_concept_μονωδία_el">
                <ontolex:isEvokedBy rdf:resource="#μονωδία_el"/>
                <skos:definition xml:lang="el">Οι μονωδίες χαρακτηρίζονται από σόλο ερμηνείες, όπου ο ποιητής ταυτίζεται με τον τραγουδιστή και εκφράζει προσωπικές σκέψεις και συναισθήματα, καθώς προσφέρουν μια άμεση και ελεύθερη έκφραση της προσωπικότητας. Για παράδειγμα, στις σαπφικές ωδές, η ποιήτρια δίνει προτεραιότητα στη δική της φωνή έναντι των άλλων.</skos:definition>
            </ontolex:LexicalConcept>
        </ontolex:evokes>
        <ontolex:denotes rdf:resource="#Archaic_Lyric_Poem_in_ionic_or_in_doric_or_in_aeolic_dialect_performed_by_a_single_performer"/>
    </ontolex:LexicalEntry>

    <ontolex:LexicalEntry rdf:about="#επίνικος_el">
        <ontolex:lexicalForm>
            <ontolex:Form rdf:about="#form_επίνικος_el">
                <ontolex:writtenRep xml:lang="el">επίνικος</ontolex:writtenRep>
            </ontolex:Form>
        </ontolex:lexicalForm>
        <ontolex:evokes>
            <ontolex:LexicalConcept rdf:about="#lexical_concept_επίνικος_el">
                <ontolex:isEvokedBy rdf:resource="#επίνικος_el"/>
                <skos:definition xml:lang="el">Λυρικό τραγούδι αφιερωμένο σε νικητή αθλητικών αγώνων. Ο Πίνδαρος, ο Βακχυλίδης και ο Ίβυκος είναι αυτοί που συνέθεσαν επινίκια τραγούδια.</skos:definition>
            </ontolex:LexicalConcept>
        </ontolex:evokes>
        <ontolex:denotes rdf:resource="#Archaic_Lyric_Poem_in_ionic_or_in_doric_or_in_aeolic_dialect_performed_by_a_chorus_or_by_a_single_performer_dedicated_to_winners_in_athletic_events"/>
    </ontolex:LexicalEntry>

    <ontolex:LexicalEntry rdf:about="#προσόδιο_el">
        <ontolex:lexicalForm>
            <ontolex:Form rdf:about="#form_προσόδιο_el">
                <ontolex:writtenRep xml:lang="el">προσόδιο</ontolex:writtenRep>
            </ontolex:Form>
        </ontolex:lexicalForm>
        <ontolex:evokes>
            <ontolex:LexicalConcept rdf:about="#lexical_concept_προσόδιο_el">
                <ontolex:isEvokedBy rdf:resource="#προσόδιο_el"/>
                <skos:definition xml:lang="el">Ένα λυρικό τραγούδι που ερμηνεύεται στο δρόμο προς το ιερό από μια χορωδία. Ο Αλκμάν, ο Βακχυλίδης και ο Πίνδαρος είναι διάσημοι συνθέτες προσοδίων.</skos:definition>
            </ontolex:LexicalConcept>
        </ontolex:evokes>
        <ontolex:denotes rdf:resource="#Archaic_Lyric_Poem_in_ionic_or_in_doric_or_in_aeolic_dialect_performed_by_a_chorus_on_the_way_to_an_altar"/>
    </ontolex:LexicalEntry>

    <ontolex:LexicalEntry rdf:about="#μέλος_el">
        <ontolex:lexicalForm>
            <ontolex:Form rdf:about="#form_μέλος_el">
                <ontolex:writtenRep xml:lang="el">μέλος</ontolex:writtenRep>
            </ontolex:Form>
        </ontolex:lexicalForm>
        <ontolex:evokes>
            <ontolex:LexicalConcept rdf:about="#lexical_concept_μέλος_el">
                <ontolex:isEvokedBy rdf:resource="#μέλος_el"/>
                <skos:definition xml:lang="el">Το Μέλος είναι το υπερώνυμο των αρχαϊκών λυρικών ποιημάτων, τα οποία ήταν γραμμένα σε ιωνική (εκτός από τον ίαμβο και την ελεγεία), αιολική και δωρική διάλεκτο.</skos:definition>
            </ontolex:LexicalConcept>
        </ontolex:evokes>
        <ontolex:denotes rdf:resource="#Archaic_Lyric_Poem_in_ionic_or_in_doric_or_in_aeolic_dialect"/>
    </ontolex:LexicalEntry>

    <ontolex:LexicalEntry rdf:about="#ελεγεία_el">
        <ontolex:lexicalForm>
            <ontolex:Form rdf:about="#form_ελεγεία_el">
                <ontolex:writtenRep xml:lang="el">ελεγεία</ontolex:writtenRep>
            </ontolex:Form>
        </ontolex:lexicalForm>
        <ontolex:evokes>
            <ontolex:LexicalConcept rdf:about="#lexical_concept_ελεγεία_el">
                <ontolex:isEvokedBy rdf:resource="#ελεγεία_el"/>
                <skos:definition xml:lang="el">Οι ελεγείες είναι ποιήματα γραμμένα σε ελεγειακά δίστιχα, με τον πρώτο στίχο σε εξάμετρο και τον δεύτερο σε πεντάμετρο. Αρχικά, χρησιμοποιήθηκαν για θρήνους (αλλά αργότερα είχαν ένα ευρύ φάσμα θεμάτων) και πιθανόν προέρχονται από τις ανατολίτικες θρηνητικές πρακτικές. Μπορεί να είναι μικρές σε έκταση (όσο ένα απλό κουπλέ) ή μεγαλύτερες.</skos:definition>
            </ontolex:LexicalConcept>
        </ontolex:evokes>
        <ontolex:denotes rdf:resource="#Archaic_Lyric_Poem_only_in_ionic_dialect_in_elegiac_couplet"/>
    </ontolex:LexicalEntry>

    <ontolex:LexicalEntry rdf:about="#αρχαϊκό_λυρικό_ποίημα_el">
        <ontolex:lexicalForm>
            <ontolex:Form rdf:about="#form_αρχαϊκό_λυρικό_ποίημα_el">
                <ontolex:writtenRep xml:lang="el">αρχαϊκό λυρικό ποίημα</ontolex:writtenRep>
            </ontolex:Form>
        </ontolex:lexicalForm>
        <ontolex:evokes>
            <ontolex:LexicalConcept rdf:about="#lexical_concept_αρχαϊκό_λυρικό_ποίημα_el">
                <ontolex:isEvokedBy rdf:resource="#αρχαϊκό_λυρικό_ποίημα_el"/>
                <skos:definition xml:lang="el">"Η Λυρική ποίηση ξεκίνησε ως θεσμός της αρχαίας Ελλάδας, ταξινομημένος σε σχέση με άλλες κατηγορίες ποίησης κατά την εποχή της κλασικής αρχαιότητας: τα δραματικά (γραμμένα σε στίχους) και τα επικά ποιήματα. Η λυρική ποίηση ήταν πολύ πιο σύντομη, ενώ διακρινόταν επίσης από την εστίασή της στην ψυχική κατάσταση του ποιητή και σε προσωπικά θέματα και όχι στο αφηγηματικό τόξο" (Ακαδημία Αμερικανών Ποιητών). Έτσι, ένα αρχαϊκό λυρικό ποίημα είναι ένα τέτοιο ποίημα που γράφτηκε από τον 7ο-αρχές του 5ου αιώνα π.Χ.</skos:definition>
            </ontolex:LexicalConcept>
        </ontolex:evokes>
        <ontolex:denotes rdf:resource="#Archaic_Lyric_Poem"/>
    </ontolex:LexicalEntry>


<!-- *********************************************** -->
<!-- ONTOTERMINOLOGY VOCABULARY (OTV) -->
<!-- http://ontoterminology.com/ -->
<!-- *********************************************** -->

<!-- ***********************************************
                     OTV CLASSES
     *********************************************** -->

<!-- Conceptual dimension -->

<!-- CTT concepts are represented as OWL classes
     and as instances of the OTVConcept  class -->

<owl:Class rdf:about="http://www.ontologia.fr/OTB/otv#OTVCore">
        <rdfs:label>OTVCore</rdfs:label>      
        <rdfs:comment>The Generic Concept of OTV Concepts</rdfs:comment>
        <rdfs:isDefinedBy>http://www.ontologia.fr/OTB/otv.rdf</rdfs:isDefinedBy>
</owl:Class>

<owl:Class rdf:about="http://www.ontologia.fr/OTB/otv#Concept">
        <rdfs:label>Concept</rdfs:label>
        <rdfs:subClassOf rdf:resource="http://www.ontologia.fr/OTB/otv#OTVCore"/>     
        <rdfs:comment>The class of OTV Concept</rdfs:comment>
        <rdfs:comment>Les concepts sont des instances de la classe Concept</rdfs:comment>
        <rdfs:isDefinedBy>http://www.ontologia.fr/OTB/otv.rdf</rdfs:isDefinedBy>
        <owl:disjointWith rdf:resource="http://www.ontologia.fr/OTB/otv#AxisOfAnalysis"/>
        <owl:disjointWith rdf:resource="http://www.ontologia.fr/OTB/otv#Difference"/>
        <owl:disjointWith rdf:resource="http://www.ontologia.fr/OTB/otv#Relation"/>
        <owl:disjointWith rdf:resource="http://www.ontologia.fr/OTB/otv#Attribute"/>
        <owl:disjointWith rdf:resource="http://www.ontologia.fr/OTB/otv#Object"/>
        <owl:disjointWith rdf:resource="http://www.ontologia.fr/OTB/otv#Term"/>
        <owl:disjointWith rdf:resource="http://www.ontologia.fr/OTB/otv#ProperName"/>
</owl:Class>

<owl:Class rdf:about="http://www.ontologia.fr/OTB/otv#AxisOfAnalysis">
        <rdfs:label>AxisOfAnalysis</rdfs:label>
        <rdfs:subClassOf rdf:resource="http://www.ontologia.fr/OTB/otv#OTVCore"/>     
        <rdfs:comment>The class of OTV AxesOfAnalysis</rdfs:comment>
        <rdfs:comment>Les axes d analyse sont des instances de la classe AxesOfAnalysis</rdfs:comment>
        <rdfs:isDefinedBy>http://www.ontologia.fr/OTB/otv.rdf</rdfs:isDefinedBy>
        <owl:disjointWith rdf:resource="http://www.ontologia.fr/OTB/otv#Concept"/>
        <owl:disjointWith rdf:resource="http://www.ontologia.fr/OTB/otv#Difference"/>
        <owl:disjointWith rdf:resource="http://www.ontologia.fr/OTB/otv#Relation"/>
        <owl:disjointWith rdf:resource="http://www.ontologia.fr/OTB/otv#Attribute"/>
        <owl:disjointWith rdf:resource="http://www.ontologia.fr/OTB/otv#Object"/>
        <owl:disjointWith rdf:resource="http://www.ontologia.fr/OTB/otv#Term"/>
        <owl:disjointWith rdf:resource="http://www.ontologia.fr/OTB/otv#ProperName"/>
</owl:Class>

<owl:Class rdf:about="http://www.ontologia.fr/OTB/otv#Difference">
        <rdfs:label>Difference</rdfs:label>
        <rdfs:subClassOf rdf:resource="http://www.ontologia.fr/OTB/otv#OTVCore"/>    
        <rdfs:comment>The class of OTV Differences</rdfs:comment>
       <rdfs:comment>Les différence sont des instances de la classe Difference</rdfs:comment>
        <rdfs:isDefinedBy>http://www.ontologia.fr/OTB/otv.rdf</rdfs:isDefinedBy>
        <owl:disjointWith rdf:resource="http://www.ontologia.fr/OTB/otv#AxisOfAnalysis"/>
        <owl:disjointWith rdf:resource="http://www.ontologia.fr/OTB/otv#Concept"/>
        <owl:disjointWith rdf:resource="http://www.ontologia.fr/OTB/otv#Relation"/>
        <owl:disjointWith rdf:resource="http://www.ontologia.fr/OTB/otv#Attribute"/>
        <owl:disjointWith rdf:resource="http://www.ontologia.fr/OTB/otv#Object"/>
        <owl:disjointWith rdf:resource="http://www.ontologia.fr/OTB/otv#Term"/>
        <owl:disjointWith rdf:resource="http://www.ontologia.fr/OTB/otv#ProperName"/>
</owl:Class>

<owl:Class rdf:about="http://www.ontologia.fr/OTB/otv#Relation">
        <rdfs:label>Relation</rdfs:label>
        <rdfs:subClassOf rdf:resource="http://www.ontologia.fr/OTB/otv#OTVCore"/>    
        <rdfs:comment>The class of OTV Relations</rdfs:comment>
        <rdfs:isDefinedBy>http://www.ontologia.fr/OTB/otv.rdf</rdfs:isDefinedBy>
        <owl:disjointWith rdf:resource="http://www.ontologia.fr/OTB/otv#AxisOfAnalysis"/>
        <owl:disjointWith rdf:resource="http://www.ontologia.fr/OTB/otv#Difference"/>
        <owl:disjointWith rdf:resource="http://www.ontologia.fr/OTB/otv#Concept"/>
        <owl:disjointWith rdf:resource="http://www.ontologia.fr/OTB/otv#Attribute"/>
        <owl:disjointWith rdf:resource="http://www.ontologia.fr/OTB/otv#Object"/>
        <owl:disjointWith rdf:resource="http://www.ontologia.fr/OTB/otv#Term"/>
        <owl:disjointWith rdf:resource="http://www.ontologia.fr/OTB/otv#ProperName"/>
</owl:Class>

<owl:Class rdf:about="http://www.ontologia.fr/OTB/otv#Attribute">
        <rdfs:label>Attribute</rdfs:label>
        <rdfs:subClassOf rdf:resource="http://www.ontologia.fr/OTB/otv#OTVCore"/>    
        <rdfs:comment>The class of OTV Attributes</rdfs:comment>
        <rdfs:isDefinedBy>http://www.ontologia.fr/OTB/otv.rdf</rdfs:isDefinedBy>
        <owl:disjointWith rdf:resource="http://www.ontologia.fr/OTB/otv#AxisOfAnalysis"/>
        <owl:disjointWith rdf:resource="http://www.ontologia.fr/OTB/otv#Difference"/>
        <owl:disjointWith rdf:resource="http://www.ontologia.fr/OTB/otv#Relation"/>
        <owl:disjointWith rdf:resource="http://www.ontologia.fr/OTB/otv#Concept"/>
        <owl:disjointWith rdf:resource="http://www.ontologia.fr/OTB/otv#Object"/>
        <owl:disjointWith rdf:resource="http://www.ontologia.fr/OTB/otv#Term"/>
        <owl:disjointWith rdf:resource="http://www.ontologia.fr/OTB/otv#ProperName"/>
</owl:Class>

<owl:Class rdf:about="http://www.ontologia.fr/OTB/otv#Object">
        <rdfs:label>Object</rdfs:label>
        <rdfs:subClassOf rdf:resource="http://www.ontologia.fr/OTB/otv#OTVCore"/>
        <rdfs:comment>The class of OTV Objects</rdfs:comment>
        <rdfs:isDefinedBy>http://www.ontologia.fr/OTB/otv.rdf</rdfs:isDefinedBy>
        <owl:disjointWith rdf:resource="http://www.ontologia.fr/OTB/otv#AxisOfAnalysis"/>
        <owl:disjointWith rdf:resource="http://www.ontologia.fr/OTB/otv#Difference"/>
        <owl:disjointWith rdf:resource="http://www.ontologia.fr/OTB/otv#Relation"/>
        <owl:disjointWith rdf:resource="http://www.ontologia.fr/OTB/otv#Attribute"/>
        <owl:disjointWith rdf:resource="http://www.ontologia.fr/OTB/otv#Concept"/>
        <owl:disjointWith rdf:resource="http://www.ontologia.fr/OTB/otv#Term"/>
        <owl:disjointWith rdf:resource="http://www.ontologia.fr/OTB/otv#ProperName"/>
</owl:Class>

<!-- Linguistic dimension -->

<owl:Class rdf:about="http://www.ontologia.fr/OTB/otv#Term">
 	      <rdfs:label>Term</rdfs:label>
        <rdfs:subClassOf rdf:resource="http://www.ontologia.fr/OTB/otv#OTVCore"/>
        <rdfs:comment>The class of OTV Terms</rdfs:comment>
        <rdfs:isDefinedBy>http://www.ontologia.fr/OTB/otv.rdf</rdfs:isDefinedBy>
        <owl:disjointWith rdf:resource="http://www.ontologia.fr/OTB/otv#AxisOfAnalysis"/>
        <owl:disjointWith rdf:resource="http://www.ontologia.fr/OTB/otv#Difference"/>
        <owl:disjointWith rdf:resource="http://www.ontologia.fr/OTB/otv#Relation"/>
        <owl:disjointWith rdf:resource="http://www.ontologia.fr/OTB/otv#Attribute"/>
        <owl:disjointWith rdf:resource="http://www.ontologia.fr/OTB/otv#Object"/>
        <owl:disjointWith rdf:resource="http://www.ontologia.fr/OTB/otv#Concept"/>
        <owl:disjointWith rdf:resource="http://www.ontologia.fr/OTB/otv#ProperName"/>
</owl:Class>

<owl:Class rdf:about="http://www.ontologia.fr/OTB/otv#ProperName">
        <rdfs:label>ProperName</rdfs:label>
        <rdfs:subClassOf rdf:resource="http://www.ontologia.fr/OTB/otv#OTVCore"/>
        <rdfs:comment>The class of OTV ProperName</rdfs:comment>
        <rdfs:isDefinedBy>http://www.ontologia.fr/OTB/otv.rdf</rdfs:isDefinedBy>
        <owl:disjointWith rdf:resource="http://www.ontologia.fr/OTB/otv#AxisOfAnalysis"/>
        <owl:disjointWith rdf:resource="http://www.ontologia.fr/OTB/otv#Difference"/>
        <owl:disjointWith rdf:resource="http://www.ontologia.fr/OTB/otv#Relation"/>
        <owl:disjointWith rdf:resource="http://www.ontologia.fr/OTB/otv#Attribute"/>
        <owl:disjointWith rdf:resource="http://www.ontologia.fr/OTB/otv#Object"/>
        <owl:disjointWith rdf:resource="http://www.ontologia.fr/OTB/otv#Term"/>
        <owl:disjointWith rdf:resource="http://www.ontologia.fr/OTB/otv#Concept"/>
</owl:Class>

<!-- ***********************************************
                     OTV OBJECT PROPERTIES
     *********************************************** -->

<!-- Conceptual dimension -->

<owl:ObjectProperty rdf:about="http://www.ontologia.fr/OTB/otv#isA">
    <rdfs:label>isA</rdfs:label> 
    <rdfs:comment>Generic relationship between 2 concepts</rdfs:comment>
    <rdfs:domain rdf:resource="http://www.ontologia.fr/OTB/otv#Concept"/>
    <rdfs:range rdf:resource="http://www.ontologia.fr/OTB/otv#Concept"/>
    <rdfs:isDefinedBy>http://www.ontologia.fr/OTB/otv.rdf</rdfs:isDefinedBy>
</owl:ObjectProperty>

<owl:ObjectProperty rdf:about="http://www.ontologia.fr/OTB/otv#ownDifference">
  <rdfs:label>ownDifference</rdfs:label>
  <rdfs:comment>Link a concept to one of its specific differences</rdfs:comment>
    <rdfs:domain rdf:resource="http://www.ontologia.fr/OTB/otv#Concept"/>
    <rdfs:range rdf:resource="http://www.ontologia.fr/OTB/otv#Difference"/>
</owl:ObjectProperty>

<owl:ObjectProperty rdf:about="http://www.ontologia.fr/OTB/otv#inheritedDifference">
  <rdfs:label>inheritedDifference</rdfs:label>
  <rdfs:comment>Link a concept to one of its inherited differences</rdfs:comment>
    <rdfs:domain rdf:resource="http://www.ontologia.fr/OTB/otv#Concept"/>
    <rdfs:range rdf:resource="http://www.ontologia.fr/OTB/otv#Difference"/>
</owl:ObjectProperty>

<owl:ObjectProperty rdf:about="http://www.ontologia.fr/OTB/otv#difference">
  <rdfs:label>difference</rdfs:label>
  <rdfs:comment>Link a concept to one of its differences either inherited or specific</rdfs:comment>
    <rdfs:domain rdf:resource="http://www.ontologia.fr/OTB/otv#Concept"/>
    <rdfs:range rdf:resource="http://www.ontologia.fr/OTB/otv#Difference"/>
</owl:ObjectProperty>

<owl:ObjectProperty rdf:about="http://www.ontologia.fr/OTB/otv#belongsToAxis">
  <rdfs:label>belongsToAxis</rdfs:label>
  <rdfs:comment>Indicate the axis of analysis to which the difference belongs</rdfs:comment>
    <rdfs:domain rdf:resource="http://www.ontologia.fr/OTB/otv#Difference"/>
    <rdfs:range rdf:resource="http://www.ontologia.fr/OTB/otv#AxisOfAnalysis"/>
</owl:ObjectProperty>

<owl:ObjectProperty rdf:about="http://www.ontologia.fr/OTB/otv#containsDifference">
  <rdfs:label>containsDifference</rdfs:label>
  <rdfs:comment>Indicate the differences which belongs to the axis of analysis</rdfs:comment>
    <rdfs:domain rdf:resource="http://www.ontologia.fr/OTB/otv#AxisOfAnalysis"/>
    <rdfs:range rdf:resource="http://www.ontologia.fr/OTB/otv#Difference"/>
</owl:ObjectProperty>

<owl:ObjectProperty rdf:about="http://www.ontologia.fr/OTB/otv#attribute">
  <rdfs:label>attribute</rdfs:label>
  <rdfs:comment>Link a concept to one of its attributes either inherited or specific</rdfs:comment>
    <rdfs:domain rdf:resource="http://www.ontologia.fr/OTB/otv#Concept"/>
    <rdfs:range rdf:resource="http://www.ontologia.fr/OTB/otv#Attribute"/>
</owl:ObjectProperty>

<owl:ObjectProperty rdf:about="http://www.ontologia.fr/OTB/otv#instanceOf">
    <rdfs:label>instanceOf</rdfs:label> 
    <rdfs:comment>instance relationship</rdfs:comment>
    <rdfs:domain rdf:resource="http://www.ontologia.fr/OTB/otv#Object"/>
    <rdfs:range rdf:resource="http://www.ontologia.fr/OTB/otv#Concept"/>
  <rdfs:isDefinedBy>http://www.ontologia.fr/OTB/otv.rdf</rdfs:isDefinedBy>
</owl:ObjectProperty>

<!-- Relations between the 2 dimensions -->

<owl:ObjectProperty rdf:about="http://www.ontologia.fr/OTB/otv#denotedByTerm">
    <rdfs:label>denotedByTerm</rdfs:label> 
    <rdfs:comment>Link a concept to a term which denotes it</rdfs:comment>
    <rdfs:domain rdf:resource="http://www.ontologia.fr/OTB/otv#Concept"/>
    <rdfs:range rdf:resource="http://www.ontologia.fr/OTB/otv#Term"/>
  <rdfs:isDefinedBy>http://www.ontologia.fr/OTB/otv.rdf</rdfs:isDefinedBy>
</owl:ObjectProperty>

<owl:ObjectProperty rdf:about="http://www.ontologia.fr/OTB/otv#denotedConcept">
    <rdfs:label>denotedConcept</rdfs:label> 
    <rdfs:comment>Property whose value is the OTV concept denoted by the term: &apos;a term is a verbal designation of a concept&apos; (ISO 1087)</rdfs:comment>
    <rdfs:domain rdf:resource="http://www.ontologia.fr/OTB/otv#Term"/>
    <rdfs:range rdf:resource="http://www.ontologia.fr/OTB/otv#Concept"/>
    <rdfs:isDefinedBy>http://www.ontologia.fr/OTB/otv.rdf</rdfs:isDefinedBy>
</owl:ObjectProperty>

<owl:ObjectProperty rdf:about="http://www.ontologia.fr/OTB/otv#denotedByProperName">
    <rdfs:label>denotedByProperName</rdfs:label>
    <rdfs:comment>The denotedByPrperName property links an individual (object) to a proper name which denotes it</rdfs:comment>
 	<rdfs:domain rdf:resource="http://www.ontologia.fr/OTB/otv#Object"/>
 	<rdfs:range rdf:resource="http://www.ontologia.fr/OTB/otv#ProperName"/>
    <rdfs:isDefinedBy>http://www.ontologia.fr/OTB/otv.rdf</rdfs:isDefinedBy>
</owl:ObjectProperty>

<owl:ObjectProperty rdf:about="http://www.ontologia.fr/OTB/otv#denotedObject">
   	<rdfs:label>denotedObject</rdfs:label>
    <rdfs:comment>Property whose value is the OTV object denoted by the proper name</rdfs:comment>
 	<rdfs:domain rdf:resource="http://www.ontologia.fr/OTB/otv#ProperName"/>
 	<rdfs:range rdf:resource="http://www.ontologia.fr/OTB/otv#Object"/>
    <rdfs:isDefinedBy>http://www.ontologia.fr/OTB/otv.rdf</rdfs:isDefinedBy>
</owl:ObjectProperty>


<!-- ***********************************************
                      OTV ANNOTATION PROPERTIES
       *********************************************** -->

<owl:AnnotationProperty rdf:about="http://www.ontologia.fr/OTB/otv#conceptName">
    <rdfs:label>conceptName</rdfs:label> 
    <rdfs:comment>Name of the concept</rdfs:comment>
    <rdfs:domain rdf:resource="http://www.ontologia.fr/OTB/otv#Concept"/>
    <rdfs:range rdf:resource="http://www.w3.org/2001/XMLSchema#string"/>
    <rdfs:isDefinedBy>http://www.ontologia.fr/OTB/otv.rdf</rdfs:isDefinedBy>
</owl:AnnotationProperty>

<owl:AnnotationProperty rdf:about="http://www.ontologia.fr/OTB/otv#termName">
    <rdfs:label>termName</rdfs:label> <!-- équivalent à rdfs:label -->
    <rdfs:comment>String representing the term</rdfs:comment>
 	  <rdfs:domain rdf:resource="http://www.ontologia.fr/OTB/otv#Term"/>
 	  <rdfs:range rdf:resource="http://www.w3.org/2001/XMLSchema#string"/>
   	<rdfs:isDefinedBy>http://www.ontologia.fr/OTB/otv.rdf</rdfs:isDefinedBy>
</owl:AnnotationProperty>

<owl:AnnotationProperty rdf:about="http://www.ontologia.fr/OTB/otv#properName">
 	  <rdfs:label>properName</rdfs:label>
    <rdfs:comment>String representing the proper name</rdfs:comment>
 	  <rdfs:domain rdf:resource="http://www.ontologia.fr/OTB/otv#ProperName"/>
 	  <rdfs:range rdf:resource="http://www.w3.org/2001/XMLSchema#string"/>
   	<rdfs:isDefinedBy>http://www.ontologia.fr/OTB/otv.rdf</rdfs:isDefinedBy>
</owl:AnnotationProperty>

<owl:AnnotationProperty rdf:about="http://www.ontologia.fr/OTB/otv#language">
 	  <rdfs:label>language</rdfs:label>
    <rdfs:comment>Property that denotes the language of the term</rdfs:comment>
    <rdfs:domain>
      <owl:Class>
        <owl:unionOf rdf:parseType="Collection">
          <rdf:Description rdf:about="http://www.ontologia.fr/OTB/otv#Term"/>
          <rdf:Description rdf:about="http://www.ontologia.fr/OTB/otv#ProperName"/>
        </owl:unionOf>
      </owl:Class>
    </rdfs:domain>
 	  <rdfs:range rdf:resource="http://www.w3.org/2001/XMLSchema#string"/>
   	<rdfs:isDefinedBy>http://www.ontologia.fr/OTB/otv.rdf</rdfs:isDefinedBy>
</owl:AnnotationProperty>

<owl:AnnotationProperty rdf:about="http://www.ontologia.fr/OTB/otv#termStatus">
	 <rdfs:label>termStatus</rdfs:label>
    <rdfs:comment>Property that indicates the status of the term</rdfs:comment>
 	  <rdfs:domain rdf:resource="http://www.ontologia.fr/OTB/otv#Term"/>
 	  <rdfs:range rdf:resource="http://www.w3.org/2001/XMLSchema#string"/>
   	<rdfs:isDefinedBy>http://www.ontologia.fr/OTB/otv.rdf</rdfs:isDefinedBy>
</owl:AnnotationProperty>

<owl:AnnotationProperty rdf:about="http://www.ontologia.fr/OTB/otv#termDefinition">
   <rdfs:label>termDefinition</rdfs:label>
    <rdfs:comment>Defintion of the term in natural language</rdfs:comment>
    <rdfs:domain rdf:resource="http://www.ontologia.fr/OTB/otv#Term"/>
    <rdfs:range rdf:resource="http://www.w3.org/2001/XMLSchema#string"/>
    <rdfs:isDefinedBy>http://www.ontologia.fr/OTB/otv.rdf</rdfs:isDefinedBy>
</owl:AnnotationProperty>

<owl:AnnotationProperty rdf:about="http://www.ontologia.fr/OTB/otv#context">
   <rdfs:label>context</rdfs:label>
    <rdfs:comment>Context associated to the term</rdfs:comment>
    <rdfs:domain rdf:resource="http://www.ontologia.fr/OTB/otv#Term"/>
    <rdfs:isDefinedBy>http://www.ontologia.fr/OTB/otv.rdf</rdfs:isDefinedBy>
</owl:AnnotationProperty>

<owl:AnnotationProperty rdf:about="http://www.ontologia.fr/OTB/otv#note">
   <rdfs:label>note</rdfs:label>
    <rdfs:comment>Note associated to the term</rdfs:comment>
    <rdfs:domain rdf:resource="http://www.ontologia.fr/OTB/otv#Term"/>
    <rdfs:isDefinedBy>http://www.ontologia.fr/OTB/otv.rdf</rdfs:isDefinedBy>
</owl:AnnotationProperty>

<owl:AnnotationProperty rdf:about="http://www.ontologia.fr/OTB/otv#partOfSpeech">
   <rdfs:label>partOfSpeech</rdfs:label>
    <rdfs:comment>Part of Speech of the term</rdfs:comment>
    <rdfs:domain rdf:resource="http://www.ontologia.fr/OTB/otv#Term"/>
    <rdfs:range rdf:resource="http://www.w3.org/2001/XMLSchema#string"/>
    <rdfs:isDefinedBy>http://www.ontologia.fr/OTB/otv.rdf</rdfs:isDefinedBy>
</owl:AnnotationProperty>

<owl:AnnotationProperty rdf:about="http://www.ontologia.fr/OTB/otv#gender">
   <rdfs:label>gender</rdfs:label>
    <rdfs:comment>Gender of the term</rdfs:comment>
    <rdfs:domain rdf:resource="http://www.ontologia.fr/OTB/otv#Term"/>
    <rdfs:range rdf:resource="http://www.w3.org/2001/XMLSchema#string"/>
    <rdfs:isDefinedBy>http://www.ontologia.fr/OTB/otv.rdf</rdfs:isDefinedBy>
</owl:AnnotationProperty>

<owl:AnnotationProperty rdf:about="http://www.ontologia.fr/OTB/otv#beginDate">
    <rdfs:label>beginDate</rdfs:label>
   	<rdfs:comment>Property that indicates the begin date of of an axis of analysis, concept, term, object</rdfs:comment>
    <rdfs:domain rdf:resource="http://www.ontologia.fr/OTB/otv#OTVCore"/>
    <rdfs:range rdf:resource="http://www.w3.org/2001/XMLSchema#dateTime"/>
   	<rdfs:isDefinedBy>http://www.ontologia.fr/OTB/otv.rdf</rdfs:isDefinedBy>
</owl:AnnotationProperty>

<owl:AnnotationProperty rdf:about="http://www.ontologia.fr/OTB/otv#endDate">
	 <rdfs:label>endDate</rdfs:label>
 	  <rdfs:comment>Property that indicates the end date of of an axis of analysis, concept, term, object</rdfs:comment>
    <rdfs:domain rdf:resource="http://www.ontologia.fr/OTB/otv#OTVCore"/>
    <rdfs:range rdf:resource="http://www.w3.org/2001/XMLSchema#dateTime"/>
   	<rdfs:isDefinedBy>http://www.ontologia.fr/OTB/otv.rdf</rdfs:isDefinedBy>
</owl:AnnotationProperty>


	<!-- 
	//////////////////////////////////////////////////////////
	//
	// OTV
	//
	//////////////////////////////////////////////////////////
	-->

<!-- ONTOTERMINOLOGY

	Ontoterminology: ALyrA_ontoterminology
	Author: Rafail Giannadakis
	Creation date: May 18, 2024
	Export date: August 25, 2024 time: 10:01:59 PM
	Generated by Tedi version: 3.7
	http://ontoterminology.com/tedi -->

	<!--  OTV Axes of Analysis and Differences -->

    <!-- Axis of Analysis: 11 Content -->

    <otv:AxisOfAnalysis rdf:about="#11_Content">
        <rdfs:label>11 Content</rdfs:label>
        <otv:containsDifference rdf:resource="#with_erotic_content"/>
        <otv:containsDifference rdf:resource="#with_gnomic_content"/>
        <otv:containsDifference rdf:resource="#with_imitation_content"/>
        <otv:containsDifference rdf:resource="#with_political_content"/>
        <otv:containsDifference rdf:resource="#with_war_content"/>
    </otv:AxisOfAnalysis>

    <otv:Difference rdf:about="#with_erotic_content">
        <rdf:type rdf:resource="http://www.ontologia.fr/OTB/otv#Difference"/>
        <rdfs:label>with erotic content</rdfs:label>
        <otv:belongsToAxis rdf:resource="#11_Content"/>
    </otv:Difference>

    <otv:Difference rdf:about="#with_gnomic_content">
        <rdf:type rdf:resource="http://www.ontologia.fr/OTB/otv#Difference"/>
        <rdfs:label>with gnomic content</rdfs:label>
        <otv:belongsToAxis rdf:resource="#11_Content"/>
    </otv:Difference>

    <otv:Difference rdf:about="#with_imitation_content">
        <rdf:type rdf:resource="http://www.ontologia.fr/OTB/otv#Difference"/>
        <rdfs:label>with imitation content</rdfs:label>
        <otv:belongsToAxis rdf:resource="#11_Content"/>
    </otv:Difference>

    <otv:Difference rdf:about="#with_political_content">
        <rdf:type rdf:resource="http://www.ontologia.fr/OTB/otv#Difference"/>
        <rdfs:label>with political content</rdfs:label>
        <otv:belongsToAxis rdf:resource="#11_Content"/>
    </otv:Difference>

    <otv:Difference rdf:about="#with_war_content">
        <rdf:type rdf:resource="http://www.ontologia.fr/OTB/otv#Difference"/>
        <rdfs:label>with war content</rdfs:label>
        <otv:belongsToAxis rdf:resource="#11_Content"/>
    </otv:Difference>

    <!-- Axis of Analysis: 8 Ancient Greek Subject -->

    <otv:AxisOfAnalysis rdf:about="#8_Ancient_Greek_Subject">
        <rdfs:label>8 Ancient Greek Subject</rdfs:label>
        <otv:containsDifference rdf:resource="#dedicated_to_a_god"/>
        <otv:containsDifference rdf:resource="#dedicated_to_mortal"/>
        <otv:containsDifference rdf:resource="#with_specific_content"/>
    </otv:AxisOfAnalysis>

    <otv:Difference rdf:about="#dedicated_to_a_god">
        <rdf:type rdf:resource="http://www.ontologia.fr/OTB/otv#Difference"/>
        <rdfs:label>dedicated to a god</rdfs:label>
        <otv:belongsToAxis rdf:resource="#8_Ancient_Greek_Subject"/>
    </otv:Difference>

    <otv:Difference rdf:about="#dedicated_to_mortal">
        <rdf:type rdf:resource="http://www.ontologia.fr/OTB/otv#Difference"/>
        <rdfs:label>dedicated to mortal</rdfs:label>
        <otv:belongsToAxis rdf:resource="#8_Ancient_Greek_Subject"/>
    </otv:Difference>

    <otv:Difference rdf:about="#with_specific_content">
        <rdf:type rdf:resource="http://www.ontologia.fr/OTB/otv#Difference"/>
        <rdfs:label>with specific content</rdfs:label>
        <otv:belongsToAxis rdf:resource="#8_Ancient_Greek_Subject"/>
    </otv:Difference>

    <!-- Axis of Analysis: 10 Dedicated to a mortal -->

    <otv:AxisOfAnalysis rdf:about="#10_Dedicated_to_a_mortal">
        <rdfs:label>10 Dedicated to a mortal</rdfs:label>
        <otv:containsDifference rdf:resource="#dedicated_to_a_dead_being"/>
        <otv:containsDifference rdf:resource="#dedicated_to_wedding_couple"/>
        <otv:containsDifference rdf:resource="#dedicated_to_winners_in_athletic_events"/>
    </otv:AxisOfAnalysis>

    <otv:Difference rdf:about="#dedicated_to_a_dead_being">
        <rdf:type rdf:resource="http://www.ontologia.fr/OTB/otv#Difference"/>
        <rdfs:label>dedicated to a dead being</rdfs:label>
        <otv:belongsToAxis rdf:resource="#10_Dedicated_to_a_mortal"/>
    </otv:Difference>

    <otv:Difference rdf:about="#dedicated_to_wedding_couple">
        <rdf:type rdf:resource="http://www.ontologia.fr/OTB/otv#Difference"/>
        <rdfs:label>dedicated to wedding couple</rdfs:label>
        <otv:belongsToAxis rdf:resource="#10_Dedicated_to_a_mortal"/>
    </otv:Difference>

    <otv:Difference rdf:about="#dedicated_to_winners_in_athletic_events">
        <rdf:type rdf:resource="http://www.ontologia.fr/OTB/otv#Difference"/>
        <rdfs:label>dedicated to winners in athletic events</rdfs:label>
        <otv:belongsToAxis rdf:resource="#10_Dedicated_to_a_mortal"/>
    </otv:Difference>

    <!-- Axis of Analysis: 9 Dedicated to a god -->

    <otv:AxisOfAnalysis rdf:about="#9_Dedicated_to_a_god">
        <rdfs:label>9 Dedicated to a god</rdfs:label>
        <otv:containsDifference rdf:resource="#dedicated_to_apollo"/>
        <otv:containsDifference rdf:resource="#dedicated_to_dionysus"/>
    </otv:AxisOfAnalysis>

    <otv:Difference rdf:about="#dedicated_to_apollo">
        <rdf:type rdf:resource="http://www.ontologia.fr/OTB/otv#Difference"/>
        <rdfs:label>dedicated to apollo</rdfs:label>
        <otv:belongsToAxis rdf:resource="#9_Dedicated_to_a_god"/>
    </otv:Difference>

    <otv:Difference rdf:about="#dedicated_to_dionysus">
        <rdf:type rdf:resource="http://www.ontologia.fr/OTB/otv#Difference"/>
        <rdfs:label>dedicated to dionysus</rdfs:label>
        <otv:belongsToAxis rdf:resource="#9_Dedicated_to_a_god"/>
    </otv:Difference>

    <!-- Axis of Analysis: 4 Ancient Greek Occassion -->

    <otv:AxisOfAnalysis rdf:about="#4_Ancient_Greek_Occassion">
        <rdfs:label>4 Ancient Greek Occassion</rdfs:label>
        <otv:containsDifference rdf:resource="#during_bride_procession"/>
        <otv:containsDifference rdf:resource="#on_the_way_to_an_altar"/>
    </otv:AxisOfAnalysis>

    <otv:Difference rdf:about="#during_bride_procession">
        <rdf:type rdf:resource="http://www.ontologia.fr/OTB/otv#Difference"/>
        <rdfs:label>during bride procession</rdfs:label>
        <otv:belongsToAxis rdf:resource="#4_Ancient_Greek_Occassion"/>
    </otv:Difference>

    <otv:Difference rdf:about="#on_the_way_to_an_altar">
        <rdf:type rdf:resource="http://www.ontologia.fr/OTB/otv#Difference"/>
        <rdfs:label>on the way to an altar</rdfs:label>
        <otv:belongsToAxis rdf:resource="#4_Ancient_Greek_Occassion"/>
    </otv:Difference>

    <!-- Axis of Analysis: 5 Ancient Greek Performer -->

    <otv:AxisOfAnalysis rdf:about="#5_Ancient_Greek_Performer">
        <rdfs:label>5 Ancient Greek Performer</rdfs:label>
        <otv:containsDifference rdf:resource="#performed_by_a_chorus_or_by_a_single_performer"/>
        <otv:containsDifference rdf:resource="#performed_by_a_chorus"/>
        <otv:containsDifference rdf:resource="#performed_by_a_single_performer"/>
    </otv:AxisOfAnalysis>

    <otv:Difference rdf:about="#performed_by_a_chorus_or_by_a_single_performer">
        <rdf:type rdf:resource="http://www.ontologia.fr/OTB/otv#Difference"/>
        <rdfs:label>performed by a chorus or by a single performer</rdfs:label>
        <otv:belongsToAxis rdf:resource="#5_Ancient_Greek_Performer"/>
    </otv:Difference>

    <otv:Difference rdf:about="#performed_by_a_chorus">
        <rdf:type rdf:resource="http://www.ontologia.fr/OTB/otv#Difference"/>
        <rdfs:label>performed by a chorus</rdfs:label>
        <otv:belongsToAxis rdf:resource="#5_Ancient_Greek_Performer"/>
    </otv:Difference>

    <otv:Difference rdf:about="#performed_by_a_single_performer">
        <rdf:type rdf:resource="http://www.ontologia.fr/OTB/otv#Difference"/>
        <rdfs:label>performed by a single performer</rdfs:label>
        <otv:belongsToAxis rdf:resource="#5_Ancient_Greek_Performer"/>
    </otv:Difference>

    <!-- Axis of Analysis: 7 Gender -->

    <otv:AxisOfAnalysis rdf:about="#7_Gender">
        <rdfs:label>7 Gender</rdfs:label>
        <otv:containsDifference rdf:resource="#female"/>
        <otv:containsDifference rdf:resource="#male"/>
    </otv:AxisOfAnalysis>

    <otv:Difference rdf:about="#female">
        <rdf:type rdf:resource="http://www.ontologia.fr/OTB/otv#Difference"/>
        <rdfs:label>female</rdfs:label>
        <otv:belongsToAxis rdf:resource="#7_Gender"/>
    </otv:Difference>

    <otv:Difference rdf:about="#male">
        <rdf:type rdf:resource="http://www.ontologia.fr/OTB/otv#Difference"/>
        <rdfs:label>male</rdfs:label>
        <otv:belongsToAxis rdf:resource="#7_Gender"/>
    </otv:Difference>

    <!-- Axis of Analysis: 1 Category -->

    <otv:AxisOfAnalysis rdf:about="#1_Category">
        <rdfs:label>1 Category</rdfs:label>
        <otv:containsDifference rdf:resource="#ancient_location"/>
        <otv:containsDifference rdf:resource="#archaic_lyric_composer"/>
        <otv:containsDifference rdf:resource="#archaic_lyric_poem"/>
        <otv:containsDifference rdf:resource="#before_common_era_century"/>
    </otv:AxisOfAnalysis>

    <otv:Difference rdf:about="#ancient_location">
        <rdf:type rdf:resource="http://www.ontologia.fr/OTB/otv#Difference"/>
        <rdfs:label>ancient location</rdfs:label>
        <otv:belongsToAxis rdf:resource="#1_Category"/>
    </otv:Difference>

    <otv:Difference rdf:about="#archaic_lyric_composer">
        <rdf:type rdf:resource="http://www.ontologia.fr/OTB/otv#Difference"/>
        <rdfs:label>archaic lyric composer</rdfs:label>
        <otv:belongsToAxis rdf:resource="#1_Category"/>
    </otv:Difference>

    <otv:Difference rdf:about="#archaic_lyric_poem">
        <rdf:type rdf:resource="http://www.ontologia.fr/OTB/otv#Difference"/>
        <rdfs:label>archaic lyric poem</rdfs:label>
        <otv:belongsToAxis rdf:resource="#1_Category"/>
    </otv:Difference>

    <otv:Difference rdf:about="#before_common_era_century">
        <rdf:type rdf:resource="http://www.ontologia.fr/OTB/otv#Difference"/>
        <rdfs:label>before common era century</rdfs:label>
        <otv:belongsToAxis rdf:resource="#1_Category"/>
    </otv:Difference>

    <!-- Axis of Analysis: 6 Type of chorus -->

    <otv:AxisOfAnalysis rdf:about="#6_Type_of_chorus">
        <rdfs:label>6 Type of chorus</rdfs:label>
        <otv:containsDifference rdf:resource="#performed_by_a_maidens_chorus"/>
        <otv:containsDifference rdf:resource="#performed_by_a_non-specific_type_of_chorus"/>
    </otv:AxisOfAnalysis>

    <otv:Difference rdf:about="#performed_by_a_maidens_chorus">
        <rdf:type rdf:resource="http://www.ontologia.fr/OTB/otv#Difference"/>
        <rdfs:label>performed by a maidens chorus</rdfs:label>
        <otv:belongsToAxis rdf:resource="#6_Type_of_chorus"/>
    </otv:Difference>

    <otv:Difference rdf:about="#performed_by_a_non-specific_type_of_chorus">
        <rdf:type rdf:resource="http://www.ontologia.fr/OTB/otv#Difference"/>
        <rdfs:label>performed by a non-specific type of chorus</rdfs:label>
        <otv:belongsToAxis rdf:resource="#6_Type_of_chorus"/>
    </otv:Difference>

    <!-- Axis of Analysis: 2 Ancient Greek Dialect -->

    <otv:AxisOfAnalysis rdf:about="#2_Ancient_Greek_Dialect">
        <rdfs:label>2 Ancient Greek Dialect</rdfs:label>
        <otv:containsDifference rdf:resource="#in_ionic_or_in_doric_or_in_aeolic_dialect"/>
        <otv:containsDifference rdf:resource="#only_in_ionic_dialect"/>
    </otv:AxisOfAnalysis>

    <otv:Difference rdf:about="#in_ionic_or_in_doric_or_in_aeolic_dialect">
        <rdf:type rdf:resource="http://www.ontologia.fr/OTB/otv#Difference"/>
        <rdfs:label>in ionic or in doric or in aeolic dialect</rdfs:label>
        <otv:belongsToAxis rdf:resource="#2_Ancient_Greek_Dialect"/>
    </otv:Difference>

    <otv:Difference rdf:about="#only_in_ionic_dialect">
        <rdf:type rdf:resource="http://www.ontologia.fr/OTB/otv#Difference"/>
        <rdfs:label>only in ionic dialect</rdfs:label>
        <otv:belongsToAxis rdf:resource="#2_Ancient_Greek_Dialect"/>
    </otv:Difference>

    <!-- Axis of Analysis: 3 Ancient Greek Metre -->

    <otv:AxisOfAnalysis rdf:about="#3_Ancient_Greek_Metre">
        <rdfs:label>3 Ancient Greek Metre</rdfs:label>
        <otv:containsDifference rdf:resource="#in_elegiac_couplet"/>
        <otv:containsDifference rdf:resource="#in_iambic_or_trochaic_metre"/>
    </otv:AxisOfAnalysis>

    <otv:Difference rdf:about="#in_elegiac_couplet">
        <rdf:type rdf:resource="http://www.ontologia.fr/OTB/otv#Difference"/>
        <rdfs:label>in elegiac couplet</rdfs:label>
        <otv:belongsToAxis rdf:resource="#3_Ancient_Greek_Metre"/>
    </otv:Difference>

    <otv:Difference rdf:about="#in_iambic_or_trochaic_metre">
        <rdf:type rdf:resource="http://www.ontologia.fr/OTB/otv#Difference"/>
        <rdfs:label>in iambic or trochaic metre</rdfs:label>
        <otv:belongsToAxis rdf:resource="#3_Ancient_Greek_Metre"/>
    </otv:Difference>

	<!--  OTV Relations -->

    <otv:Relation rdf:about="#bornIn"/>
    <otv:Relation rdf:about="#centuryOfLiving"/>
    <otv:Relation rdf:about="#hasFunction"/>
    <otv:Relation rdf:about="#hasPart"/>
    <otv:Relation rdf:about="#hasWritten"/>
    <otv:Relation rdf:about="#isBirthPlaceOf"/>
    <otv:Relation rdf:about="#isCenturyOf"/>
    <otv:Relation rdf:about="#isRelatedTo"/>
    <otv:Relation rdf:about="#isWrittenBy"/>
    <otv:Relation rdf:about="#residentedBy"/>
    <otv:Relation rdf:about="#stayedIn"/>
	<!--  OTV Attributes -->

    <otv:Attribute rdf:about="#endsIn"/>
    <otv:Attribute rdf:about="#passageChoselEl"/>
    <otv:Attribute rdf:about="#passageChosenEn"/>
    <otv:Attribute rdf:about="#pleiadesCoordinates"/>
    <otv:Attribute rdf:about="#startsIn"/>
    <otv:Attribute rdf:about="#tlgIdentifyingNumber"/>
	<!--  OTV Concepts -->

    <otv:Concept rdf:about="#Archaic_Lyric_Composer">
        <otv:conceptName>&lt;Archaic Lyric Composer&gt;</otv:conceptName>
        <otv:ownDifference rdf:resource="#archaic_lyric_composer"/>
        <otv:difference rdf:resource="#archaic_lyric_composer"/>
        <bornIn rdf:resource="#Ancient_Location"/>
        <centuryOfLiving rdf:resource="#BCE_century"/>
        <hasWritten rdf:resource="#Archaic_Lyric_Poem"/>
        <stayedIn rdf:resource="#Ancient_Location"/>
        <otv:attribute rdf:resource="#tlgIdentifyingNumber"/>
        <otv:attribute rdf:resource="#passageChosenEn"/>
        <otv:attribute rdf:resource="#passageChoselEl"/>
        <otv:denotedByTerm rdf:resource="#archaic_lyric_composer_en"/>
        <otv:denotedByTerm rdf:resource="#αρχαϊκός_λυρικός_συνθέτης_el"/>
    </otv:Concept>

    <otv:Concept rdf:about="#Archaic_Lyric_Poem_only_in_ionic_dialect_in_elegiac_couplet">
        <otv:conceptName>&lt;Archaic Lyric Poem only in ionic dialect in elegiac couplet&gt;</otv:conceptName>
        <otv:isA rdf:resource="#Archaic_Lyric_Poem_only_in_ionic_dialect"/>
        <otv:ownDifference rdf:resource="#in_elegiac_couplet"/>
        <otv:inheritedDifference rdf:resource="#only_in_ionic_dialect"/>
        <otv:inheritedDifference rdf:resource="#archaic_lyric_poem"/>
        <otv:difference rdf:resource="#in_elegiac_couplet"/>
        <otv:difference rdf:resource="#only_in_ionic_dialect"/>
        <otv:difference rdf:resource="#archaic_lyric_poem"/>
        <isWrittenBy rdf:resource="#Archaic_Lyric_Composer"/>
        <otv:denotedByTerm rdf:resource="#elegy_en"/>
        <otv:denotedByTerm rdf:resource="#ελεγεία_el"/>
    </otv:Concept>

    <otv:Concept rdf:about="#Archaic_Lyric_Poem">
        <otv:conceptName>&lt;Archaic Lyric Poem&gt;</otv:conceptName>
        <otv:ownDifference rdf:resource="#archaic_lyric_poem"/>
        <otv:difference rdf:resource="#archaic_lyric_poem"/>
        <isWrittenBy rdf:resource="#Archaic_Lyric_Composer"/>
        <otv:denotedByTerm rdf:resource="#archaic_lyric_poem_en"/>
        <otv:denotedByTerm rdf:resource="#αρχαϊκό_λυρικό_ποίημα_el"/>
    </otv:Concept>

    <otv:Concept rdf:about="#Archaic_Lyric_Poem_in_ionic_or_in_doric_or_in_aeolic_dialect_performed_by_a_chorus_or_by_a_single_performer_dedicated_to_apollo">
        <otv:conceptName>&lt;Archaic Lyric Poem in ionic or in doric or in aeolic dialect performed by a chorus or by a single performer dedicated to apollo&gt;</otv:conceptName>
        <otv:isA rdf:resource="#Archaic_Lyric_Poem_in_ionic_or_in_doric_or_in_aeolic_dialect_performed_by_a_chorus_or_by_a_single_performer_dedicated_to_a_god"/>
        <otv:ownDifference rdf:resource="#dedicated_to_apollo"/>
        <otv:inheritedDifference rdf:resource="#dedicated_to_a_god"/>
        <otv:inheritedDifference rdf:resource="#performed_by_a_chorus_or_by_a_single_performer"/>
        <otv:inheritedDifference rdf:resource="#in_ionic_or_in_doric_or_in_aeolic_dialect"/>
        <otv:inheritedDifference rdf:resource="#archaic_lyric_poem"/>
        <otv:difference rdf:resource="#dedicated_to_apollo"/>
        <otv:difference rdf:resource="#dedicated_to_a_god"/>
        <otv:difference rdf:resource="#performed_by_a_chorus_or_by_a_single_performer"/>
        <otv:difference rdf:resource="#in_ionic_or_in_doric_or_in_aeolic_dialect"/>
        <otv:difference rdf:resource="#archaic_lyric_poem"/>
        <isWrittenBy rdf:resource="#Archaic_Lyric_Composer"/>
        <otv:denotedByTerm rdf:resource="#paean_en"/>
        <otv:denotedByTerm rdf:resource="#παιάνας_el"/>
    </otv:Concept>

    <otv:Concept rdf:about="#Archaic_Lyric_Poem_only_in_ionic_dialect_in_elegiac_couplet_with_gnomic_content">
        <otv:conceptName>&lt;Archaic Lyric Poem only in ionic dialect in elegiac couplet with gnomic content&gt;</otv:conceptName>
        <otv:isA rdf:resource="#Archaic_Lyric_Poem_only_in_ionic_dialect_in_elegiac_couplet"/>
        <otv:ownDifference rdf:resource="#with_specific_content"/>
        <otv:ownDifference rdf:resource="#with_gnomic_content"/>
        <otv:inheritedDifference rdf:resource="#in_elegiac_couplet"/>
        <otv:inheritedDifference rdf:resource="#only_in_ionic_dialect"/>
        <otv:inheritedDifference rdf:resource="#archaic_lyric_poem"/>
        <otv:difference rdf:resource="#with_gnomic_content"/>
        <otv:difference rdf:resource="#with_specific_content"/>
        <otv:difference rdf:resource="#in_elegiac_couplet"/>
        <otv:difference rdf:resource="#only_in_ionic_dialect"/>
        <otv:difference rdf:resource="#archaic_lyric_poem"/>
        <isWrittenBy rdf:resource="#Archaic_Lyric_Composer"/>
        <otv:denotedByTerm rdf:resource="#gnomic_elegy_en"/>
        <otv:denotedByTerm rdf:resource="#γνωμική_ελεγεία_el"/>
    </otv:Concept>

    <otv:Concept rdf:about="#Archaic_Lyric_Poem_in_ionic_or_in_doric_or_in_aeolic_dialect_performed_by_a_chorus">
        <otv:conceptName>&lt;Archaic Lyric Poem in ionic or in doric or in aeolic dialect performed by a chorus&gt;</otv:conceptName>
        <otv:isA rdf:resource="#Archaic_Lyric_Poem_in_ionic_or_in_doric_or_in_aeolic_dialect"/>
        <otv:ownDifference rdf:resource="#performed_by_a_chorus"/>
        <otv:inheritedDifference rdf:resource="#in_ionic_or_in_doric_or_in_aeolic_dialect"/>
        <otv:inheritedDifference rdf:resource="#archaic_lyric_poem"/>
        <otv:difference rdf:resource="#performed_by_a_chorus"/>
        <otv:difference rdf:resource="#in_ionic_or_in_doric_or_in_aeolic_dialect"/>
        <otv:difference rdf:resource="#archaic_lyric_poem"/>
        <isWrittenBy rdf:resource="#Archaic_Lyric_Composer"/>
        <otv:denotedByTerm rdf:resource="#archaic_lyric_poem_in_ionic_or_in_doric_or_in_aeolic_dialect_performed_by_a_chorus_en"/>
        <otv:denotedByTerm rdf:resource="#αρχαϊκό_λυρικό_ποίημα_σε_ιωνική_ή_δωρική_ή_αιολική_διάλεκτο_που_εκτελείται_από_χορό_el"/>
    </otv:Concept>

    <otv:Concept rdf:about="#Archaic_Lyric_Poem_in_ionic_or_in_doric_or_in_aeolic_dialect_performed_by_a_chorus_on_the_way_to_an_altar">
        <otv:conceptName>&lt;Archaic Lyric Poem in ionic or in doric or in aeolic dialect performed by a chorus on the way to an altar&gt;</otv:conceptName>
        <otv:isA rdf:resource="#Archaic_Lyric_Poem_in_ionic_or_in_doric_or_in_aeolic_dialect_performed_by_a_chorus_performed_by_a_non-specific_type_of_chorus"/>
        <otv:ownDifference rdf:resource="#on_the_way_to_an_altar"/>
        <otv:inheritedDifference rdf:resource="#performed_by_a_non-specific_type_of_chorus"/>
        <otv:inheritedDifference rdf:resource="#performed_by_a_chorus"/>
        <otv:inheritedDifference rdf:resource="#in_ionic_or_in_doric_or_in_aeolic_dialect"/>
        <otv:inheritedDifference rdf:resource="#archaic_lyric_poem"/>
        <otv:difference rdf:resource="#on_the_way_to_an_altar"/>
        <otv:difference rdf:resource="#performed_by_a_non-specific_type_of_chorus"/>
        <otv:difference rdf:resource="#performed_by_a_chorus"/>
        <otv:difference rdf:resource="#in_ionic_or_in_doric_or_in_aeolic_dialect"/>
        <otv:difference rdf:resource="#archaic_lyric_poem"/>
        <isWrittenBy rdf:resource="#Archaic_Lyric_Composer"/>
        <otv:denotedByTerm rdf:resource="#prosodion_en"/>
        <otv:denotedByTerm rdf:resource="#προσόδιο_el"/>
    </otv:Concept>

    <otv:Concept rdf:about="#Archaic_Lyric_Poem_in_ionic_or_in_doric_or_in_aeolic_dialect_performed_by_a_single_performer">
        <otv:conceptName>&lt;Archaic Lyric Poem in ionic or in doric or in aeolic dialect performed by a single performer&gt;</otv:conceptName>
        <otv:isA rdf:resource="#Archaic_Lyric_Poem_in_ionic_or_in_doric_or_in_aeolic_dialect"/>
        <otv:ownDifference rdf:resource="#performed_by_a_single_performer"/>
        <otv:inheritedDifference rdf:resource="#in_ionic_or_in_doric_or_in_aeolic_dialect"/>
        <otv:inheritedDifference rdf:resource="#archaic_lyric_poem"/>
        <otv:difference rdf:resource="#performed_by_a_single_performer"/>
        <otv:difference rdf:resource="#in_ionic_or_in_doric_or_in_aeolic_dialect"/>
        <otv:difference rdf:resource="#archaic_lyric_poem"/>
        <isWrittenBy rdf:resource="#Archaic_Lyric_Composer"/>
        <otv:denotedByTerm rdf:resource="#monody_en"/>
        <otv:denotedByTerm rdf:resource="#μονωδία_el"/>
    </otv:Concept>

    <otv:Concept rdf:about="#Archaic_Lyric_Poem_only_in_ionic_dialect">
        <otv:conceptName>&lt;Archaic Lyric Poem only in ionic dialect&gt;</otv:conceptName>
        <otv:isA rdf:resource="#Archaic_Lyric_Poem"/>
        <otv:ownDifference rdf:resource="#only_in_ionic_dialect"/>
        <otv:inheritedDifference rdf:resource="#archaic_lyric_poem"/>
        <otv:difference rdf:resource="#only_in_ionic_dialect"/>
        <otv:difference rdf:resource="#archaic_lyric_poem"/>
        <isWrittenBy rdf:resource="#Archaic_Lyric_Composer"/>
        <otv:denotedByTerm rdf:resource="#archaic_lyric_poem_only_in_ionic_dialect_en"/>
        <otv:denotedByTerm rdf:resource="#αρχαϊκό_λυρικό_ποίημα_μόνο_στην_ιωνική_διάλεκτο_el"/>
    </otv:Concept>

    <otv:Concept rdf:about="#Ancient_Location">
        <otv:conceptName>&lt;Ancient Location&gt;</otv:conceptName>
        <otv:ownDifference rdf:resource="#ancient_location"/>
        <otv:difference rdf:resource="#ancient_location"/>
        <isBirthPlaceOf rdf:resource="#Archaic_Lyric_Composer"/>
        <residentedBy rdf:resource="#Archaic_Lyric_Composer"/>
        <otv:attribute rdf:resource="#pleiadesCoordinates"/>
        <otv:denotedByTerm rdf:resource="#ancient_location_en"/>
        <otv:denotedByTerm rdf:resource="#αρχαία_τοποθεσία_el"/>
    </otv:Concept>

    <otv:Concept rdf:about="#Archaic_Lyric_Poem_in_ionic_or_in_doric_or_in_aeolic_dialect_performed_by_a_chorus_or_by_a_single_performer_dedicated_to_dionysus">
        <otv:conceptName>&lt;Archaic Lyric Poem in ionic or in doric or in aeolic dialect performed by a chorus or by a single performer dedicated to dionysus&gt;</otv:conceptName>
        <otv:isA rdf:resource="#Archaic_Lyric_Poem_in_ionic_or_in_doric_or_in_aeolic_dialect_performed_by_a_chorus_or_by_a_single_performer_dedicated_to_a_god"/>
        <otv:ownDifference rdf:resource="#dedicated_to_dionysus"/>
        <otv:inheritedDifference rdf:resource="#dedicated_to_a_god"/>
        <otv:inheritedDifference rdf:resource="#performed_by_a_chorus_or_by_a_single_performer"/>
        <otv:inheritedDifference rdf:resource="#in_ionic_or_in_doric_or_in_aeolic_dialect"/>
        <otv:inheritedDifference rdf:resource="#archaic_lyric_poem"/>
        <otv:difference rdf:resource="#dedicated_to_dionysus"/>
        <otv:difference rdf:resource="#dedicated_to_a_god"/>
        <otv:difference rdf:resource="#performed_by_a_chorus_or_by_a_single_performer"/>
        <otv:difference rdf:resource="#in_ionic_or_in_doric_or_in_aeolic_dialect"/>
        <otv:difference rdf:resource="#archaic_lyric_poem"/>
        <isWrittenBy rdf:resource="#Archaic_Lyric_Composer"/>
        <otv:denotedByTerm rdf:resource="#dithyramb_en"/>
        <otv:denotedByTerm rdf:resource="#διθύραμβος_el"/>
    </otv:Concept>

    <otv:Concept rdf:about="#Archaic_Lyric_Poem_in_ionic_or_in_doric_or_in_aeolic_dialect_performed_by_a_chorus_or_by_a_single_performer_dedicated_to_a_god">
        <otv:conceptName>&lt;Archaic Lyric Poem in ionic or in doric or in aeolic dialect performed by a chorus or by a single performer dedicated to a god&gt;</otv:conceptName>
        <otv:isA rdf:resource="#Archaic_Lyric_Poem_in_ionic_or_in_doric_or_in_aeolic_dialect_performed_by_a_chorus_or_by_a_single_performer"/>
        <otv:ownDifference rdf:resource="#dedicated_to_a_god"/>
        <otv:inheritedDifference rdf:resource="#performed_by_a_chorus_or_by_a_single_performer"/>
        <otv:inheritedDifference rdf:resource="#in_ionic_or_in_doric_or_in_aeolic_dialect"/>
        <otv:inheritedDifference rdf:resource="#archaic_lyric_poem"/>
        <otv:difference rdf:resource="#dedicated_to_a_god"/>
        <otv:difference rdf:resource="#performed_by_a_chorus_or_by_a_single_performer"/>
        <otv:difference rdf:resource="#in_ionic_or_in_doric_or_in_aeolic_dialect"/>
        <otv:difference rdf:resource="#archaic_lyric_poem"/>
        <isWrittenBy rdf:resource="#Archaic_Lyric_Composer"/>
        <otv:denotedByTerm rdf:resource="#hymn_en"/>
        <otv:denotedByTerm rdf:resource="#ύμνος_el"/>
    </otv:Concept>

    <otv:Concept rdf:about="#Archaic_Lyric_Poem_only_in_ionic_dialect_in_iambic_or_trochaic_metre">
        <otv:conceptName>&lt;Archaic Lyric Poem only in ionic dialect in iambic or trochaic metre&gt;</otv:conceptName>
        <otv:isA rdf:resource="#Archaic_Lyric_Poem_only_in_ionic_dialect"/>
        <otv:ownDifference rdf:resource="#in_iambic_or_trochaic_metre"/>
        <otv:inheritedDifference rdf:resource="#only_in_ionic_dialect"/>
        <otv:inheritedDifference rdf:resource="#archaic_lyric_poem"/>
        <otv:difference rdf:resource="#in_iambic_or_trochaic_metre"/>
        <otv:difference rdf:resource="#only_in_ionic_dialect"/>
        <otv:difference rdf:resource="#archaic_lyric_poem"/>
        <isWrittenBy rdf:resource="#Archaic_Lyric_Composer"/>
        <otv:denotedByTerm rdf:resource="#iamb_en"/>
        <otv:denotedByTerm rdf:resource="#ίαμβος_el"/>
    </otv:Concept>

    <otv:Concept rdf:about="#Archaic_Lyric_Poem_in_ionic_or_in_doric_or_in_aeolic_dialect_performed_by_a_chorus_or_by_a_single_performer">
        <otv:conceptName>&lt;Archaic Lyric Poem in ionic or in doric or in aeolic dialect performed by a chorus or by a single performer&gt;</otv:conceptName>
        <otv:isA rdf:resource="#Archaic_Lyric_Poem_in_ionic_or_in_doric_or_in_aeolic_dialect"/>
        <otv:ownDifference rdf:resource="#performed_by_a_chorus_or_by_a_single_performer"/>
        <otv:inheritedDifference rdf:resource="#in_ionic_or_in_doric_or_in_aeolic_dialect"/>
        <otv:inheritedDifference rdf:resource="#archaic_lyric_poem"/>
        <otv:difference rdf:resource="#performed_by_a_chorus_or_by_a_single_performer"/>
        <otv:difference rdf:resource="#in_ionic_or_in_doric_or_in_aeolic_dialect"/>
        <otv:difference rdf:resource="#archaic_lyric_poem"/>
        <isWrittenBy rdf:resource="#Archaic_Lyric_Composer"/>
        <otv:denotedByTerm rdf:resource="#archaic_lyric_poem_in_ionic_or_in_doric_or_in_aeolic_dialect_performed_by_a_chorus_or_by_a_single_performer_en"/>
        <otv:denotedByTerm rdf:resource="#αρχαϊκό_λυρικό_ποίημα_σε_ιωνική_ή_δωρική_ή_αιολική_διάλεκτο_που_εκτελείται_από_χορό_ή_από_έναν_μόνο_ερμηνευτή_el"/>
    </otv:Concept>

    <otv:Concept rdf:about="#Archaic_Lyric_Poem_in_ionic_or_in_doric_or_in_aeolic_dialect_performed_by_a_chorus_or_by_a_single_performer_dedicated_to_dead">
        <otv:conceptName>&lt;Archaic Lyric Poem in ionic or in doric or in aeolic dialect performed by a chorus or by a single performer dedicated to dead&gt;</otv:conceptName>
        <otv:isA rdf:resource="#Archaic_Lyric_Poem_in_ionic_or_in_doric_or_in_aeolic_dialect_performed_by_a_chorus_or_by_a_single_performer_dedicated_to_living"/>
        <otv:ownDifference rdf:resource="#dedicated_to_a_dead_being"/>
        <otv:inheritedDifference rdf:resource="#dedicated_to_mortal"/>
        <otv:inheritedDifference rdf:resource="#performed_by_a_chorus_or_by_a_single_performer"/>
        <otv:inheritedDifference rdf:resource="#in_ionic_or_in_doric_or_in_aeolic_dialect"/>
        <otv:inheritedDifference rdf:resource="#archaic_lyric_poem"/>
        <otv:difference rdf:resource="#dedicated_to_a_dead_being"/>
        <otv:difference rdf:resource="#dedicated_to_mortal"/>
        <otv:difference rdf:resource="#performed_by_a_chorus_or_by_a_single_performer"/>
        <otv:difference rdf:resource="#in_ionic_or_in_doric_or_in_aeolic_dialect"/>
        <otv:difference rdf:resource="#archaic_lyric_poem"/>
        <isWrittenBy rdf:resource="#Archaic_Lyric_Composer"/>
        <otv:denotedByTerm rdf:resource="#threnos_en"/>
        <otv:denotedByTerm rdf:resource="#θρήνος_el"/>
    </otv:Concept>

    <otv:Concept rdf:about="#Archaic_Lyric_Poem_in_ionic_or_in_doric_or_in_aeolic_dialect">
        <otv:conceptName>&lt;Archaic Lyric Poem in ionic or in doric or in aeolic dialect&gt;</otv:conceptName>
        <otv:isA rdf:resource="#Archaic_Lyric_Poem"/>
        <otv:ownDifference rdf:resource="#in_ionic_or_in_doric_or_in_aeolic_dialect"/>
        <otv:inheritedDifference rdf:resource="#archaic_lyric_poem"/>
        <otv:difference rdf:resource="#in_ionic_or_in_doric_or_in_aeolic_dialect"/>
        <otv:difference rdf:resource="#archaic_lyric_poem"/>
        <isWrittenBy rdf:resource="#Archaic_Lyric_Composer"/>
        <otv:denotedByTerm rdf:resource="#melos_en"/>
        <otv:denotedByTerm rdf:resource="#μέλος_el"/>
    </otv:Concept>

    <otv:Concept rdf:about="#Archaic_Lyric_Poem_only_in_ionic_dialect_in_elegiac_couplet_with_war_content">
        <otv:conceptName>&lt;Archaic Lyric Poem only in ionic dialect in elegiac couplet with war content&gt;</otv:conceptName>
        <otv:isA rdf:resource="#Archaic_Lyric_Poem_only_in_ionic_dialect_in_elegiac_couplet"/>
        <otv:ownDifference rdf:resource="#with_specific_content"/>
        <otv:ownDifference rdf:resource="#with_war_content"/>
        <otv:inheritedDifference rdf:resource="#in_elegiac_couplet"/>
        <otv:inheritedDifference rdf:resource="#only_in_ionic_dialect"/>
        <otv:inheritedDifference rdf:resource="#archaic_lyric_poem"/>
        <otv:difference rdf:resource="#with_war_content"/>
        <otv:difference rdf:resource="#with_specific_content"/>
        <otv:difference rdf:resource="#in_elegiac_couplet"/>
        <otv:difference rdf:resource="#only_in_ionic_dialect"/>
        <otv:difference rdf:resource="#archaic_lyric_poem"/>
        <isWrittenBy rdf:resource="#Archaic_Lyric_Composer"/>
        <otv:denotedByTerm rdf:resource="#war_elegy_en"/>
        <otv:denotedByTerm rdf:resource="#πολεμική_ελεγεία_el"/>
    </otv:Concept>

    <otv:Concept rdf:about="#Archaic_Lyric_Poem_in_ionic_or_in_doric_or_in_aeolic_dialect_performed_by_a_chorus_with_imitation_expressions">
        <otv:conceptName>&lt;Archaic Lyric Poem in ionic or in doric or in aeolic dialect performed by a chorus with imitation expressions&gt;</otv:conceptName>
        <otv:isA rdf:resource="#Archaic_Lyric_Poem_in_ionic_or_in_doric_or_in_aeolic_dialect_performed_by_a_chorus_performed_by_a_non-specific_type_of_chorus"/>
        <otv:ownDifference rdf:resource="#with_specific_content"/>
        <otv:ownDifference rdf:resource="#with_imitation_content"/>
        <otv:inheritedDifference rdf:resource="#performed_by_a_non-specific_type_of_chorus"/>
        <otv:inheritedDifference rdf:resource="#performed_by_a_chorus"/>
        <otv:inheritedDifference rdf:resource="#in_ionic_or_in_doric_or_in_aeolic_dialect"/>
        <otv:inheritedDifference rdf:resource="#archaic_lyric_poem"/>
        <otv:difference rdf:resource="#with_imitation_content"/>
        <otv:difference rdf:resource="#with_specific_content"/>
        <otv:difference rdf:resource="#performed_by_a_non-specific_type_of_chorus"/>
        <otv:difference rdf:resource="#performed_by_a_chorus"/>
        <otv:difference rdf:resource="#in_ionic_or_in_doric_or_in_aeolic_dialect"/>
        <otv:difference rdf:resource="#archaic_lyric_poem"/>
        <isWrittenBy rdf:resource="#Archaic_Lyric_Composer"/>
        <otv:denotedByTerm rdf:resource="#hyporcheme_en"/>
        <otv:denotedByTerm rdf:resource="#υπόρχημα_el"/>
    </otv:Concept>

    <otv:Concept rdf:about="#Archaic_Lyric_Poem_in_ionic_or_in_doric_or_in_aeolic_dialect_performed_by_a_chorus_or_by_a_single_performer_dedicated_to_wedding_couple">
        <otv:conceptName>&lt;Archaic Lyric Poem in ionic or in doric or in aeolic dialect performed by a chorus or by a single performer dedicated to wedding couple&gt;</otv:conceptName>
        <otv:isA rdf:resource="#Archaic_Lyric_Poem_in_ionic_or_in_doric_or_in_aeolic_dialect_performed_by_a_chorus_or_by_a_single_performer_dedicated_to_living"/>
        <otv:ownDifference rdf:resource="#dedicated_to_wedding_couple"/>
        <otv:inheritedDifference rdf:resource="#dedicated_to_mortal"/>
        <otv:inheritedDifference rdf:resource="#performed_by_a_chorus_or_by_a_single_performer"/>
        <otv:inheritedDifference rdf:resource="#in_ionic_or_in_doric_or_in_aeolic_dialect"/>
        <otv:inheritedDifference rdf:resource="#archaic_lyric_poem"/>
        <otv:difference rdf:resource="#dedicated_to_wedding_couple"/>
        <otv:difference rdf:resource="#dedicated_to_mortal"/>
        <otv:difference rdf:resource="#performed_by_a_chorus_or_by_a_single_performer"/>
        <otv:difference rdf:resource="#in_ionic_or_in_doric_or_in_aeolic_dialect"/>
        <otv:difference rdf:resource="#archaic_lyric_poem"/>
        <isWrittenBy rdf:resource="#Archaic_Lyric_Composer"/>
        <otv:denotedByTerm rdf:resource="#epithalamion_en"/>
        <otv:denotedByTerm rdf:resource="#επιθαλάμιο_el"/>
    </otv:Concept>

    <otv:Concept rdf:about="#Archaic_Lyric_Poem_only_in_ionic_dialect_in_elegiac_couplet_with_political_content">
        <otv:conceptName>&lt;Archaic Lyric Poem only in ionic dialect in elegiac couplet with political content&gt;</otv:conceptName>
        <otv:isA rdf:resource="#Archaic_Lyric_Poem_only_in_ionic_dialect_in_elegiac_couplet"/>
        <otv:ownDifference rdf:resource="#with_specific_content"/>
        <otv:ownDifference rdf:resource="#with_political_content"/>
        <otv:inheritedDifference rdf:resource="#in_elegiac_couplet"/>
        <otv:inheritedDifference rdf:resource="#only_in_ionic_dialect"/>
        <otv:inheritedDifference rdf:resource="#archaic_lyric_poem"/>
        <otv:difference rdf:resource="#with_political_content"/>
        <otv:difference rdf:resource="#with_specific_content"/>
        <otv:difference rdf:resource="#in_elegiac_couplet"/>
        <otv:difference rdf:resource="#only_in_ionic_dialect"/>
        <otv:difference rdf:resource="#archaic_lyric_poem"/>
        <isWrittenBy rdf:resource="#Archaic_Lyric_Composer"/>
        <otv:denotedByTerm rdf:resource="#political_elegy_en"/>
        <otv:denotedByTerm rdf:resource="#πολιτική_ελεγεία_el"/>
    </otv:Concept>

    <otv:Concept rdf:about="#Archaic_Lyric_Poem_in_ionic_or_in_doric_or_in_aeolic_dialect_performed_by_a_chorus_performed_by_a_non-specific_type_of_chorus">
        <otv:conceptName>&lt;Archaic Lyric Poem in ionic or in doric or in aeolic dialect performed by a chorus performed by a non-specific type of chorus&gt;</otv:conceptName>
        <otv:isA rdf:resource="#Archaic_Lyric_Poem_in_ionic_or_in_doric_or_in_aeolic_dialect_performed_by_a_chorus"/>
        <otv:ownDifference rdf:resource="#performed_by_a_non-specific_type_of_chorus"/>
        <otv:inheritedDifference rdf:resource="#performed_by_a_chorus"/>
        <otv:inheritedDifference rdf:resource="#in_ionic_or_in_doric_or_in_aeolic_dialect"/>
        <otv:inheritedDifference rdf:resource="#archaic_lyric_poem"/>
        <otv:difference rdf:resource="#performed_by_a_non-specific_type_of_chorus"/>
        <otv:difference rdf:resource="#performed_by_a_chorus"/>
        <otv:difference rdf:resource="#in_ionic_or_in_doric_or_in_aeolic_dialect"/>
        <otv:difference rdf:resource="#archaic_lyric_poem"/>
        <isWrittenBy rdf:resource="#Archaic_Lyric_Composer"/>
        <otv:denotedByTerm rdf:resource="#archaic_lyric_poem_in_ionic_or_doric_or_aeolic_dialect_performed_by_a_chorus_of_no_particular_type_en"/>
        <otv:denotedByTerm rdf:resource="#αρχαϊκό_λυρικό_ποίημα_σε_ιωνική_ή_δωρική_ή_αιολική_διάλεκτο_που_εκτελείται_από_χορό_μη_συγκεκριμένου_τύπου_el"/>
    </otv:Concept>

    <otv:Concept rdf:about="#BCE_century">
        <otv:conceptName>&lt;BCE century&gt;</otv:conceptName>
        <otv:ownDifference rdf:resource="#before_common_era_century"/>
        <otv:difference rdf:resource="#before_common_era_century"/>
        <isCenturyOf rdf:resource="#Archaic_Lyric_Composer"/>
        <otv:attribute rdf:resource="#startsIn"/>
        <otv:attribute rdf:resource="#endsIn"/>
        <otv:denotedByTerm rdf:resource="#before_common_era_century_en"/>
        <otv:denotedByTerm rdf:resource="#προχριστιανικός_αιώνας_el"/>
    </otv:Concept>

    <otv:Concept rdf:about="#Archaic_Lyric_Poetess">
        <otv:conceptName>&lt;Archaic Lyric Poetess&gt;</otv:conceptName>
        <otv:isA rdf:resource="#Archaic_Lyric_Composer"/>
        <otv:ownDifference rdf:resource="#female"/>
        <otv:inheritedDifference rdf:resource="#archaic_lyric_composer"/>
        <otv:difference rdf:resource="#female"/>
        <otv:difference rdf:resource="#archaic_lyric_composer"/>
        <bornIn rdf:resource="#Ancient_Location"/>
        <centuryOfLiving rdf:resource="#BCE_century"/>
        <hasWritten rdf:resource="#Archaic_Lyric_Poem"/>
        <stayedIn rdf:resource="#Ancient_Location"/>
        <otv:attribute rdf:resource="#tlgIdentifyingNumber"/>
        <otv:attribute rdf:resource="#passageChosenEn"/>
        <otv:attribute rdf:resource="#passageChoselEl"/>
        <otv:denotedByTerm rdf:resource="#archaic_lyric_poetess_en"/>
        <otv:denotedByTerm rdf:resource="#αρχαϊκή_λυρική_ποιήτρια_el"/>
    </otv:Concept>

    <otv:Concept rdf:about="#Archaic_Lyric_Poem_in_ionic_or_in_doric_or_in_aeolic_dialect_performed_by_a_chorus_performed_by_a_maidens_chorus">
        <otv:conceptName>&lt;Archaic Lyric Poem in ionic or in doric or in aeolic dialect performed by a chorus performed by a maidens chorus&gt;</otv:conceptName>
        <otv:isA rdf:resource="#Archaic_Lyric_Poem_in_ionic_or_in_doric_or_in_aeolic_dialect_performed_by_a_chorus"/>
        <otv:ownDifference rdf:resource="#performed_by_a_maidens_chorus"/>
        <otv:inheritedDifference rdf:resource="#performed_by_a_chorus"/>
        <otv:inheritedDifference rdf:resource="#in_ionic_or_in_doric_or_in_aeolic_dialect"/>
        <otv:inheritedDifference rdf:resource="#archaic_lyric_poem"/>
        <otv:difference rdf:resource="#performed_by_a_maidens_chorus"/>
        <otv:difference rdf:resource="#performed_by_a_chorus"/>
        <otv:difference rdf:resource="#in_ionic_or_in_doric_or_in_aeolic_dialect"/>
        <otv:difference rdf:resource="#archaic_lyric_poem"/>
        <isWrittenBy rdf:resource="#Archaic_Lyric_Composer"/>
        <otv:denotedByTerm rdf:resource="#partheneion_en"/>
        <otv:denotedByTerm rdf:resource="#παρθένειο_el"/>
    </otv:Concept>

    <otv:Concept rdf:about="#Archaic_Lyric_Poem_in_ionic_or_in_doric_or_in_aeolic_dialect_performed_by_a_chorus_or_by_a_single_performer_dedicated_to_winners_in_athletic_events">
        <otv:conceptName>&lt;Archaic Lyric Poem in ionic or in doric or in aeolic dialect performed by a chorus or by a single performer dedicated to winners in athletic events&gt;</otv:conceptName>
        <otv:isA rdf:resource="#Archaic_Lyric_Poem_in_ionic_or_in_doric_or_in_aeolic_dialect_performed_by_a_chorus_or_by_a_single_performer_dedicated_to_living"/>
        <otv:ownDifference rdf:resource="#dedicated_to_winners_in_athletic_events"/>
        <otv:inheritedDifference rdf:resource="#dedicated_to_mortal"/>
        <otv:inheritedDifference rdf:resource="#performed_by_a_chorus_or_by_a_single_performer"/>
        <otv:inheritedDifference rdf:resource="#in_ionic_or_in_doric_or_in_aeolic_dialect"/>
        <otv:inheritedDifference rdf:resource="#archaic_lyric_poem"/>
        <otv:difference rdf:resource="#dedicated_to_winners_in_athletic_events"/>
        <otv:difference rdf:resource="#dedicated_to_mortal"/>
        <otv:difference rdf:resource="#performed_by_a_chorus_or_by_a_single_performer"/>
        <otv:difference rdf:resource="#in_ionic_or_in_doric_or_in_aeolic_dialect"/>
        <otv:difference rdf:resource="#archaic_lyric_poem"/>
        <isWrittenBy rdf:resource="#Archaic_Lyric_Composer"/>
        <otv:denotedByTerm rdf:resource="#epinikion_en"/>
        <otv:denotedByTerm rdf:resource="#επίνικος_el"/>
    </otv:Concept>

    <otv:Concept rdf:about="#Archaic_Lyric_Poem_in_ionic_or_in_doric_or_in_aeolic_dialect_performed_by_a_chorus_or_by_a_single_performer_dedicated_to_living">
        <otv:conceptName>&lt;Archaic Lyric Poem in ionic or in doric or in aeolic dialect performed by a chorus or by a single performer dedicated to living&gt;</otv:conceptName>
        <otv:isA rdf:resource="#Archaic_Lyric_Poem_in_ionic_or_in_doric_or_in_aeolic_dialect_performed_by_a_chorus_or_by_a_single_performer"/>
        <otv:ownDifference rdf:resource="#dedicated_to_mortal"/>
        <otv:inheritedDifference rdf:resource="#performed_by_a_chorus_or_by_a_single_performer"/>
        <otv:inheritedDifference rdf:resource="#in_ionic_or_in_doric_or_in_aeolic_dialect"/>
        <otv:inheritedDifference rdf:resource="#archaic_lyric_poem"/>
        <otv:difference rdf:resource="#dedicated_to_mortal"/>
        <otv:difference rdf:resource="#performed_by_a_chorus_or_by_a_single_performer"/>
        <otv:difference rdf:resource="#in_ionic_or_in_doric_or_in_aeolic_dialect"/>
        <otv:difference rdf:resource="#archaic_lyric_poem"/>
        <isWrittenBy rdf:resource="#Archaic_Lyric_Composer"/>
        <otv:denotedByTerm rdf:resource="#enkomion_en"/>
        <otv:denotedByTerm rdf:resource="#εγκώμιο_el"/>
    </otv:Concept>

    <otv:Concept rdf:about="#Archaic_Lyric_Poem_in_ionic_or_in_doric_or_in_aeolic_dialect_performed_by_a_chorus_during_bride_procession">
        <otv:conceptName>&lt;Archaic Lyric Poem in ionic or in doric or in aeolic dialect performed by a chorus during bride procession&gt;</otv:conceptName>
        <otv:isA rdf:resource="#Archaic_Lyric_Poem_in_ionic_or_in_doric_or_in_aeolic_dialect_performed_by_a_chorus_performed_by_a_non-specific_type_of_chorus"/>
        <otv:ownDifference rdf:resource="#during_bride_procession"/>
        <otv:inheritedDifference rdf:resource="#performed_by_a_non-specific_type_of_chorus"/>
        <otv:inheritedDifference rdf:resource="#performed_by_a_chorus"/>
        <otv:inheritedDifference rdf:resource="#in_ionic_or_in_doric_or_in_aeolic_dialect"/>
        <otv:inheritedDifference rdf:resource="#archaic_lyric_poem"/>
        <otv:difference rdf:resource="#during_bride_procession"/>
        <otv:difference rdf:resource="#performed_by_a_non-specific_type_of_chorus"/>
        <otv:difference rdf:resource="#performed_by_a_chorus"/>
        <otv:difference rdf:resource="#in_ionic_or_in_doric_or_in_aeolic_dialect"/>
        <otv:difference rdf:resource="#archaic_lyric_poem"/>
        <isWrittenBy rdf:resource="#Archaic_Lyric_Composer"/>
        <otv:denotedByTerm rdf:resource="#hymenaios_en"/>
        <otv:denotedByTerm rdf:resource="#υμέναιος_el"/>
    </otv:Concept>

    <otv:Concept rdf:about="#Archaic_Lyric_Poet">
        <otv:conceptName>&lt;Archaic Lyric Poet&gt;</otv:conceptName>
        <otv:isA rdf:resource="#Archaic_Lyric_Composer"/>
        <otv:ownDifference rdf:resource="#male"/>
        <otv:inheritedDifference rdf:resource="#archaic_lyric_composer"/>
        <otv:difference rdf:resource="#male"/>
        <otv:difference rdf:resource="#archaic_lyric_composer"/>
        <bornIn rdf:resource="#Ancient_Location"/>
        <centuryOfLiving rdf:resource="#BCE_century"/>
        <hasWritten rdf:resource="#Archaic_Lyric_Poem"/>
        <stayedIn rdf:resource="#Ancient_Location"/>
        <otv:attribute rdf:resource="#tlgIdentifyingNumber"/>
        <otv:attribute rdf:resource="#passageChosenEn"/>
        <otv:attribute rdf:resource="#passageChoselEl"/>
        <otv:denotedByTerm rdf:resource="#archaic_lyric_poet_en"/>
        <otv:denotedByTerm rdf:resource="#αρχαϊκός_λυρικός_ποιητής_el"/>
    </otv:Concept>

    <otv:Concept rdf:about="#Archaic_Lyric_Poem_only_in_ionic_dialect_in_elegiac_couplet_with_erotic_content">
        <otv:conceptName>&lt;Archaic Lyric Poem only in ionic dialect in elegiac couplet with erotic content&gt;</otv:conceptName>
        <otv:isA rdf:resource="#Archaic_Lyric_Poem_only_in_ionic_dialect_in_elegiac_couplet"/>
        <otv:ownDifference rdf:resource="#with_specific_content"/>
        <otv:ownDifference rdf:resource="#with_erotic_content"/>
        <otv:inheritedDifference rdf:resource="#in_elegiac_couplet"/>
        <otv:inheritedDifference rdf:resource="#only_in_ionic_dialect"/>
        <otv:inheritedDifference rdf:resource="#archaic_lyric_poem"/>
        <otv:difference rdf:resource="#with_erotic_content"/>
        <otv:difference rdf:resource="#with_specific_content"/>
        <otv:difference rdf:resource="#in_elegiac_couplet"/>
        <otv:difference rdf:resource="#only_in_ionic_dialect"/>
        <otv:difference rdf:resource="#archaic_lyric_poem"/>
        <isWrittenBy rdf:resource="#Archaic_Lyric_Composer"/>
        <otv:denotedByTerm rdf:resource="#erotic_elegy_en"/>
        <otv:denotedByTerm rdf:resource="#ερωτική_ελεγεία_el"/>
    </otv:Concept>

	<!--  OTV Terms -->

    <otv:Term rdf:about="#epithalamion_en">
        <rdfs:label xml:lang="en">epithalamion</rdfs:label>
        <otv:termName>epithalamion</otv:termName>
        <otv:language>en</otv:language>
        <otv:denotedConcept rdf:resource="#Archaic_Lyric_Poem_in_ionic_or_in_doric_or_in_aeolic_dialect_performed_by_a_chorus_or_by_a_single_performer_dedicated_to_wedding_couple"/>
        <otv:termStatus>preferred</otv:termStatus>
        <otv:partOfSpeech>none</otv:partOfSpeech>
        <otv:gender>none</otv:gender>
        <otv:termDefinition>Epithalamium is a song dedicated to a wedding couple sung at the nuptial residence. Sappho is famous for her such songs.</otv:termDefinition>
        <skos:definition xml:lang="en">Epithalamium is a song dedicated to a wedding couple sung at the nuptial residence. Sappho is famous for her such songs.</skos:definition>
    </otv:Term>

    <otv:Term rdf:about="#threnos_en">
        <rdfs:label xml:lang="en">threnos</rdfs:label>
        <otv:termName>threnos</otv:termName>
        <otv:language>en</otv:language>
        <otv:denotedConcept rdf:resource="#Archaic_Lyric_Poem_in_ionic_or_in_doric_or_in_aeolic_dialect_performed_by_a_chorus_or_by_a_single_performer_dedicated_to_dead"/>
        <otv:termStatus>preferred</otv:termStatus>
        <otv:partOfSpeech>none</otv:partOfSpeech>
        <otv:gender>none</otv:gender>
        <otv:termDefinition>Lyric song dedicated to a dead human being. Anacreon, Pindar and Simonides are famous for their such compositions.</otv:termDefinition>
        <skos:definition xml:lang="en">Lyric song dedicated to a dead human being. Anacreon, Pindar and Simonides are famous for their such compositions.</skos:definition>
    </otv:Term>

    <otv:Term rdf:about="#archaic_lyric_poetess_en">
        <rdfs:label xml:lang="en">archaic lyric poetess</rdfs:label>
        <otv:termName>archaic lyric poetess</otv:termName>
        <otv:language>en</otv:language>
        <otv:denotedConcept rdf:resource="#Archaic_Lyric_Poetess"/>
        <otv:termStatus>preferred</otv:termStatus>
        <otv:partOfSpeech>none</otv:partOfSpeech>
        <otv:gender>none</otv:gender>
        <otv:termDefinition>An Archaic Lyric poetess (woman) is a person who lived during 7th-early 5th century BCE and wrote Archaic Lyric poetry.</otv:termDefinition>
        <skos:definition xml:lang="en">An Archaic Lyric poetess (woman) is a person who lived during 7th-early 5th century BCE and wrote Archaic Lyric poetry.</skos:definition>
    </otv:Term>

    <otv:Term rdf:about="#dithyramb_en">
        <rdfs:label xml:lang="en">dithyramb</rdfs:label>
        <otv:termName>dithyramb</otv:termName>
        <otv:language>en</otv:language>
        <otv:denotedConcept rdf:resource="#Archaic_Lyric_Poem_in_ionic_or_in_doric_or_in_aeolic_dialect_performed_by_a_chorus_or_by_a_single_performer_dedicated_to_dionysus"/>
        <otv:termStatus>preferred</otv:termStatus>
        <otv:partOfSpeech>none</otv:partOfSpeech>
        <otv:gender>none</otv:gender>
        <otv:termDefinition>Devotional hymns of Dionysus. Bacchylides, Pindar and Simonides are known to have composed dithyrambs.</otv:termDefinition>
        <skos:definition xml:lang="en">Devotional hymns of Dionysus. Bacchylides, Pindar and Simonides are known to have composed dithyrambs.</skos:definition>
    </otv:Term>

    <otv:Term rdf:about="#archaic_lyric_poem_in_ionic_or_in_doric_or_in_aeolic_dialect_performed_by_a_chorus_or_by_a_single_performer_en">
        <rdfs:label xml:lang="en">archaic lyric poem in ionic or in doric or in aeolic dialect performed by a chorus or by a single performer</rdfs:label>
        <otv:termName>archaic lyric poem in ionic or in doric or in aeolic dialect performed by a chorus or by a single performer</otv:termName>
        <otv:language>en</otv:language>
        <otv:denotedConcept rdf:resource="#Archaic_Lyric_Poem_in_ionic_or_in_doric_or_in_aeolic_dialect_performed_by_a_chorus_or_by_a_single_performer"/>
        <otv:termStatus>preferred</otv:termStatus>
        <otv:partOfSpeech>none</otv:partOfSpeech>
        <otv:gender>none</otv:gender>
        <otv:termDefinition>Melos which was performed either by one person or by a chorus.</otv:termDefinition>
        <skos:definition xml:lang="en">Melos which was performed either by one person or by a chorus.</skos:definition>
    </otv:Term>

    <otv:Term rdf:about="#hyporcheme_en">
        <rdfs:label xml:lang="en">hyporcheme</rdfs:label>
        <otv:termName>hyporcheme</otv:termName>
        <otv:language>en</otv:language>
        <otv:denotedConcept rdf:resource="#Archaic_Lyric_Poem_in_ionic_or_in_doric_or_in_aeolic_dialect_performed_by_a_chorus_with_imitation_expressions"/>
        <otv:termStatus>preferred</otv:termStatus>
        <otv:partOfSpeech>none</otv:partOfSpeech>
        <otv:gender>none</otv:gender>
        <otv:termDefinition>A lyric song accompanied by imitative movements. Bacchylides and Pindar are famous for composing hyporchemes.</otv:termDefinition>
        <skos:definition xml:lang="en">A lyric song accompanied by imitative movements. Bacchylides and Pindar are famous for composing hyporchemes.</skos:definition>
    </otv:Term>

    <otv:Term rdf:about="#archaic_lyric_poem_en">
        <rdfs:label xml:lang="en">archaic lyric poem</rdfs:label>
        <otv:termName>archaic lyric poem</otv:termName>
        <otv:language>en</otv:language>
        <otv:denotedConcept rdf:resource="#Archaic_Lyric_Poem"/>
        <otv:termStatus>preferred</otv:termStatus>
        <otv:partOfSpeech>none</otv:partOfSpeech>
        <otv:gender>none</otv:gender>
        <otv:termDefinition>"Lyric poetry began as a fixture of ancient Greece, classified against other categories of poetry at the time of classical antiquity: dramas (written in verse) and epic poems. The lyric was far shorter, distinguished also by its focus on the poet’s state of mind and personal themes rather than narrative arc" (Academy of American Poets). So, an Archaic Lyric Poem is such poem written from 7th-early 5th century BCE.</otv:termDefinition>
        <skos:definition xml:lang="en">"Lyric poetry began as a fixture of ancient Greece, classified against other categories of poetry at the time of classical antiquity: dramas (written in verse) and epic poems. The lyric was far shorter, distinguished also by its focus on the poet’s state of mind and personal themes rather than narrative arc" (Academy of American Poets). So, an Archaic Lyric Poem is such poem written from 7th-early 5th century BCE.</skos:definition>
    </otv:Term>

    <otv:Term rdf:about="#before_common_era_century_en">
        <rdfs:label xml:lang="en">before common era century</rdfs:label>
        <otv:termName>before common era century</otv:termName>
        <otv:language>en</otv:language>
        <otv:denotedConcept rdf:resource="#BCE_century"/>
        <otv:termStatus>preferred</otv:termStatus>
        <otv:partOfSpeech>none</otv:partOfSpeech>
        <otv:gender>none</otv:gender>
        <otv:termDefinition>Century that is BCE.</otv:termDefinition>
        <skos:definition xml:lang="en">Century that is BCE.</skos:definition>
    </otv:Term>

    <otv:Term rdf:about="#elegy_en">
        <rdfs:label xml:lang="en">elegy</rdfs:label>
        <otv:termName>elegy</otv:termName>
        <otv:language>en</otv:language>
        <otv:denotedConcept rdf:resource="#Archaic_Lyric_Poem_only_in_ionic_dialect_in_elegiac_couplet"/>
        <otv:termStatus>preferred</otv:termStatus>
        <otv:partOfSpeech>none</otv:partOfSpeech>
        <otv:gender>none</otv:gender>
        <otv:termDefinition>Elegies are poems written in elegiac couplets, with the first line in hexameter and the second line in pentameter, initially used for lamentation (but later had a wide range of themes) and possibly originating from Eastern mourning practices. They can be as short as a single couplet or longer sequences as needed.</otv:termDefinition>
        <skos:definition xml:lang="en">Elegies are poems written in elegiac couplets, with the first line in hexameter and the second line in pentameter, initially used for lamentation (but later had a wide range of themes) and possibly originating from Eastern mourning practices. They can be as short as a single couplet or longer sequences as needed.</skos:definition>
    </otv:Term>

    <otv:Term rdf:about="#archaic_lyric_poem_only_in_ionic_dialect_en">
        <rdfs:label xml:lang="en">archaic lyric poem only in ionic dialect</rdfs:label>
        <otv:termName>archaic lyric poem only in ionic dialect</otv:termName>
        <otv:language>en</otv:language>
        <otv:denotedConcept rdf:resource="#Archaic_Lyric_Poem_only_in_ionic_dialect"/>
        <otv:termStatus>preferred</otv:termStatus>
        <otv:partOfSpeech>none</otv:partOfSpeech>
        <otv:gender>none</otv:gender>
        <otv:termDefinition>Archaic Lyric poem written only in ionic dialect. Ionic greek dialect, a subset of Eastern Greek, originated on the mainland and spread during the Dorian invasions. By the 5th century BC, it was primarily spoken in Ionia, including Asia Minor, Chios, and Samos. It also extended to Euboea and through Ionian colonization to the northern Aegean, Black Sea, and western Mediterranean.</otv:termDefinition>
        <skos:definition xml:lang="en">Archaic Lyric poem written only in ionic dialect. Ionic greek dialect, a subset of Eastern Greek, originated on the mainland and spread during the Dorian invasions. By the 5th century BC, it was primarily spoken in Ionia, including Asia Minor, Chios, and Samos. It also extended to Euboea and through Ionian colonization to the northern Aegean, Black Sea, and western Mediterranean.</skos:definition>
    </otv:Term>

    <otv:Term rdf:about="#paean_en">
        <rdfs:label xml:lang="en">paean</rdfs:label>
        <otv:termName>paean</otv:termName>
        <otv:language>en</otv:language>
        <otv:denotedConcept rdf:resource="#Archaic_Lyric_Poem_in_ionic_or_in_doric_or_in_aeolic_dialect_performed_by_a_chorus_or_by_a_single_performer_dedicated_to_apollo"/>
        <otv:termStatus>preferred</otv:termStatus>
        <otv:partOfSpeech>none</otv:partOfSpeech>
        <otv:gender>none</otv:gender>
        <otv:termDefinition>Lyric song dedicated to Ancient Greek god Apollo. Alcman, Pindar and Bacchylides are famous composers of paeans.</otv:termDefinition>
        <skos:definition xml:lang="en">Lyric song dedicated to Ancient Greek god Apollo. Alcman, Pindar and Bacchylides are famous composers of paeans.</skos:definition>
    </otv:Term>

    <otv:Term rdf:about="#melos_en">
        <rdfs:label xml:lang="en">melos</rdfs:label>
        <otv:termName>melos</otv:termName>
        <otv:language>en</otv:language>
        <otv:denotedConcept rdf:resource="#Archaic_Lyric_Poem_in_ionic_or_in_doric_or_in_aeolic_dialect"/>
        <otv:termStatus>preferred</otv:termStatus>
        <otv:partOfSpeech>none</otv:partOfSpeech>
        <otv:gender>none</otv:gender>
        <otv:termDefinition>Melos is the hypernym of the Archaic Lyric poems, which were written in ionic (except of the iamb and elegy), aeolic and doric dialect.</otv:termDefinition>
        <skos:definition xml:lang="en">Melos is the hypernym of the Archaic Lyric poems, which were written in ionic (except of the iamb and elegy), aeolic and doric dialect.</skos:definition>
    </otv:Term>

    <otv:Term rdf:about="#archaic_lyric_composer_en">
        <rdfs:label xml:lang="en">archaic lyric composer</rdfs:label>
        <otv:termName>archaic lyric composer</otv:termName>
        <otv:language>en</otv:language>
        <otv:denotedConcept rdf:resource="#Archaic_Lyric_Composer"/>
        <otv:termStatus>preferred</otv:termStatus>
        <otv:partOfSpeech>none</otv:partOfSpeech>
        <otv:gender>none</otv:gender>
        <otv:termDefinition>An Archaic Lyric composer is a person who lived during 7th-early 5th century BCE and wrote a lyric poem.</otv:termDefinition>
        <skos:definition xml:lang="en">An Archaic Lyric composer is a person who lived during 7th-early 5th century BCE and wrote a lyric poem.</skos:definition>
    </otv:Term>

    <otv:Term rdf:about="#hymn_en">
        <rdfs:label xml:lang="en">hymn</rdfs:label>
        <otv:termName>hymn</otv:termName>
        <otv:language>en</otv:language>
        <otv:denotedConcept rdf:resource="#Archaic_Lyric_Poem_in_ionic_or_in_doric_or_in_aeolic_dialect_performed_by_a_chorus_or_by_a_single_performer_dedicated_to_a_god"/>
        <otv:termStatus>preferred</otv:termStatus>
        <otv:partOfSpeech>none</otv:partOfSpeech>
        <otv:gender>none</otv:gender>
        <otv:termDefinition>Lyric song dedicated to gods. Multiple poets has composed hymns, sych as Alcaeus, Terpander, Sappho, Alcman et. al.</otv:termDefinition>
        <skos:definition xml:lang="en">Lyric song dedicated to gods. Multiple poets has composed hymns, sych as Alcaeus, Terpander, Sappho, Alcman et. al.</skos:definition>
    </otv:Term>

    <otv:Term rdf:about="#archaic_lyric_poet_en">
        <rdfs:label xml:lang="en">archaic lyric poet</rdfs:label>
        <otv:termName>archaic lyric poet</otv:termName>
        <otv:language>en</otv:language>
        <otv:denotedConcept rdf:resource="#Archaic_Lyric_Poet"/>
        <otv:termStatus>preferred</otv:termStatus>
        <otv:partOfSpeech>none</otv:partOfSpeech>
        <otv:gender>none</otv:gender>
        <otv:termDefinition>An Archaic Lyric poet is a person (man) who lived during 7th-early 5th century BCE and wrote Archaic Lyric poetry.</otv:termDefinition>
        <skos:definition xml:lang="en">An Archaic Lyric poet is a person (man) who lived during 7th-early 5th century BCE and wrote Archaic Lyric poetry.</skos:definition>
    </otv:Term>

    <otv:Term rdf:about="#prosodion_en">
        <rdfs:label xml:lang="en">prosodion</rdfs:label>
        <otv:termName>prosodion</otv:termName>
        <otv:language>en</otv:language>
        <otv:denotedConcept rdf:resource="#Archaic_Lyric_Poem_in_ionic_or_in_doric_or_in_aeolic_dialect_performed_by_a_chorus_on_the_way_to_an_altar"/>
        <otv:termStatus>preferred</otv:termStatus>
        <otv:partOfSpeech>none</otv:partOfSpeech>
        <otv:gender>none</otv:gender>
        <otv:termDefinition>A lyric song performed on the way to an altar by a chorus. Alcman, Bacchylides and Pindar are famous prosodia composers.</otv:termDefinition>
        <skos:definition xml:lang="en">A lyric song performed on the way to an altar by a chorus. Alcman, Bacchylides and Pindar are famous prosodia composers.</skos:definition>
    </otv:Term>

    <otv:Term rdf:about="#hymenaios_en">
        <rdfs:label xml:lang="en">hymenaios</rdfs:label>
        <otv:termName>hymenaios</otv:termName>
        <otv:language>en</otv:language>
        <otv:denotedConcept rdf:resource="#Archaic_Lyric_Poem_in_ionic_or_in_doric_or_in_aeolic_dialect_performed_by_a_chorus_during_bride_procession"/>
        <otv:termStatus>preferred</otv:termStatus>
        <otv:partOfSpeech>none</otv:partOfSpeech>
        <otv:gender>none</otv:gender>
        <otv:termDefinition>A lyric song sung during the procession of the bride to the groom's house. Sappho is famous for her such songs.</otv:termDefinition>
        <skos:definition xml:lang="en">A lyric song sung during the procession of the bride to the groom's house. Sappho is famous for her such songs.</skos:definition>
    </otv:Term>

    <otv:Term rdf:about="#enkomion_en">
        <rdfs:label xml:lang="en">enkomion</rdfs:label>
        <otv:termName>enkomion</otv:termName>
        <otv:language>en</otv:language>
        <otv:denotedConcept rdf:resource="#Archaic_Lyric_Poem_in_ionic_or_in_doric_or_in_aeolic_dialect_performed_by_a_chorus_or_by_a_single_performer_dedicated_to_living"/>
        <otv:termStatus>preferred</otv:termStatus>
        <otv:partOfSpeech>none</otv:partOfSpeech>
        <otv:gender>none</otv:gender>
        <otv:termDefinition>Lyric song of praise for living people. Pindar, Bacchylides and Ibicus are important figures in enkomion composition.</otv:termDefinition>
        <skos:definition xml:lang="en">Lyric song of praise for living people. Pindar, Bacchylides and Ibicus are important figures in enkomion composition.</skos:definition>
    </otv:Term>

    <otv:Term rdf:about="#iamb_en">
        <rdfs:label xml:lang="en">iamb</rdfs:label>
        <otv:termName>iamb</otv:termName>
        <otv:language>en</otv:language>
        <otv:denotedConcept rdf:resource="#Archaic_Lyric_Poem_only_in_ionic_dialect_in_iambic_or_trochaic_metre"/>
        <otv:termStatus>preferred</otv:termStatus>
        <otv:partOfSpeech>none</otv:partOfSpeech>
        <otv:gender>none</otv:gender>
        <otv:termDefinition>Initially associated with Dionysus, the iamb may have a pre-Hellenic origin as a poetic form. Typically composed in iambic trimeter or trochaic tetrameter, its Ionic version often adopts a first-person perspective, though its context can vary.</otv:termDefinition>
        <skos:definition xml:lang="en">Initially associated with Dionysus, the iamb may have a pre-Hellenic origin as a poetic form. Typically composed in iambic trimeter or trochaic tetrameter, its Ionic version often adopts a first-person perspective, though its context can vary.</skos:definition>
    </otv:Term>

    <otv:Term rdf:about="#epinikion_en">
        <rdfs:label xml:lang="en">epinikion</rdfs:label>
        <otv:termName>epinikion</otv:termName>
        <otv:language>en</otv:language>
        <otv:denotedConcept rdf:resource="#Archaic_Lyric_Poem_in_ionic_or_in_doric_or_in_aeolic_dialect_performed_by_a_chorus_or_by_a_single_performer_dedicated_to_winners_in_athletic_events"/>
        <otv:termStatus>preferred</otv:termStatus>
        <otv:partOfSpeech>none</otv:partOfSpeech>
        <otv:gender>none</otv:gender>
        <otv:termDefinition>Lyric song of praise winners of sports games. Pindar, Bacchylides and Ibicus are who composed epinikia.</otv:termDefinition>
        <skos:definition xml:lang="en">Lyric song of praise winners of sports games. Pindar, Bacchylides and Ibicus are who composed epinikia.</skos:definition>
    </otv:Term>

    <otv:Term rdf:about="#gnomic_elegy_en">
        <rdfs:label xml:lang="en">gnomic elegy</rdfs:label>
        <otv:termName>gnomic elegy</otv:termName>
        <otv:language>en</otv:language>
        <otv:denotedConcept rdf:resource="#Archaic_Lyric_Poem_only_in_ionic_dialect_in_elegiac_couplet_with_gnomic_content"/>
        <otv:termStatus>preferred</otv:termStatus>
        <otv:partOfSpeech>none</otv:partOfSpeech>
        <otv:gender>none</otv:gender>
        <otv:termDefinition>Elegy with gnomic, counseling, biosophical content. Known poets of gnomic elegies are Phocylides and Theognis.</otv:termDefinition>
        <skos:definition xml:lang="en">Elegy with gnomic, counseling, biosophical content. Known poets of gnomic elegies are Phocylides and Theognis.</skos:definition>
    </otv:Term>

    <otv:Term rdf:about="#political_elegy_en">
        <rdfs:label xml:lang="en">political elegy</rdfs:label>
        <otv:termName>political elegy</otv:termName>
        <otv:language>en</otv:language>
        <otv:denotedConcept rdf:resource="#Archaic_Lyric_Poem_only_in_ionic_dialect_in_elegiac_couplet_with_political_content"/>
        <otv:termStatus>preferred</otv:termStatus>
        <otv:partOfSpeech>none</otv:partOfSpeech>
        <otv:gender>none</otv:gender>
        <otv:termDefinition>Elegy with political content. Solon Atheniensis is a famous poet who composed such elegies.</otv:termDefinition>
        <skos:definition xml:lang="en">Elegy with political content. Solon Atheniensis is a famous poet who composed such elegies.</skos:definition>
    </otv:Term>

    <otv:Term rdf:about="#ancient_location_en">
        <rdfs:label xml:lang="en">ancient location</rdfs:label>
        <otv:termName>ancient location</otv:termName>
        <otv:language>en</otv:language>
        <otv:denotedConcept rdf:resource="#Ancient_Location"/>
        <otv:termStatus>preferred</otv:termStatus>
        <otv:partOfSpeech>none</otv:partOfSpeech>
        <otv:gender>none</otv:gender>
        <otv:termDefinition>In the current ontoterminology Ancient Location objects concern the places where the Archaic Lyric Poets were born or lived, while they are inserted with coordinates from the pleiades gazetteer of ancient places (https:pleiades.stoa.orgplaces).</otv:termDefinition>
        <skos:definition xml:lang="en">In the current ontoterminology Ancient Location objects concern the places where the Archaic Lyric Poets were born or lived, while they are inserted with coordinates from the pleiades gazetteer of ancient places (https:pleiades.stoa.orgplaces).</skos:definition>
    </otv:Term>

    <otv:Term rdf:about="#erotic_elegy_en">
        <rdfs:label xml:lang="en">erotic elegy</rdfs:label>
        <otv:termName>erotic elegy</otv:termName>
        <otv:language>en</otv:language>
        <otv:denotedConcept rdf:resource="#Archaic_Lyric_Poem_only_in_ionic_dialect_in_elegiac_couplet_with_erotic_content"/>
        <otv:termStatus>preferred</otv:termStatus>
        <otv:partOfSpeech>none</otv:partOfSpeech>
        <otv:gender>none</otv:gender>
        <otv:termDefinition>Elegy with erotic content. Famous poet who composed erotic elegies is Mimnermus.</otv:termDefinition>
        <skos:definition xml:lang="en">Elegy with erotic content. Famous poet who composed erotic elegies is Mimnermus.</skos:definition>
    </otv:Term>

    <otv:Term rdf:about="#partheneion_en">
        <rdfs:label xml:lang="en">partheneion</rdfs:label>
        <otv:termName>partheneion</otv:termName>
        <otv:language>en</otv:language>
        <otv:denotedConcept rdf:resource="#Archaic_Lyric_Poem_in_ionic_or_in_doric_or_in_aeolic_dialect_performed_by_a_chorus_performed_by_a_maidens_chorus"/>
        <otv:termStatus>preferred</otv:termStatus>
        <otv:partOfSpeech>none</otv:partOfSpeech>
        <otv:gender>none</otv:gender>
        <otv:termDefinition>A lyric song performed by a maidens chorus. Alcman, Pindar and Bacchylides are famous for composing Partheneia.</otv:termDefinition>
        <skos:definition xml:lang="en">A lyric song performed by a maidens chorus. Alcman, Pindar and Bacchylides are famous for composing Partheneia.</skos:definition>
    </otv:Term>

    <otv:Term rdf:about="#archaic_lyric_poem_in_ionic_or_in_doric_or_in_aeolic_dialect_performed_by_a_chorus_en">
        <rdfs:label xml:lang="en">archaic lyric poem in ionic or in doric or in aeolic dialect performed by a chorus</rdfs:label>
        <otv:termName>archaic lyric poem in ionic or in doric or in aeolic dialect performed by a chorus</otv:termName>
        <otv:language>en</otv:language>
        <otv:denotedConcept rdf:resource="#Archaic_Lyric_Poem_in_ionic_or_in_doric_or_in_aeolic_dialect_performed_by_a_chorus"/>
        <otv:termStatus>preferred</otv:termStatus>
        <otv:partOfSpeech>none</otv:partOfSpeech>
        <otv:gender>none</otv:gender>
        <otv:termDefinition>Lyric song performed by a group (chorus) of people (women, men), which were dancing and singing.</otv:termDefinition>
        <skos:definition xml:lang="en">Lyric song performed by a group (chorus) of people (women, men), which were dancing and singing.</skos:definition>
    </otv:Term>

    <otv:Term rdf:about="#archaic_lyric_poem_in_ionic_or_doric_or_aeolic_dialect_performed_by_a_chorus_of_no_particular_type_en">
        <rdfs:label xml:lang="en">archaic lyric poem in ionic or doric or aeolic dialect performed by a chorus of no particular type</rdfs:label>
        <otv:termName>archaic lyric poem in ionic or doric or aeolic dialect performed by a chorus of no particular type</otv:termName>
        <otv:language>en</otv:language>
        <otv:denotedConcept rdf:resource="#Archaic_Lyric_Poem_in_ionic_or_in_doric_or_in_aeolic_dialect_performed_by_a_chorus_performed_by_a_non-specific_type_of_chorus"/>
        <otv:termStatus>none</otv:termStatus>
        <otv:partOfSpeech>none</otv:partOfSpeech>
        <otv:gender>none</otv:gender>
        <otv:termDefinition>An Archaic Lyric poem in Ionic or Doric or Aeolic dialect performed by a chorus of no particular type.</otv:termDefinition>
        <skos:definition xml:lang="en">An Archaic Lyric poem in Ionic or Doric or Aeolic dialect performed by a chorus of no particular type.</skos:definition>
    </otv:Term>

    <otv:Term rdf:about="#monody_en">
        <rdfs:label xml:lang="en">monody</rdfs:label>
        <otv:termName>monody</otv:termName>
        <otv:language>en</otv:language>
        <otv:denotedConcept rdf:resource="#Archaic_Lyric_Poem_in_ionic_or_in_doric_or_in_aeolic_dialect_performed_by_a_single_performer"/>
        <otv:termStatus>preferred</otv:termStatus>
        <otv:partOfSpeech>none</otv:partOfSpeech>
        <otv:gender>none</otv:gender>
        <otv:termDefinition>Monodies are characterized by solo performances, where the poet identifies with the singer and expresses personal thoughts and emotions, as they offer a direct and free expression of personality. For instance, in Sapphic odes, the poetess prioritizes her own voice over others.</otv:termDefinition>
        <skos:definition xml:lang="en">Monodies are characterized by solo performances, where the poet identifies with the singer and expresses personal thoughts and emotions, as they offer a direct and free expression of personality. For instance, in Sapphic odes, the poetess prioritizes her own voice over others.</skos:definition>
    </otv:Term>

    <otv:Term rdf:about="#war_elegy_en">
        <rdfs:label xml:lang="en">war elegy</rdfs:label>
        <otv:termName>war elegy</otv:termName>
        <otv:language>en</otv:language>
        <otv:denotedConcept rdf:resource="#Archaic_Lyric_Poem_only_in_ionic_dialect_in_elegiac_couplet_with_war_content"/>
        <otv:termStatus>preferred</otv:termStatus>
        <otv:partOfSpeech>none</otv:partOfSpeech>
        <otv:gender>none</otv:gender>
        <otv:termDefinition>Elegy with war content. Tyrtaeus and Callinus are famous poets of such elegy.</otv:termDefinition>
        <skos:definition xml:lang="en">Elegy with war content. Tyrtaeus and Callinus are famous poets of such elegy.</skos:definition>
    </otv:Term>

    <otv:Term rdf:about="#αρχαϊκό_λυρικό_ποίημα_μόνο_στην_ιωνική_διάλεκτο_el">
        <rdfs:label xml:lang="el">αρχαϊκό λυρικό ποίημα μόνο στην ιωνική διάλεκτο</rdfs:label>
        <otv:termName>αρχαϊκό λυρικό ποίημα μόνο στην ιωνική διάλεκτο</otv:termName>
        <otv:language>el</otv:language>
        <otv:denotedConcept rdf:resource="#Archaic_Lyric_Poem_only_in_ionic_dialect"/>
        <otv:termStatus>preferred</otv:termStatus>
        <otv:partOfSpeech>none</otv:partOfSpeech>
        <otv:gender>none</otv:gender>
        <otv:termDefinition>Αρχαϊκό λυρικό ποίημα μόνο στην ιωνική διάλεκτο.</otv:termDefinition>
        <skos:definition xml:lang="el">Αρχαϊκό λυρικό ποίημα μόνο στην ιωνική διάλεκτο.</skos:definition>
    </otv:Term>

    <otv:Term rdf:about="#αρχαία_τοποθεσία_el">
        <rdfs:label xml:lang="el">αρχαία τοποθεσία</rdfs:label>
        <otv:termName>αρχαία τοποθεσία</otv:termName>
        <otv:language>el</otv:language>
        <otv:denotedConcept rdf:resource="#Ancient_Location"/>
        <otv:termStatus>preferred</otv:termStatus>
        <otv:partOfSpeech>none</otv:partOfSpeech>
        <otv:gender>none</otv:gender>
        <otv:termDefinition>Στην παρούσα οντοορολογία γίνεται αναφορά στους τόπους όπου γεννήθηκαν ή έζησαν οι αρχαϊκοί λυρικοί ποιητές. Η ακριβής τους τοποθεσία εισάγεται με συντεταγμένες από το ευρετήριο αρχαίων τόπων pleiades (https:pleiades.stoa.orgplaces).</otv:termDefinition>
        <skos:definition xml:lang="el">Στην παρούσα οντοορολογία γίνεται αναφορά στους τόπους όπου γεννήθηκαν ή έζησαν οι αρχαϊκοί λυρικοί ποιητές. Η ακριβής τους τοποθεσία εισάγεται με συντεταγμένες από το ευρετήριο αρχαίων τόπων pleiades (https:pleiades.stoa.orgplaces).</skos:definition>
    </otv:Term>

    <otv:Term rdf:about="#πολεμική_ελεγεία_el">
        <rdfs:label xml:lang="el">πολεμική ελεγεία</rdfs:label>
        <otv:termName>πολεμική ελεγεία</otv:termName>
        <otv:language>el</otv:language>
        <otv:denotedConcept rdf:resource="#Archaic_Lyric_Poem_only_in_ionic_dialect_in_elegiac_couplet_with_war_content"/>
        <otv:termStatus>preferred</otv:termStatus>
        <otv:partOfSpeech>none</otv:partOfSpeech>
        <otv:gender>none</otv:gender>
        <otv:termDefinition>Ελεγεία με πολεμικό χαρακτήρα. Ο Τυρταίος και ο Καλλίνικος είναι διάσημοι ποιητές τέτοιων ελεγειών.</otv:termDefinition>
        <skos:definition xml:lang="el">Ελεγεία με πολεμικό χαρακτήρα. Ο Τυρταίος και ο Καλλίνικος είναι διάσημοι ποιητές τέτοιων ελεγειών.</skos:definition>
    </otv:Term>

    <otv:Term rdf:about="#αρχαϊκή_λυρική_ποιήτρια_el">
        <rdfs:label xml:lang="el">αρχαϊκή λυρική ποιήτρια</rdfs:label>
        <otv:termName>αρχαϊκή λυρική ποιήτρια</otv:termName>
        <otv:language>el</otv:language>
        <otv:denotedConcept rdf:resource="#Archaic_Lyric_Poetess"/>
        <otv:termStatus>preferred</otv:termStatus>
        <otv:partOfSpeech>none</otv:partOfSpeech>
        <otv:gender>none</otv:gender>
        <otv:termDefinition>Η αρχαϊκή λυρική ποιήτρια είναι πρόσωπο που έζησε κατά τον 7ο-αρχές του 5ου αιώνα π.Χ. και έγραψε αρχαϊκή λυρική ποίηση.</otv:termDefinition>
        <skos:definition xml:lang="el">Η αρχαϊκή λυρική ποιήτρια είναι πρόσωπο που έζησε κατά τον 7ο-αρχές του 5ου αιώνα π.Χ. και έγραψε αρχαϊκή λυρική ποίηση.</skos:definition>
    </otv:Term>

    <otv:Term rdf:about="#αρχαϊκός_λυρικός_συνθέτης_el">
        <rdfs:label xml:lang="el">αρχαϊκός λυρικός συνθέτης</rdfs:label>
        <otv:termName>αρχαϊκός λυρικός συνθέτης</otv:termName>
        <otv:language>el</otv:language>
        <otv:denotedConcept rdf:resource="#Archaic_Lyric_Composer"/>
        <otv:termStatus>preferred</otv:termStatus>
        <otv:partOfSpeech>none</otv:partOfSpeech>
        <otv:gender>none</otv:gender>
        <otv:termDefinition>Ο αρχαϊκός λυρικός συνθέτης είναι ένα πρόσωπο που έζησε κατά τη διάρκεια του 7ου-αρχές του 5ου αιώνα π.Χ. και έγραψε λυρικό ποίημα.</otv:termDefinition>
        <skos:definition xml:lang="el">Ο αρχαϊκός λυρικός συνθέτης είναι ένα πρόσωπο που έζησε κατά τη διάρκεια του 7ου-αρχές του 5ου αιώνα π.Χ. και έγραψε λυρικό ποίημα.</skos:definition>
    </otv:Term>

    <otv:Term rdf:about="#αρχαϊκό_λυρικό_ποίημα_σε_ιωνική_ή_δωρική_ή_αιολική_διάλεκτο_που_εκτελείται_από_χορό_ή_από_έναν_μόνο_ερμηνευτή_el">
        <rdfs:label xml:lang="el">αρχαϊκό λυρικό ποίημα σε ιωνική ή δωρική ή αιολική διάλεκτο που εκτελείται από χορό ή από έναν μόνο ερμηνευτή</rdfs:label>
        <otv:termName>αρχαϊκό λυρικό ποίημα σε ιωνική ή δωρική ή αιολική διάλεκτο που εκτελείται από χορό ή από έναν μόνο ερμηνευτή</otv:termName>
        <otv:language>el</otv:language>
        <otv:denotedConcept rdf:resource="#Archaic_Lyric_Poem_in_ionic_or_in_doric_or_in_aeolic_dialect_performed_by_a_chorus_or_by_a_single_performer"/>
        <otv:termStatus>preferred</otv:termStatus>
        <otv:partOfSpeech>none</otv:partOfSpeech>
        <otv:gender>none</otv:gender>
        <otv:termDefinition>Μέλος που εκτελείται από χορό ή από έναν μόνο ερμηνευτή.</otv:termDefinition>
        <skos:definition xml:lang="el">Μέλος που εκτελείται από χορό ή από έναν μόνο ερμηνευτή.</skos:definition>
    </otv:Term>

    <otv:Term rdf:about="#θρήνος_el">
        <rdfs:label xml:lang="el">θρήνος</rdfs:label>
        <otv:termName>θρήνος</otv:termName>
        <otv:language>el</otv:language>
        <otv:denotedConcept rdf:resource="#Archaic_Lyric_Poem_in_ionic_or_in_doric_or_in_aeolic_dialect_performed_by_a_chorus_or_by_a_single_performer_dedicated_to_dead"/>
        <otv:termStatus>preferred</otv:termStatus>
        <otv:partOfSpeech>none</otv:partOfSpeech>
        <otv:gender>none</otv:gender>
        <otv:termDefinition>Λυρικό τραγούδι αφιερωμένο σε έναν νεκρό άνθρωπο. Ο Ανακρέων, ο Πίνδαρος και ο Σιμωνίδης είναι διάσημοι για τέτοιες συνθέσεις τους.</otv:termDefinition>
        <skos:definition xml:lang="el">Λυρικό τραγούδι αφιερωμένο σε έναν νεκρό άνθρωπο. Ο Ανακρέων, ο Πίνδαρος και ο Σιμωνίδης είναι διάσημοι για τέτοιες συνθέσεις τους.</skos:definition>
    </otv:Term>

    <otv:Term rdf:about="#διθύραμβος_el">
        <rdfs:label xml:lang="el">διθύραμβος</rdfs:label>
        <otv:termName>διθύραμβος</otv:termName>
        <otv:language>el</otv:language>
        <otv:denotedConcept rdf:resource="#Archaic_Lyric_Poem_in_ionic_or_in_doric_or_in_aeolic_dialect_performed_by_a_chorus_or_by_a_single_performer_dedicated_to_dionysus"/>
        <otv:termStatus>preferred</otv:termStatus>
        <otv:partOfSpeech>none</otv:partOfSpeech>
        <otv:gender>none</otv:gender>
        <otv:termDefinition>Λατρευτικοί ύμνοι του Διονύσου. Ο Βακχυλίδης, ο Πίνδαρος και ο Σιμωνίδης είναι γνωστό ότι συνέθεσαν διθύραμβους.</otv:termDefinition>
        <skos:definition xml:lang="el">Λατρευτικοί ύμνοι του Διονύσου. Ο Βακχυλίδης, ο Πίνδαρος και ο Σιμωνίδης είναι γνωστό ότι συνέθεσαν διθύραμβους.</skos:definition>
    </otv:Term>

    <otv:Term rdf:about="#ερωτική_ελεγεία_el">
        <rdfs:label xml:lang="el">ερωτική ελεγεία</rdfs:label>
        <otv:termName>ερωτική ελεγεία</otv:termName>
        <otv:language>el</otv:language>
        <otv:denotedConcept rdf:resource="#Archaic_Lyric_Poem_only_in_ionic_dialect_in_elegiac_couplet_with_erotic_content"/>
        <otv:termStatus>preferred</otv:termStatus>
        <otv:partOfSpeech>none</otv:partOfSpeech>
        <otv:gender>none</otv:gender>
        <otv:termDefinition>Ελεγεία με ερωτικό χαρακτήρα. Διάσημος ποιητής που συνέθεσε ερωτικές ελεγείες είναι ο Μίμνερμος.</otv:termDefinition>
        <skos:definition xml:lang="el">Ελεγεία με ερωτικό χαρακτήρα. Διάσημος ποιητής που συνέθεσε ερωτικές ελεγείες είναι ο Μίμνερμος.</skos:definition>
    </otv:Term>

    <otv:Term rdf:about="#πολιτική_ελεγεία_el">
        <rdfs:label xml:lang="el">πολιτική ελεγεία</rdfs:label>
        <otv:termName>πολιτική ελεγεία</otv:termName>
        <otv:language>el</otv:language>
        <otv:denotedConcept rdf:resource="#Archaic_Lyric_Poem_only_in_ionic_dialect_in_elegiac_couplet_with_political_content"/>
        <otv:termStatus>preferred</otv:termStatus>
        <otv:partOfSpeech>none</otv:partOfSpeech>
        <otv:gender>none</otv:gender>
        <otv:termDefinition>Ελεγεία με πολιτικό χαρακτήρα. Ο Τυρταίος και ο Καλλίνικος είναι διάσημοι ποιητές τέτοιων ελεγειών.</otv:termDefinition>
        <skos:definition xml:lang="el">Ελεγεία με πολιτικό χαρακτήρα. Ο Τυρταίος και ο Καλλίνικος είναι διάσημοι ποιητές τέτοιων ελεγειών.</skos:definition>
    </otv:Term>

    <otv:Term rdf:about="#ύμνος_el">
        <rdfs:label xml:lang="el">ύμνος</rdfs:label>
        <otv:termName>ύμνος</otv:termName>
        <otv:language>el</otv:language>
        <otv:denotedConcept rdf:resource="#Archaic_Lyric_Poem_in_ionic_or_in_doric_or_in_aeolic_dialect_performed_by_a_chorus_or_by_a_single_performer_dedicated_to_a_god"/>
        <otv:termStatus>preferred</otv:termStatus>
        <otv:partOfSpeech>none</otv:partOfSpeech>
        <otv:gender>none</otv:gender>
        <otv:termDefinition>Λυρικό τραγούδι αφιερωμένο στους θεούς. Πολλοί ποιητές έχουν συνθέσει ύμνους, όπως ο Αλκαίος, ο Τέρπανδρος, η Σαπφώ, ο Αλκμάνας κ.ά.</otv:termDefinition>
        <skos:definition xml:lang="el">Λυρικό τραγούδι αφιερωμένο στους θεούς. Πολλοί ποιητές έχουν συνθέσει ύμνους, όπως ο Αλκαίος, ο Τέρπανδρος, η Σαπφώ, ο Αλκμάνας κ.ά.</skos:definition>
    </otv:Term>

    <otv:Term rdf:about="#επιθαλάμιο_el">
        <rdfs:label xml:lang="el">επιθαλάμιο</rdfs:label>
        <otv:termName>επιθαλάμιο</otv:termName>
        <otv:language>el</otv:language>
        <otv:denotedConcept rdf:resource="#Archaic_Lyric_Poem_in_ionic_or_in_doric_or_in_aeolic_dialect_performed_by_a_chorus_or_by_a_single_performer_dedicated_to_wedding_couple"/>
        <otv:termStatus>preferred</otv:termStatus>
        <otv:partOfSpeech>none</otv:partOfSpeech>
        <otv:gender>none</otv:gender>
        <otv:termDefinition>Το Επιθαλάμιο είναι ένα τραγούδι αφιερωμένο σε ένα γαμήλιο ζευγάρι που τραγουδιέται στη γαμήλια κατοικία. Η Σαπφώ είναι γνωστή για τα επιθαλάμιά της.</otv:termDefinition>
        <skos:definition xml:lang="el">Το Επιθαλάμιο είναι ένα τραγούδι αφιερωμένο σε ένα γαμήλιο ζευγάρι που τραγουδιέται στη γαμήλια κατοικία. Η Σαπφώ είναι γνωστή για τα επιθαλάμιά της.</skos:definition>
    </otv:Term>

    <otv:Term rdf:about="#αρχαϊκό_λυρικό_ποίημα_σε_ιωνική_ή_δωρική_ή_αιολική_διάλεκτο_που_εκτελείται_από_χορό_μη_συγκεκριμένου_τύπου_el">
        <rdfs:label xml:lang="el">αρχαϊκό λυρικό ποίημα σε ιωνική ή δωρική ή αιολική διάλεκτο που εκτελείται από χορό μη συγκεκριμένου τύπου</rdfs:label>
        <otv:termName>αρχαϊκό λυρικό ποίημα σε ιωνική ή δωρική ή αιολική διάλεκτο που εκτελείται από χορό μη συγκεκριμένου τύπου</otv:termName>
        <otv:language>el</otv:language>
        <otv:denotedConcept rdf:resource="#Archaic_Lyric_Poem_in_ionic_or_in_doric_or_in_aeolic_dialect_performed_by_a_chorus_performed_by_a_non-specific_type_of_chorus"/>
        <otv:termStatus>preferred</otv:termStatus>
        <otv:partOfSpeech>none</otv:partOfSpeech>
        <otv:gender>none</otv:gender>
        <otv:termDefinition>Αρχαϊκό λυρικό ποίημα σε ιωνική ή δωρική ή αιολική διάλεκτο που εκτελείται από χορό μη συγκεκριμένου τύπου.</otv:termDefinition>
        <skos:definition xml:lang="el">Αρχαϊκό λυρικό ποίημα σε ιωνική ή δωρική ή αιολική διάλεκτο που εκτελείται από χορό μη συγκεκριμένου τύπου.</skos:definition>
    </otv:Term>

    <otv:Term rdf:about="#υμέναιος_el">
        <rdfs:label xml:lang="el">υμέναιος</rdfs:label>
        <otv:termName>υμέναιος</otv:termName>
        <otv:language>el</otv:language>
        <otv:denotedConcept rdf:resource="#Archaic_Lyric_Poem_in_ionic_or_in_doric_or_in_aeolic_dialect_performed_by_a_chorus_during_bride_procession"/>
        <otv:termStatus>preferred</otv:termStatus>
        <otv:partOfSpeech>none</otv:partOfSpeech>
        <otv:gender>none</otv:gender>
        <otv:termDefinition>Ένα λυρικό τραγούδι που εκτελείται κατά τη διάρκεια της πομπής της νύφης προς το σπίτι του γαμπρού. Η Σαπφώ είναι διάσημη για τους υμεναίους της.</otv:termDefinition>
        <skos:definition xml:lang="el">Ένα λυρικό τραγούδι που εκτελείται κατά τη διάρκεια της πομπής της νύφης προς το σπίτι του γαμπρού. Η Σαπφώ είναι διάσημη για τους υμεναίους της.</skos:definition>
    </otv:Term>

    <otv:Term rdf:about="#παιάνας_el">
        <rdfs:label xml:lang="el">παιάνας</rdfs:label>
        <otv:termName>παιάνας</otv:termName>
        <otv:language>el</otv:language>
        <otv:denotedConcept rdf:resource="#Archaic_Lyric_Poem_in_ionic_or_in_doric_or_in_aeolic_dialect_performed_by_a_chorus_or_by_a_single_performer_dedicated_to_apollo"/>
        <otv:termStatus>preferred</otv:termStatus>
        <otv:partOfSpeech>none</otv:partOfSpeech>
        <otv:gender>none</otv:gender>
        <otv:termDefinition>Λυρικό τραγούδι αφιερωμένο στον αρχαίο Έλληνα θεό Απόλλωνα. Ο Αλκμάνας, ο Πίνδαρος και ο Βακχυλίδης είναι διάσημοι συνθέτες παιάνων.</otv:termDefinition>
        <skos:definition xml:lang="el">Λυρικό τραγούδι αφιερωμένο στον αρχαίο Έλληνα θεό Απόλλωνα. Ο Αλκμάνας, ο Πίνδαρος και ο Βακχυλίδης είναι διάσημοι συνθέτες παιάνων.</skos:definition>
    </otv:Term>

    <otv:Term rdf:about="#αρχαϊκός_λυρικός_ποιητής_el">
        <rdfs:label xml:lang="el">αρχαϊκός λυρικός ποιητής</rdfs:label>
        <otv:termName>αρχαϊκός λυρικός ποιητής</otv:termName>
        <otv:language>el</otv:language>
        <otv:denotedConcept rdf:resource="#Archaic_Lyric_Poet"/>
        <otv:termStatus>preferred</otv:termStatus>
        <otv:partOfSpeech>none</otv:partOfSpeech>
        <otv:gender>none</otv:gender>
        <otv:termDefinition>Ο αρχαϊκός λυρικός ποιητής είναι ένα πρόσωπο που έζησε κατά τον 7ο-αρχές του 5ου αιώνα π.Χ. και έγραψε αρχαϊκή λυρική ποίηση.</otv:termDefinition>
        <skos:definition xml:lang="el">Ο αρχαϊκός λυρικός ποιητής είναι ένα πρόσωπο που έζησε κατά τον 7ο-αρχές του 5ου αιώνα π.Χ. και έγραψε αρχαϊκή λυρική ποίηση.</skos:definition>
    </otv:Term>

    <otv:Term rdf:about="#προχριστιανικός_αιώνας_el">
        <rdfs:label xml:lang="el">προχριστιανικός αιώνας</rdfs:label>
        <otv:termName>προχριστιανικός αιώνας</otv:termName>
        <otv:language>el</otv:language>
        <otv:denotedConcept rdf:resource="#BCE_century"/>
        <otv:termStatus>preferred</otv:termStatus>
        <otv:partOfSpeech>none</otv:partOfSpeech>
        <otv:gender>none</otv:gender>
        <otv:termDefinition> Προχριστιανικός αιώνας.</otv:termDefinition>
        <skos:definition xml:lang="el"> Προχριστιανικός αιώνας.</skos:definition>
    </otv:Term>

    <otv:Term rdf:about="#υπόρχημα_el">
        <rdfs:label xml:lang="el">υπόρχημα</rdfs:label>
        <otv:termName>υπόρχημα</otv:termName>
        <otv:language>el</otv:language>
        <otv:denotedConcept rdf:resource="#Archaic_Lyric_Poem_in_ionic_or_in_doric_or_in_aeolic_dialect_performed_by_a_chorus_with_imitation_expressions"/>
        <otv:termStatus>preferred</otv:termStatus>
        <otv:partOfSpeech>none</otv:partOfSpeech>
        <otv:gender>none</otv:gender>
        <otv:termDefinition>Ένα λυρικό τραγούδι που συνοδεύεται από μιμητικές κινήσεις. Ο Βακχυλίδης και ο Πίνδαρος φημίζονται για τη σύνθεση υπορχημάτων.</otv:termDefinition>
        <skos:definition xml:lang="el">Ένα λυρικό τραγούδι που συνοδεύεται από μιμητικές κινήσεις. Ο Βακχυλίδης και ο Πίνδαρος φημίζονται για τη σύνθεση υπορχημάτων.</skos:definition>
    </otv:Term>

    <otv:Term rdf:about="#γνωμική_ελεγεία_el">
        <rdfs:label xml:lang="el">γνωμική ελεγεία</rdfs:label>
        <otv:termName>γνωμική ελεγεία</otv:termName>
        <otv:language>el</otv:language>
        <otv:denotedConcept rdf:resource="#Archaic_Lyric_Poem_only_in_ionic_dialect_in_elegiac_couplet_with_gnomic_content"/>
        <otv:termStatus>preferred</otv:termStatus>
        <otv:partOfSpeech>none</otv:partOfSpeech>
        <otv:gender>none</otv:gender>
        <otv:termDefinition>Ελεγεία με γνωμικό, συμβουλευτικό, βιοσοφικό περιεχόμενο. Γνωστοί ποιητές γνωστών γνωμικών ελεγειών είναι ο Φωκυλίδης και ο Θεογένης.</otv:termDefinition>
        <skos:definition xml:lang="el">Ελεγεία με γνωμικό, συμβουλευτικό, βιοσοφικό περιεχόμενο. Γνωστοί ποιητές γνωστών γνωμικών ελεγειών είναι ο Φωκυλίδης και ο Θεογένης.</skos:definition>
    </otv:Term>

    <otv:Term rdf:about="#αρχαϊκό_λυρικό_ποίημα_σε_ιωνική_ή_δωρική_ή_αιολική_διάλεκτο_που_εκτελείται_από_χορό_el">
        <rdfs:label xml:lang="el">αρχαϊκό λυρικό ποίημα σε ιωνική ή δωρική ή αιολική διάλεκτο που εκτελείται από χορό</rdfs:label>
        <otv:termName>αρχαϊκό λυρικό ποίημα σε ιωνική ή δωρική ή αιολική διάλεκτο που εκτελείται από χορό</otv:termName>
        <otv:language>el</otv:language>
        <otv:denotedConcept rdf:resource="#Archaic_Lyric_Poem_in_ionic_or_in_doric_or_in_aeolic_dialect_performed_by_a_chorus"/>
        <otv:termStatus>preferred</otv:termStatus>
        <otv:partOfSpeech>none</otv:partOfSpeech>
        <otv:gender>none</otv:gender>
        <otv:termDefinition>Μέλος που εκτελείται από Χορό.</otv:termDefinition>
        <skos:definition xml:lang="el">Μέλος που εκτελείται από Χορό.</skos:definition>
    </otv:Term>

    <otv:Term rdf:about="#εγκώμιο_el">
        <rdfs:label xml:lang="el">εγκώμιο</rdfs:label>
        <otv:termName>εγκώμιο</otv:termName>
        <otv:language>el</otv:language>
        <otv:denotedConcept rdf:resource="#Archaic_Lyric_Poem_in_ionic_or_in_doric_or_in_aeolic_dialect_performed_by_a_chorus_or_by_a_single_performer_dedicated_to_living"/>
        <otv:termStatus>preferred</otv:termStatus>
        <otv:partOfSpeech>none</otv:partOfSpeech>
        <otv:gender>none</otv:gender>
        <otv:termDefinition>Λυρικό τραγούδι επαίνου για ανθρώπους στη διάρκεια της ζωής τους. Ο Πίνδαρος, ο Βακχυλίδης και ο Ίβυκος είναι σημαντικές μορφές της σύνθεσης του εγκωμίου.</otv:termDefinition>
        <skos:definition xml:lang="el">Λυρικό τραγούδι επαίνου για ανθρώπους στη διάρκεια της ζωής τους. Ο Πίνδαρος, ο Βακχυλίδης και ο Ίβυκος είναι σημαντικές μορφές της σύνθεσης του εγκωμίου.</skos:definition>
    </otv:Term>

    <otv:Term rdf:about="#παρθένειο_el">
        <rdfs:label xml:lang="el">παρθένειο</rdfs:label>
        <otv:termName>παρθένειο</otv:termName>
        <otv:language>el</otv:language>
        <otv:denotedConcept rdf:resource="#Archaic_Lyric_Poem_in_ionic_or_in_doric_or_in_aeolic_dialect_performed_by_a_chorus_performed_by_a_maidens_chorus"/>
        <otv:termStatus>preferred</otv:termStatus>
        <otv:partOfSpeech>none</otv:partOfSpeech>
        <otv:gender>none</otv:gender>
        <otv:termDefinition>Ένα λυρικό τραγούδι που ερμηνεύεται από μια χορωδία νεανίδων. Ο Αλκμάνας, ο Πίνδαρος και ο Βακχυλίδης φημίζονται για τη σύνθεση των Παρθενείων.</otv:termDefinition>
        <skos:definition xml:lang="el">Ένα λυρικό τραγούδι που ερμηνεύεται από μια χορωδία νεανίδων. Ο Αλκμάνας, ο Πίνδαρος και ο Βακχυλίδης φημίζονται για τη σύνθεση των Παρθενείων.</skos:definition>
    </otv:Term>

    <otv:Term rdf:about="#ίαμβος_el">
        <rdfs:label xml:lang="el">ίαμβος</rdfs:label>
        <otv:termName>ίαμβος</otv:termName>
        <otv:language>el</otv:language>
        <otv:denotedConcept rdf:resource="#Archaic_Lyric_Poem_only_in_ionic_dialect_in_iambic_or_trochaic_metre"/>
        <otv:termStatus>preferred</otv:termStatus>
        <otv:partOfSpeech>none</otv:partOfSpeech>
        <otv:gender>none</otv:gender>
        <otv:termDefinition>Αρχικά συνδεόμενος με τον Διόνυσο, ο ίαμβος μπορεί να έχει προελληνική προέλευση ως ποιητική μορφή. Συνήθως συντίθεται σε ιαμβικό τρίμετρο ή τροχαϊκό τετράμετρο, η ιωνική εκδοχή του συχνά υιοθετεί την πρωτοπρόσωπη σκοπιά, αν και τα συμφραζόμενα μπορεί να ποικίλλουν.</otv:termDefinition>
        <skos:definition xml:lang="el">Αρχικά συνδεόμενος με τον Διόνυσο, ο ίαμβος μπορεί να έχει προελληνική προέλευση ως ποιητική μορφή. Συνήθως συντίθεται σε ιαμβικό τρίμετρο ή τροχαϊκό τετράμετρο, η ιωνική εκδοχή του συχνά υιοθετεί την πρωτοπρόσωπη σκοπιά, αν και τα συμφραζόμενα μπορεί να ποικίλλουν.</skos:definition>
    </otv:Term>

    <otv:Term rdf:about="#μονωδία_el">
        <rdfs:label xml:lang="el">μονωδία</rdfs:label>
        <otv:termName>μονωδία</otv:termName>
        <otv:language>el</otv:language>
        <otv:denotedConcept rdf:resource="#Archaic_Lyric_Poem_in_ionic_or_in_doric_or_in_aeolic_dialect_performed_by_a_single_performer"/>
        <otv:termStatus>preferred</otv:termStatus>
        <otv:partOfSpeech>none</otv:partOfSpeech>
        <otv:gender>none</otv:gender>
        <otv:termDefinition>Οι μονωδίες χαρακτηρίζονται από σόλο ερμηνείες, όπου ο ποιητής ταυτίζεται με τον τραγουδιστή και εκφράζει προσωπικές σκέψεις και συναισθήματα, καθώς προσφέρουν μια άμεση και ελεύθερη έκφραση της προσωπικότητας. Για παράδειγμα, στις σαπφικές ωδές, η ποιήτρια δίνει προτεραιότητα στη δική της φωνή έναντι των άλλων.</otv:termDefinition>
        <skos:definition xml:lang="el">Οι μονωδίες χαρακτηρίζονται από σόλο ερμηνείες, όπου ο ποιητής ταυτίζεται με τον τραγουδιστή και εκφράζει προσωπικές σκέψεις και συναισθήματα, καθώς προσφέρουν μια άμεση και ελεύθερη έκφραση της προσωπικότητας. Για παράδειγμα, στις σαπφικές ωδές, η ποιήτρια δίνει προτεραιότητα στη δική της φωνή έναντι των άλλων.</skos:definition>
    </otv:Term>

    <otv:Term rdf:about="#επίνικος_el">
        <rdfs:label xml:lang="el">επίνικος</rdfs:label>
        <otv:termName>επίνικος</otv:termName>
        <otv:language>el</otv:language>
        <otv:denotedConcept rdf:resource="#Archaic_Lyric_Poem_in_ionic_or_in_doric_or_in_aeolic_dialect_performed_by_a_chorus_or_by_a_single_performer_dedicated_to_winners_in_athletic_events"/>
        <otv:termStatus>preferred</otv:termStatus>
        <otv:partOfSpeech>none</otv:partOfSpeech>
        <otv:gender>none</otv:gender>
        <otv:termDefinition>Λυρικό τραγούδι αφιερωμένο σε νικητή αθλητικών αγώνων. Ο Πίνδαρος, ο Βακχυλίδης και ο Ίβυκος είναι αυτοί που συνέθεσαν επινίκια τραγούδια.</otv:termDefinition>
        <skos:definition xml:lang="el">Λυρικό τραγούδι αφιερωμένο σε νικητή αθλητικών αγώνων. Ο Πίνδαρος, ο Βακχυλίδης και ο Ίβυκος είναι αυτοί που συνέθεσαν επινίκια τραγούδια.</skos:definition>
    </otv:Term>

    <otv:Term rdf:about="#προσόδιο_el">
        <rdfs:label xml:lang="el">προσόδιο</rdfs:label>
        <otv:termName>προσόδιο</otv:termName>
        <otv:language>el</otv:language>
        <otv:denotedConcept rdf:resource="#Archaic_Lyric_Poem_in_ionic_or_in_doric_or_in_aeolic_dialect_performed_by_a_chorus_on_the_way_to_an_altar"/>
        <otv:termStatus>preferred</otv:termStatus>
        <otv:partOfSpeech>none</otv:partOfSpeech>
        <otv:gender>none</otv:gender>
        <otv:termDefinition>Ένα λυρικό τραγούδι που ερμηνεύεται στο δρόμο προς το ιερό από μια χορωδία. Ο Αλκμάν, ο Βακχυλίδης και ο Πίνδαρος είναι διάσημοι συνθέτες προσοδίων.</otv:termDefinition>
        <skos:definition xml:lang="el">Ένα λυρικό τραγούδι που ερμηνεύεται στο δρόμο προς το ιερό από μια χορωδία. Ο Αλκμάν, ο Βακχυλίδης και ο Πίνδαρος είναι διάσημοι συνθέτες προσοδίων.</skos:definition>
    </otv:Term>

    <otv:Term rdf:about="#μέλος_el">
        <rdfs:label xml:lang="el">μέλος</rdfs:label>
        <otv:termName>μέλος</otv:termName>
        <otv:language>el</otv:language>
        <otv:denotedConcept rdf:resource="#Archaic_Lyric_Poem_in_ionic_or_in_doric_or_in_aeolic_dialect"/>
        <otv:termStatus>preferred</otv:termStatus>
        <otv:partOfSpeech>none</otv:partOfSpeech>
        <otv:gender>none</otv:gender>
        <otv:termDefinition>Το Μέλος είναι το υπερώνυμο των αρχαϊκών λυρικών ποιημάτων, τα οποία ήταν γραμμένα σε ιωνική (εκτός από τον ίαμβο και την ελεγεία), αιολική και δωρική διάλεκτο.</otv:termDefinition>
        <skos:definition xml:lang="el">Το Μέλος είναι το υπερώνυμο των αρχαϊκών λυρικών ποιημάτων, τα οποία ήταν γραμμένα σε ιωνική (εκτός από τον ίαμβο και την ελεγεία), αιολική και δωρική διάλεκτο.</skos:definition>
    </otv:Term>

    <otv:Term rdf:about="#ελεγεία_el">
        <rdfs:label xml:lang="el">ελεγεία</rdfs:label>
        <otv:termName>ελεγεία</otv:termName>
        <otv:language>el</otv:language>
        <otv:denotedConcept rdf:resource="#Archaic_Lyric_Poem_only_in_ionic_dialect_in_elegiac_couplet"/>
        <otv:termStatus>preferred</otv:termStatus>
        <otv:partOfSpeech>none</otv:partOfSpeech>
        <otv:gender>none</otv:gender>
        <otv:termDefinition>Οι ελεγείες είναι ποιήματα γραμμένα σε ελεγειακά δίστιχα, με τον πρώτο στίχο σε εξάμετρο και τον δεύτερο σε πεντάμετρο. Αρχικά, χρησιμοποιήθηκαν για θρήνους (αλλά αργότερα είχαν ένα ευρύ φάσμα θεμάτων) και πιθανόν προέρχονται από τις ανατολίτικες θρηνητικές πρακτικές. Μπορεί να είναι μικρές σε έκταση (όσο ένα απλό κουπλέ) ή μεγαλύτερες.</otv:termDefinition>
        <skos:definition xml:lang="el">Οι ελεγείες είναι ποιήματα γραμμένα σε ελεγειακά δίστιχα, με τον πρώτο στίχο σε εξάμετρο και τον δεύτερο σε πεντάμετρο. Αρχικά, χρησιμοποιήθηκαν για θρήνους (αλλά αργότερα είχαν ένα ευρύ φάσμα θεμάτων) και πιθανόν προέρχονται από τις ανατολίτικες θρηνητικές πρακτικές. Μπορεί να είναι μικρές σε έκταση (όσο ένα απλό κουπλέ) ή μεγαλύτερες.</skos:definition>
    </otv:Term>

    <otv:Term rdf:about="#αρχαϊκό_λυρικό_ποίημα_el">
        <rdfs:label xml:lang="el">αρχαϊκό λυρικό ποίημα</rdfs:label>
        <otv:termName>αρχαϊκό λυρικό ποίημα</otv:termName>
        <otv:language>el</otv:language>
        <otv:denotedConcept rdf:resource="#Archaic_Lyric_Poem"/>
        <otv:termStatus>preferred</otv:termStatus>
        <otv:partOfSpeech>none</otv:partOfSpeech>
        <otv:gender>none</otv:gender>
        <otv:termDefinition>"Η Λυρική ποίηση ξεκίνησε ως θεσμός της αρχαίας Ελλάδας, ταξινομημένος σε σχέση με άλλες κατηγορίες ποίησης κατά την εποχή της κλασικής αρχαιότητας: τα δραματικά (γραμμένα σε στίχους) και τα επικά ποιήματα. Η λυρική ποίηση ήταν πολύ πιο σύντομη, ενώ διακρινόταν επίσης από την εστίασή της στην ψυχική κατάσταση του ποιητή και σε προσωπικά θέματα και όχι στο αφηγηματικό τόξο" (Ακαδημία Αμερικανών Ποιητών). Έτσι, ένα αρχαϊκό λυρικό ποίημα είναι ένα τέτοιο ποίημα που γράφτηκε από τον 7ο-αρχές του 5ου αιώνα π.Χ.</otv:termDefinition>
        <skos:definition xml:lang="el">"Η Λυρική ποίηση ξεκίνησε ως θεσμός της αρχαίας Ελλάδας, ταξινομημένος σε σχέση με άλλες κατηγορίες ποίησης κατά την εποχή της κλασικής αρχαιότητας: τα δραματικά (γραμμένα σε στίχους) και τα επικά ποιήματα. Η λυρική ποίηση ήταν πολύ πιο σύντομη, ενώ διακρινόταν επίσης από την εστίασή της στην ψυχική κατάσταση του ποιητή και σε προσωπικά θέματα και όχι στο αφηγηματικό τόξο" (Ακαδημία Αμερικανών Ποιητών). Έτσι, ένα αρχαϊκό λυρικό ποίημα είναι ένα τέτοιο ποίημα που γράφτηκε από τον 7ο-αρχές του 5ου αιώνα π.Χ.</skos:definition>
    </otv:Term>

	<!--  OTV Proper Names -->

    <otv:ProperName rdf:about="#Pindar_en">
        <otv:properName>Pindar</otv:properName>
        <otv:language>en</otv:language>
        <otv:denotedObject rdf:resource="#pindarus_boeotus"/>
    </otv:ProperName>

    <otv:ProperName rdf:about="#Erotic_odes_of_Anacreon_Teius_en">
        <otv:properName>Erotic odes of Anacreon Teius</otv:properName>
        <otv:language>en</otv:language>
        <otv:denotedObject rdf:resource="#erotic_odes_anacreon"/>
    </otv:ProperName>

    <otv:ProperName rdf:about="#Anacreon_Lyricus_en">
        <otv:properName>Anacreon Lyricus</otv:properName>
        <otv:language>en</otv:language>
        <otv:denotedObject rdf:resource="#anacreon_teius"/>
    </otv:ProperName>

    <otv:ProperName rdf:about="#Archilochus_Lyricus_en">
        <otv:properName>Archilochus Lyricus</otv:properName>
        <otv:language>en</otv:language>
        <otv:denotedObject rdf:resource="#archilochus_parius"/>
    </otv:ProperName>

    <otv:ProperName rdf:about="#7th_century_BCE_en">
        <otv:properName>7th century BCE</otv:properName>
        <otv:language>en</otv:language>
        <otv:denotedObject rdf:resource="#7th_century_BCE"/>
    </otv:ProperName>

    <otv:ProperName rdf:about="#Enkomion_of_Ibycus_Rheginus_en">
        <otv:properName>Enkomion of Ibycus Rheginus</otv:properName>
        <otv:language>en</otv:language>
        <otv:denotedObject rdf:resource="#enkomion_ibycus"/>
    </otv:ProperName>

    <otv:ProperName rdf:about="#Sapphus_en">
        <otv:properName>Sapphus</otv:properName>
        <otv:language>en</otv:language>
        <otv:denotedObject rdf:resource="#sappho_lesbia"/>
    </otv:ProperName>

    <otv:ProperName rdf:about="#Iambs_of_Ananius_en">
        <otv:properName>Iambs of Ananius</otv:properName>
        <otv:language>en</otv:language>
        <otv:denotedObject rdf:resource="#iambs_ananius"/>
    </otv:ProperName>

    <otv:ProperName rdf:about="#War_elegies_of_Tyrtaeus_Lacedaemonius_en">
        <otv:properName>War elegies of Tyrtaeus Lacedaemonius</otv:properName>
        <otv:language>en</otv:language>
        <otv:denotedObject rdf:resource="#war_elegies_tyrtaeus"/>
    </otv:ProperName>

    <otv:ProperName rdf:about="#Ephesus_en">
        <otv:properName>Ephesus</otv:properName>
        <otv:language>en</otv:language>
        <otv:denotedObject rdf:resource="#ephesus"/>
    </otv:ProperName>

    <otv:ProperName rdf:about="#Anacreon_Teius_en">
        <otv:properName>Anacreon Teius</otv:properName>
        <otv:language>en</otv:language>
        <otv:denotedObject rdf:resource="#anacreon_teius"/>
    </otv:ProperName>

    <otv:ProperName rdf:about="#Thasos-_settlement_en">
        <otv:properName>Thasos- settlement</otv:properName>
        <otv:language>en</otv:language>
        <otv:denotedObject rdf:resource="#thasos_settlement"/>
    </otv:ProperName>

    <otv:ProperName rdf:about="#Paros_en">
        <otv:properName>Paros</otv:properName>
        <otv:language>en</otv:language>
        <otv:denotedObject rdf:resource="#paros"/>
    </otv:ProperName>

    <otv:ProperName rdf:about="#Epinikoi_of_Simonides_Ceus_en">
        <otv:properName>Epinikoi of Simonides Ceus</otv:properName>
        <otv:language>en</otv:language>
        <otv:denotedObject rdf:resource="#epinikoi_simonides"/>
    </otv:ProperName>

    <otv:ProperName rdf:about="#Pindarus_Lyricus_en">
        <otv:properName>Pindarus Lyricus</otv:properName>
        <otv:language>en</otv:language>
        <otv:denotedObject rdf:resource="#pindarus_boeotus"/>
    </otv:ProperName>

    <otv:ProperName rdf:about="#Terpander_Lesbius_en">
        <otv:properName>Terpander Lesbius</otv:properName>
        <otv:language>en</otv:language>
        <otv:denotedObject rdf:resource="#terpander_lesbius"/>
    </otv:ProperName>

    <otv:ProperName rdf:about="#Sicilia_en">
        <otv:properName>Sicilia</otv:properName>
        <otv:language>en</otv:language>
        <otv:denotedObject rdf:resource="#sicilia"/>
    </otv:ProperName>

    <otv:ProperName rdf:about="#Solon_Atheniensis_en">
        <otv:properName>Solon Atheniensis</otv:properName>
        <otv:language>en</otv:language>
        <otv:denotedObject rdf:resource="#solon_atheniensis"/>
    </otv:ProperName>

    <otv:ProperName rdf:about="#Mimnermo_of_Colophon_en">
        <otv:properName>Mimnermo of Colophon</otv:properName>
        <otv:language>en</otv:language>
        <otv:denotedObject rdf:resource="#mimnermus_lyricus"/>
    </otv:ProperName>

    <otv:ProperName rdf:about="#Choral_songs_of_Stesichorus_Himeraeus_en">
        <otv:properName>Choral songs of Stesichorus Himeraeus</otv:properName>
        <otv:language>en</otv:language>
        <otv:denotedObject rdf:resource="#choral_stesichorus"/>
    </otv:ProperName>

    <otv:ProperName rdf:about="#Miletus_en">
        <otv:properName>Miletus</otv:properName>
        <otv:language>en</otv:language>
        <otv:denotedObject rdf:resource="#miletus"/>
    </otv:ProperName>

    <otv:ProperName rdf:about="#Hymns_of_Sappho_Lesbia_en">
        <otv:properName>Hymns of Sappho Lesbia</otv:properName>
        <otv:language>en</otv:language>
        <otv:denotedObject rdf:resource="#hymns_sappho"/>
    </otv:ProperName>

    <otv:ProperName rdf:about="#Alcaeus_Lyricus_en">
        <otv:properName>Alcaeus Lyricus</otv:properName>
        <otv:language>en</otv:language>
        <otv:denotedObject rdf:resource="#alcaeus_lesbius"/>
    </otv:ProperName>

    <otv:ProperName rdf:about="#Mimnermus_Lyricus_en">
        <otv:properName>Mimnermus Lyricus</otv:properName>
        <otv:language>en</otv:language>
        <otv:denotedObject rdf:resource="#mimnermus_lyricus"/>
    </otv:ProperName>

    <otv:ProperName rdf:about="#Erotic_poetry_of_Alcman_Lacedaemonius_en">
        <otv:properName>Erotic poetry of Alcman Lacedaemonius</otv:properName>
        <otv:language>en</otv:language>
        <otv:denotedObject rdf:resource="#erotic_odes_alcman"/>
    </otv:ProperName>

    <otv:ProperName rdf:about="#Samos_en">
        <otv:properName>Samos</otv:properName>
        <otv:language>en</otv:language>
        <otv:denotedObject rdf:resource="#samos"/>
    </otv:ProperName>

    <otv:ProperName rdf:about="#Partheneia_of_Alcman_Lacedaemonius_en">
        <otv:properName>Partheneia of Alcman Lacedaemonius</otv:properName>
        <otv:language>en</otv:language>
        <otv:denotedObject rdf:resource="#partheneia_alcman"/>
    </otv:ProperName>

    <otv:ProperName rdf:about="#Prosodia_of_Bacchylides_Ceus_en">
        <otv:properName>Prosodia of Bacchylides Ceus</otv:properName>
        <otv:language>en</otv:language>
        <otv:denotedObject rdf:resource="#prosodia_bacchylides"/>
    </otv:ProperName>

    <otv:ProperName rdf:about="#Simonides_of_Ceos_en">
        <otv:properName>Simonides of Ceos</otv:properName>
        <otv:language>en</otv:language>
        <otv:denotedObject rdf:resource="#simonides_ceus"/>
    </otv:ProperName>

    <otv:ProperName rdf:about="#Sappho_Lyrica_en">
        <otv:properName>Sappho Lyrica</otv:properName>
        <otv:language>en</otv:language>
        <otv:denotedObject rdf:resource="#sappho_lesbia"/>
    </otv:ProperName>

    <otv:ProperName rdf:about="#Phocylides_of_Miletus_en">
        <otv:properName>Phocylides of Miletus</otv:properName>
        <otv:language>en</otv:language>
        <otv:denotedObject rdf:resource="#phocylides_milesius"/>
    </otv:ProperName>

    <otv:ProperName rdf:about="#Bacchylides_Lyricus_en">
        <otv:properName>Bacchylides Lyricus</otv:properName>
        <otv:language>en</otv:language>
        <otv:denotedObject rdf:resource="#bacchylides_ceus"/>
    </otv:ProperName>

    <otv:ProperName rdf:about="#Prosodia_of_Alcman_Lacedaemonius_en">
        <otv:properName>Prosodia of Alcman Lacedaemonius</otv:properName>
        <otv:language>en</otv:language>
        <otv:denotedObject rdf:resource="#prosodia_alcman"/>
    </otv:ProperName>

    <otv:ProperName rdf:about="#Alcman_Lyricus_en">
        <otv:properName>Alcman Lyricus</otv:properName>
        <otv:language>en</otv:language>
        <otv:denotedObject rdf:resource="#alcman_lacedaemonius"/>
    </otv:ProperName>

    <otv:ProperName rdf:about="#Smyrna_en">
        <otv:properName>Smyrna</otv:properName>
        <otv:language>en</otv:language>
        <otv:denotedObject rdf:resource="#smyrna"/>
    </otv:ProperName>

    <otv:ProperName rdf:about="#Colophon_en">
        <otv:properName>Colophon</otv:properName>
        <otv:language>en</otv:language>
        <otv:denotedObject rdf:resource="#colophon"/>
    </otv:ProperName>

    <otv:ProperName rdf:about="#Alcaeus_Mytilenaeus_en">
        <otv:properName>Alcaeus Mytilenaeus</otv:properName>
        <otv:language>en</otv:language>
        <otv:denotedObject rdf:resource="#alcaeus_lesbius"/>
    </otv:ProperName>

    <otv:ProperName rdf:about="#Iambs_of_Anacreon_Teius_en">
        <otv:properName>Iambs of Anacreon Teius</otv:properName>
        <otv:language>en</otv:language>
        <otv:denotedObject rdf:resource="#iambs_anacreon"/>
    </otv:ProperName>

    <otv:ProperName rdf:about="#Theognis_Megarensis_en">
        <otv:properName>Theognis Megarensis</otv:properName>
        <otv:language>en</otv:language>
        <otv:denotedObject rdf:resource="#theognis_megarensis"/>
    </otv:ProperName>

    <otv:ProperName rdf:about="#Sparta_en">
        <otv:properName>Sparta</otv:properName>
        <otv:language>en</otv:language>
        <otv:denotedObject rdf:resource="#sparta"/>
    </otv:ProperName>

    <otv:ProperName rdf:about="#Terpandrus_en">
        <otv:properName>Terpandrus</otv:properName>
        <otv:language>en</otv:language>
        <otv:denotedObject rdf:resource="#terpander_lesbius"/>
    </otv:ProperName>

    <otv:ProperName rdf:about="#Ananius_Lyricus_en">
        <otv:properName>Ananius Lyricus</otv:properName>
        <otv:language>en</otv:language>
        <otv:denotedObject rdf:resource="#ananius_iambographus"/>
    </otv:ProperName>

    <otv:ProperName rdf:about="#Stesichorus_Himeraeus_en">
        <otv:properName>Stesichorus Himeraeus</otv:properName>
        <otv:language>en</otv:language>
        <otv:denotedObject rdf:resource="#stesichorus_himeraeus"/>
    </otv:ProperName>

    <otv:ProperName rdf:about="#Elegies_of_Simonides_Ceus_en">
        <otv:properName>Elegies of Simonides Ceus</otv:properName>
        <otv:language>en</otv:language>
        <otv:denotedObject rdf:resource="#elegies_simonides"/>
    </otv:ProperName>

    <otv:ProperName rdf:about="#Simonides_of_Amorgos_en">
        <otv:properName>Simonides of Amorgos</otv:properName>
        <otv:language>en</otv:language>
        <otv:denotedObject rdf:resource="#semonides_amorginus"/>
    </otv:ProperName>

    <otv:ProperName rdf:about="#Hymns_of_Alcaeus_Lesbius_en">
        <otv:properName>Hymns of Alcaeus Lesbius</otv:properName>
        <otv:language>en</otv:language>
        <otv:denotedObject rdf:resource="#hymns_alcaeus"/>
    </otv:ProperName>

    <otv:ProperName rdf:about="#Warlike_odes_of_Alcaeus_Lesbius_en">
        <otv:properName>Warlike odes of Alcaeus Lesbius</otv:properName>
        <otv:language>en</otv:language>
        <otv:denotedObject rdf:resource="#warlike_odes_alcaeus"/>
    </otv:ProperName>

    <otv:ProperName rdf:about="#Athens_en">
        <otv:properName>Athens</otv:properName>
        <otv:language>en</otv:language>
        <otv:denotedObject rdf:resource="#athens"/>
    </otv:ProperName>

    <otv:ProperName rdf:about="#Semonides_Amorginus_en">
        <otv:properName>Semonides Amorginus</otv:properName>
        <otv:language>en</otv:language>
        <otv:denotedObject rdf:resource="#semonides_amorginus"/>
    </otv:ProperName>

    <otv:ProperName rdf:about="#Semonides_Iambographus_en">
        <otv:properName>Semonides Iambographus</otv:properName>
        <otv:language>en</otv:language>
        <otv:denotedObject rdf:resource="#semonides_amorginus"/>
    </otv:ProperName>

    <otv:ProperName rdf:about="#Rhegium_en">
        <otv:properName>Rhegium</otv:properName>
        <otv:language>en</otv:language>
        <otv:denotedObject rdf:resource="#rhegium"/>
    </otv:ProperName>

    <otv:ProperName rdf:about="#Abdera_en">
        <otv:properName>Abdera</otv:properName>
        <otv:language>en</otv:language>
        <otv:denotedObject rdf:resource="#abdera"/>
    </otv:ProperName>

    <otv:ProperName rdf:about="#Klazomenai_en">
        <otv:properName>Klazomenai</otv:properName>
        <otv:language>en</otv:language>
        <otv:denotedObject rdf:resource="#klazomenai"/>
    </otv:ProperName>

    <otv:ProperName rdf:about="#Threnoi_of_Pindarus_Boeotus_en">
        <otv:properName>Threnoi of Pindarus Boeotus</otv:properName>
        <otv:language>en</otv:language>
        <otv:denotedObject rdf:resource="#threnoi_pindarus"/>
    </otv:ProperName>

    <otv:ProperName rdf:about="#Ibycus_Rheginus_en">
        <otv:properName>Ibycus Rheginus</otv:properName>
        <otv:language>en</otv:language>
        <otv:denotedObject rdf:resource="#ibycus_rheginus"/>
    </otv:ProperName>

    <otv:ProperName rdf:about="#Elegies_of_Archilochus_Parius_en">
        <otv:properName>Elegies of Archilochus Parius</otv:properName>
        <otv:language>en</otv:language>
        <otv:denotedObject rdf:resource="#elegies_archilochus"/>
    </otv:ProperName>

    <otv:ProperName rdf:about="#Megara_en">
        <otv:properName>Megara</otv:properName>
        <otv:language>en</otv:language>
        <otv:denotedObject rdf:resource="#megara"/>
    </otv:ProperName>

    <otv:ProperName rdf:about="#Pindarus_en">
        <otv:properName>Pindarus</otv:properName>
        <otv:language>en</otv:language>
        <otv:denotedObject rdf:resource="#pindarus_boeotus"/>
    </otv:ProperName>

    <otv:ProperName rdf:about="#Enkomion_of_Bacchylides_Ceus_en">
        <otv:properName>Enkomion of Bacchylides Ceus</otv:properName>
        <otv:language>en</otv:language>
        <otv:denotedObject rdf:resource="#enkomion_bacchylides"/>
    </otv:ProperName>

    <otv:ProperName rdf:about="#Hymns_of_Anacreon_Teius_en">
        <otv:properName>Hymns of Anacreon Teius</otv:properName>
        <otv:language>en</otv:language>
        <otv:denotedObject rdf:resource="#hymns_anacreon"/>
    </otv:ProperName>

    <otv:ProperName rdf:about="#Prosodia_of_Pindarus_Boeotus_en">
        <otv:properName>Prosodia of Pindarus Boeotus</otv:properName>
        <otv:language>en</otv:language>
        <otv:denotedObject rdf:resource="#prosodia_pindarus"/>
    </otv:ProperName>

    <otv:ProperName rdf:about="#Callinus_Ephesius_en">
        <otv:properName>Callinus Ephesius</otv:properName>
        <otv:language>en</otv:language>
        <otv:denotedObject rdf:resource="#callinus_ephesius"/>
    </otv:ProperName>

    <otv:ProperName rdf:about="#Alcman_Lacedaemonius_en">
        <otv:properName>Alcman Lacedaemonius</otv:properName>
        <otv:language>en</otv:language>
        <otv:denotedObject rdf:resource="#alcman_lacedaemonius"/>
    </otv:ProperName>

    <otv:ProperName rdf:about="#Epithalamia_of_Sappho_Lesbia_en">
        <otv:properName>Epithalamia of Sappho Lesbia</otv:properName>
        <otv:language>en</otv:language>
        <otv:denotedObject rdf:resource="#epithalamia_sappho"/>
    </otv:ProperName>

    <otv:ProperName rdf:about="#Gnomic_elegies_of_Phocylides_Milesius_en">
        <otv:properName>Gnomic elegies of Phocylides Milesius</otv:properName>
        <otv:language>en</otv:language>
        <otv:denotedObject rdf:resource="#gnomic_elegies_phocylides"/>
    </otv:ProperName>

    <otv:ProperName rdf:about="#Simonides_Ceus_en">
        <otv:properName>Simonides Ceus</otv:properName>
        <otv:language>en</otv:language>
        <otv:denotedObject rdf:resource="#simonides_ceus"/>
    </otv:ProperName>

    <otv:ProperName rdf:about="#Ananius_Iambographus_en">
        <otv:properName>Ananius Iambographus</otv:properName>
        <otv:language>en</otv:language>
        <otv:denotedObject rdf:resource="#ananius_iambographus"/>
    </otv:ProperName>

    <otv:ProperName rdf:about="#Enkomion_of_Pindarus_Boeotus_en">
        <otv:properName>Enkomion of Pindarus Boeotus</otv:properName>
        <otv:language>en</otv:language>
        <otv:denotedObject rdf:resource="#enkomion_pindarus"/>
    </otv:ProperName>

    <otv:ProperName rdf:about="#Ananios_Iambograph_en">
        <otv:properName>Ananios Iambograph</otv:properName>
        <otv:language>en</otv:language>
        <otv:denotedObject rdf:resource="#ananius_iambographus"/>
    </otv:ProperName>

    <otv:ProperName rdf:about="#Boeotia_en">
        <otv:properName>Boeotia</otv:properName>
        <otv:language>en</otv:language>
        <otv:denotedObject rdf:resource="#boeotia"/>
    </otv:ProperName>

    <otv:ProperName rdf:about="#Phocylides_Lyricus_en">
        <otv:properName>Phocylides Lyricus</otv:properName>
        <otv:language>en</otv:language>
        <otv:denotedObject rdf:resource="#phocylides_milesius"/>
    </otv:ProperName>

    <otv:ProperName rdf:about="#Akragas_en">
        <otv:properName>Akragas</otv:properName>
        <otv:language>en</otv:language>
        <otv:denotedObject rdf:resource="#akragas"/>
    </otv:ProperName>

    <otv:ProperName rdf:about="#Hymenaios_of_Sappho_Lesbia_en">
        <otv:properName>Hymenaios of Sappho Lesbia</otv:properName>
        <otv:language>en</otv:language>
        <otv:denotedObject rdf:resource="#hymenaios_sappho"/>
    </otv:ProperName>

    <otv:ProperName rdf:about="#Bacchylides_Ceus_en">
        <otv:properName>Bacchylides Ceus</otv:properName>
        <otv:language>en</otv:language>
        <otv:denotedObject rdf:resource="#bacchylides_ceus"/>
    </otv:ProperName>

    <otv:ProperName rdf:about="#Amorgos_en">
        <otv:properName>Amorgos</otv:properName>
        <otv:language>en</otv:language>
        <otv:denotedObject rdf:resource="#amorgos"/>
    </otv:ProperName>

    <otv:ProperName rdf:about="#Hipponax_Iambographus_en">
        <otv:properName>Hipponax Iambographus</otv:properName>
        <otv:language>en</otv:language>
        <otv:denotedObject rdf:resource="#hipponax_ephesius"/>
    </otv:ProperName>

    <otv:ProperName rdf:about="#Lesbos_en">
        <otv:properName>Lesbos</otv:properName>
        <otv:language>en</otv:language>
        <otv:denotedObject rdf:resource="#lesbos"/>
    </otv:ProperName>

    <otv:ProperName rdf:about="#Sympotic_odes_of_Anacreon_Teius_en">
        <otv:properName>Sympotic odes of Anacreon Teius</otv:properName>
        <otv:language>en</otv:language>
        <otv:denotedObject rdf:resource="#sympotic_odes_anacreon"/>
    </otv:ProperName>

    <otv:ProperName rdf:about="#Hipponax_Ephesius_en">
        <otv:properName>Hipponax Ephesius</otv:properName>
        <otv:language>en</otv:language>
        <otv:denotedObject rdf:resource="#hipponax_ephesius"/>
    </otv:ProperName>

    <otv:ProperName rdf:about="#Terpandros_en">
        <otv:properName>Terpandros</otv:properName>
        <otv:language>en</otv:language>
        <otv:denotedObject rdf:resource="#terpander_lesbius"/>
    </otv:ProperName>

    <otv:ProperName rdf:about="#Paeans_of_Alcman_Lacedaemonius_en">
        <otv:properName>Paeans of Alcman Lacedaemonius</otv:properName>
        <otv:language>en</otv:language>
        <otv:denotedObject rdf:resource="#paeans_alcman"/>
    </otv:ProperName>

    <otv:ProperName rdf:about="#Hymns_of_Archilochus_Parius_en">
        <otv:properName>Hymns of Archilochus Parius</otv:properName>
        <otv:language>en</otv:language>
        <otv:denotedObject rdf:resource="#hymns_archilochus"/>
    </otv:ProperName>

    <otv:ProperName rdf:about="#Erotic_odes_of_Alcaeus_Lesbius_en">
        <otv:properName>Erotic odes of Alcaeus Lesbius</otv:properName>
        <otv:language>en</otv:language>
        <otv:denotedObject rdf:resource="#erotic_odes_alcaeus"/>
    </otv:ProperName>

    <otv:ProperName rdf:about="#Sappho_Lesbia_en">
        <otv:properName>Sappho Lesbia</otv:properName>
        <otv:language>en</otv:language>
        <otv:denotedObject rdf:resource="#sappho_lesbia"/>
    </otv:ProperName>

    <otv:ProperName rdf:about="#Simonides_Lyricus_en">
        <otv:properName>Simonides Lyricus</otv:properName>
        <otv:language>en</otv:language>
        <otv:denotedObject rdf:resource="#simonides_ceus"/>
    </otv:ProperName>

    <otv:ProperName rdf:about="#Threnoi_of_Anacreon_Teius_en">
        <otv:properName>Threnoi of Anacreon Teius</otv:properName>
        <otv:language>en</otv:language>
        <otv:denotedObject rdf:resource="#threnoi_anacreon"/>
    </otv:ProperName>

    <otv:ProperName rdf:about="#Keos_en">
        <otv:properName>Keos</otv:properName>
        <otv:language>en</otv:language>
        <otv:denotedObject rdf:resource="#keos"/>
    </otv:ProperName>

    <otv:ProperName rdf:about="#Pindarus_Boeotus_en">
        <otv:properName>Pindarus Boeotus</otv:properName>
        <otv:language>en</otv:language>
        <otv:denotedObject rdf:resource="#pindarus_boeotus"/>
    </otv:ProperName>

    <otv:ProperName rdf:about="#5th_century_BCE_en">
        <otv:properName>5th century BCE</otv:properName>
        <otv:language>en</otv:language>
        <otv:denotedObject rdf:resource="#5th_century_BCE"/>
    </otv:ProperName>

    <otv:ProperName rdf:about="#Archilochus_Iamb._et_Eleg._en">
        <otv:properName>Archilochus Iamb. et Eleg.</otv:properName>
        <otv:language>en</otv:language>
        <otv:denotedObject rdf:resource="#archilochus_parius"/>
    </otv:ProperName>

    <otv:ProperName rdf:about="#Himera_en">
        <otv:properName>Himera</otv:properName>
        <otv:language>en</otv:language>
        <otv:denotedObject rdf:resource="#himera"/>
    </otv:ProperName>

    <otv:ProperName rdf:about="#Teos_en">
        <otv:properName>Teos</otv:properName>
        <otv:language>en</otv:language>
        <otv:denotedObject rdf:resource="#teos"/>
    </otv:ProperName>

    <otv:ProperName rdf:about="#Aegypt_en">
        <otv:properName>Aegypt</otv:properName>
        <otv:language>en</otv:language>
        <otv:denotedObject rdf:resource="#aegypt"/>
    </otv:ProperName>

    <otv:ProperName rdf:about="#Hymns_of_Alcman_Lacedaemonius_en">
        <otv:properName>Hymns of Alcman Lacedaemonius</otv:properName>
        <otv:language>en</otv:language>
        <otv:denotedObject rdf:resource="#hymns_alcman"/>
    </otv:ProperName>

    <otv:ProperName rdf:about="#Partheneia_of_Bacchylides_Ceus_en">
        <otv:properName>Partheneia of Bacchylides Ceus</otv:properName>
        <otv:language>en</otv:language>
        <otv:denotedObject rdf:resource="#partheneia_bacchylides"/>
    </otv:ProperName>

    <otv:ProperName rdf:about="#Hymns_of_Terpander_Lesbius_en">
        <otv:properName>Hymns of Terpander Lesbius</otv:properName>
        <otv:language>en</otv:language>
        <otv:denotedObject rdf:resource="#hymns_terpander"/>
    </otv:ProperName>

    <otv:ProperName rdf:about="#Tyrtaeus_Lacedaemonius_en">
        <otv:properName>Tyrtaeus Lacedaemonius</otv:properName>
        <otv:language>en</otv:language>
        <otv:denotedObject rdf:resource="#tyrtaeus_lacedaemonius"/>
    </otv:ProperName>

    <otv:ProperName rdf:about="#Sympotic_odes_of_Alcaeus_Lesbius_en">
        <otv:properName>Sympotic odes of Alcaeus Lesbius</otv:properName>
        <otv:language>en</otv:language>
        <otv:denotedObject rdf:resource="#sympotic_odes_alcaeus"/>
    </otv:ProperName>

    <otv:ProperName rdf:about="#Iambs_of_Archilochus_Parius_en">
        <otv:properName>Iambs of Archilochus Parius</otv:properName>
        <otv:language>en</otv:language>
        <otv:denotedObject rdf:resource="#iambs_archilochus"/>
    </otv:ProperName>

    <otv:ProperName rdf:about="#Dithyrambs_of_Simonides_Ceus_en">
        <otv:properName>Dithyrambs of Simonides Ceus</otv:properName>
        <otv:language>en</otv:language>
        <otv:denotedObject rdf:resource="#dithyrambs_simonides"/>
    </otv:ProperName>

    <otv:ProperName rdf:about="#Simonides_of_Samos_en">
        <otv:properName>Simonides of Samos</otv:properName>
        <otv:language>en</otv:language>
        <otv:denotedObject rdf:resource="#semonides_amorginus"/>
    </otv:ProperName>

    <otv:ProperName rdf:about="#Iambs_of_Hipponax_Ephesius_en">
        <otv:properName>Iambs of Hipponax Ephesius</otv:properName>
        <otv:language>en</otv:language>
        <otv:denotedObject rdf:resource="#iambs_hipponax"/>
    </otv:ProperName>

    <otv:ProperName rdf:about="#Choral_songs_of_Ibycus_Rheginus_en">
        <otv:properName>Choral songs of Ibycus Rheginus</otv:properName>
        <otv:language>en</otv:language>
        <otv:denotedObject rdf:resource="#choral_ibycus"/>
    </otv:ProperName>

    <otv:ProperName rdf:about="#Hyporchemes_of_Bacchylides_Ceus_en">
        <otv:properName>Hyporchemes of Bacchylides Ceus</otv:properName>
        <otv:language>en</otv:language>
        <otv:denotedObject rdf:resource="#hyporcheme_bacchylides"/>
    </otv:ProperName>

    <otv:ProperName rdf:about="#Alcaeus_Lesbius_en">
        <otv:properName>Alcaeus Lesbius</otv:properName>
        <otv:language>en</otv:language>
        <otv:denotedObject rdf:resource="#alcaeus_lesbius"/>
    </otv:ProperName>

    <otv:ProperName rdf:about="#Theognis_Elegiacus_en">
        <otv:properName>Theognis Elegiacus</otv:properName>
        <otv:language>en</otv:language>
        <otv:denotedObject rdf:resource="#theognis_megarensis"/>
    </otv:ProperName>

    <otv:ProperName rdf:about="#Gnomic_elegies_of_Theognis_Megarensis_en">
        <otv:properName>Gnomic elegies of Theognis Megarensis</otv:properName>
        <otv:language>en</otv:language>
        <otv:denotedObject rdf:resource="#gnomic_elegies_theognis"/>
    </otv:ProperName>

    <otv:ProperName rdf:about="#Partheneia_of_Pindarus_Boeotus_en">
        <otv:properName>Partheneia of Pindarus Boeotus</otv:properName>
        <otv:language>en</otv:language>
        <otv:denotedObject rdf:resource="#partheneia_pindarus"/>
    </otv:ProperName>

    <otv:ProperName rdf:about="#Epinikoi_of_Pindarus_Boeotus_en">
        <otv:properName>Epinikoi of Pindarus Boeotus</otv:properName>
        <otv:language>en</otv:language>
        <otv:denotedObject rdf:resource="#epinikoi_pindarus"/>
    </otv:ProperName>

    <otv:ProperName rdf:about="#Dithyrambs_of_Bacchylides_Ceus_en">
        <otv:properName>Dithyrambs of Bacchylides Ceus</otv:properName>
        <otv:language>en</otv:language>
        <otv:denotedObject rdf:resource="#dithyrambs_bacchylides"/>
    </otv:ProperName>

    <otv:ProperName rdf:about="#Paeans_of_Bacchylides_Ceus_en">
        <otv:properName>Paeans of Bacchylides Ceus</otv:properName>
        <otv:language>en</otv:language>
        <otv:denotedObject rdf:resource="#paeans_bacchylides"/>
    </otv:ProperName>

    <otv:ProperName rdf:about="#Erotic_poetry_of_Sappho_Lesbia_en">
        <otv:properName>Erotic poetry of Sappho Lesbia</otv:properName>
        <otv:language>en</otv:language>
        <otv:denotedObject rdf:resource="#erotic_odes_sappho"/>
    </otv:ProperName>

    <otv:ProperName rdf:about="#Political_elegy_of_Solon_Athenienis_en">
        <otv:properName>Political elegy of Solon Athenienis</otv:properName>
        <otv:language>en</otv:language>
        <otv:denotedObject rdf:resource="#political_elegies_solon"/>
    </otv:ProperName>

    <otv:ProperName rdf:about="#Alcaeus_Mytilenensis_en">
        <otv:properName>Alcaeus Mytilenensis</otv:properName>
        <otv:language>en</otv:language>
        <otv:denotedObject rdf:resource="#alcaeus_lesbius"/>
    </otv:ProperName>

    <otv:ProperName rdf:about="#Hyporchemes_of_Pindarus_Boeotus_en">
        <otv:properName>Hyporchemes of Pindarus Boeotus</otv:properName>
        <otv:language>en</otv:language>
        <otv:denotedObject rdf:resource="#hyporchemes_pindarus"/>
    </otv:ProperName>

    <otv:ProperName rdf:about="#War_elegy_of_Callinus_Ephesius_en">
        <otv:properName>War elegy of Callinus Ephesius</otv:properName>
        <otv:language>en</otv:language>
        <otv:denotedObject rdf:resource="#war_elegy_callinus"/>
    </otv:ProperName>

    <otv:ProperName rdf:about="#Archilochus_Parius_en">
        <otv:properName>Archilochus Parius</otv:properName>
        <otv:language>en</otv:language>
        <otv:denotedObject rdf:resource="#archilochus_parius"/>
    </otv:ProperName>

    <otv:ProperName rdf:about="#Sardis_en">
        <otv:properName>Sardis</otv:properName>
        <otv:language>en</otv:language>
        <otv:denotedObject rdf:resource="#sardis"/>
    </otv:ProperName>

    <otv:ProperName rdf:about="#Erotic_elegies_of_Mimnermus_Lyricus_en">
        <otv:properName>Erotic elegies of Mimnermus Lyricus</otv:properName>
        <otv:language>en</otv:language>
        <otv:denotedObject rdf:resource="#erotic_elegies_mimnermus"/>
    </otv:ProperName>

    <otv:ProperName rdf:about="#Phocylides_Milesius_en">
        <otv:properName>Phocylides Milesius</otv:properName>
        <otv:language>en</otv:language>
        <otv:denotedObject rdf:resource="#phocylides_milesius"/>
    </otv:ProperName>

    <otv:ProperName rdf:about="#Syrakousai_en">
        <otv:properName>Syrakousai</otv:properName>
        <otv:language>en</otv:language>
        <otv:denotedObject rdf:resource="#syrakousai"/>
    </otv:ProperName>

    <otv:ProperName rdf:about="#Elegies_of_Anacreon_Teius_en">
        <otv:properName>Elegies of Anacreon Teius</otv:properName>
        <otv:language>en</otv:language>
        <otv:denotedObject rdf:resource="#elegies_anacreon"/>
    </otv:ProperName>

    <otv:ProperName rdf:about="#Dithyrambs_of_Pindarus_Boeotus_en">
        <otv:properName>Dithyrambs of Pindarus Boeotus</otv:properName>
        <otv:language>en</otv:language>
        <otv:denotedObject rdf:resource="#dithyrambs_pindarus"/>
    </otv:ProperName>

    <otv:ProperName rdf:about="#Iambs_of_Semonides_Amorginus_en">
        <otv:properName>Iambs of Semonides Amorginus</otv:properName>
        <otv:language>en</otv:language>
        <otv:denotedObject rdf:resource="#iambs_semonides"/>
    </otv:ProperName>

    <otv:ProperName rdf:about="#Epinikoi_of_Bacchylides_Ceus_en">
        <otv:properName>Epinikoi of Bacchylides Ceus</otv:properName>
        <otv:language>en</otv:language>
        <otv:denotedObject rdf:resource="#epinikoi_bacchylides"/>
    </otv:ProperName>

    <otv:ProperName rdf:about="#Paeans_of_Pindarus_Boeotus_en">
        <otv:properName>Paeans of Pindarus Boeotus</otv:properName>
        <otv:language>en</otv:language>
        <otv:denotedObject rdf:resource="#paeans_pindarus"/>
    </otv:ProperName>

    <otv:ProperName rdf:about="#6th_century_BCE_en">
        <otv:properName>6th century BCE</otv:properName>
        <otv:language>en</otv:language>
        <otv:denotedObject rdf:resource="#6th_century_BCE"/>
    </otv:ProperName>

    <otv:ProperName rdf:about="#Threnoi_of_Simonides_Ceus_en">
        <otv:properName>Threnoi of Simonides Ceus</otv:properName>
        <otv:language>en</otv:language>
        <otv:denotedObject rdf:resource="#threnoi_simonides"/>
    </otv:ProperName>

    <otv:ProperName rdf:about="#Archilochus_of_Paros_en">
        <otv:properName>Archilochus of Paros</otv:properName>
        <otv:language>en</otv:language>
        <otv:denotedObject rdf:resource="#archilochus_parius"/>
    </otv:ProperName>

    <otv:ProperName rdf:about="#Μίλητος_el">
        <otv:properName>Μίλητος</otv:properName>
        <otv:language>el</otv:language>
        <otv:denotedObject rdf:resource="#miletus"/>
    </otv:ProperName>

    <otv:ProperName rdf:about="#Σμύρνη_el">
        <otv:properName>Σμύρνη</otv:properName>
        <otv:language>el</otv:language>
        <otv:denotedObject rdf:resource="#smyrna"/>
    </otv:ProperName>

    <otv:ProperName rdf:about="#Πολεμικές_ωδές_του_Αλκαίου_el">
        <otv:properName>Πολεμικές ωδές του Αλκαίου</otv:properName>
        <otv:language>el</otv:language>
        <otv:denotedObject rdf:resource="#warlike_odes_alcaeus"/>
    </otv:ProperName>

    <otv:ProperName rdf:about="#Ανακρέων_ο_Τήιος_el">
        <otv:properName>Ανακρέων ο Τήιος</otv:properName>
        <otv:language>el</otv:language>
        <otv:denotedObject rdf:resource="#anacreon_teius"/>
    </otv:ProperName>

    <otv:ProperName rdf:about="#Τέως_el">
        <otv:properName>Τέως</otv:properName>
        <otv:language>el</otv:language>
        <otv:denotedObject rdf:resource="#teos"/>
    </otv:ProperName>

    <otv:ProperName rdf:about="#Παρθένεια_του_Αλκμάνα_el">
        <otv:properName>Παρθένεια του Αλκμάνα</otv:properName>
        <otv:language>el</otv:language>
        <otv:denotedObject rdf:resource="#partheneia_alcman"/>
    </otv:ProperName>

    <otv:ProperName rdf:about="#Ανάνιος_ο_Ιαμβογράφος_el">
        <otv:properName>Ανάνιος ο Ιαμβογράφος</otv:properName>
        <otv:language>el</otv:language>
        <otv:denotedObject rdf:resource="#ananius_iambographus"/>
    </otv:ProperName>

    <otv:ProperName rdf:about="#Σόλων_ο_Αθηναίος_el">
        <otv:properName>Σόλων ο Αθηναίος</otv:properName>
        <otv:language>el</otv:language>
        <otv:denotedObject rdf:resource="#solon_atheniensis"/>
    </otv:ProperName>

    <otv:ProperName rdf:about="#Χορική_ποίηση_του_Ίβυκου_του_Ρηγίνου_el">
        <otv:properName>Χορική ποίηση του Ίβυκου του Ρηγίνου</otv:properName>
        <otv:language>el</otv:language>
        <otv:denotedObject rdf:resource="#choral_ibycus"/>
    </otv:ProperName>

    <otv:ProperName rdf:about="#Λέσβος_el">
        <otv:properName>Λέσβος</otv:properName>
        <otv:language>el</otv:language>
        <otv:denotedObject rdf:resource="#lesbos"/>
    </otv:ProperName>

    <otv:ProperName rdf:about="#Έφεσος_el">
        <otv:properName>Έφεσος</otv:properName>
        <otv:language>el</otv:language>
        <otv:denotedObject rdf:resource="#ephesus"/>
    </otv:ProperName>

    <otv:ProperName rdf:about="#Συμποτικές_ωδές_του_Ανακρέοντα_el">
        <otv:properName>Συμποτικές ωδές του Ανακρέοντα</otv:properName>
        <otv:language>el</otv:language>
        <otv:denotedObject rdf:resource="#sympotic_odes_anacreon"/>
    </otv:ProperName>

    <otv:ProperName rdf:about="#Παιάνες_του_Πινδάρου_el">
        <otv:properName>Παιάνες του Πινδάρου</otv:properName>
        <otv:language>el</otv:language>
        <otv:denotedObject rdf:resource="#paeans_pindarus"/>
    </otv:ProperName>

    <otv:ProperName rdf:about="#Αλκαίος_ο_Μυτιληναίος_el">
        <otv:properName>Αλκαίος ο Μυτιληναίος</otv:properName>
        <otv:language>el</otv:language>
        <otv:denotedObject rdf:resource="#alcaeus_lesbius"/>
    </otv:ProperName>

    <otv:ProperName rdf:about="#Σημωνίδης_ο_Αμοργίνος_el">
        <otv:properName>Σημωνίδης ο Αμοργίνος</otv:properName>
        <otv:language>el</otv:language>
        <otv:denotedObject rdf:resource="#semonides_amorginus"/>
    </otv:ProperName>

    <otv:ProperName rdf:about="#Ερωτική_ποίηση_της_Σαπφούς_el">
        <otv:properName>Ερωτική ποίηση της Σαπφούς</otv:properName>
        <otv:language>el</otv:language>
        <otv:denotedObject rdf:resource="#erotic_odes_sappho"/>
    </otv:ProperName>

    <otv:ProperName rdf:about="#Αλκαίος_ο_Λέσβιος_el">
        <otv:properName>Αλκαίος ο Λέσβιος</otv:properName>
        <otv:language>el</otv:language>
        <otv:denotedObject rdf:resource="#alcaeus_lesbius"/>
    </otv:ProperName>

    <otv:ProperName rdf:about="#Διθύραμβοι_του_Σιμωνίδη_του_Κείου_el">
        <otv:properName>Διθύραμβοι του Σιμωνίδη του Κείου</otv:properName>
        <otv:language>el</otv:language>
        <otv:denotedObject rdf:resource="#dithyrambs_simonides"/>
    </otv:ProperName>

    <otv:ProperName rdf:about="#6ος_αιώνας_π.Χ._el">
        <otv:properName>6ος αιώνας π.Χ.</otv:properName>
        <otv:language>el</otv:language>
        <otv:denotedObject rdf:resource="#6th_century_BCE"/>
    </otv:ProperName>

    <otv:ProperName rdf:about="#Πολεμικές_ελεγείες_του_Τυρταίου_el">
        <otv:properName>Πολεμικές ελεγείες του Τυρταίου</otv:properName>
        <otv:language>el</otv:language>
        <otv:denotedObject rdf:resource="#war_elegies_tyrtaeus"/>
    </otv:ProperName>

    <otv:ProperName rdf:about="#Αλκμάνας_ο_Λυρικός_el">
        <otv:properName>Αλκμάνας ο Λυρικός</otv:properName>
        <otv:language>el</otv:language>
        <otv:denotedObject rdf:resource="#alcman_lacedaemonius"/>
    </otv:ProperName>

    <otv:ProperName rdf:about="#Γνωμικές_ελεγείς_του_Φωκυλίδη_el">
        <otv:properName>Γνωμικές ελεγείς του Φωκυλίδη</otv:properName>
        <otv:language>el</otv:language>
        <otv:denotedObject rdf:resource="#gnomic_elegies_phocylides"/>
    </otv:ProperName>

    <otv:ProperName rdf:about="#Ίαμβοι_του_Ανακρέοντα_el">
        <otv:properName>Ίαμβοι του Ανακρέοντα</otv:properName>
        <otv:language>el</otv:language>
        <otv:denotedObject rdf:resource="#iambs_anacreon"/>
    </otv:ProperName>

    <otv:ProperName rdf:about="#Ύμνοι_του_Αλκμάνα_του_Λακεδαιμόνιου_el">
        <otv:properName>Ύμνοι του Αλκμάνα του Λακεδαιμόνιου</otv:properName>
        <otv:language>el</otv:language>
        <otv:denotedObject rdf:resource="#hymns_alcman"/>
    </otv:ProperName>

    <otv:ProperName rdf:about="#Κέα_el">
        <otv:properName>Κέα</otv:properName>
        <otv:language>el</otv:language>
        <otv:denotedObject rdf:resource="#keos"/>
    </otv:ProperName>

    <otv:ProperName rdf:about="#Αθήνα_el">
        <otv:properName>Αθήνα</otv:properName>
        <otv:language>el</otv:language>
        <otv:denotedObject rdf:resource="#athens"/>
    </otv:ProperName>

    <otv:ProperName rdf:about="#Υπορχήματα_του_Βακχυλίδη_el">
        <otv:properName>Υπορχήματα του Βακχυλίδη</otv:properName>
        <otv:language>el</otv:language>
        <otv:denotedObject rdf:resource="#hyporcheme_bacchylides"/>
    </otv:ProperName>

    <otv:ProperName rdf:about="#Πίνδαρος_ο_Βοιωτός_el">
        <otv:properName>Πίνδαρος ο Βοιωτός</otv:properName>
        <otv:language>el</otv:language>
        <otv:denotedObject rdf:resource="#pindarus_boeotus"/>
    </otv:ProperName>

    <otv:ProperName rdf:about="#Πίνδαρος_από_τη_Βοιωτία_el">
        <otv:properName>Πίνδαρος από τη Βοιωτία</otv:properName>
        <otv:language>el</otv:language>
        <otv:denotedObject rdf:resource="#pindarus_boeotus"/>
    </otv:ProperName>

    <otv:ProperName rdf:about="#Πολεμικές_ελεγείες_του_Καλλίνου_el">
        <otv:properName>Πολεμικές ελεγείες του Καλλίνου</otv:properName>
        <otv:language>el</otv:language>
        <otv:denotedObject rdf:resource="#war_elegy_callinus"/>
    </otv:ProperName>

    <otv:ProperName rdf:about="#Θρήνοι_του_Ανακρέοντα_el">
        <otv:properName>Θρήνοι του Ανακρέοντα</otv:properName>
        <otv:language>el</otv:language>
        <otv:denotedObject rdf:resource="#threnoi_anacreon"/>
    </otv:ProperName>

    <otv:ProperName rdf:about="#Ιππώναξ_ο_Εφέσιος_el">
        <otv:properName>Ιππώναξ ο Εφέσιος</otv:properName>
        <otv:language>el</otv:language>
        <otv:denotedObject rdf:resource="#hipponax_ephesius"/>
    </otv:ProperName>

    <otv:ProperName rdf:about="#Παιάνες_του_Αλκμάνα_el">
        <otv:properName>Παιάνες του Αλκμάνα</otv:properName>
        <otv:language>el</otv:language>
        <otv:denotedObject rdf:resource="#paeans_alcman"/>
    </otv:ProperName>

    <otv:ProperName rdf:about="#Αρχίλοχος_ο_Πάριος_el">
        <otv:properName>Αρχίλοχος ο Πάριος</otv:properName>
        <otv:language>el</otv:language>
        <otv:denotedObject rdf:resource="#archilochus_parius"/>
    </otv:ProperName>

    <otv:ProperName rdf:about="#Ελεγείες_του_Σιμωνίδη_από_την_Κέα_el">
        <otv:properName>Ελεγείες του Σιμωνίδη από την Κέα</otv:properName>
        <otv:language>el</otv:language>
        <otv:denotedObject rdf:resource="#elegies_simonides"/>
    </otv:ProperName>

    <otv:ProperName rdf:about="#Μίμνερμος_ο_Λυρικός_el">
        <otv:properName>Μίμνερμος ο Λυρικός</otv:properName>
        <otv:language>el</otv:language>
        <otv:denotedObject rdf:resource="#mimnermus_lyricus"/>
    </otv:ProperName>

    <otv:ProperName rdf:about="#Σαπφώ_el">
        <otv:properName>Σαπφώ</otv:properName>
        <otv:language>el</otv:language>
        <otv:denotedObject rdf:resource="#sappho_lesbia"/>
    </otv:ProperName>

    <otv:ProperName rdf:about="#Θέογνις_από_τα_Μέγαρα_el">
        <otv:properName>Θέογνις από τα Μέγαρα</otv:properName>
        <otv:language>el</otv:language>
        <otv:denotedObject rdf:resource="#theognis_megarensis"/>
    </otv:ProperName>

    <otv:ProperName rdf:about="#Σάμος_el">
        <otv:properName>Σάμος</otv:properName>
        <otv:language>el</otv:language>
        <otv:denotedObject rdf:resource="#samos"/>
    </otv:ProperName>

    <otv:ProperName rdf:about="#Κλαζομενές_el">
        <otv:properName>Κλαζομενές</otv:properName>
        <otv:language>el</otv:language>
        <otv:denotedObject rdf:resource="#klazomenai"/>
    </otv:ProperName>

    <otv:ProperName rdf:about="#Φωκυλίδης_από_τη_Μίλητο_el">
        <otv:properName>Φωκυλίδης από τη Μίλητο</otv:properName>
        <otv:language>el</otv:language>
        <otv:denotedObject rdf:resource="#phocylides_milesius"/>
    </otv:ProperName>

    <otv:ProperName rdf:about="#Διθυραμβική_ποίηση_του_Πινδάρου_el">
        <otv:properName>Διθυραμβική ποίηση του Πινδάρου</otv:properName>
        <otv:language>el</otv:language>
        <otv:denotedObject rdf:resource="#dithyrambs_pindarus"/>
    </otv:ProperName>

    <otv:ProperName rdf:about="#Αλκμάν_el">
        <otv:properName>Αλκμάν</otv:properName>
        <otv:language>el</otv:language>
        <otv:denotedObject rdf:resource="#alcman_lacedaemonius"/>
    </otv:ProperName>

    <otv:ProperName rdf:about="#Άβδηρα_el">
        <otv:properName>Άβδηρα</otv:properName>
        <otv:language>el</otv:language>
        <otv:denotedObject rdf:resource="#abdera"/>
    </otv:ProperName>

    <otv:ProperName rdf:about="#Καλλίνος_ο_Εφέσιος_el">
        <otv:properName>Καλλίνος ο Εφέσιος</otv:properName>
        <otv:language>el</otv:language>
        <otv:denotedObject rdf:resource="#callinus_ephesius"/>
    </otv:ProperName>

    <otv:ProperName rdf:about="#Ίαμβοι_του_Σημωνίδη_του_Αμοργίνου_el">
        <otv:properName>Ίαμβοι του Σημωνίδη του Αμοργίνου</otv:properName>
        <otv:language>el</otv:language>
        <otv:denotedObject rdf:resource="#iambs_semonides"/>
    </otv:ProperName>

    <otv:ProperName rdf:about="#Αμοργός_el">
        <otv:properName>Αμοργός</otv:properName>
        <otv:language>el</otv:language>
        <otv:denotedObject rdf:resource="#amorgos"/>
    </otv:ProperName>

    <otv:ProperName rdf:about="#Παρθένεια_του_Βακχυλίδη_el">
        <otv:properName>Παρθένεια του Βακχυλίδη</otv:properName>
        <otv:language>el</otv:language>
        <otv:denotedObject rdf:resource="#partheneia_bacchylides"/>
    </otv:ProperName>

    <otv:ProperName rdf:about="#Εγκωμιαστική_ποίηση_του_Πινδάρου_el">
        <otv:properName>Εγκωμιαστική ποίηση του Πινδάρου</otv:properName>
        <otv:language>el</otv:language>
        <otv:denotedObject rdf:resource="#enkomion_pindarus"/>
    </otv:ProperName>

    <otv:ProperName rdf:about="#Εγκωμιαστική_ποίηση_του_Ιβύκου_el">
        <otv:properName>Εγκωμιαστική ποίηση του Ιβύκου</otv:properName>
        <otv:language>el</otv:language>
        <otv:denotedObject rdf:resource="#enkomion_ibycus"/>
    </otv:ProperName>

    <otv:ProperName rdf:about="#Ύμνοι_της_Σαπφούς_της_Λεσβίας_el">
        <otv:properName>Ύμνοι της Σαπφούς της Λεσβίας</otv:properName>
        <otv:language>el</otv:language>
        <otv:denotedObject rdf:resource="#hymns_sappho"/>
    </otv:ProperName>

    <otv:ProperName rdf:about="#Στησίχορος_από_την_Ιμέρα_el">
        <otv:properName>Στησίχορος από την Ιμέρα</otv:properName>
        <otv:language>el</otv:language>
        <otv:denotedObject rdf:resource="#stesichorus_himeraeus"/>
    </otv:ProperName>

    <otv:ProperName rdf:about="#Βακχυλίδης_ο_Λυρικός_el">
        <otv:properName>Βακχυλίδης ο Λυρικός</otv:properName>
        <otv:language>el</otv:language>
        <otv:denotedObject rdf:resource="#bacchylides_ceus"/>
    </otv:ProperName>

    <otv:ProperName rdf:about="#Πολιτική_ελεγεία_του_Σόλωνα_el">
        <otv:properName>Πολιτική ελεγεία του Σόλωνα</otv:properName>
        <otv:language>el</otv:language>
        <otv:denotedObject rdf:resource="#political_elegies_solon"/>
    </otv:ProperName>

    <otv:ProperName rdf:about="#Διθυραμβική_ποίηση_του_Βακχυλίδη_από_την_Κέα_el">
        <otv:properName>Διθυραμβική ποίηση του Βακχυλίδη από την Κέα</otv:properName>
        <otv:language>el</otv:language>
        <otv:denotedObject rdf:resource="#dithyrambs_bacchylides"/>
    </otv:ProperName>

    <otv:ProperName rdf:about="#Φωκυλίδης_ο_Λυρικός_el">
        <otv:properName>Φωκυλίδης ο Λυρικός</otv:properName>
        <otv:language>el</otv:language>
        <otv:denotedObject rdf:resource="#phocylides_milesius"/>
    </otv:ProperName>

    <otv:ProperName rdf:about="#Θρήνοι_του_Σιμωνίδη_από_την_Κέα_el">
        <otv:properName>Θρήνοι του Σιμωνίδη από την Κέα</otv:properName>
        <otv:language>el</otv:language>
        <otv:denotedObject rdf:resource="#threnoi_simonides"/>
    </otv:ProperName>

    <otv:ProperName rdf:about="#Σημωνίδης_ο_Ιαμβογράφος_el">
        <otv:properName>Σημωνίδης ο Ιαμβογράφος</otv:properName>
        <otv:language>el</otv:language>
        <otv:denotedObject rdf:resource="#semonides_amorginus"/>
    </otv:ProperName>

    <otv:ProperName rdf:about="#Βακχυλίδης_από_την_Κέα_el">
        <otv:properName>Βακχυλίδης από την Κέα</otv:properName>
        <otv:language>el</otv:language>
        <otv:denotedObject rdf:resource="#bacchylides_ceus"/>
    </otv:ProperName>

    <otv:ProperName rdf:about="#Ερωτική_ελεγεία_του_Μίμνερμου_el">
        <otv:properName>Ερωτική ελεγεία του Μίμνερμου</otv:properName>
        <otv:language>el</otv:language>
        <otv:denotedObject rdf:resource="#erotic_elegies_mimnermus"/>
    </otv:ProperName>

    <otv:ProperName rdf:about="#Πάρος_el">
        <otv:properName>Πάρος</otv:properName>
        <otv:language>el</otv:language>
        <otv:denotedObject rdf:resource="#paros"/>
    </otv:ProperName>

    <otv:ProperName rdf:about="#Ίαμβοι_του_Ανάνιου_el">
        <otv:properName>Ίαμβοι του Ανάνιου</otv:properName>
        <otv:language>el</otv:language>
        <otv:denotedObject rdf:resource="#iambs_ananius"/>
    </otv:ProperName>

    <otv:ProperName rdf:about="#Θρήνοι_του_Πινδάρου_el">
        <otv:properName>Θρήνοι του Πινδάρου</otv:properName>
        <otv:language>el</otv:language>
        <otv:denotedObject rdf:resource="#threnoi_pindarus"/>
    </otv:ProperName>

    <otv:ProperName rdf:about="#Επίνικοι_του_Βακχυλίδη_el">
        <otv:properName>Επίνικοι του Βακχυλίδη</otv:properName>
        <otv:language>el</otv:language>
        <otv:denotedObject rdf:resource="#epinikoi_bacchylides"/>
    </otv:ProperName>

    <otv:ProperName rdf:about="#Συρακούσες_el">
        <otv:properName>Συρακούσες</otv:properName>
        <otv:language>el</otv:language>
        <otv:denotedObject rdf:resource="#syrakousai"/>
    </otv:ProperName>

    <otv:ProperName rdf:about="#7ος_αιώνας_π.Χ._el">
        <otv:properName>7ος αιώνας π.Χ.</otv:properName>
        <otv:language>el</otv:language>
        <otv:denotedObject rdf:resource="#7th_century_BCE"/>
    </otv:ProperName>

    <otv:ProperName rdf:about="#Επίνικοι_του_Πινδάρου_el">
        <otv:properName>Επίνικοι του Πινδάρου</otv:properName>
        <otv:language>el</otv:language>
        <otv:denotedObject rdf:resource="#epinikoi_pindarus"/>
    </otv:ProperName>

    <otv:ProperName rdf:about="#Ερωτικές_ωδές_του_Αλκαίου_el">
        <otv:properName>Ερωτικές ωδές του Αλκαίου</otv:properName>
        <otv:language>el</otv:language>
        <otv:denotedObject rdf:resource="#erotic_odes_alcaeus"/>
    </otv:ProperName>

    <otv:ProperName rdf:about="#Επίνικοι_του_Σιμωνίδη_από_την_Κέα_el">
        <otv:properName>Επίνικοι του Σιμωνίδη από την Κέα</otv:properName>
        <otv:language>el</otv:language>
        <otv:denotedObject rdf:resource="#epinikoi_simonides"/>
    </otv:ProperName>

    <otv:ProperName rdf:about="#Ύμνοι_του_Τέρπανδρου_el">
        <otv:properName>Ύμνοι του Τέρπανδρου</otv:properName>
        <otv:language>el</otv:language>
        <otv:denotedObject rdf:resource="#hymns_terpander"/>
    </otv:ProperName>

    <otv:ProperName rdf:about="#Επιθαλάμια_της_Σαπφούς_της_Λεσβίας_el">
        <otv:properName>Επιθαλάμια της Σαπφούς της Λεσβίας</otv:properName>
        <otv:language>el</otv:language>
        <otv:denotedObject rdf:resource="#epithalamia_sappho"/>
    </otv:ProperName>

    <otv:ProperName rdf:about="#Κολοφώνα_el">
        <otv:properName>Κολοφώνα</otv:properName>
        <otv:language>el</otv:language>
        <otv:denotedObject rdf:resource="#colophon"/>
    </otv:ProperName>

    <otv:ProperName rdf:about="#Παρθένεια_του_Πινδάρου_el">
        <otv:properName>Παρθένεια του Πινδάρου</otv:properName>
        <otv:language>el</otv:language>
        <otv:denotedObject rdf:resource="#partheneia_pindarus"/>
    </otv:ProperName>

    <otv:ProperName rdf:about="#Μέγαρα_el">
        <otv:properName>Μέγαρα</otv:properName>
        <otv:language>el</otv:language>
        <otv:denotedObject rdf:resource="#megara"/>
    </otv:ProperName>

    <otv:ProperName rdf:about="#Αλκμάνας_ο_Λακεδαιμόνιος_el">
        <otv:properName>Αλκμάνας ο Λακεδαιμόνιος</otv:properName>
        <otv:language>el</otv:language>
        <otv:denotedObject rdf:resource="#alcman_lacedaemonius"/>
    </otv:ProperName>

    <otv:ProperName rdf:about="#Χορική_ποίηση_του_Στησίχορου_από_την_Ιμέρα_el">
        <otv:properName>Χορική ποίηση του Στησίχορου από την Ιμέρα</otv:properName>
        <otv:language>el</otv:language>
        <otv:denotedObject rdf:resource="#choral_stesichorus"/>
    </otv:ProperName>

    <otv:ProperName rdf:about="#Ερωτικές_ωδές_του_Ανακρέοντα_el">
        <otv:properName>Ερωτικές ωδές του Ανακρέοντα</otv:properName>
        <otv:language>el</otv:language>
        <otv:denotedObject rdf:resource="#erotic_odes_anacreon"/>
    </otv:ProperName>

    <otv:ProperName rdf:about="#Ιμέρα_el">
        <otv:properName>Ιμέρα</otv:properName>
        <otv:language>el</otv:language>
        <otv:denotedObject rdf:resource="#himera"/>
    </otv:ProperName>

    <otv:ProperName rdf:about="#Γνωμικές_ελεγείες_του_Θέογνη_el">
        <otv:properName>Γνωμικές ελεγείες του Θέογνη</otv:properName>
        <otv:language>el</otv:language>
        <otv:denotedObject rdf:resource="#gnomic_elegies_theognis"/>
    </otv:ProperName>

    <otv:ProperName rdf:about="#Ελεγείες_του_Αρχιλόχου_του_Πάριου_el">
        <otv:properName>Ελεγείες του Αρχιλόχου του Πάριου</otv:properName>
        <otv:language>el</otv:language>
        <otv:denotedObject rdf:resource="#elegies_archilochus"/>
    </otv:ProperName>

    <otv:ProperName rdf:about="#Ίαμβοι_του_Ιππώνακτα_el">
        <otv:properName>Ίαμβοι του Ιππώνακτα</otv:properName>
        <otv:language>el</otv:language>
        <otv:denotedObject rdf:resource="#iambs_hipponax"/>
    </otv:ProperName>

    <otv:ProperName rdf:about="#Ύμνοι_του_Ανακρέοντα_el">
        <otv:properName>Ύμνοι του Ανακρέοντα</otv:properName>
        <otv:language>el</otv:language>
        <otv:denotedObject rdf:resource="#hymns_anacreon"/>
    </otv:ProperName>

    <otv:ProperName rdf:about="#Σαπφώ_η_Λεσβία_el">
        <otv:properName>Σαπφώ η Λεσβία</otv:properName>
        <otv:language>el</otv:language>
        <otv:denotedObject rdf:resource="#sappho_lesbia"/>
    </otv:ProperName>

    <otv:ProperName rdf:about="#Ίαμβοι_του_Αρχιλόχου_el">
        <otv:properName>Ίαμβοι του Αρχιλόχου</otv:properName>
        <otv:language>el</otv:language>
        <otv:denotedObject rdf:resource="#iambs_archilochus"/>
    </otv:ProperName>

    <otv:ProperName rdf:about="#Πίνδαρος_ο_Λυρικός_el">
        <otv:properName>Πίνδαρος ο Λυρικός</otv:properName>
        <otv:language>el</otv:language>
        <otv:denotedObject rdf:resource="#pindarus_boeotus"/>
    </otv:ProperName>

    <otv:ProperName rdf:about="#Μίμνερμος_από_την_Κολοφώνα_el">
        <otv:properName>Μίμνερμος από την Κολοφώνα</otv:properName>
        <otv:language>el</otv:language>
        <otv:denotedObject rdf:resource="#mimnermus_lyricus"/>
    </otv:ProperName>

    <otv:ProperName rdf:about="#Ιππώναξ_ο_Ιαμβογράφος_el">
        <otv:properName>Ιππώναξ ο Ιαμβογράφος</otv:properName>
        <otv:language>el</otv:language>
        <otv:denotedObject rdf:resource="#hipponax_ephesius"/>
    </otv:ProperName>

    <otv:ProperName rdf:about="#Ύμνοι_του_Αρχιλόχου_el">
        <otv:properName>Ύμνοι του Αρχιλόχου</otv:properName>
        <otv:language>el</otv:language>
        <otv:denotedObject rdf:resource="#hymns_archilochus"/>
    </otv:ProperName>

    <otv:ProperName rdf:about="#Σιμωνίδης_από_την_Κέα_el">
        <otv:properName>Σιμωνίδης από την Κέα</otv:properName>
        <otv:language>el</otv:language>
        <otv:denotedObject rdf:resource="#simonides_ceus"/>
    </otv:ProperName>

    <otv:ProperName rdf:about="#Συμποτικές_ωδές_του_Αλκαίου_el">
        <otv:properName>Συμποτικές ωδές του Αλκαίου</otv:properName>
        <otv:language>el</otv:language>
        <otv:denotedObject rdf:resource="#sympotic_odes_alcaeus"/>
    </otv:ProperName>

    <otv:ProperName rdf:about="#Εγκωμιαστική_ποίηση_του_Βακχυλίδη_el">
        <otv:properName>Εγκωμιαστική ποίηση του Βακχυλίδη</otv:properName>
        <otv:language>el</otv:language>
        <otv:denotedObject rdf:resource="#enkomion_bacchylides"/>
    </otv:ProperName>

    <otv:ProperName rdf:about="#Τέρπανδρος_ο_Λέσβιος_el">
        <otv:properName>Τέρπανδρος ο Λέσβιος</otv:properName>
        <otv:language>el</otv:language>
        <otv:denotedObject rdf:resource="#terpander_lesbius"/>
    </otv:ProperName>

    <otv:ProperName rdf:about="#Υπορχήματα_του_Πινδάρου_el">
        <otv:properName>Υπορχήματα του Πινδάρου</otv:properName>
        <otv:language>el</otv:language>
        <otv:denotedObject rdf:resource="#hyporchemes_pindarus"/>
    </otv:ProperName>

    <otv:ProperName rdf:about="#Φωκυλίδης_ο_Μιλήσιος_el">
        <otv:properName>Φωκυλίδης ο Μιλήσιος</otv:properName>
        <otv:language>el</otv:language>
        <otv:denotedObject rdf:resource="#phocylides_milesius"/>
    </otv:ProperName>

    <otv:ProperName rdf:about="#Ερωτική_ποίηση_του_Αλκμάνα_el">
        <otv:properName>Ερωτική ποίηση του Αλκμάνα</otv:properName>
        <otv:language>el</otv:language>
        <otv:denotedObject rdf:resource="#erotic_odes_alcman"/>
    </otv:ProperName>

    <otv:ProperName rdf:about="#Προσόδια_του_Αλκμάνα_el">
        <otv:properName>Προσόδια του Αλκμάνα</otv:properName>
        <otv:language>el</otv:language>
        <otv:denotedObject rdf:resource="#prosodia_alcman"/>
    </otv:ProperName>

    <otv:ProperName rdf:about="#Πίνδαρος_el">
        <otv:properName>Πίνδαρος</otv:properName>
        <otv:language>el</otv:language>
        <otv:denotedObject rdf:resource="#pindarus_boeotus"/>
    </otv:ProperName>

    <otv:ProperName rdf:about="#Ακράγας_el">
        <otv:properName>Ακράγας</otv:properName>
        <otv:language>el</otv:language>
        <otv:denotedObject rdf:resource="#akragas"/>
    </otv:ProperName>

    <otv:ProperName rdf:about="#Βοιωτία_el">
        <otv:properName>Βοιωτία</otv:properName>
        <otv:language>el</otv:language>
        <otv:denotedObject rdf:resource="#boeotia"/>
    </otv:ProperName>

    <otv:ProperName rdf:about="#Ανακρέων_ο_Λυρικός_el">
        <otv:properName>Ανακρέων ο Λυρικός</otv:properName>
        <otv:language>el</otv:language>
        <otv:denotedObject rdf:resource="#anacreon_teius"/>
    </otv:ProperName>

    <otv:ProperName rdf:about="#Ελεγείες_του_Ανακρέοντα_του_Τηίου_el">
        <otv:properName>Ελεγείες του Ανακρέοντα του Τηίου</otv:properName>
        <otv:language>el</otv:language>
        <otv:denotedObject rdf:resource="#elegies_anacreon"/>
    </otv:ProperName>

    <otv:ProperName rdf:about="#Παιάνες_του_Βακχυλίδη_el">
        <otv:properName>Παιάνες του Βακχυλίδη</otv:properName>
        <otv:language>el</otv:language>
        <otv:denotedObject rdf:resource="#paeans_bacchylides"/>
    </otv:ProperName>

    <otv:ProperName rdf:about="#5ος_αιώνας_π.Χ._el">
        <otv:properName>5ος αιώνας π.Χ.</otv:properName>
        <otv:language>el</otv:language>
        <otv:denotedObject rdf:resource="#5th_century_BCE"/>
    </otv:ProperName>

    <otv:ProperName rdf:about="#Σπάρτη_el">
        <otv:properName>Σπάρτη</otv:properName>
        <otv:language>el</otv:language>
        <otv:denotedObject rdf:resource="#sparta"/>
    </otv:ProperName>

    <otv:ProperName rdf:about="#Σιμωνίδης_ο_Λυρικός_el">
        <otv:properName>Σιμωνίδης ο Λυρικός</otv:properName>
        <otv:language>el</otv:language>
        <otv:denotedObject rdf:resource="#simonides_ceus"/>
    </otv:ProperName>

    <otv:ProperName rdf:about="#Σικελία_el">
        <otv:properName>Σικελία</otv:properName>
        <otv:language>el</otv:language>
        <otv:denotedObject rdf:resource="#sicilia"/>
    </otv:ProperName>

    <otv:ProperName rdf:about="#Υμέναιοι_της_Σαπφούς_el">
        <otv:properName>Υμέναιοι της Σαπφούς</otv:properName>
        <otv:language>el</otv:language>
        <otv:denotedObject rdf:resource="#hymenaios_sappho"/>
    </otv:ProperName>

    <otv:ProperName rdf:about="#Ίβυκος_ο_Ρηγίνος_el">
        <otv:properName>Ίβυκος ο Ρηγίνος</otv:properName>
        <otv:language>el</otv:language>
        <otv:denotedObject rdf:resource="#ibycus_rheginus"/>
    </otv:ProperName>

    <otv:ProperName rdf:about="#Ανάνιος_ο_Λυρικός_el">
        <otv:properName>Ανάνιος ο Λυρικός</otv:properName>
        <otv:language>el</otv:language>
        <otv:denotedObject rdf:resource="#ananius_iambographus"/>
    </otv:ProperName>

    <otv:ProperName rdf:about="#Σάρδεις_el">
        <otv:properName>Σάρδεις</otv:properName>
        <otv:language>el</otv:language>
        <otv:denotedObject rdf:resource="#sardis"/>
    </otv:ProperName>

    <otv:ProperName rdf:about="#Ύμνοι_του_Αλκαίου_el">
        <otv:properName>Ύμνοι του Αλκαίου</otv:properName>
        <otv:language>el</otv:language>
        <otv:denotedObject rdf:resource="#hymns_alcaeus"/>
    </otv:ProperName>

    <otv:ProperName rdf:about="#Αλκαίος_ο_Λυρικός_el">
        <otv:properName>Αλκαίος ο Λυρικός</otv:properName>
        <otv:language>el</otv:language>
        <otv:denotedObject rdf:resource="#alcaeus_lesbius"/>
    </otv:ProperName>

    <otv:ProperName rdf:about="#Ρήγιο_el">
        <otv:properName>Ρήγιο</otv:properName>
        <otv:language>el</otv:language>
        <otv:denotedObject rdf:resource="#rhegium"/>
    </otv:ProperName>

    <otv:ProperName rdf:about="#Προσόδια_του_Πινδάρου_el">
        <otv:properName>Προσόδια του Πινδάρου</otv:properName>
        <otv:language>el</otv:language>
        <otv:denotedObject rdf:resource="#prosodia_pindarus"/>
    </otv:ProperName>

    <otv:ProperName rdf:about="#Θάσος-αποικία_el">
        <otv:properName>Θάσος-αποικία</otv:properName>
        <otv:language>el</otv:language>
        <otv:denotedObject rdf:resource="#thasos_settlement"/>
    </otv:ProperName>

    <otv:ProperName rdf:about="#Προσόδια_του_Βακχυλίδη_el">
        <otv:properName>Προσόδια του Βακχυλίδη</otv:properName>
        <otv:language>el</otv:language>
        <otv:denotedObject rdf:resource="#prosodia_bacchylides"/>
    </otv:ProperName>

    <otv:ProperName rdf:about="#Τυρταίος_ο_Λακεδαιμόνιος_el">
        <otv:properName>Τυρταίος ο Λακεδαιμόνιος</otv:properName>
        <otv:language>el</otv:language>
        <otv:denotedObject rdf:resource="#tyrtaeus_lacedaemonius"/>
    </otv:ProperName>

    <otv:ProperName rdf:about="#Αίγυπτος_el">
        <otv:properName>Αίγυπτος</otv:properName>
        <otv:language>el</otv:language>
        <otv:denotedObject rdf:resource="#aegypt"/>
    </otv:ProperName>

	<!--  OTV Individuals -->

    <otv:Object rdf:about="#elegies_simonides">
        <otv:instanceOf rdf:resource="#Archaic_Lyric_Poem_only_in_ionic_dialect_in_elegiac_couplet"/>
        <otv:denotedByProperName rdf:resource="#Elegies_of_Simonides_Ceus_en"/>
        <otv:denotedByProperName rdf:resource="#Ελεγείες_του_Σιμωνίδη_από_την_Κέα_el"/>
    </otv:Object>

    <otv:Object rdf:about="#erotic_odes_alcman">
        <otv:instanceOf rdf:resource="#Archaic_Lyric_Poem_in_ionic_or_in_doric_or_in_aeolic_dialect_performed_by_a_single_performer"/>
        <otv:denotedByProperName rdf:resource="#Erotic_poetry_of_Alcman_Lacedaemonius_en"/>
        <otv:denotedByProperName rdf:resource="#Ερωτική_ποίηση_του_Αλκμάνα_el"/>
    </otv:Object>

    <otv:Object rdf:about="#threnoi_anacreon">
        <otv:instanceOf rdf:resource="#Archaic_Lyric_Poem_in_ionic_or_in_doric_or_in_aeolic_dialect_performed_by_a_chorus_or_by_a_single_performer_dedicated_to_dead"/>
        <otv:denotedByProperName rdf:resource="#Threnoi_of_Anacreon_Teius_en"/>
        <otv:denotedByProperName rdf:resource="#Θρήνοι_του_Ανακρέοντα_el"/>
    </otv:Object>

    <otv:Object rdf:about="#partheneia_pindarus">
        <otv:instanceOf rdf:resource="#Archaic_Lyric_Poem_in_ionic_or_in_doric_or_in_aeolic_dialect_performed_by_a_chorus_performed_by_a_maidens_chorus"/>
        <otv:denotedByProperName rdf:resource="#Partheneia_of_Pindarus_Boeotus_en"/>
        <otv:denotedByProperName rdf:resource="#Παρθένεια_του_Πινδάρου_el"/>
    </otv:Object>

    <otv:Object rdf:about="#war_elegies_tyrtaeus">
        <otv:instanceOf rdf:resource="#Archaic_Lyric_Poem_only_in_ionic_dialect_in_elegiac_couplet_with_war_content"/>
        <otv:denotedByProperName rdf:resource="#War_elegies_of_Tyrtaeus_Lacedaemonius_en"/>
        <otv:denotedByProperName rdf:resource="#Πολεμικές_ελεγείες_του_Τυρταίου_el"/>
    </otv:Object>

    <otv:Object rdf:about="#callinus_ephesius">
        <otv:instanceOf rdf:resource="#Archaic_Lyric_Poet"/>
        <otv:denotedByProperName rdf:resource="#Callinus_Ephesius_en"/>
        <otv:denotedByProperName rdf:resource="#Καλλίνος_ο_Εφέσιος_el"/>
    </otv:Object>

    <otv:Object rdf:about="#archilochus_parius">
        <otv:instanceOf rdf:resource="#Archaic_Lyric_Poet"/>
        <otv:denotedByProperName rdf:resource="#Archilochus_Parius_en"/>
        <otv:denotedByProperName rdf:resource="#Archilochus_Lyricus_en"/>
        <otv:denotedByProperName rdf:resource="#Archilochus_of_Paros_en"/>
        <otv:denotedByProperName rdf:resource="#Archilochus_Iamb._et_Eleg._en"/>
        <otv:denotedByProperName rdf:resource="#Αρχίλοχος_ο_Πάριος_el"/>
    </otv:Object>

    <otv:Object rdf:about="#sappho_lesbia">
        <otv:instanceOf rdf:resource="#Archaic_Lyric_Poetess"/>
        <otv:denotedByProperName rdf:resource="#Sappho_Lesbia_en"/>
        <otv:denotedByProperName rdf:resource="#Sappho_Lyrica_en"/>
        <otv:denotedByProperName rdf:resource="#Sapphus_en"/>
        <otv:denotedByProperName rdf:resource="#Σαπφώ_el"/>
        <otv:denotedByProperName rdf:resource="#Σαπφώ_η_Λεσβία_el"/>
    </otv:Object>

    <otv:Object rdf:about="#anacreon_teius">
        <otv:instanceOf rdf:resource="#Archaic_Lyric_Poet"/>
        <otv:denotedByProperName rdf:resource="#Anacreon_Teius_en"/>
        <otv:denotedByProperName rdf:resource="#Anacreon_Lyricus_en"/>
        <otv:denotedByProperName rdf:resource="#Ανακρέων_ο_Λυρικός_el"/>
        <otv:denotedByProperName rdf:resource="#Ανακρέων_ο_Τήιος_el"/>
    </otv:Object>

    <otv:Object rdf:about="#erotic_odes_alcaeus">
        <otv:instanceOf rdf:resource="#Archaic_Lyric_Poem_in_ionic_or_in_doric_or_in_aeolic_dialect_performed_by_a_single_performer"/>
        <otv:denotedByProperName rdf:resource="#Erotic_odes_of_Alcaeus_Lesbius_en"/>
        <otv:denotedByProperName rdf:resource="#Ερωτικές_ωδές_του_Αλκαίου_el"/>
    </otv:Object>

    <otv:Object rdf:about="#mimnermus_lyricus">
        <otv:instanceOf rdf:resource="#Archaic_Lyric_Poet"/>
        <otv:denotedByProperName rdf:resource="#Mimnermus_Lyricus_en"/>
        <otv:denotedByProperName rdf:resource="#Mimnermo_of_Colophon_en"/>
        <otv:denotedByProperName rdf:resource="#Μίμνερμος_από_την_Κολοφώνα_el"/>
        <otv:denotedByProperName rdf:resource="#Μίμνερμος_ο_Λυρικός_el"/>
    </otv:Object>

    <otv:Object rdf:about="#7th_century_BCE">
        <otv:instanceOf rdf:resource="#BCE_century"/>
        <otv:denotedByProperName rdf:resource="#7th_century_BCE_en"/>
        <otv:denotedByProperName rdf:resource="#7ος_αιώνας_π.Χ._el"/>
    </otv:Object>

    <otv:Object rdf:about="#enkomion_pindarus">
        <otv:instanceOf rdf:resource="#Archaic_Lyric_Poem_in_ionic_or_in_doric_or_in_aeolic_dialect_performed_by_a_chorus_or_by_a_single_performer_dedicated_to_living"/>
        <otv:denotedByProperName rdf:resource="#Enkomion_of_Pindarus_Boeotus_en"/>
        <otv:denotedByProperName rdf:resource="#Εγκωμιαστική_ποίηση_του_Πινδάρου_el"/>
    </otv:Object>

    <otv:Object rdf:about="#erotic_odes_anacreon">
        <otv:instanceOf rdf:resource="#Archaic_Lyric_Poem_in_ionic_or_in_doric_or_in_aeolic_dialect_performed_by_a_single_performer"/>
        <otv:denotedByProperName rdf:resource="#Erotic_odes_of_Anacreon_Teius_en"/>
        <otv:denotedByProperName rdf:resource="#Ερωτικές_ωδές_του_Ανακρέοντα_el"/>
    </otv:Object>

    <otv:Object rdf:about="#smyrna">
        <otv:instanceOf rdf:resource="#Ancient_Location"/>
        <otv:denotedByProperName rdf:resource="#Smyrna_en"/>
        <otv:denotedByProperName rdf:resource="#Σμύρνη_el"/>
    </otv:Object>

    <otv:Object rdf:about="#partheneia_alcman">
        <otv:instanceOf rdf:resource="#Archaic_Lyric_Poem_in_ionic_or_in_doric_or_in_aeolic_dialect_performed_by_a_chorus_performed_by_a_maidens_chorus"/>
        <otv:denotedByProperName rdf:resource="#Partheneia_of_Alcman_Lacedaemonius_en"/>
        <otv:denotedByProperName rdf:resource="#Παρθένεια_του_Αλκμάνα_el"/>
    </otv:Object>

    <otv:Object rdf:about="#akragas">
        <otv:instanceOf rdf:resource="#Ancient_Location"/>
        <otv:denotedByProperName rdf:resource="#Akragas_en"/>
        <otv:denotedByProperName rdf:resource="#Ακράγας_el"/>
    </otv:Object>

    <otv:Object rdf:about="#paeans_bacchylides">
        <otv:instanceOf rdf:resource="#Archaic_Lyric_Poem_in_ionic_or_in_doric_or_in_aeolic_dialect_performed_by_a_chorus_or_by_a_single_performer_dedicated_to_apollo"/>
        <otv:denotedByProperName rdf:resource="#Paeans_of_Bacchylides_Ceus_en"/>
        <otv:denotedByProperName rdf:resource="#Παιάνες_του_Βακχυλίδη_el"/>
    </otv:Object>

    <otv:Object rdf:about="#iambs_hipponax">
        <otv:instanceOf rdf:resource="#Archaic_Lyric_Poem_only_in_ionic_dialect_in_iambic_or_trochaic_metre"/>
        <otv:denotedByProperName rdf:resource="#Iambs_of_Hipponax_Ephesius_en"/>
        <otv:denotedByProperName rdf:resource="#Ίαμβοι_του_Ιππώνακτα_el"/>
    </otv:Object>

    <otv:Object rdf:about="#alcman_lacedaemonius">
        <otv:instanceOf rdf:resource="#Archaic_Lyric_Poet"/>
        <otv:denotedByProperName rdf:resource="#Alcman_Lacedaemonius_en"/>
        <otv:denotedByProperName rdf:resource="#Alcman_Lyricus_en"/>
        <otv:denotedByProperName rdf:resource="#Αλκμάν_el"/>
        <otv:denotedByProperName rdf:resource="#Αλκμάνας_ο_Λακεδαιμόνιος_el"/>
        <otv:denotedByProperName rdf:resource="#Αλκμάνας_ο_Λυρικός_el"/>
    </otv:Object>

    <otv:Object rdf:about="#miletus">
        <otv:instanceOf rdf:resource="#Ancient_Location"/>
        <otv:denotedByProperName rdf:resource="#Miletus_en"/>
        <otv:denotedByProperName rdf:resource="#Μίλητος_el"/>
    </otv:Object>

    <otv:Object rdf:about="#enkomion_ibycus">
        <otv:instanceOf rdf:resource="#Archaic_Lyric_Poem_in_ionic_or_in_doric_or_in_aeolic_dialect_performed_by_a_chorus_or_by_a_single_performer_dedicated_to_living"/>
        <otv:denotedByProperName rdf:resource="#Enkomion_of_Ibycus_Rheginus_en"/>
        <otv:denotedByProperName rdf:resource="#Εγκωμιαστική_ποίηση_του_Ιβύκου_el"/>
    </otv:Object>

    <otv:Object rdf:about="#colophon">
        <otv:instanceOf rdf:resource="#Ancient_Location"/>
        <otv:denotedByProperName rdf:resource="#Colophon_en"/>
        <otv:denotedByProperName rdf:resource="#Κολοφώνα_el"/>
    </otv:Object>

    <otv:Object rdf:about="#epinikoi_simonides">
        <otv:instanceOf rdf:resource="#Archaic_Lyric_Poem_in_ionic_or_in_doric_or_in_aeolic_dialect_performed_by_a_chorus_or_by_a_single_performer_dedicated_to_winners_in_athletic_events"/>
        <otv:denotedByProperName rdf:resource="#Epinikoi_of_Simonides_Ceus_en"/>
        <otv:denotedByProperName rdf:resource="#Επίνικοι_του_Σιμωνίδη_από_την_Κέα_el"/>
    </otv:Object>

    <otv:Object rdf:about="#amorgos">
        <otv:instanceOf rdf:resource="#Ancient_Location"/>
        <otv:denotedByProperName rdf:resource="#Amorgos_en"/>
        <otv:denotedByProperName rdf:resource="#Αμοργός_el"/>
    </otv:Object>

    <otv:Object rdf:about="#paros">
        <otv:instanceOf rdf:resource="#Ancient_Location"/>
        <otv:denotedByProperName rdf:resource="#Paros_en"/>
        <otv:denotedByProperName rdf:resource="#Πάρος_el"/>
    </otv:Object>

    <otv:Object rdf:about="#alcaeus_lesbius">
        <otv:instanceOf rdf:resource="#Archaic_Lyric_Poet"/>
        <otv:denotedByProperName rdf:resource="#Alcaeus_Lesbius_en"/>
        <otv:denotedByProperName rdf:resource="#Alcaeus_Lyricus_en"/>
        <otv:denotedByProperName rdf:resource="#Alcaeus_Mytilenaeus_en"/>
        <otv:denotedByProperName rdf:resource="#Alcaeus_Mytilenensis_en"/>
        <otv:denotedByProperName rdf:resource="#Αλκαίος_ο_Λέσβιος_el"/>
        <otv:denotedByProperName rdf:resource="#Αλκαίος_ο_Λυρικός_el"/>
        <otv:denotedByProperName rdf:resource="#Αλκαίος_ο_Μυτιληναίος_el"/>
    </otv:Object>

    <otv:Object rdf:about="#gnomic_elegies_phocylides">
        <otv:instanceOf rdf:resource="#Archaic_Lyric_Poem_only_in_ionic_dialect_in_elegiac_couplet_with_gnomic_content"/>
        <otv:denotedByProperName rdf:resource="#Gnomic_elegies_of_Phocylides_Milesius_en"/>
        <otv:denotedByProperName rdf:resource="#Γνωμικές_ελεγείς_του_Φωκυλίδη_el"/>
    </otv:Object>

    <otv:Object rdf:about="#boeotia">
        <otv:instanceOf rdf:resource="#Ancient_Location"/>
        <otv:denotedByProperName rdf:resource="#Boeotia_en"/>
        <otv:denotedByProperName rdf:resource="#Βοιωτία_el"/>
    </otv:Object>

    <otv:Object rdf:about="#prosodia_alcman">
        <otv:instanceOf rdf:resource="#Archaic_Lyric_Poem_in_ionic_or_in_doric_or_in_aeolic_dialect_performed_by_a_chorus_on_the_way_to_an_altar"/>
        <otv:denotedByProperName rdf:resource="#Prosodia_of_Alcman_Lacedaemonius_en"/>
        <otv:denotedByProperName rdf:resource="#Προσόδια_του_Αλκμάνα_el"/>
    </otv:Object>

    <otv:Object rdf:about="#threnoi_pindarus">
        <otv:instanceOf rdf:resource="#Archaic_Lyric_Poem_in_ionic_or_in_doric_or_in_aeolic_dialect_performed_by_a_chorus_or_by_a_single_performer_dedicated_to_dead"/>
        <otv:denotedByProperName rdf:resource="#Threnoi_of_Pindarus_Boeotus_en"/>
        <otv:denotedByProperName rdf:resource="#Θρήνοι_του_Πινδάρου_el"/>
    </otv:Object>

    <otv:Object rdf:about="#lesbos">
        <otv:instanceOf rdf:resource="#Ancient_Location"/>
        <otv:denotedByProperName rdf:resource="#Lesbos_en"/>
        <otv:denotedByProperName rdf:resource="#Λέσβος_el"/>
    </otv:Object>

    <otv:Object rdf:about="#solon_atheniensis">
        <otv:instanceOf rdf:resource="#Archaic_Lyric_Poet"/>
        <otv:denotedByProperName rdf:resource="#Solon_Atheniensis_en"/>
        <otv:denotedByProperName rdf:resource="#Σόλων_ο_Αθηναίος_el"/>
    </otv:Object>

    <otv:Object rdf:about="#prosodia_bacchylides">
        <otv:instanceOf rdf:resource="#Archaic_Lyric_Poem_in_ionic_or_in_doric_or_in_aeolic_dialect_performed_by_a_chorus_on_the_way_to_an_altar"/>
        <otv:denotedByProperName rdf:resource="#Prosodia_of_Bacchylides_Ceus_en"/>
        <otv:denotedByProperName rdf:resource="#Προσόδια_του_Βακχυλίδη_el"/>
    </otv:Object>

    <otv:Object rdf:about="#klazomenai">
        <otv:instanceOf rdf:resource="#Ancient_Location"/>
        <otv:denotedByProperName rdf:resource="#Klazomenai_en"/>
        <otv:denotedByProperName rdf:resource="#Κλαζομενές_el"/>
    </otv:Object>

    <otv:Object rdf:about="#phocylides_milesius">
        <otv:instanceOf rdf:resource="#Archaic_Lyric_Poet"/>
        <otv:denotedByProperName rdf:resource="#Phocylides_Milesius_en"/>
        <otv:denotedByProperName rdf:resource="#Phocylides_of_Miletus_en"/>
        <otv:denotedByProperName rdf:resource="#Phocylides_Lyricus_en"/>
        <otv:denotedByProperName rdf:resource="#Φωκυλίδης_ο_Λυρικός_el"/>
        <otv:denotedByProperName rdf:resource="#Φωκυλίδης_ο_Μιλήσιος_el"/>
        <otv:denotedByProperName rdf:resource="#Φωκυλίδης_από_τη_Μίλητο_el"/>
    </otv:Object>

    <otv:Object rdf:about="#elegies_anacreon">
        <otv:instanceOf rdf:resource="#Archaic_Lyric_Poem_only_in_ionic_dialect_in_elegiac_couplet"/>
        <otv:denotedByProperName rdf:resource="#Elegies_of_Anacreon_Teius_en"/>
        <otv:denotedByProperName rdf:resource="#Ελεγείες_του_Ανακρέοντα_του_Τηίου_el"/>
    </otv:Object>

    <otv:Object rdf:about="#sparta">
        <otv:instanceOf rdf:resource="#Ancient_Location"/>
        <otv:denotedByProperName rdf:resource="#Sparta_en"/>
        <otv:denotedByProperName rdf:resource="#Σπάρτη_el"/>
    </otv:Object>

    <otv:Object rdf:about="#megara">
        <otv:instanceOf rdf:resource="#Ancient_Location"/>
        <otv:denotedByProperName rdf:resource="#Megara_en"/>
        <otv:denotedByProperName rdf:resource="#Μέγαρα_el"/>
    </otv:Object>

    <otv:Object rdf:about="#sicilia">
        <otv:instanceOf rdf:resource="#Ancient_Location"/>
        <otv:denotedByProperName rdf:resource="#Sicilia_en"/>
        <otv:denotedByProperName rdf:resource="#Σικελία_el"/>
    </otv:Object>

    <otv:Object rdf:about="#enkomion_bacchylides">
        <otv:instanceOf rdf:resource="#Archaic_Lyric_Poem_in_ionic_or_in_doric_or_in_aeolic_dialect_performed_by_a_chorus_or_by_a_single_performer_dedicated_to_living"/>
        <otv:denotedByProperName rdf:resource="#Enkomion_of_Bacchylides_Ceus_en"/>
        <otv:denotedByProperName rdf:resource="#Εγκωμιαστική_ποίηση_του_Βακχυλίδη_el"/>
    </otv:Object>

    <otv:Object rdf:about="#paeans_pindarus">
        <otv:instanceOf rdf:resource="#Archaic_Lyric_Poem_in_ionic_or_in_doric_or_in_aeolic_dialect_performed_by_a_chorus_or_by_a_single_performer_dedicated_to_apollo"/>
        <otv:denotedByProperName rdf:resource="#Paeans_of_Pindarus_Boeotus_en"/>
        <otv:denotedByProperName rdf:resource="#Παιάνες_του_Πινδάρου_el"/>
    </otv:Object>

    <otv:Object rdf:about="#choral_ibycus">
        <otv:instanceOf rdf:resource="#Archaic_Lyric_Poem_in_ionic_or_in_doric_or_in_aeolic_dialect_performed_by_a_chorus"/>
        <otv:denotedByProperName rdf:resource="#Choral_songs_of_Ibycus_Rheginus_en"/>
        <otv:denotedByProperName rdf:resource="#Χορική_ποίηση_του_Ίβυκου_του_Ρηγίνου_el"/>
    </otv:Object>

    <otv:Object rdf:about="#elegies_archilochus">
        <otv:instanceOf rdf:resource="#Archaic_Lyric_Poem_only_in_ionic_dialect_in_elegiac_couplet"/>
        <otv:denotedByProperName rdf:resource="#Elegies_of_Archilochus_Parius_en"/>
        <otv:denotedByProperName rdf:resource="#Ελεγείες_του_Αρχιλόχου_του_Πάριου_el"/>
    </otv:Object>

    <otv:Object rdf:about="#dithyrambs_simonides">
        <otv:instanceOf rdf:resource="#Archaic_Lyric_Poem_in_ionic_or_in_doric_or_in_aeolic_dialect_performed_by_a_chorus_or_by_a_single_performer_dedicated_to_dionysus"/>
        <otv:denotedByProperName rdf:resource="#Dithyrambs_of_Simonides_Ceus_en"/>
        <otv:denotedByProperName rdf:resource="#Διθύραμβοι_του_Σιμωνίδη_του_Κείου_el"/>
    </otv:Object>

    <otv:Object rdf:about="#pindarus_boeotus">
        <otv:instanceOf rdf:resource="#Archaic_Lyric_Poet"/>
        <otv:denotedByProperName rdf:resource="#Pindarus_Boeotus_en"/>
        <otv:denotedByProperName rdf:resource="#Pindar_en"/>
        <otv:denotedByProperName rdf:resource="#Pindarus_Lyricus_en"/>
        <otv:denotedByProperName rdf:resource="#Pindarus_en"/>
        <otv:denotedByProperName rdf:resource="#Πίνδαρος_el"/>
        <otv:denotedByProperName rdf:resource="#Πίνδαρος_από_τη_Βοιωτία_el"/>
        <otv:denotedByProperName rdf:resource="#Πίνδαρος_ο_Βοιωτός_el"/>
        <otv:denotedByProperName rdf:resource="#Πίνδαρος_ο_Λυρικός_el"/>
    </otv:Object>

    <otv:Object rdf:about="#threnoi_simonides">
        <otv:instanceOf rdf:resource="#Archaic_Lyric_Poem_in_ionic_or_in_doric_or_in_aeolic_dialect_performed_by_a_chorus_or_by_a_single_performer_dedicated_to_dead"/>
        <otv:denotedByProperName rdf:resource="#Threnoi_of_Simonides_Ceus_en"/>
        <otv:denotedByProperName rdf:resource="#Θρήνοι_του_Σιμωνίδη_από_την_Κέα_el"/>
    </otv:Object>

    <otv:Object rdf:about="#political_elegies_solon">
        <otv:instanceOf rdf:resource="#Archaic_Lyric_Poem_only_in_ionic_dialect_in_elegiac_couplet_with_political_content"/>
        <otv:denotedByProperName rdf:resource="#Political_elegy_of_Solon_Athenienis_en"/>
        <otv:denotedByProperName rdf:resource="#Πολιτική_ελεγεία_του_Σόλωνα_el"/>
    </otv:Object>

    <otv:Object rdf:about="#partheneia_bacchylides">
        <otv:instanceOf rdf:resource="#Archaic_Lyric_Poem_in_ionic_or_in_doric_or_in_aeolic_dialect_performed_by_a_chorus_performed_by_a_maidens_chorus"/>
        <otv:denotedByProperName rdf:resource="#Partheneia_of_Bacchylides_Ceus_en"/>
        <otv:denotedByProperName rdf:resource="#Παρθένεια_του_Βακχυλίδη_el"/>
    </otv:Object>

    <otv:Object rdf:about="#iambs_archilochus">
        <otv:instanceOf rdf:resource="#Archaic_Lyric_Poem_only_in_ionic_dialect_in_iambic_or_trochaic_metre"/>
        <otv:denotedByProperName rdf:resource="#Iambs_of_Archilochus_Parius_en"/>
        <otv:denotedByProperName rdf:resource="#Ίαμβοι_του_Αρχιλόχου_el"/>
    </otv:Object>

    <otv:Object rdf:about="#keos">
        <otv:instanceOf rdf:resource="#Ancient_Location"/>
        <otv:denotedByProperName rdf:resource="#Keos_en"/>
        <otv:denotedByProperName rdf:resource="#Κέα_el"/>
    </otv:Object>

    <otv:Object rdf:about="#epithalamia_sappho">
        <otv:instanceOf rdf:resource="#Archaic_Lyric_Poem_in_ionic_or_in_doric_or_in_aeolic_dialect_performed_by_a_chorus_or_by_a_single_performer_dedicated_to_wedding_couple"/>
        <otv:denotedByProperName rdf:resource="#Epithalamia_of_Sappho_Lesbia_en"/>
        <otv:denotedByProperName rdf:resource="#Επιθαλάμια_της_Σαπφούς_της_Λεσβίας_el"/>
    </otv:Object>

    <otv:Object rdf:about="#stesichorus_himeraeus">
        <otv:instanceOf rdf:resource="#Archaic_Lyric_Poet"/>
        <otv:denotedByProperName rdf:resource="#Stesichorus_Himeraeus_en"/>
        <otv:denotedByProperName rdf:resource="#Στησίχορος_από_την_Ιμέρα_el"/>
    </otv:Object>

    <otv:Object rdf:about="#iambs_semonides">
        <otv:instanceOf rdf:resource="#Archaic_Lyric_Poem_only_in_ionic_dialect_in_iambic_or_trochaic_metre"/>
        <otv:denotedByProperName rdf:resource="#Iambs_of_Semonides_Amorginus_en"/>
        <otv:denotedByProperName rdf:resource="#Ίαμβοι_του_Σημωνίδη_του_Αμοργίνου_el"/>
    </otv:Object>

    <otv:Object rdf:about="#sympotic_odes_anacreon">
        <otv:instanceOf rdf:resource="#Archaic_Lyric_Poem_in_ionic_or_in_doric_or_in_aeolic_dialect_performed_by_a_single_performer"/>
        <otv:denotedByProperName rdf:resource="#Sympotic_odes_of_Anacreon_Teius_en"/>
        <otv:denotedByProperName rdf:resource="#Συμποτικές_ωδές_του_Ανακρέοντα_el"/>
    </otv:Object>

    <otv:Object rdf:about="#ananius_iambographus">
        <otv:instanceOf rdf:resource="#Archaic_Lyric_Poet"/>
        <otv:denotedByProperName rdf:resource="#Ananius_Iambographus_en"/>
        <otv:denotedByProperName rdf:resource="#Ananios_Iambograph_en"/>
        <otv:denotedByProperName rdf:resource="#Ananius_Lyricus_en"/>
        <otv:denotedByProperName rdf:resource="#Ανάνιος_ο_Ιαμβογράφος_el"/>
        <otv:denotedByProperName rdf:resource="#Ανάνιος_ο_Λυρικός_el"/>
    </otv:Object>

    <otv:Object rdf:about="#sardis">
        <otv:instanceOf rdf:resource="#Ancient_Location"/>
        <otv:denotedByProperName rdf:resource="#Sardis_en"/>
        <otv:denotedByProperName rdf:resource="#Σάρδεις_el"/>
    </otv:Object>

    <otv:Object rdf:about="#rhegium">
        <otv:instanceOf rdf:resource="#Ancient_Location"/>
        <otv:denotedByProperName rdf:resource="#Rhegium_en"/>
        <otv:denotedByProperName rdf:resource="#Ρήγιο_el"/>
    </otv:Object>

    <otv:Object rdf:about="#warlike_odes_alcaeus">
        <otv:instanceOf rdf:resource="#Archaic_Lyric_Poem_in_ionic_or_in_doric_or_in_aeolic_dialect_performed_by_a_single_performer"/>
        <otv:denotedByProperName rdf:resource="#Warlike_odes_of_Alcaeus_Lesbius_en"/>
        <otv:denotedByProperName rdf:resource="#Πολεμικές_ωδές_του_Αλκαίου_el"/>
    </otv:Object>

    <otv:Object rdf:about="#hyporchemes_pindarus">
        <otv:instanceOf rdf:resource="#Archaic_Lyric_Poem_in_ionic_or_in_doric_or_in_aeolic_dialect_performed_by_a_chorus_with_imitation_expressions"/>
        <otv:denotedByProperName rdf:resource="#Hyporchemes_of_Pindarus_Boeotus_en"/>
        <otv:denotedByProperName rdf:resource="#Υπορχήματα_του_Πινδάρου_el"/>
    </otv:Object>

    <otv:Object rdf:about="#hymns_anacreon">
        <otv:instanceOf rdf:resource="#Archaic_Lyric_Poem_in_ionic_or_in_doric_or_in_aeolic_dialect_performed_by_a_chorus_or_by_a_single_performer_dedicated_to_a_god"/>
        <otv:denotedByProperName rdf:resource="#Hymns_of_Anacreon_Teius_en"/>
        <otv:denotedByProperName rdf:resource="#Ύμνοι_του_Ανακρέοντα_el"/>
    </otv:Object>

    <otv:Object rdf:about="#himera">
        <otv:instanceOf rdf:resource="#Ancient_Location"/>
        <otv:denotedByProperName rdf:resource="#Himera_en"/>
        <otv:denotedByProperName rdf:resource="#Ιμέρα_el"/>
    </otv:Object>

    <otv:Object rdf:about="#hymns_alcaeus">
        <otv:instanceOf rdf:resource="#Archaic_Lyric_Poem_in_ionic_or_in_doric_or_in_aeolic_dialect_performed_by_a_chorus_or_by_a_single_performer_dedicated_to_a_god"/>
        <otv:denotedByProperName rdf:resource="#Hymns_of_Alcaeus_Lesbius_en"/>
        <otv:denotedByProperName rdf:resource="#Ύμνοι_του_Αλκαίου_el"/>
    </otv:Object>

    <otv:Object rdf:about="#teos">
        <otv:instanceOf rdf:resource="#Ancient_Location"/>
        <otv:denotedByProperName rdf:resource="#Teos_en"/>
        <otv:denotedByProperName rdf:resource="#Τέως_el"/>
    </otv:Object>

    <otv:Object rdf:about="#dithyrambs_pindarus">
        <otv:instanceOf rdf:resource="#Archaic_Lyric_Poem_in_ionic_or_in_doric_or_in_aeolic_dialect_performed_by_a_chorus_or_by_a_single_performer_dedicated_to_dionysus"/>
        <otv:denotedByProperName rdf:resource="#Dithyrambs_of_Pindarus_Boeotus_en"/>
        <otv:denotedByProperName rdf:resource="#Διθυραμβική_ποίηση_του_Πινδάρου_el"/>
    </otv:Object>

    <otv:Object rdf:about="#theognis_megarensis">
        <otv:instanceOf rdf:resource="#Archaic_Lyric_Poet"/>
        <otv:denotedByProperName rdf:resource="#Theognis_Megarensis_en"/>
        <otv:denotedByProperName rdf:resource="#Theognis_Elegiacus_en"/>
        <otv:denotedByProperName rdf:resource="#Θέογνις_από_τα_Μέγαρα_el"/>
    </otv:Object>

    <otv:Object rdf:about="#athens">
        <otv:instanceOf rdf:resource="#Ancient_Location"/>
        <otv:denotedByProperName rdf:resource="#Athens_en"/>
        <otv:denotedByProperName rdf:resource="#Αθήνα_el"/>
    </otv:Object>

    <otv:Object rdf:about="#sympotic_odes_alcaeus">
        <otv:instanceOf rdf:resource="#Archaic_Lyric_Poem_in_ionic_or_in_doric_or_in_aeolic_dialect_performed_by_a_single_performer"/>
        <otv:denotedByProperName rdf:resource="#Sympotic_odes_of_Alcaeus_Lesbius_en"/>
        <otv:denotedByProperName rdf:resource="#Συμποτικές_ωδές_του_Αλκαίου_el"/>
    </otv:Object>

    <otv:Object rdf:about="#aegypt">
        <otv:instanceOf rdf:resource="#Ancient_Location"/>
        <otv:denotedByProperName rdf:resource="#Aegypt_en"/>
        <otv:denotedByProperName rdf:resource="#Αίγυπτος_el"/>
    </otv:Object>

    <otv:Object rdf:about="#choral_stesichorus">
        <otv:instanceOf rdf:resource="#Archaic_Lyric_Poem_in_ionic_or_in_doric_or_in_aeolic_dialect_performed_by_a_chorus"/>
        <otv:denotedByProperName rdf:resource="#Choral_songs_of_Stesichorus_Himeraeus_en"/>
        <otv:denotedByProperName rdf:resource="#Χορική_ποίηση_του_Στησίχορου_από_την_Ιμέρα_el"/>
    </otv:Object>

    <otv:Object rdf:about="#erotic_elegies_mimnermus">
        <otv:instanceOf rdf:resource="#Archaic_Lyric_Poem_only_in_ionic_dialect_in_elegiac_couplet_with_erotic_content"/>
        <otv:denotedByProperName rdf:resource="#Erotic_elegies_of_Mimnermus_Lyricus_en"/>
        <otv:denotedByProperName rdf:resource="#Ερωτική_ελεγεία_του_Μίμνερμου_el"/>
    </otv:Object>

    <otv:Object rdf:about="#thasos_settlement">
        <otv:instanceOf rdf:resource="#Ancient_Location"/>
        <otv:denotedByProperName rdf:resource="#Thasos-_settlement_en"/>
        <otv:denotedByProperName rdf:resource="#Θάσος-αποικία_el"/>
    </otv:Object>

    <otv:Object rdf:about="#5th_century_BCE">
        <otv:instanceOf rdf:resource="#BCE_century"/>
        <otv:denotedByProperName rdf:resource="#5th_century_BCE_en"/>
        <otv:denotedByProperName rdf:resource="#5ος_αιώνας_π.Χ._el"/>
    </otv:Object>

    <otv:Object rdf:about="#samos">
        <otv:instanceOf rdf:resource="#Ancient_Location"/>
        <otv:denotedByProperName rdf:resource="#Samos_en"/>
        <otv:denotedByProperName rdf:resource="#Σάμος_el"/>
    </otv:Object>

    <otv:Object rdf:about="#gnomic_elegies_theognis">
        <otv:instanceOf rdf:resource="#Archaic_Lyric_Poem_only_in_ionic_dialect_in_elegiac_couplet_with_gnomic_content"/>
        <otv:denotedByProperName rdf:resource="#Gnomic_elegies_of_Theognis_Megarensis_en"/>
        <otv:denotedByProperName rdf:resource="#Γνωμικές_ελεγείες_του_Θέογνη_el"/>
    </otv:Object>

    <otv:Object rdf:about="#simonides_ceus">
        <otv:instanceOf rdf:resource="#Archaic_Lyric_Poet"/>
        <otv:denotedByProperName rdf:resource="#Simonides_Ceus_en"/>
        <otv:denotedByProperName rdf:resource="#Simonides_Lyricus_en"/>
        <otv:denotedByProperName rdf:resource="#Simonides_of_Ceos_en"/>
        <otv:denotedByProperName rdf:resource="#Σιμωνίδης_από_την_Κέα_el"/>
        <otv:denotedByProperName rdf:resource="#Σιμωνίδης_ο_Λυρικός_el"/>
    </otv:Object>

    <otv:Object rdf:about="#ibycus_rheginus">
        <otv:instanceOf rdf:resource="#Archaic_Lyric_Poet"/>
        <otv:denotedByProperName rdf:resource="#Ibycus_Rheginus_en"/>
        <otv:denotedByProperName rdf:resource="#Ίβυκος_ο_Ρηγίνος_el"/>
    </otv:Object>

    <otv:Object rdf:about="#hyporcheme_bacchylides">
        <otv:instanceOf rdf:resource="#Archaic_Lyric_Poem_in_ionic_or_in_doric_or_in_aeolic_dialect_performed_by_a_chorus_with_imitation_expressions"/>
        <otv:denotedByProperName rdf:resource="#Hyporchemes_of_Bacchylides_Ceus_en"/>
        <otv:denotedByProperName rdf:resource="#Υπορχήματα_του_Βακχυλίδη_el"/>
    </otv:Object>

    <otv:Object rdf:about="#epinikoi_pindarus">
        <otv:instanceOf rdf:resource="#Archaic_Lyric_Poem_in_ionic_or_in_doric_or_in_aeolic_dialect_performed_by_a_chorus_or_by_a_single_performer_dedicated_to_winners_in_athletic_events"/>
        <otv:denotedByProperName rdf:resource="#Epinikoi_of_Pindarus_Boeotus_en"/>
        <otv:denotedByProperName rdf:resource="#Επίνικοι_του_Πινδάρου_el"/>
    </otv:Object>

    <otv:Object rdf:about="#6th_century_BCE">
        <otv:instanceOf rdf:resource="#BCE_century"/>
        <otv:denotedByProperName rdf:resource="#6th_century_BCE_en"/>
        <otv:denotedByProperName rdf:resource="#6ος_αιώνας_π.Χ._el"/>
    </otv:Object>

    <otv:Object rdf:about="#epinikoi_bacchylides">
        <otv:instanceOf rdf:resource="#Archaic_Lyric_Poem_in_ionic_or_in_doric_or_in_aeolic_dialect_performed_by_a_chorus_or_by_a_single_performer_dedicated_to_winners_in_athletic_events"/>
        <otv:denotedByProperName rdf:resource="#Epinikoi_of_Bacchylides_Ceus_en"/>
        <otv:denotedByProperName rdf:resource="#Επίνικοι_του_Βακχυλίδη_el"/>
    </otv:Object>

    <otv:Object rdf:about="#abdera">
        <otv:instanceOf rdf:resource="#Ancient_Location"/>
        <otv:denotedByProperName rdf:resource="#Abdera_en"/>
        <otv:denotedByProperName rdf:resource="#Άβδηρα_el"/>
    </otv:Object>

    <otv:Object rdf:about="#paeans_alcman">
        <otv:instanceOf rdf:resource="#Archaic_Lyric_Poem_in_ionic_or_in_doric_or_in_aeolic_dialect_performed_by_a_chorus_or_by_a_single_performer_dedicated_to_apollo"/>
        <otv:denotedByProperName rdf:resource="#Paeans_of_Alcman_Lacedaemonius_en"/>
        <otv:denotedByProperName rdf:resource="#Παιάνες_του_Αλκμάνα_el"/>
    </otv:Object>

    <otv:Object rdf:about="#iambs_anacreon">
        <otv:instanceOf rdf:resource="#Archaic_Lyric_Poem_only_in_ionic_dialect_in_iambic_or_trochaic_metre"/>
        <otv:denotedByProperName rdf:resource="#Iambs_of_Anacreon_Teius_en"/>
        <otv:denotedByProperName rdf:resource="#Ίαμβοι_του_Ανακρέοντα_el"/>
    </otv:Object>

    <otv:Object rdf:about="#hymns_terpander">
        <otv:instanceOf rdf:resource="#Archaic_Lyric_Poem_in_ionic_or_in_doric_or_in_aeolic_dialect_performed_by_a_chorus_or_by_a_single_performer_dedicated_to_a_god"/>
        <otv:denotedByProperName rdf:resource="#Hymns_of_Terpander_Lesbius_en"/>
        <otv:denotedByProperName rdf:resource="#Ύμνοι_του_Τέρπανδρου_el"/>
    </otv:Object>

    <otv:Object rdf:about="#hipponax_ephesius">
        <otv:instanceOf rdf:resource="#Archaic_Lyric_Poet"/>
        <otv:denotedByProperName rdf:resource="#Hipponax_Ephesius_en"/>
        <otv:denotedByProperName rdf:resource="#Hipponax_Iambographus_en"/>
        <otv:denotedByProperName rdf:resource="#Ιππώναξ_ο_Εφέσιος_el"/>
        <otv:denotedByProperName rdf:resource="#Ιππώναξ_ο_Ιαμβογράφος_el"/>
    </otv:Object>

    <otv:Object rdf:about="#hymns_sappho">
        <otv:instanceOf rdf:resource="#Archaic_Lyric_Poem_in_ionic_or_in_doric_or_in_aeolic_dialect_performed_by_a_chorus_or_by_a_single_performer_dedicated_to_a_god"/>
        <otv:denotedByProperName rdf:resource="#Hymns_of_Sappho_Lesbia_en"/>
        <otv:denotedByProperName rdf:resource="#Ύμνοι_της_Σαπφούς_της_Λεσβίας_el"/>
    </otv:Object>

    <otv:Object rdf:about="#hymns_archilochus">
        <otv:instanceOf rdf:resource="#Archaic_Lyric_Poem_in_ionic_or_in_doric_or_in_aeolic_dialect_performed_by_a_chorus_or_by_a_single_performer_dedicated_to_a_god"/>
        <otv:denotedByProperName rdf:resource="#Hymns_of_Archilochus_Parius_en"/>
        <otv:denotedByProperName rdf:resource="#Ύμνοι_του_Αρχιλόχου_el"/>
    </otv:Object>

    <otv:Object rdf:about="#hymenaios_sappho">
        <otv:instanceOf rdf:resource="#Archaic_Lyric_Poem_in_ionic_or_in_doric_or_in_aeolic_dialect_performed_by_a_chorus_during_bride_procession"/>
        <otv:denotedByProperName rdf:resource="#Hymenaios_of_Sappho_Lesbia_en"/>
        <otv:denotedByProperName rdf:resource="#Υμέναιοι_της_Σαπφούς_el"/>
    </otv:Object>

    <otv:Object rdf:about="#erotic_odes_sappho">
        <otv:instanceOf rdf:resource="#Archaic_Lyric_Poem_in_ionic_or_in_doric_or_in_aeolic_dialect_performed_by_a_single_performer"/>
        <otv:denotedByProperName rdf:resource="#Erotic_poetry_of_Sappho_Lesbia_en"/>
        <otv:denotedByProperName rdf:resource="#Ερωτική_ποίηση_της_Σαπφούς_el"/>
    </otv:Object>

    <otv:Object rdf:about="#iambs_ananius">
        <otv:instanceOf rdf:resource="#Archaic_Lyric_Poem_only_in_ionic_dialect_in_iambic_or_trochaic_metre"/>
        <otv:denotedByProperName rdf:resource="#Iambs_of_Ananius_en"/>
        <otv:denotedByProperName rdf:resource="#Ίαμβοι_του_Ανάνιου_el"/>
    </otv:Object>

    <otv:Object rdf:about="#dithyrambs_bacchylides">
        <otv:instanceOf rdf:resource="#Archaic_Lyric_Poem_in_ionic_or_in_doric_or_in_aeolic_dialect_performed_by_a_chorus_or_by_a_single_performer_dedicated_to_dionysus"/>
        <otv:denotedByProperName rdf:resource="#Dithyrambs_of_Bacchylides_Ceus_en"/>
        <otv:denotedByProperName rdf:resource="#Διθυραμβική_ποίηση_του_Βακχυλίδη_από_την_Κέα_el"/>
    </otv:Object>

    <otv:Object rdf:about="#war_elegy_callinus">
        <otv:instanceOf rdf:resource="#Archaic_Lyric_Poem_only_in_ionic_dialect_in_elegiac_couplet_with_war_content"/>
        <otv:denotedByProperName rdf:resource="#War_elegy_of_Callinus_Ephesius_en"/>
        <otv:denotedByProperName rdf:resource="#Πολεμικές_ελεγείες_του_Καλλίνου_el"/>
    </otv:Object>

    <otv:Object rdf:about="#bacchylides_ceus">
        <otv:instanceOf rdf:resource="#Archaic_Lyric_Poet"/>
        <otv:denotedByProperName rdf:resource="#Bacchylides_Ceus_en"/>
        <otv:denotedByProperName rdf:resource="#Bacchylides_Lyricus_en"/>
        <otv:denotedByProperName rdf:resource="#Βακχυλίδης_από_την_Κέα_el"/>
        <otv:denotedByProperName rdf:resource="#Βακχυλίδης_ο_Λυρικός_el"/>
    </otv:Object>

    <otv:Object rdf:about="#terpander_lesbius">
        <otv:instanceOf rdf:resource="#Archaic_Lyric_Poet"/>
        <otv:denotedByProperName rdf:resource="#Terpander_Lesbius_en"/>
        <otv:denotedByProperName rdf:resource="#Terpandros_en"/>
        <otv:denotedByProperName rdf:resource="#Terpandrus_en"/>
        <otv:denotedByProperName rdf:resource="#Τέρπανδρος_ο_Λέσβιος_el"/>
    </otv:Object>

    <otv:Object rdf:about="#tyrtaeus_lacedaemonius">
        <otv:instanceOf rdf:resource="#Archaic_Lyric_Poet"/>
        <otv:denotedByProperName rdf:resource="#Tyrtaeus_Lacedaemonius_en"/>
        <otv:denotedByProperName rdf:resource="#Τυρταίος_ο_Λακεδαιμόνιος_el"/>
    </otv:Object>

    <otv:Object rdf:about="#hymns_alcman">
        <otv:instanceOf rdf:resource="#Archaic_Lyric_Poem_in_ionic_or_in_doric_or_in_aeolic_dialect_performed_by_a_chorus_or_by_a_single_performer_dedicated_to_a_god"/>
        <otv:denotedByProperName rdf:resource="#Hymns_of_Alcman_Lacedaemonius_en"/>
        <otv:denotedByProperName rdf:resource="#Ύμνοι_του_Αλκμάνα_του_Λακεδαιμόνιου_el"/>
    </otv:Object>

    <otv:Object rdf:about="#semonides_amorginus">
        <otv:instanceOf rdf:resource="#Archaic_Lyric_Poet"/>
        <otv:denotedByProperName rdf:resource="#Semonides_Amorginus_en"/>
        <otv:denotedByProperName rdf:resource="#Simonides_of_Amorgos_en"/>
        <otv:denotedByProperName rdf:resource="#Semonides_Iambographus_en"/>
        <otv:denotedByProperName rdf:resource="#Simonides_of_Samos_en"/>
        <otv:denotedByProperName rdf:resource="#Σημωνίδης_ο_Αμοργίνος_el"/>
        <otv:denotedByProperName rdf:resource="#Σημωνίδης_ο_Ιαμβογράφος_el"/>
    </otv:Object>

    <otv:Object rdf:about="#ephesus">
        <otv:instanceOf rdf:resource="#Ancient_Location"/>
        <otv:denotedByProperName rdf:resource="#Ephesus_en"/>
        <otv:denotedByProperName rdf:resource="#Έφεσος_el"/>
    </otv:Object>

    <otv:Object rdf:about="#syrakousai">
        <otv:instanceOf rdf:resource="#Ancient_Location"/>
        <otv:denotedByProperName rdf:resource="#Syrakousai_en"/>
        <otv:denotedByProperName rdf:resource="#Συρακούσες_el"/>
    </otv:Object>

    <otv:Object rdf:about="#prosodia_pindarus">
        <otv:instanceOf rdf:resource="#Archaic_Lyric_Poem_in_ionic_or_in_doric_or_in_aeolic_dialect_performed_by_a_chorus_on_the_way_to_an_altar"/>
        <otv:denotedByProperName rdf:resource="#Prosodia_of_Pindarus_Boeotus_en"/>
        <otv:denotedByProperName rdf:resource="#Προσόδια_του_Πινδάρου_el"/>
    </otv:Object>

</rdf:RDF>
